# baseURI: http://data.europa.eu/a4g/ontology
# imports: http://purl.org/dc/terms/
# imports: http://www.w3.org/2004/02/skos/core
# prefix: epo

@prefix : <http://data.europa.eu/a4g/ontology#> .
@prefix cc: <http://creativecommons.org/ns#> .
@prefix dc: <http://www.omg.org/spec/UML/20131001/UMLDC> .
@prefix dct: <http://purl.org/dc/terms/> .
@prefix epo: <http://data.europa.eu/a4g/ontology#> .
@prefix foaf: <http://xmlns.com/foaf/0.1/> .
@prefix org: <http://www.w3.org/ns/org#> .
@prefix owl: <http://www.w3.org/2002/07/owl#> .
@prefix rdf: <http://www.w3.org/1999/02/22-rdf-syntax-ns#> .
@prefix rdfs: <http://www.w3.org/2000/01/rdf-schema#> .
@prefix skos: <http://www.w3.org/2004/02/skos/core#> .
@prefix vann: <http://purl.org/vocab/vann/> .
@prefix xsd: <http://www.w3.org/2001/XMLSchema#> .

<http://data.europa.eu/Nuts>
  rdf:type skos:ConceptScheme ;
  rdfs:comment "e.g. NUTS 2016"@en ;
  rdfs:isDefinedBy <http://data.europa.eu/a4g/ontology> ;
  rdfs:label "Nuts"@en ;
  skos:definition "e.g. NUTS 2016"@en ;
  skos:prefLabel "Nuts" ;
.
<http://data.europa.eu/a4g/ontology>
  rdf:type owl:Ontology ;
  cc:attributionName "PublicationsOffice of the European Union" ;
  cc:attributionURL <http://publications.europa.eu/resource/authority/corporate-body/PUBL> ;
  dct:date "2020-05-25+02:00"^^xsd:date ;
  dct:description """Procurement data has been identified as data with a
            high-reuse potential. Given the increasing importance of data standards for
            eProcurement, a number of initiatives driven by the public sector, the industry and
            academia have been kick-started in recent years. Some have grown organically, while
            others are the result of standardisation work. The vocabularies and the semantics that
            they are introducing, the phases of public procurement that they are covering, and the
            technologies that they are using all differ. These differences hamper data
            interoperability and thus its reuse by them or by the wider public. This creates the
            need for a common data standard for publishing procurement data, hence allowing data
            from different sources to be easily accessed and linked, and consequently
            reused."""@en ;
  dct:license <http://creativecommons.org/licenses/by-sa/4.0/> ;
  dct:title "eProcurement ontology"@en ;
  vann:preferredNamespacePrefix "epo" ;
  vann:preferredNamespaceUri "http://data.europa.eu/a4g/ontology#" ;
  rdfs:label "eProcurement ontology"@en ;
  rdfs:seeAlso <https://github.com/eprocurementontology/eprocurementontology> ;
  rdfs:seeAlso <https://joinup.ec.europa.eu/solution/eprocurement-ontology/about> ;
  rdfs:seeAlso <https://op.europa.eu/en/web/eu-vocabularies/e-procurement> ;
  owl:imports dct: ;
  owl:imports <http://www.w3.org/2004/02/skos/core> ;
  owl:versionInfo "eProcurement Ontology version auto generated on 25/05/2020" ;
.
epo:ABW
  rdf:type skos:Concept ;
  rdfs:isDefinedBy <http://data.europa.eu/a4g/ontology> ;
  rdfs:label "Aruba"@en ;
  skos:inScheme <http://publications.europa.eu/resource/authority/Country> ;
  skos:prefLabel "Aruba"@en ;
.
epo:AFG
  rdf:type skos:Concept ;
  rdfs:isDefinedBy <http://data.europa.eu/a4g/ontology> ;
  rdfs:label "Afghanistan"@en ;
  skos:inScheme <http://publications.europa.eu/resource/authority/Country> ;
  skos:prefLabel "Afghanistan"@en ;
.
epo:AGO
  rdf:type skos:Concept ;
  rdfs:isDefinedBy <http://data.europa.eu/a4g/ontology> ;
  rdfs:label "Angola"@en ;
  skos:inScheme <http://publications.europa.eu/resource/authority/Country> ;
  skos:prefLabel "Angola"@en ;
.
epo:AIA
  rdf:type skos:Concept ;
  rdfs:isDefinedBy <http://data.europa.eu/a4g/ontology> ;
  rdfs:label "Anguilla"@en ;
  skos:inScheme <http://publications.europa.eu/resource/authority/Country> ;
  skos:prefLabel "Anguilla"@en ;
.
epo:ALA
  rdf:type skos:Concept ;
  rdfs:isDefinedBy <http://data.europa.eu/a4g/ontology> ;
  rdfs:label "Aland Islands"@en ;
  skos:inScheme <http://publications.europa.eu/resource/authority/Country> ;
  skos:prefLabel "Aland Islands"@en ;
.
epo:ALB
  rdf:type skos:Concept ;
  rdfs:isDefinedBy <http://data.europa.eu/a4g/ontology> ;
  rdfs:label "Albania"@en ;
  skos:inScheme <http://publications.europa.eu/resource/authority/Country> ;
  skos:prefLabel "Albania"@en ;
.
epo:AND
  rdf:type skos:Concept ;
  rdfs:isDefinedBy <http://data.europa.eu/a4g/ontology> ;
  rdfs:label "Andorra"@en ;
  skos:inScheme <http://publications.europa.eu/resource/authority/Country> ;
  skos:prefLabel "Andorra"@en ;
.
epo:APR
  rdf:type skos:Concept ;
  rdfs:isDefinedBy <http://data.europa.eu/a4g/ontology> ;
  rdfs:label "April"@en ;
  skos:inScheme <http://publications.europa.eu/resource/authority/Timeperiods> ;
  skos:prefLabel "April"@en ;
.
epo:ARG
  rdf:type skos:Concept ;
  rdfs:isDefinedBy <http://data.europa.eu/a4g/ontology> ;
  rdfs:label "Argentina"@en ;
  skos:inScheme <http://publications.europa.eu/resource/authority/Country> ;
  skos:prefLabel "Argentina"@en ;
.
epo:ARM
  rdf:type skos:Concept ;
  rdfs:isDefinedBy <http://data.europa.eu/a4g/ontology> ;
  rdfs:label "Armenia"@en ;
  skos:inScheme <http://publications.europa.eu/resource/authority/Country> ;
  skos:prefLabel "Armenia"@en ;
.
epo:ASM
  rdf:type skos:Concept ;
  rdfs:isDefinedBy <http://data.europa.eu/a4g/ontology> ;
  rdfs:label "American Samoa"@en ;
  skos:inScheme <http://publications.europa.eu/resource/authority/Country> ;
  skos:prefLabel "American Samoa"@en ;
.
epo:ATA
  rdf:type skos:Concept ;
  rdfs:isDefinedBy <http://data.europa.eu/a4g/ontology> ;
  rdfs:label "Antartica"@en ;
  skos:inScheme <http://publications.europa.eu/resource/authority/Country> ;
  skos:prefLabel "Antartica"@en ;
.
epo:ATG
  rdf:type skos:Concept ;
  rdfs:isDefinedBy <http://data.europa.eu/a4g/ontology> ;
  rdfs:label "Antigua and Barbuda"@en ;
  skos:inScheme <http://publications.europa.eu/resource/authority/Country> ;
  skos:prefLabel "Antigua and Barbuda"@en ;
.
epo:AUG
  rdf:type skos:Concept ;
  rdfs:isDefinedBy <http://data.europa.eu/a4g/ontology> ;
  rdfs:label "August"@en ;
  skos:inScheme <http://publications.europa.eu/resource/authority/Timeperiods> ;
  skos:prefLabel "August"@en ;
.
epo:AUS
  rdf:type skos:Concept ;
  rdfs:isDefinedBy <http://data.europa.eu/a4g/ontology> ;
  rdfs:label "Australia"@en ;
  skos:inScheme <http://publications.europa.eu/resource/authority/Country> ;
  skos:prefLabel "Australia"@en ;
.
epo:AUT
  rdf:type skos:Concept ;
  rdfs:isDefinedBy <http://data.europa.eu/a4g/ontology> ;
  rdfs:label "Austria"@en ;
  skos:inScheme <http://publications.europa.eu/resource/authority/Country> ;
  skos:prefLabel "Austria"@en ;
.
epo:AUTUMN
  rdf:type skos:Concept ;
  rdfs:isDefinedBy <http://data.europa.eu/a4g/ontology> ;
  rdfs:label "Autumn"@en ;
  skos:inScheme <http://publications.europa.eu/resource/authority/Timeperiods> ;
  skos:prefLabel "Autumn"@en ;
.
epo:AZE
  rdf:type skos:Concept ;
  rdfs:isDefinedBy <http://data.europa.eu/a4g/ontology> ;
  rdfs:label "Azerbaijan"@en ;
  skos:inScheme <http://publications.europa.eu/resource/authority/Country> ;
  skos:prefLabel "Azerbaijan"@en ;
.
epo:Abs-comp
  rdf:type skos:Concept ;
  rdfs:isDefinedBy <http://data.europa.eu/a4g/ontology> ;
  rdfs:label "The contract can be provided only by a particular economic operator because of an absence of competition for technical reasons"@en ;
  skos:inScheme <http://publications.europa.eu/resource/authority/Direct-award-justification> ;
  skos:prefLabel "The contract can be provided only by a particular economic operator because of an absence of competition for technical reasons"@en ;
.
epo:Accelerated-procedure-justification-type
  rdf:type skos:ConceptScheme ;
  rdfs:comment "A procurement procedure where the time limit for receipt of tenders can be reduced due to a state of urgency."@en ;
  rdfs:isDefinedBy <http://data.europa.eu/a4g/ontology> ;
  rdfs:label "Accelerated-procedure-justification-type"@en ;
  skos:definition "A procurement procedure where the time limit for receipt of tenders can be reduced due to a state of urgency."@en ;
  skos:prefLabel "Accelerated-procedure-justification-type" ;
.
epo:AccessTerms
  rdf:type owl:Class ;
  rdfs:comment """Conditions and stipulations about where and how to access the procurement documents.

"""@en ;
  rdfs:isDefinedBy <http://data.europa.eu/a4g/ontology> ;
  rdfs:label "Access terms"@en ;
  skos:definition """Conditions and stipulations about where and how to access the procurement documents.

"""@en ;
  skos:prefLabel "Access terms"@en ;
.
epo:Add-work-serv-supp
  rdf:type skos:Concept ;
  rdfs:isDefinedBy <http://data.europa.eu/a4g/ontology> ;
  rdfs:label "Need for additional works, services or supplies by the original contractor. "@en ;
  skos:inScheme <http://publications.europa.eu/resource/authority/Modification-justification> ;
  skos:prefLabel "Need for additional works, services or supplies by the original contractor. "@en ;
.
epo:AdditionalDocument
  rdf:type owl:Class ;
  rdfs:comment "Supplementary interrelated document."@en ;
  rdfs:isDefinedBy <http://data.europa.eu/a4g/ontology> ;
  rdfs:label "Additional document"@en ;
  rdfs:subClassOf epo:ProcurementDocument ;
  owl:disjointWith epo:CallForCompetition ;
  owl:disjointWith epo:ContractTemplate ;
  owl:disjointWith epo:DescriptiveDocument ;
  owl:disjointWith epo:DraftCV ;
  owl:disjointWith epo:ESPDRequest ;
  owl:disjointWith epo:InvitationToTender ;
  owl:disjointWith epo:PreAwardCatalogueRequest ;
  owl:disjointWith epo:TechnicalSpecifications ;
  skos:definition "Supplementary interrelated document."@en ;
  skos:prefLabel "Additional document"@en ;
.
epo:Address
  rdf:type owl:Class ;
  rdfs:comment """The particulars of the place where a person or an organization is located.

WG Approval 28/04/2020"""@en ;
  rdfs:isDefinedBy <http://data.europa.eu/a4g/ontology> ;
  rdfs:label "Address"@en ;
  skos:definition """The particulars of the place where a person or an organization is located.

WG Approval 28/04/2020"""@en ;
  skos:prefLabel "Address"@en ;
.
epo:AdmistrativeCriterion
  rdf:type skos:Concept ;
  rdfs:isDefinedBy <http://data.europa.eu/a4g/ontology> ;
  rdfs:label "Admistrative criterion"@en ;
  skos:inScheme epo:E-evaluation-criterion-type ;
  skos:prefLabel "Admistrative criterion"@en ;
.
epo:Agent
  rdf:type owl:Class ;
  rdfs:comment """A  person, an organization, or a system that act in procurement or have the power to act in procurement.

WG Approval 28/04/2020"""@en ;
  rdfs:isDefinedBy <http://data.europa.eu/a4g/ontology> ;
  rdfs:label "Agent"@en ;
  rdfs:subClassOf dct:Agent ;
  skos:definition """A  person, an organization, or a system that act in procurement or have the power to act in procurement.

WG Approval 28/04/2020"""@en ;
  skos:prefLabel "Agent"@en ;
.
epo:Air
  rdf:type skos:Concept ;
  rdfs:isDefinedBy <http://data.europa.eu/a4g/ontology> ;
  rdfs:label "Airport-related activities"@en ;
  skos:inScheme <http://publications.europa.eu/resource/authority/Main-activity> ;
  skos:prefLabel "Airport-related activities"@en ;
.
epo:All-rej
  rdf:type skos:Concept ;
  rdfs:isDefinedBy <http://data.europa.eu/a4g/ontology> ;
  rdfs:label "All tenders, requests to participate or porjects were rejected"@en ;
  skos:inScheme <http://publications.europa.eu/resource/authority/Non-award-justification> ;
  skos:prefLabel "All tenders, requests to participate or porjects were rejected"@en ;
.
epo:Allowed
  rdf:type skos:Concept ;
  rdfs:isDefinedBy <http://data.europa.eu/a4g/ontology> ;
  rdfs:label "Allowed"@en ;
  skos:inScheme <http://publications.europa.eu/resource/authority/Permission> ;
  skos:prefLabel "Allowed"@en ;
.
epo:Amount
  rdf:type rdfs:Datatype ;
  rdf:type owl:Class ;
  rdfs:isDefinedBy <http://data.europa.eu/a4g/ontology> ;
  rdfs:label "Amount"@en ;
  rdfs:subClassOf <http://www.unece.org/cefact#Amount> ;
  skos:prefLabel "Amount"@en ;
.
epo:Anyw
  rdf:type skos:Concept ;
  rdfs:isDefinedBy <http://data.europa.eu/a4g/ontology> ;
  rdfs:label "Anywhere"@en ;
  skos:inScheme <http://publications.europa.eu/resource/authority/Other-place-service> ;
  skos:prefLabel "Anywhere"@en ;
.
epo:Anyw-cou
  rdf:type skos:Concept ;
  rdfs:isDefinedBy <http://data.europa.eu/a4g/ontology> ;
  rdfs:label "Anywhere in the given country"@en ;
  skos:inScheme <http://publications.europa.eu/resource/authority/Other-place-service> ;
  skos:prefLabel "Anywhere in the given country"@en ;
.
epo:Anyw-eea
  rdf:type skos:Concept ;
  rdfs:isDefinedBy <http://data.europa.eu/a4g/ontology> ;
  rdfs:label "Anywhere in the European Economic Area"@en ;
  skos:inScheme <http://publications.europa.eu/resource/authority/Other-place-service> ;
  skos:prefLabel "Anywhere in the European Economic Area"@en ;
.
epo:Authority-type
  rdf:type skos:ConceptScheme ;
  rdfs:comment """Aternative name to this code list:

- Authority Competency Level Type
"""@en ;
  rdfs:isDefinedBy <http://data.europa.eu/a4g/ontology> ;
  rdfs:label "Authority-type"@en ;
  skos:definition """Aternative name to this code list:

- Authority Competency Level Type
"""@en ;
  skos:prefLabel "Authority-type" ;
.
epo:Award-dimension-parent-criterion-relation
  rdf:type skos:ConceptScheme ;
  rdfs:isDefinedBy <http://data.europa.eu/a4g/ontology> ;
  rdfs:label "Award-dimension-parent-criterion-relation"@en ;
  skos:prefLabel "Award-dimension-parent-criterion-relation" ;
.
epo:Award-evaluation-method-type
  rdf:type skos:ConceptScheme ;
  rdfs:comment "A code signifying the type of criterion."@en ;
  rdfs:isDefinedBy <http://data.europa.eu/a4g/ontology> ;
  rdfs:label "Award-evaluation-method-type"@en ;
  skos:definition "A code signifying the type of criterion."@en ;
  skos:prefLabel "Award-evaluation-method-type" ;
.
epo:Award-type
  rdf:type skos:ConceptScheme ;
  rdfs:isDefinedBy <http://data.europa.eu/a4g/ontology> ;
  rdfs:label "Award-type"@en ;
  skos:prefLabel "Award-type" ;
.
epo:AwardCriterion
  rdf:type owl:Class ;
  rdf:type skos:Concept ;
  rdfs:comment """Describes a requirement that the tender needs to resolve and on which the tender is evaluated and ranked.

(WG approval 05/11/2018)"""@en ;
  rdfs:isDefinedBy <http://data.europa.eu/a4g/ontology> ;
  rdfs:label "Award criterion"@en ;
  rdfs:subClassOf epo:ProcurementCriterion ;
  owl:disjointWith epo:ExclusionGround ;
  owl:disjointWith epo:SelectionCriterion ;
  skos:definition """Describes a requirement that the tender needs to resolve and on which the tender is evaluated and ranked.

(WG approval 05/11/2018)"""@en ;
  skos:inScheme epo:E-evaluation-criterion-type ;
  skos:prefLabel "Award criterion"@en ;
.
epo:AwardDecision
  rdf:type owl:Class ;
  rdfs:comment """Resolution of the buyer as to the result of the procurement procedure.

(WG approval 14/11/2018)"""@en ;
  rdfs:isDefinedBy <http://data.europa.eu/a4g/ontology> ;
  rdfs:label "Award decision"@en ;
  skos:definition """Resolution of the buyer as to the result of the procurement procedure.

(WG approval 14/11/2018)"""@en ;
  skos:prefLabel "Award decision"@en ;
.
epo:AwardDimension
  rdf:type owl:Class ;
  rdfs:comment """The information needed to ponder award criteria dimensions, 
The award is computed on the basis of different several dimensions such as quality, price and cost. 
One dimension, e.g. quality, provides the information necessary to measure how the overall quality criteria will be evaluated, as opposed to the individual quality criterion (which has its own weight and threshold)."""@en ;
  rdfs:isDefinedBy <http://data.europa.eu/a4g/ontology> ;
  rdfs:label "Award dimension"@en ;
  rdfs:subClassOf epo:AwardCriterion ;
  skos:definition """The information needed to ponder award criteria dimensions, 
The award is computed on the basis of different several dimensions such as quality, price and cost. 
One dimension, e.g. quality, provides the information necessary to measure how the overall quality criteria will be evaluated, as opposed to the individual quality criterion (which has its own weight and threshold)."""@en ;
  skos:prefLabel "Award dimension"@en ;
.
epo:BDI
  rdf:type skos:Concept ;
  rdfs:isDefinedBy <http://data.europa.eu/a4g/ontology> ;
  rdfs:label "Burundi"@en ;
  skos:inScheme <http://publications.europa.eu/resource/authority/Country> ;
  skos:prefLabel "Burundi"@en ;
.
epo:BEL
  rdf:type skos:Concept ;
  rdfs:isDefinedBy <http://data.europa.eu/a4g/ontology> ;
  rdfs:label "Belgium"@en ;
  skos:inScheme <http://publications.europa.eu/resource/authority/Country> ;
  skos:prefLabel "Belgium"@en ;
.
epo:BEN
  rdf:type skos:Concept ;
  rdfs:isDefinedBy <http://data.europa.eu/a4g/ontology> ;
  rdfs:label "Benin"@en ;
  skos:inScheme <http://publications.europa.eu/resource/authority/Country> ;
  skos:prefLabel "Benin"@en ;
.
epo:BFA
  rdf:type skos:Concept ;
  rdfs:isDefinedBy <http://data.europa.eu/a4g/ontology> ;
  rdfs:label "Burkina Faso"@en ;
  skos:inScheme <http://publications.europa.eu/resource/authority/Country> ;
  skos:prefLabel "Burkina Faso"@en ;
.
epo:BGD
  rdf:type skos:Concept ;
  rdfs:isDefinedBy <http://data.europa.eu/a4g/ontology> ;
  rdfs:label "Bangladesh"@en ;
  skos:inScheme <http://publications.europa.eu/resource/authority/Country> ;
  skos:prefLabel "Bangladesh"@en ;
.
epo:BGPL
  rdf:type skos:Concept ;
  rdfs:isDefinedBy <http://data.europa.eu/a4g/ontology> ;
  rdfs:label "Body Governed by Public Law"@en ;
  skos:inScheme epo:Authority-type ;
  skos:prefLabel "Body Governed by Public Law"@en ;
.
epo:BGR
  rdf:type skos:Concept ;
  rdfs:isDefinedBy <http://data.europa.eu/a4g/ontology> ;
  rdfs:label "Bulgaria"@en ;
  skos:inScheme <http://publications.europa.eu/resource/authority/Country> ;
  skos:prefLabel "Bulgaria"@en ;
.
epo:BHR
  rdf:type skos:Concept ;
  rdfs:isDefinedBy <http://data.europa.eu/a4g/ontology> ;
  rdfs:label "Bahrain"@en ;
  skos:inScheme <http://publications.europa.eu/resource/authority/Country> ;
  skos:prefLabel "Bahrain"@en ;
.
epo:BHS
  rdf:type skos:Concept ;
  rdfs:isDefinedBy <http://data.europa.eu/a4g/ontology> ;
  rdfs:label "Bahamas"@en ;
  skos:inScheme <http://publications.europa.eu/resource/authority/Country> ;
  skos:prefLabel "Bahamas"@en ;
.
epo:BIH
  rdf:type skos:Concept ;
  rdfs:isDefinedBy <http://data.europa.eu/a4g/ontology> ;
  rdfs:label "Bosnia and Herzegovina"@en ;
  skos:inScheme <http://publications.europa.eu/resource/authority/Country> ;
  skos:prefLabel "Bosnia and Herzegovina"@en ;
.
epo:BLR
  rdf:type skos:Concept ;
  rdfs:isDefinedBy <http://data.europa.eu/a4g/ontology> ;
  rdfs:label "Belarus"@en ;
  skos:inScheme <http://publications.europa.eu/resource/authority/Country> ;
  skos:prefLabel "Belarus"@en ;
.
epo:BLZ
  rdf:type skos:Concept ;
  rdfs:isDefinedBy <http://data.europa.eu/a4g/ontology> ;
  rdfs:label "Belize"@en ;
  skos:inScheme <http://publications.europa.eu/resource/authority/Country> ;
  skos:prefLabel "Belize"@en ;
.
epo:BMU
  rdf:type skos:Concept ;
  rdfs:isDefinedBy <http://data.europa.eu/a4g/ontology> ;
  rdfs:label "Bermuda"@en ;
  skos:inScheme <http://publications.europa.eu/resource/authority/Country> ;
  skos:prefLabel "Bermuda"@en ;
.
epo:BOL
  rdf:type skos:Concept ;
  rdfs:isDefinedBy <http://data.europa.eu/a4g/ontology> ;
  rdfs:label "Bolivia"@en ;
  skos:inScheme <http://publications.europa.eu/resource/authority/Country> ;
  skos:prefLabel "Bolivia"@en ;
.
epo:BRA
  rdf:type skos:Concept ;
  rdfs:isDefinedBy <http://data.europa.eu/a4g/ontology> ;
  rdfs:label "Brazil"@en ;
  skos:inScheme <http://publications.europa.eu/resource/authority/Country> ;
  skos:prefLabel "Brazil"@en ;
.
epo:BRB
  rdf:type skos:Concept ;
  rdfs:isDefinedBy <http://data.europa.eu/a4g/ontology> ;
  rdfs:label "Barbados"@en ;
  skos:inScheme <http://publications.europa.eu/resource/authority/Country> ;
  skos:prefLabel "Barbados"@en ;
.
epo:BRN
  rdf:type skos:Concept ;
  rdfs:isDefinedBy <http://data.europa.eu/a4g/ontology> ;
  rdfs:label "Brunei Darussalam"@en ;
  skos:inScheme <http://publications.europa.eu/resource/authority/Country> ;
  skos:prefLabel "Brunei Darussalam"@en ;
.
epo:BTN
  rdf:type skos:Concept ;
  rdfs:isDefinedBy <http://data.europa.eu/a4g/ontology> ;
  rdfs:label "Bhutan"@en ;
  skos:inScheme <http://publications.europa.eu/resource/authority/Country> ;
  skos:prefLabel "Bhutan"@en ;
.
epo:BVT
  rdf:type skos:Concept ;
  rdfs:isDefinedBy <http://data.europa.eu/a4g/ontology> ;
  rdfs:label "Bouvet Island"@en ;
  skos:inScheme <http://publications.europa.eu/resource/authority/Country> ;
  skos:prefLabel "Bouvet Island"@en ;
.
epo:BWA
  rdf:type skos:Concept ;
  rdfs:isDefinedBy <http://data.europa.eu/a4g/ontology> ;
  rdfs:label "Botswana"@en ;
  skos:inScheme <http://publications.europa.eu/resource/authority/Country> ;
  skos:prefLabel "Botswana"@en ;
.
epo:BinaryObject
  rdf:type rdfs:Datatype ;
  rdfs:isDefinedBy <http://data.europa.eu/a4g/ontology> ;
  rdfs:label "Binary object"@en ;
  skos:prefLabel "Binary object"@en ;
.
epo:Body-pl
  rdf:type skos:Concept ;
  rdfs:isDefinedBy <http://data.europa.eu/a4g/ontology> ;
  rdfs:label "Body governed by public law"@en ;
  skos:inScheme <http://publications.europa.eu/resource/authority/Buyer-legal-type> ;
  skos:prefLabel "Body governed by public law"@en ;
.
epo:Body-pl-cga
  rdf:type skos:Concept ;
  rdfs:isDefinedBy <http://data.europa.eu/a4g/ontology> ;
  rdfs:label "Body governed by public law, controlled by a central government authority"@en ;
  skos:inScheme <http://publications.europa.eu/resource/authority/Buyer-legal-type> ;
  skos:prefLabel "Body governed by public law, controlled by a central government authority"@en ;
.
epo:Body-pl-la
  rdf:type skos:Concept ;
  rdfs:isDefinedBy <http://data.europa.eu/a4g/ontology> ;
  rdfs:label "Body governed by public law, controlled by a local authority"@en ;
  skos:inScheme <http://publications.europa.eu/resource/authority/Buyer-legal-type> ;
  skos:prefLabel "Body governed by public law, controlled by a local authority"@en ;
.
epo:Body-pl-ra
  rdf:type skos:Concept ;
  rdfs:isDefinedBy <http://data.europa.eu/a4g/ontology> ;
  rdfs:label "Body governed by public law, controlled by a regional authority"@en ;
  skos:inScheme <http://publications.europa.eu/resource/authority/Buyer-legal-type> ;
  skos:prefLabel "Body governed by public law, controlled by a regional authority"@en ;
.
epo:Bud-pay
  rdf:type skos:Concept ;
  rdfs:isDefinedBy <http://data.europa.eu/a4g/ontology> ;
  rdfs:label "Organisation whose budget is used to pay for the contract"@en ;
  skos:inScheme epo:Function-taxonomy ;
  skos:prefLabel "Organisation whose budget is used to pay for the contract"@en ;
.
epo:Business
  rdf:type owl:Class ;
  rdfs:comment """A private law company registered in a national registry.

WG Approval 28/04/2020

"""@en ;
  rdfs:isDefinedBy <http://data.europa.eu/a4g/ontology> ;
  rdfs:label "Business"@en ;
  rdfs:subClassOf epo:RegisteredOrganisation ;
  skos:definition """A private law company registered in a national registry.

WG Approval 28/04/2020

"""@en ;
  skos:prefLabel "Business"@en ;
.
epo:Buy-int-canc
  rdf:type skos:Concept ;
  rdfs:isDefinedBy <http://data.europa.eu/a4g/ontology> ;
  rdfs:label "The buyer intends to cancel the original notice"@en ;
  skos:inScheme epo:Notice-corrigendum-justification ;
  skos:prefLabel "The buyer intends to cancel the original notice"@en ;
.
epo:Buyer
  rdf:type owl:Class ;
  rdfs:comment """A role of an agent that awards the contract. 

Additional information:
Examples of a buyer can be the role of contracting authority, contracting entity, a defence contractor, an international organisation, or an organisation awarding a contract subsidized by a contracting authority.


WG Approval  28/04/2020"""@en ;
  rdfs:isDefinedBy <http://data.europa.eu/a4g/ontology> ;
  rdfs:label "Buyer"@en ;
  rdfs:subClassOf epo:Role ;
  owl:disjointWith epo:CentralPurchasingBody ;
  owl:disjointWith epo:EconomicOperator ;
  owl:disjointWith epo:ProcurementServiceProvider ;
  skos:definition """A role of an agent that awards the contract. 

Additional information:
Examples of a buyer can be the role of contracting authority, contracting entity, a defence contractor, an international organisation, or an organisation awarding a contract subsidized by a contracting authority.


WG Approval  28/04/2020"""@en ;
  skos:prefLabel "Buyer"@en ;
.
epo:BuyerProfile
  rdf:type owl:Class ;
  rdfs:comment """Website address where the buyer publishes information on its procurement procedures and general information.

WG approval 04/05/2018
"""@en ;
  rdfs:isDefinedBy <http://data.europa.eu/a4g/ontology> ;
  rdfs:label "Buyer profile"@en ;
  skos:definition """Website address where the buyer publishes information on its procurement procedures and general information.

WG approval 04/05/2018
"""@en ;
  skos:prefLabel "Buyer profile"@en ;
.
epo:BuyersListedAndNotListedInThisNotice
  rdf:type skos:Concept ;
  rdfs:isDefinedBy <http://data.europa.eu/a4g/ontology> ;
  rdfs:label "Buyers listed and not listed in this notice"@en ;
  skos:inScheme epo:Dps-scope ;
  skos:prefLabel "Buyers listed and not listed in this notice"@en ;
.
epo:BuyersOnlyListedInThisNotice
  rdf:type skos:Concept ;
  rdfs:isDefinedBy <http://data.europa.eu/a4g/ontology> ;
  rdfs:label "Buyers only listed in this notice"@en ;
  skos:inScheme epo:Dps-scope ;
  skos:prefLabel "Buyers only listed in this notice"@en ;
.
epo:C-dir200981EC
  rdf:type skos:Concept ;
  rdfs:isDefinedBy <http://data.europa.eu/a4g/ontology> ;
  rdfs:label "The contract falls within the services listed in Annex II of the Directive 2009/81/EC"@en ;
  skos:inScheme <http://publications.europa.eu/resource/authority/Direct-award-justification> ;
  skos:prefLabel "The contract falls within the services listed in Annex II of the Directive 2009/81/EC"@en ;
.
epo:CAF
  rdf:type skos:Concept ;
  rdfs:isDefinedBy <http://data.europa.eu/a4g/ontology> ;
  rdfs:label "Central African Republic"@en ;
  skos:inScheme <http://publications.europa.eu/resource/authority/Country> ;
  skos:prefLabel "Central African Republic"@en ;
.
epo:CALENDAR_DAY
  rdf:type skos:Concept ;
  rdfs:isDefinedBy <http://data.europa.eu/a4g/ontology> ;
  rdfs:label "Calendar Day"@en ;
  skos:inScheme <http://publications.europa.eu/resource/authority/Timeperiods> ;
  skos:prefLabel "Calendar Day"@en ;
.
epo:CAN
  rdf:type skos:Concept ;
  rdfs:isDefinedBy <http://data.europa.eu/a4g/ontology> ;
  rdfs:label "Canada"@en ;
  skos:inScheme <http://publications.europa.eu/resource/authority/Country> ;
  skos:prefLabel "Canada"@en ;
.
epo:CCK
  rdf:type skos:Concept ;
  rdfs:isDefinedBy <http://data.europa.eu/a4g/ontology> ;
  rdfs:label "Cocos (Keeling Islands)"@en ;
  skos:inScheme <http://publications.europa.eu/resource/authority/Country> ;
  skos:prefLabel "Cocos (Keeling Islands)"@en ;
.
epo:CGA
  rdf:type skos:Concept ;
  rdfs:isDefinedBy <http://data.europa.eu/a4g/ontology> ;
  rdfs:label "Central Government Authority"@en ;
  skos:inScheme epo:Authority-type ;
  skos:prefLabel "Central Government Authority"@en ;
.
epo:CHL
  rdf:type skos:Concept ;
  rdfs:isDefinedBy <http://data.europa.eu/a4g/ontology> ;
  rdfs:label "Chile"@en ;
  skos:inScheme <http://publications.europa.eu/resource/authority/Country> ;
  skos:prefLabel "Chile"@en ;
.
epo:CHN
  rdf:type skos:Concept ;
  rdfs:isDefinedBy <http://data.europa.eu/a4g/ontology> ;
  rdfs:label "China"@en ;
  skos:inScheme <http://publications.europa.eu/resource/authority/Country> ;
  skos:prefLabel "China"@en ;
.
epo:CMR
  rdf:type skos:Concept ;
  rdfs:isDefinedBy <http://data.europa.eu/a4g/ontology> ;
  rdfs:label "Cameroon"@en ;
  skos:inScheme <http://publications.europa.eu/resource/authority/Country> ;
  skos:prefLabel "Cameroon"@en ;
.
epo:COD
  rdf:type skos:Concept ;
  rdfs:isDefinedBy <http://data.europa.eu/a4g/ontology> ;
  rdfs:label "Congo (Kinshasa)"@en ;
  skos:inScheme <http://publications.europa.eu/resource/authority/Country> ;
  skos:prefLabel "Congo (Kinshasa)"@en ;
.
epo:COG
  rdf:type skos:Concept ;
  rdfs:isDefinedBy <http://data.europa.eu/a4g/ontology> ;
  rdfs:label "Congo (Brazzaville)"@en ;
  skos:inScheme <http://publications.europa.eu/resource/authority/Country> ;
  skos:prefLabel "Congo (Brazzaville)"@en ;
.
epo:COK
  rdf:type skos:Concept ;
  rdfs:isDefinedBy <http://data.europa.eu/a4g/ontology> ;
  rdfs:label "Cook Islands"@en ;
  skos:inScheme <http://publications.europa.eu/resource/authority/Country> ;
  skos:prefLabel "Cook Islands"@en ;
.
epo:COL
  rdf:type skos:Concept ;
  rdfs:isDefinedBy <http://data.europa.eu/a4g/ontology> ;
  rdfs:label "Colombia"@en ;
  skos:inScheme <http://publications.europa.eu/resource/authority/Country> ;
  skos:prefLabel "Colombia"@en ;
.
epo:COM
  rdf:type skos:Concept ;
  rdfs:isDefinedBy <http://data.europa.eu/a4g/ontology> ;
  rdfs:label "Comoros"@en ;
  skos:inScheme <http://publications.europa.eu/resource/authority/Country> ;
  skos:prefLabel "Comoros"@en ;
.
epo:COMPETITIONCN
  rdf:type skos:Concept ;
  rdfs:isDefinedBy <http://data.europa.eu/a4g/ontology> ;
  rdfs:label "C o m p e t i t i o n c n"@en ;
  skos:inScheme epo:Notification-phases-content-types ;
  skos:prefLabel "C o m p e t i t i o n c n"@en ;
.
epo:COMPETITIONPIN
  rdf:type skos:Concept ;
  rdfs:isDefinedBy <http://data.europa.eu/a4g/ontology> ;
  rdfs:label "C o m p e t i t i o n p i n"@en ;
  skos:inScheme epo:Notification-phases-content-types ;
  skos:prefLabel "C o m p e t i t i o n p i n"@en ;
.
epo:COMPETITIONQS
  rdf:type skos:Concept ;
  rdfs:isDefinedBy <http://data.europa.eu/a4g/ontology> ;
  rdfs:label "C o m p e t i t i o n q s"@en ;
  skos:inScheme epo:Notification-phases-content-types ;
  skos:prefLabel "C o m p e t i t i o n q s"@en ;
.
epo:CONFIDENTIAL
  rdf:type skos:Concept ;
  rdfs:isDefinedBy <http://data.europa.eu/a4g/ontology> ;
  rdfs:label "Information and material the unauthorised disclosure of which could harm the essential interests of the European Union, of one or more of the Member States or of one or more parties participating in a Procedure."@en ;
  skos:inScheme <https://github.com/ESPD/ESPD-EDM/Confidentiality-level> ;
  skos:prefLabel "Information and material the unauthorised disclosure of which could harm the essential interests of the European Union, of one or more of the Member States or of one or more parties participating in a Procedure."@en ;
.
epo:CONSORTIUM
  rdf:type skos:Concept ;
  rdfs:isDefinedBy <http://data.europa.eu/a4g/ontology> ;
  rdfs:label "Consortium"@en ;
  skos:inScheme epo:Eo-group-type ;
  skos:prefLabel "Consortium"@en ;
.
epo:CONTRACTCM
  rdf:type skos:Concept ;
  rdfs:isDefinedBy <http://data.europa.eu/a4g/ontology> ;
  rdfs:label "C o n t r a c t c m"@en ;
  skos:inScheme epo:Notification-phases-content-types ;
  skos:prefLabel "C o n t r a c t c m"@en ;
.
epo:CONTRACTOR
  rdf:type skos:Concept ;
  rdfs:isDefinedBy <http://data.europa.eu/a4g/ontology> ;
  rdfs:label "C o n t r a c t o r"@en ;
  skos:inScheme epo:Security-clearance-address ;
  skos:prefLabel "C o n t r a c t o r"@en ;
.
epo:COST
  rdf:type skos:Concept ;
  rdfs:isDefinedBy <http://data.europa.eu/a4g/ontology> ;
  rdfs:label "C o s t"@en ;
  skos:inScheme epo:Award-dimension-parent-criterion-relation ;
  skos:prefLabel "C o s t"@en ;
.
epo:CPV
  rdf:type skos:Concept ;
  rdfs:isDefinedBy <http://data.europa.eu/a4g/ontology> ;
  rdfs:label "Cape Verde"@en ;
  skos:inScheme <http://publications.europa.eu/resource/authority/Country> ;
  skos:prefLabel "Cape Verde"@en ;
.
epo:CRITERIONAWARDLOWEST
  rdf:type skos:Concept ;
  rdfs:isDefinedBy <http://data.europa.eu/a4g/ontology> ;
  rdfs:label "C r i t e r i o n a w a r d l o w e s t"@en ;
  skos:inScheme epo:Award-evaluation-method-type ;
  skos:prefLabel "C r i t e r i o n a w a r d l o w e s t"@en ;
.
epo:CRITERIONAWARDMIXED
  rdf:type skos:Concept ;
  rdfs:isDefinedBy <http://data.europa.eu/a4g/ontology> ;
  rdfs:label "C r i t e r i o n a w a r d m i x e d"@en ;
  skos:inScheme epo:Award-evaluation-method-type ;
  skos:prefLabel "C r i t e r i o n a w a r d m i x e d"@en ;
.
epo:CRITERIONAWARDMOST_ECONOMIC_TENDER
  rdf:type skos:Concept ;
  rdfs:isDefinedBy <http://data.europa.eu/a4g/ontology> ;
  rdfs:label "C r i t e r i o n a w a r d m o s t_ e c o n o m i c_ t e n d e r"@en ;
  skos:inScheme epo:Award-evaluation-method-type ;
  skos:prefLabel "C r i t e r i o n a w a r d m o s t_ e c o n o m i c_ t e n d e r"@en ;
.
epo:CRITERIONAWARDOTHER
  rdf:type skos:Concept ;
  rdfs:isDefinedBy <http://data.europa.eu/a4g/ontology> ;
  rdfs:label "C r i t e r i o n a w a r d o t h e r"@en ;
  skos:inScheme epo:Award-evaluation-method-type ;
  skos:prefLabel "C r i t e r i o n a w a r d o t h e r"@en ;
.
epo:CRITERIONEXCLUSIONMISCONDUCTMC_PROFESSIONAL
  rdf:type skos:Concept ;
  rdfs:isDefinedBy <http://data.europa.eu/a4g/ontology> ;
  rdfs:label "C r i t e r i o n e x c l u s i o n m i s c o n d u c t m c_ p r o f e s s i o n a l"@en ;
  skos:inScheme epo:Award-evaluation-method-type ;
  skos:prefLabel "C r i t e r i o n e x c l u s i o n m i s c o n d u c t m c_ p r o f e s s i o n a l"@en ;
.
epo:CRITERIONSELECTIONECONOMIC_FINANCIAL_STANDINGTURNOVERGENERAL_YEARLY
  rdf:type skos:Concept ;
  rdfs:isDefinedBy <http://data.europa.eu/a4g/ontology> ;
  rdfs:label "C r i t e r i o n s e l e c t i o n e c o n o m i c_ f i n a n c i a l_ s t a n d i n g t u r n o v e r g e n e r a l_ y e a r l y"@en ;
  skos:inScheme epo:Award-evaluation-method-type ;
  skos:prefLabel "C r i t e r i o n s e l e c t i o n e c o n o m i c_ f i n a n c i a l_ s t a n d i n g t u r n o v e r g e n e r a l_ y e a r l y"@en ;
.
epo:CXR
  rdf:type skos:Concept ;
  rdfs:isDefinedBy <http://data.europa.eu/a4g/ontology> ;
  rdfs:label "Christmas Island"@en ;
  skos:inScheme <http://publications.europa.eu/resource/authority/Country> ;
  skos:prefLabel "Christmas Island"@en ;
.
epo:CYM
  rdf:type skos:Concept ;
  rdfs:isDefinedBy <http://data.europa.eu/a4g/ontology> ;
  rdfs:label "Cayman Islands"@en ;
  skos:inScheme <http://publications.europa.eu/resource/authority/Country> ;
  skos:prefLabel "Cayman Islands"@en ;
.
epo:CallForCompetition
  rdf:type owl:Class ;
  rdfs:comment """A public announcement of the launch of a procurement procedure.

(WG approval 14/05/2017)"""@en ;
  rdfs:isDefinedBy <http://data.europa.eu/a4g/ontology> ;
  rdfs:label "Call for competition"@en ;
  rdfs:subClassOf epo:ProcurementDocument ;
  owl:disjointWith epo:AdditionalDocument ;
  owl:disjointWith epo:ContractTemplate ;
  owl:disjointWith epo:DescriptiveDocument ;
  owl:disjointWith epo:DraftCV ;
  owl:disjointWith epo:ESPDRequest ;
  owl:disjointWith epo:InvitationToTender ;
  owl:disjointWith epo:PreAwardCatalogueRequest ;
  owl:disjointWith epo:TechnicalSpecifications ;
  skos:definition """A public announcement of the launch of a procurement procedure.

(WG approval 14/05/2017)"""@en ;
  skos:prefLabel "Call for competition"@en ;
.
epo:CallForExpressionOfInterest
  rdf:type owl:Class ;
  rdfs:comment """A call to potential providers of goods and/or services to register interest in supplying them. It is a document that describes a set of requirements or specifications and that service providers have to demonstrate their ability to meet those requirements. 
"""@en ;
  rdfs:isDefinedBy <http://data.europa.eu/a4g/ontology> ;
  rdfs:label "Call for expression of interest"@en ;
  rdfs:subClassOf epo:Notice ;
  owl:disjointWith epo:ContractAwardNotice ;
  owl:disjointWith epo:ContractModificationNotice ;
  owl:disjointWith epo:ContractNotice ;
  owl:disjointWith epo:PriorInformationNotice ;
  owl:disjointWith epo:VoluntaryEx-anteTransparencyNotice ;
  skos:definition """A call to potential providers of goods and/or services to register interest in supplying them. It is a document that describes a set of requirements or specifications and that service providers have to demonstrate their ability to meet those requirements. 
"""@en ;
  skos:prefLabel "Call for expression of interest"@en ;
.
epo:CandidateShortList
  rdf:type owl:Class ;
  rdfs:comment """The tenderers that have been selected in a two stage procedure.

Additional information: the types of procedures this shortlist applies to are restricted procedures, competitive procedures with negotiation, competitive dialogue procedures and innovation partnerships.

(WG approval 27/07/2018)"""@en ;
  rdfs:isDefinedBy <http://data.europa.eu/a4g/ontology> ;
  rdfs:label "Candidate short list"@en ;
  rdfs:subClassOf epo:EconomicOperatorShortList ;
  skos:definition """The tenderers that have been selected in a two stage procedure.

Additional information: the types of procedures this shortlist applies to are restricted procedures, competitive procedures with negotiation, competitive dialogue procedures and innovation partnerships.

(WG approval 27/07/2018)"""@en ;
  skos:prefLabel "Candidate short list"@en ;
.
epo:CentralPurchasingBody
  rdf:type owl:Class ;
  rdfs:comment """Role of a contracting authority that provides centralised purchasing activities and, possibly, ancillary purchasing activities for other procuring entities.

WG approval 18/05/2018

Contracting authority procuring activities conducted on a permanent basis, in one of the following forms:(a) the acquisition of supplies and/or services intended for contracting authorities.

Contracting authority procuring activities conducted on a permanent basis, in one of the following forms:[...](b) the award of public contracts or the conclusion of framework agreements for works, supplies or services intended for contracting authorities;"""@en ;
  rdfs:isDefinedBy <http://data.europa.eu/a4g/ontology> ;
  rdfs:label "Central purchasing body"@en ;
  rdfs:subClassOf epo:Role ;
  owl:disjointWith epo:Buyer ;
  owl:disjointWith epo:EconomicOperator ;
  owl:disjointWith epo:ProcurementServiceProvider ;
  skos:definition """Role of a contracting authority that provides centralised purchasing activities and, possibly, ancillary purchasing activities for other procuring entities.

WG approval 18/05/2018

Contracting authority procuring activities conducted on a permanent basis, in one of the following forms:(a) the acquisition of supplies and/or services intended for contracting authorities.

Contracting authority procuring activities conducted on a permanent basis, in one of the following forms:[...](b) the award of public contracts or the conclusion of framework agreements for works, supplies or services intended for contracting authorities;"""@en ;
  skos:prefLabel "Central purchasing body"@en ;
.
epo:Cga
  rdf:type skos:Concept ;
  rdfs:isDefinedBy <http://data.europa.eu/a4g/ontology> ;
  rdfs:label "Central government authority"@en ;
  skos:inScheme <http://publications.europa.eu/resource/authority/Buyer-legal-type> ;
  skos:prefLabel "Central government authority"@en ;
.
epo:Chan-need
  rdf:type skos:Concept ;
  rdfs:isDefinedBy <http://data.europa.eu/a4g/ontology> ;
  rdfs:label "Decision of the buyer, because of a change in needs"@en ;
  skos:inScheme <http://publications.europa.eu/resource/authority/Non-award-justification> ;
  skos:prefLabel "Decision of the buyer, because of a change in needs"@en ;
.
epo:Change
  rdf:type owl:Class ;
  rdf:type skos:Concept ;
  rdfs:comment """Update of information.

WG Approval 5/11/2019"""@en ;
  rdfs:isDefinedBy <http://data.europa.eu/a4g/ontology> ;
  rdfs:label "Change"@en ;
  skos:definition """Update of information.

WG Approval 5/11/2019"""@en ;
  skos:inScheme epo:Form-type ;
  skos:prefLabel "Change"@en ;
.
epo:Channel
  rdf:type owl:Class ;
  rdfs:comment """Software solutions and electronic devices for communication and exchange of information between buyers and economic operators.

Additional Information

Lots may use ad-hoc electronic means of communication that are not generally available such as specific solutions for secure and dedicated communication or non-standard eCatalogues. 

See also Directive recitals 53 to 56.

WG Suggestion to eForms 30/09/2019


"""@en ;
  rdfs:isDefinedBy <http://data.europa.eu/a4g/ontology> ;
  rdfs:label "Channel"@en ;
  skos:definition """Software solutions and electronic devices for communication and exchange of information between buyers and economic operators.

Additional Information

Lots may use ad-hoc electronic means of communication that are not generally available such as specific solutions for secure and dedicated communication or non-standard eCatalogues. 

See also Directive recitals 53 to 56.

WG Suggestion to eForms 30/09/2019


"""@en ;
  skos:prefLabel "Channel"@en ;
.
epo:Clos-nw
  rdf:type skos:Concept ;
  rdfs:isDefinedBy <http://data.europa.eu/a4g/ontology> ;
  rdfs:label "No winner was chosen and the competition is closed"@en ;
  skos:inScheme <http://publications.europa.eu/resource/authority/Winner-selection-status> ;
  skos:prefLabel "No winner was chosen and the competition is closed"@en ;
.
epo:Code
  rdf:type rdfs:Datatype ;
  rdf:type owl:Class ;
  rdfs:isDefinedBy <http://data.europa.eu/a4g/ontology> ;
  rdfs:label "Code"@en ;
  rdfs:subClassOf <http://www.unece.org/cefact#Code> ;
  skos:prefLabel "Code"@en ;
.
epo:Com-eco-ope
  rdf:type skos:Concept ;
  rdfs:isDefinedBy <http://data.europa.eu/a4g/ontology> ;
  rdfs:label "Commercial interests of an economic operator"@en ;
  skos:inScheme <http://publications.europa.eu/resource/authority/Non-publication-justification> ;
  skos:prefLabel "Commercial interests of an economic operator"@en ;
.
epo:Communication-type
  rdf:type skos:ConceptScheme ;
  rdfs:isDefinedBy <http://data.europa.eu/a4g/ontology> ;
  rdfs:label "Communication-type"@en ;
  skos:prefLabel "Communication-type" ;
.
epo:Comp
  rdf:type skos:Concept ;
  rdfs:isDefinedBy <http://data.europa.eu/a4g/ontology> ;
  rdfs:label "Competition"@en ;
  skos:inScheme epo:Form-type ;
  skos:prefLabel "Competition"@en ;
.
epo:Comp-dial
  rdf:type skos:Concept ;
  rdfs:isDefinedBy <http://data.europa.eu/a4g/ontology> ;
  rdfs:label "Competitive dialogue"@en ;
  skos:inScheme <http://publications.europa.eu/resource/authority/Procurement-procedure-type> ;
  skos:prefLabel "Competitive dialogue"@en ;
.
epo:ConflictOfInterest
  rdf:type owl:Class ;
  rdfs:isDefinedBy <http://data.europa.eu/a4g/ontology> ;
  rdfs:label "Conflict of interest"@en ;
  rdfs:subClassOf epo:ExclusionGround ;
  skos:prefLabel "Conflict of interest"@en ;
.
epo:Cont-arm-dir
  rdf:type skos:Concept ;
  rdfs:isDefinedBy <http://data.europa.eu/a4g/ontology> ;
  rdfs:label "Contract related to the provision of air and maritime transport services for the armed forces of a Member State deployed or to be deployed abroad, under the strict conditions stated in the Directive"@en ;
  skos:inScheme <http://publications.europa.eu/resource/authority/Direct-award-justification> ;
  skos:prefLabel "Contract related to the provision of air and maritime transport services for the armed forces of a Member State deployed or to be deployed abroad, under the strict conditions stated in the Directive"@en ;
.
epo:Cont-modif
  rdf:type skos:Concept ;
  rdfs:isDefinedBy <http://data.europa.eu/a4g/ontology> ;
  rdfs:label "Contract modification"@en ;
  skos:inScheme epo:Form-type ;
  skos:prefLabel "Contract modification"@en ;
.
epo:ContactPoint
  rdf:type owl:Class ;
  rdfs:comment """Details used to reach an organisation.

Additional information: 

The contact point could be a role, email address, telephone number, etc.

WG approval 5/11/2019"""@en ;
  rdfs:isDefinedBy <http://data.europa.eu/a4g/ontology> ;
  rdfs:label "Contact point"@en ;
  skos:definition """Details used to reach an organisation.

Additional information: 

The contact point could be a role, email address, telephone number, etc.

WG approval 5/11/2019"""@en ;
  skos:prefLabel "Contact point"@en ;
.
epo:Contract
  rdf:type owl:Class ;
  rdfs:comment """A voluntary, deliberate, and legally binding agreement between two or more competent parties.

(WG approval 01/06/2018)"""@en ;
  rdfs:isDefinedBy <http://data.europa.eu/a4g/ontology> ;
  rdfs:label "Contract"@en ;
  rdfs:subClassOf epo:Document ;
  owl:disjointWith epo:Notice ;
  owl:disjointWith epo:ProcurementDocument ;
  owl:disjointWith epo:RequestForParticipation ;
  owl:disjointWith epo:TenderDocument ;
  skos:definition """A voluntary, deliberate, and legally binding agreement between two or more competent parties.

(WG approval 01/06/2018)"""@en ;
  skos:prefLabel "Contract"@en ;
.
epo:ContractAwardNotice
  rdf:type owl:Class ;
  rdfs:comment """An announcement of the award or non-award of a contract by a procuring entity.

(WG approval 27/03/2019 9:41:42)"""@en ;
  rdfs:isDefinedBy <http://data.europa.eu/a4g/ontology> ;
  rdfs:label "Contract award notice"@en ;
  rdfs:subClassOf epo:Notice ;
  owl:disjointWith epo:CallForExpressionOfInterest ;
  owl:disjointWith epo:ContractModificationNotice ;
  owl:disjointWith epo:ContractNotice ;
  owl:disjointWith epo:PriorInformationNotice ;
  owl:disjointWith epo:VoluntaryEx-anteTransparencyNotice ;
  skos:definition """An announcement of the award or non-award of a contract by a procuring entity.

(WG approval 27/03/2019 9:41:42)"""@en ;
  skos:prefLabel "Contract award notice"@en ;
.
epo:ContractModificationNotice
  rdf:type owl:Class ;
  rdfs:comment """An announcement of the modification of a contract/concession during during its term by a procuring entity.

"""@en ;
  rdfs:isDefinedBy <http://data.europa.eu/a4g/ontology> ;
  rdfs:label "Contract modification notice"@en ;
  rdfs:subClassOf epo:Notice ;
  owl:disjointWith epo:CallForExpressionOfInterest ;
  owl:disjointWith epo:ContractAwardNotice ;
  owl:disjointWith epo:ContractNotice ;
  owl:disjointWith epo:PriorInformationNotice ;
  owl:disjointWith epo:VoluntaryEx-anteTransparencyNotice ;
  skos:definition """An announcement of the modification of a contract/concession during during its term by a procuring entity.

"""@en ;
  skos:prefLabel "Contract modification notice"@en ;
.
epo:ContractNotice
  rdf:type owl:Class ;
  rdfs:comment """An announcement of the launch of a procurement procedure by a procuring entity.

(WG approval 18/05/2018)"""@en ;
  rdfs:isDefinedBy <http://data.europa.eu/a4g/ontology> ;
  rdfs:label "Contract notice"@en ;
  rdfs:subClassOf epo:Notice ;
  owl:disjointWith epo:CallForExpressionOfInterest ;
  owl:disjointWith epo:ContractAwardNotice ;
  owl:disjointWith epo:ContractModificationNotice ;
  owl:disjointWith epo:PriorInformationNotice ;
  owl:disjointWith epo:VoluntaryEx-anteTransparencyNotice ;
  skos:definition """An announcement of the launch of a procurement procedure by a procuring entity.

(WG approval 18/05/2018)"""@en ;
  skos:prefLabel "Contract notice"@en ;
.
epo:ContractTemplate
  rdf:type owl:Class ;
  rdfs:isDefinedBy <http://data.europa.eu/a4g/ontology> ;
  rdfs:label "Contract template"@en ;
  rdfs:subClassOf epo:ProcurementDocument ;
  owl:disjointWith epo:AdditionalDocument ;
  owl:disjointWith epo:CallForCompetition ;
  owl:disjointWith epo:DescriptiveDocument ;
  owl:disjointWith epo:DraftCV ;
  owl:disjointWith epo:ESPDRequest ;
  owl:disjointWith epo:InvitationToTender ;
  owl:disjointWith epo:PreAwardCatalogueRequest ;
  owl:disjointWith epo:TechnicalSpecifications ;
  skos:prefLabel "Contract template"@en ;
.
epo:ContractTerms
  rdf:type owl:Class ;
  rdfs:comment """Conditions and stipulations defining particularities of the post award phase.

(WG approval 23/11/2018)
"""@en ;
  rdfs:isDefinedBy <http://data.europa.eu/a4g/ontology> ;
  rdfs:label "Contract terms"@en ;
  skos:definition """Conditions and stipulations defining particularities of the post award phase.

(WG approval 23/11/2018)
"""@en ;
  skos:prefLabel "Contract terms"@en ;
.
epo:Contractor
  rdf:type owl:Class ;
  rdfs:isDefinedBy <http://data.europa.eu/a4g/ontology> ;
  rdfs:label "Contractor"@en ;
  rdfs:subClassOf epo:Winner ;
  skos:prefLabel "Contractor"@en ;
.
epo:Cor-one-more
  rdf:type skos:Concept ;
  rdfs:isDefinedBy <http://data.europa.eu/a4g/ontology> ;
  rdfs:label "Correction of one or more mistakes"@en ;
  skos:inScheme epo:Notice-corrigendum-justification ;
  skos:prefLabel "Correction of one or more mistakes"@en ;
.
epo:Cor-pub-err
  rdf:type skos:Concept ;
  rdfs:isDefinedBy <http://data.europa.eu/a4g/ontology> ;
  rdfs:label "Correction of a publication error"@en ;
  skos:inScheme epo:Notice-corrigendum-justification ;
  skos:prefLabel "Correction of a publication error"@en ;
.
epo:Cost
  rdf:type skos:Concept ;
  rdfs:isDefinedBy <http://data.europa.eu/a4g/ontology> ;
  rdfs:label "Cost"@en ;
  skos:inScheme <http://publications.europa.eu/resource/authority/Award-criterion-type> ;
  skos:prefLabel "Cost"@en ;
.
epo:CountryIdentification
  rdf:type owl:Class ;
  rdfs:comment """A country is one of the political units which the world is divided into, covering a particular area of land.

WG approval  08/06/2018"""@en ;
  rdfs:isDefinedBy <http://data.europa.eu/a4g/ontology> ;
  rdfs:label "Country identification"@en ;
  skos:definition """A country is one of the political units which the world is divided into, covering a particular area of land.

WG approval  08/06/2018"""@en ;
  skos:prefLabel "Country identification"@en ;
.
epo:DAPVEAT
  rdf:type skos:Concept ;
  rdfs:isDefinedBy <http://data.europa.eu/a4g/ontology> ;
  rdfs:label "D a p v e a t"@en ;
  skos:inScheme epo:Notification-phases-content-types ;
  skos:prefLabel "D a p v e a t"@en ;
.
epo:DAY
  rdf:type skos:Concept ;
  rdfs:isDefinedBy <http://data.europa.eu/a4g/ontology> ;
  rdfs:label "(_S|Day)(_P|Days)"@en ;
  skos:inScheme <http://publications.europa.eu/resource/authority/Timeperiods> ;
  skos:prefLabel "(_S|Day)(_P|Days)"@en ;
.
epo:DEC
  rdf:type skos:Concept ;
  rdfs:isDefinedBy <http://data.europa.eu/a4g/ontology> ;
  rdfs:label "December"@en ;
  skos:inScheme <http://publications.europa.eu/resource/authority/Timeperiods> ;
  skos:prefLabel "December"@en ;
.
epo:DESIGN_CONTEST
  rdf:type skos:Concept ;
  rdfs:isDefinedBy <http://data.europa.eu/a4g/ontology> ;
  rdfs:label "Design contest"@en ;
  skos:inScheme epo:Procurement-regime-type ;
  skos:prefLabel "Design contest"@en ;
.
epo:DZA
  rdf:type skos:Concept ;
  rdfs:isDefinedBy <http://data.europa.eu/a4g/ontology> ;
  rdfs:label "Algeria"@en ;
  skos:inScheme <http://publications.europa.eu/resource/authority/Country> ;
  skos:prefLabel "Algeria"@en ;
.
epo:Date
  rdf:type rdfs:Datatype ;
  rdfs:isDefinedBy <http://data.europa.eu/a4g/ontology> ;
  rdfs:label "Date"@en ;
  skos:prefLabel "Date"@en ;
.
epo:DateTime
  rdf:type rdfs:Datatype ;
  rdfs:isDefinedBy <http://data.europa.eu/a4g/ontology> ;
  rdfs:label "Date time"@en ;
  skos:prefLabel "Date time"@en ;
.
epo:Def-cont
  rdf:type skos:Concept ;
  rdfs:isDefinedBy <http://data.europa.eu/a4g/ontology> ;
  rdfs:label "Defence contractor"@en ;
  skos:inScheme <http://publications.europa.eu/resource/authority/Buyer-legal-type> ;
  skos:prefLabel "Defence contractor"@en ;
.
epo:Des-con-awa
  rdf:type skos:Concept ;
  rdfs:isDefinedBy <http://data.europa.eu/a4g/ontology> ;
  rdfs:label "Service contract to be awarded to the winner or one of winners under the rules of a design contest"@en ;
  skos:inScheme <http://publications.europa.eu/resource/authority/Direct-award-justification> ;
  skos:prefLabel "Service contract to be awarded to the winner or one of winners under the rules of a design contest"@en ;
.
epo:Description
  rdf:type rdfs:Datatype ;
  rdf:type owl:Class ;
  rdfs:isDefinedBy <http://data.europa.eu/a4g/ontology> ;
  rdfs:label "Description"@en ;
  skos:prefLabel "Description"@en ;
.
epo:DescriptiveDocument
  rdf:type owl:Class ;
  rdfs:comment """Describes the object of the procurement and the properties of the procedure.
"""@en ;
  rdfs:isDefinedBy <http://data.europa.eu/a4g/ontology> ;
  rdfs:label "Descriptive document"@en ;
  rdfs:subClassOf epo:ProcurementDocument ;
  owl:disjointWith epo:AdditionalDocument ;
  owl:disjointWith epo:CallForCompetition ;
  owl:disjointWith epo:ContractTemplate ;
  owl:disjointWith epo:DraftCV ;
  owl:disjointWith epo:ESPDRequest ;
  owl:disjointWith epo:InvitationToTender ;
  owl:disjointWith epo:PreAwardCatalogueRequest ;
  owl:disjointWith epo:TechnicalSpecifications ;
  skos:definition """Describes the object of the procurement and the properties of the procedure.
"""@en ;
  skos:prefLabel "Descriptive document"@en ;
.
epo:Design-contest
  rdf:type skos:Concept ;
  rdfs:isDefinedBy <http://data.europa.eu/a4g/ontology> ;
  rdfs:label "Set of principles and rules specific of design-contests"@en ;
  skos:inScheme epo:Legal-regime ;
  skos:prefLabel "Set of principles and rules specific of design-contests"@en ;
.
epo:Design-contest-type
  rdf:type skos:ConceptScheme ;
  rdfs:isDefinedBy <http://data.europa.eu/a4g/ontology> ;
  rdfs:label "Design-contest-type"@en ;
  skos:prefLabel "Design-contest-type" ;
.
epo:DesignContestRegimeTerms
  rdf:type owl:Class ;
  rdfs:comment """Any service contract following the contest awarded to one of the winners. 

Additional information:"""@en ;
  rdfs:isDefinedBy <http://data.europa.eu/a4g/ontology> ;
  rdfs:label "Design contest regime terms"@en ;
  skos:definition """Any service contract following the contest awarded to one of the winners. 

Additional information:"""@en ;
  skos:prefLabel "Design contest regime terms"@en ;
.
epo:Dir-awa-pre
  rdf:type skos:Concept ;
  rdfs:isDefinedBy <http://data.europa.eu/a4g/ontology> ;
  rdfs:label "Direct award preannouncement"@en ;
  skos:inScheme epo:Form-type ;
  skos:prefLabel "Direct award preannouncement"@en ;
.
epo:Direct
  rdf:type skos:Concept ;
  rdfs:isDefinedBy <http://data.europa.eu/a4g/ontology> ;
  rdfs:label "Direct"@en ;
  skos:inScheme epo:Communication-type ;
  skos:prefLabel "Direct"@en ;
.
epo:DirectAwardTerms
  rdf:type owl:Class ;
  rdfs:comment """Conditions and stipulations defining particularities of the award of a contract without prior publication.

Addtional Information:

Direct award may refer to a previous procedure and/or specific Lot(s).

It may also refer to other justified situations whereby there is no previous procedure.

See Directive 2014/24/EU Article 32.

WG Approval 22/11/2019


"""@en ;
  rdfs:isDefinedBy <http://data.europa.eu/a4g/ontology> ;
  rdfs:label "Direct award terms"@en ;
  skos:definition """Conditions and stipulations defining particularities of the award of a contract without prior publication.

Addtional Information:

Direct award may refer to a previous procedure and/or specific Lot(s).

It may also refer to other justified situations whereby there is no previous procedure.

See Directive 2014/24/EU Article 32.

WG Approval 22/11/2019


"""@en ;
  skos:prefLabel "Direct award terms"@en ;
.
epo:Document
  rdf:type owl:Class ;
  rdfs:comment """A set of interrelated Business Information representing the business facts.

Additional Information:
Documents may convey information in any language, medium or form, including textual, numerical, graphic, cartographic, audio-visual forms, etc.

WG Approval 23/05/2019
"""@en ;
  rdfs:isDefinedBy <http://data.europa.eu/a4g/ontology> ;
  rdfs:label "Document"@en ;
  skos:definition """A set of interrelated Business Information representing the business facts.

Additional Information:
Documents may convey information in any language, medium or form, including textual, numerical, graphic, cartographic, audio-visual forms, etc.

WG Approval 23/05/2019
"""@en ;
  skos:prefLabel "Document"@en ;
.
epo:Dps-list
  rdf:type skos:Concept ;
  rdfs:isDefinedBy <http://data.europa.eu/a4g/ontology> ;
  rdfs:label "Dynamic purchasing system, only usable by buyers listed in this notice"@en ;
  skos:inScheme <http://publications.europa.eu/resource/authority/Dps-usage> ;
  skos:prefLabel "Dynamic purchasing system, only usable by buyers listed in this notice"@en ;
.
epo:Dps-nlist
  rdf:type skos:Concept ;
  rdfs:isDefinedBy <http://data.europa.eu/a4g/ontology> ;
  rdfs:label "Dynamic purchasing system, also usable by buyers not listed in this notice"@en ;
  skos:inScheme <http://publications.europa.eu/resource/authority/Dps-usage> ;
  skos:prefLabel "Dynamic purchasing system, also usable by buyers not listed in this notice"@en ;
.
epo:Dps-scope
  rdf:type skos:ConceptScheme ;
  rdfs:isDefinedBy <http://data.europa.eu/a4g/ontology> ;
  rdfs:label "Dps-scope"@en ;
  skos:prefLabel "Dps-scope" ;
.
epo:DraftCV
  rdf:type owl:Class ;
  rdfs:isDefinedBy <http://data.europa.eu/a4g/ontology> ;
  rdfs:label "Draft c v"@en ;
  rdfs:subClassOf epo:ProcurementDocument ;
  owl:disjointWith epo:AdditionalDocument ;
  owl:disjointWith epo:CallForCompetition ;
  owl:disjointWith epo:ContractTemplate ;
  owl:disjointWith epo:DescriptiveDocument ;
  owl:disjointWith epo:ESPDRequest ;
  owl:disjointWith epo:InvitationToTender ;
  owl:disjointWith epo:PreAwardCatalogueRequest ;
  owl:disjointWith epo:TechnicalSpecifications ;
  skos:prefLabel "Draft c v"@en ;
.
epo:DynamicPurchaseSystemTechnique
  rdf:type owl:Class ;
  rdfs:comment """An electronic system that is set up by a procuring entity which lists the economic operators that satisfy the selection and exclusion criteria.   This technique then allows the purchase via consultation of the listed tenderers using award criteria.

(WG approval 13/07/2018)"""@en ;
  rdfs:isDefinedBy <http://data.europa.eu/a4g/ontology> ;
  rdfs:label "Dynamic purchase system technique"@en ;
  rdfs:subClassOf epo:Technique ;
  owl:disjointWith epo:EAuctionTechnique ;
  owl:disjointWith epo:FrameworkAgreementTechnique ;
  skos:definition """An electronic system that is set up by a procuring entity which lists the economic operators that satisfy the selection and exclusion criteria.   This technique then allows the purchase via consultation of the listed tenderers using award criteria.

(WG approval 13/07/2018)"""@en ;
  skos:prefLabel "Dynamic purchase system technique"@en ;
.
epo:E-evaluation-criterion-type
  rdf:type skos:ConceptScheme ;
  rdfs:isDefinedBy <http://data.europa.eu/a4g/ontology> ;
  rdfs:label "E-evaluation-criterion-type"@en ;
  skos:prefLabel "E-evaluation-criterion-type" ;
.
epo:EAuctionTechnique
  rdf:type owl:Class ;
  rdfs:comment """A repetitive technique in which new prices, revised downwards, and/or new values concerning certain elements of tenders are bid on-line.

(WG approval 20/07/2018)"""@en ;
  rdfs:isDefinedBy <http://data.europa.eu/a4g/ontology> ;
  rdfs:label "E auction technique"@en ;
  rdfs:subClassOf epo:Technique ;
  owl:disjointWith epo:DynamicPurchaseSystemTechnique ;
  owl:disjointWith epo:FrameworkAgreementTechnique ;
  skos:definition """A repetitive technique in which new prices, revised downwards, and/or new values concerning certain elements of tenders are bid on-line.

(WG approval 20/07/2018)"""@en ;
  skos:prefLabel "E auction technique"@en ;
.
epo:ECONOMIC_OPERATOR
  rdf:type skos:Concept ;
  rdfs:isDefinedBy <http://data.europa.eu/a4g/ontology> ;
  rdfs:label "E c o n o m i c_ o p e r a t o r"@en ;
  skos:inScheme epo:Security-clearance-address ;
  skos:prefLabel "E c o n o m i c_ o p e r a t o r"@en ;
.
epo:ECatalogue
  rdf:type owl:Class ;
  rdfs:comment """Structured electronic format which allows for  automatic and electronic processing of listed information regarding goods and services.

(WG approval 10/08/2018)"""@en ;
  rdfs:isDefinedBy <http://data.europa.eu/a4g/ontology> ;
  rdfs:label "E catalogue"@en ;
  skos:definition """Structured electronic format which allows for  automatic and electronic processing of listed information regarding goods and services.

(WG approval 10/08/2018)"""@en ;
  skos:prefLabel "E catalogue"@en ;
.
epo:ESPDRequest
  rdf:type owl:Class ;
  rdfs:comment "European Single Procurement Document Request. Specification by the Procuring Entity of the exclusion and selection criteria for a Procurement Procedure. "@en ;
  rdfs:isDefinedBy <http://data.europa.eu/a4g/ontology> ;
  rdfs:label "E s p d request"@en ;
  rdfs:subClassOf epo:ProcurementDocument ;
  owl:disjointWith epo:AdditionalDocument ;
  owl:disjointWith epo:CallForCompetition ;
  owl:disjointWith epo:ContractTemplate ;
  owl:disjointWith epo:DescriptiveDocument ;
  owl:disjointWith epo:DraftCV ;
  owl:disjointWith epo:InvitationToTender ;
  owl:disjointWith epo:PreAwardCatalogueRequest ;
  owl:disjointWith epo:TechnicalSpecifications ;
  skos:definition "European Single Procurement Document Request. Specification by the Procuring Entity of the exclusion and selection criteria for a Procurement Procedure. "@en ;
  skos:prefLabel "E s p d request"@en ;
.
epo:ESPDResponse
  rdf:type owl:Class ;
  rdfs:comment "European Single Procurement Document Response. The declaration of the Economic Operator that it meets all the exclusion and selection criteria specified in the ESPD Request."@en ;
  rdfs:isDefinedBy <http://data.europa.eu/a4g/ontology> ;
  rdfs:label "E s p d response"@en ;
  rdfs:subClassOf epo:TenderDocument ;
  owl:disjointWith epo:FinancialTenderDocument ;
  owl:disjointWith epo:PreAwardCatalogueResponse ;
  owl:disjointWith epo:TechnicalTenderDocument ;
  skos:definition "European Single Procurement Document Response. The declaration of the Economic Operator that it meets all the exclusion and selection criteria specified in the ESPD Request."@en ;
  skos:prefLabel "E s p d response"@en ;
.
epo:EXPRESSION_OF_INTEREST
  rdf:type skos:Concept ;
  rdfs:isDefinedBy <http://data.europa.eu/a4g/ontology> ;
  rdfs:label "E x p r e s s i o n_ o f_ i n t e r e s t"@en ;
  skos:inScheme epo:Submission-document-type ;
  skos:prefLabel "E x p r e s s i o n_ o f_ i n t e r e s t"@en ;
.
epo:EconomicOperator
  rdf:type owl:Class ;
  rdfs:comment """A role played by any natural or legal person or public entity or group of such persons and/or entities, including any temporary association of undertakings, which offers the execution of works and/or a work, the supply of products or the provision of services on the market.

(WG approval 28/04/2020)
"""@en ;
  rdfs:isDefinedBy <http://data.europa.eu/a4g/ontology> ;
  rdfs:label "Economic operator"@en ;
  rdfs:subClassOf epo:Role ;
  owl:disjointWith epo:Buyer ;
  owl:disjointWith epo:CentralPurchasingBody ;
  owl:disjointWith epo:ProcurementServiceProvider ;
  skos:definition """A role played by any natural or legal person or public entity or group of such persons and/or entities, including any temporary association of undertakings, which offers the execution of works and/or a work, the supply of products or the provision of services on the market.

(WG approval 28/04/2020)
"""@en ;
  skos:prefLabel "Economic operator"@en ;
.
epo:EconomicOperatorShortList
  rdf:type owl:Class ;
  rdfs:comment """The Economic Operators that are considered for a given procedure.

WG approval 22/08/2019 """@en ;
  rdfs:isDefinedBy <http://data.europa.eu/a4g/ontology> ;
  rdfs:label "Economic operator short list"@en ;
  skos:definition """The Economic Operators that are considered for a given procedure.

WG approval 22/08/2019 """@en ;
  skos:prefLabel "Economic operator short list"@en ;
.
epo:Edu
  rdf:type skos:Concept ;
  rdfs:isDefinedBy <http://data.europa.eu/a4g/ontology> ;
  rdfs:label "Education"@en ;
  skos:inScheme <http://publications.europa.eu/resource/authority/Main-activity> ;
  skos:prefLabel "Education"@en ;
.
epo:Ef-stand
  rdf:type skos:Concept ;
  rdfs:isDefinedBy <http://data.europa.eu/a4g/ontology> ;
  rdfs:label "Economic and financial standing"@en ;
  skos:inScheme <http://publications.europa.eu/resource/authority/Selection-criterion> ;
  skos:prefLabel "Economic and financial standing"@en ;
.
epo:Elec
  rdf:type skos:Concept ;
  rdfs:isDefinedBy <http://data.europa.eu/a4g/ontology> ;
  rdfs:label "Electricity-related activities"@en ;
  skos:inScheme <http://publications.europa.eu/resource/authority/Main-activity> ;
  skos:prefLabel "Electricity-related activities"@en ;
.
epo:Eo-group-type
  rdf:type skos:ConceptScheme ;
  rdfs:isDefinedBy <http://data.europa.eu/a4g/ontology> ;
  rdfs:label "Eo-group-type"@en ;
  skos:prefLabel "Eo-group-type" ;
.
epo:Eu-ins-bod-ag
  rdf:type skos:Concept ;
  rdfs:isDefinedBy <http://data.europa.eu/a4g/ontology> ;
  rdfs:label "EU institution, body or agency"@en ;
  skos:inScheme <http://publications.europa.eu/resource/authority/Buyer-legal-type> ;
  skos:prefLabel "EU institution, body or agency"@en ;
.
epo:Evaluation-group-type
  rdf:type skos:ConceptScheme ;
  rdfs:isDefinedBy <http://data.europa.eu/a4g/ontology> ;
  rdfs:label "Evaluation-group-type"@en ;
  skos:prefLabel "Evaluation-group-type" ;
.
epo:EvaluationBoard
  rdf:type owl:Class ;
  rdfs:isDefinedBy <http://data.europa.eu/a4g/ontology> ;
  rdfs:label "Evaluation board"@en ;
  rdfs:subClassOf foaf:Group ;
  skos:prefLabel "Evaluation board"@en ;
.
epo:EvaluationResult
  rdf:type owl:Class ;
  rdfs:comment "The Evaluation Board publishes the result of tenders after completion of its evaluation."@en ;
  rdfs:isDefinedBy <http://data.europa.eu/a4g/ontology> ;
  rdfs:label "Evaluation result"@en ;
  skos:definition "The Evaluation Board publishes the result of tenders after completion of its evaluation."@en ;
  skos:prefLabel "Evaluation result"@en ;
.
epo:EvaluationSystem
  rdf:type owl:Class ;
  rdfs:comment """An automated solution that assesses structured information in tenders and proposes results.

WG approval 20/11/2018"""@en ;
  rdfs:isDefinedBy <http://data.europa.eu/a4g/ontology> ;
  rdfs:label "Evaluation system"@en ;
  skos:definition """An automated solution that assesses structured information in tenders and proposes results.

WG approval 20/11/2018"""@en ;
  skos:prefLabel "Evaluation system"@en ;
.
epo:EvaluationTerms
  rdf:type owl:Class ;
  rdfs:comment """Conditions and stipulations defining particularities of the tender evaluation.

(WG approval 23/11/2018)


"""@en ;
  rdfs:isDefinedBy <http://data.europa.eu/a4g/ontology> ;
  rdfs:label "Evaluation terms"@en ;
  skos:definition """Conditions and stipulations defining particularities of the tender evaluation.

(WG approval 23/11/2018)


"""@en ;
  skos:prefLabel "Evaluation terms"@en ;
.
epo:Evaluator
  rdf:type owl:Class ;
  rdfs:isDefinedBy <http://data.europa.eu/a4g/ontology> ;
  rdfs:label "Evaluator"@en ;
  skos:prefLabel "Evaluator"@en ;
.
epo:Exc-rights
  rdf:type skos:Concept ;
  rdfs:isDefinedBy <http://data.europa.eu/a4g/ontology> ;
  rdfs:label "The contract can be provided only by a particular economic operator because of exclusive rights, including intellectual property rights"@en ;
  skos:inScheme <http://publications.europa.eu/resource/authority/Direct-award-justification> ;
  skos:prefLabel "The contract can be provided only by a particular economic operator because of exclusive rights, including intellectual property rights"@en ;
.
epo:Exclusion-criterion
  rdf:type skos:ConceptScheme ;
  rdfs:isDefinedBy <http://data.europa.eu/a4g/ontology> ;
  rdfs:label "Exclusion-criterion"@en ;
  skos:prefLabel "Exclusion-criterion" ;
.
epo:ExclusionGround
  rdf:type owl:Class ;
  rdf:type skos:Concept ;
  rdfs:comment """Describes a legal requirement to be met by the economic operator to be a candidate in the procurement procedure.

WG approval 31/10/2018"""@en ;
  rdfs:isDefinedBy <http://data.europa.eu/a4g/ontology> ;
  rdfs:label "Exclusion ground"@en ;
  rdfs:subClassOf epo:ProcurementCriterion ;
  owl:disjointWith epo:AwardCriterion ;
  owl:disjointWith epo:SelectionCriterion ;
  skos:definition """Describes a legal requirement to be met by the economic operator to be a candidate in the procurement procedure.

WG approval 31/10/2018"""@en ;
  skos:inScheme epo:E-evaluation-criterion-type ;
  skos:prefLabel "Exclusion ground"@en ;
.
epo:Exec-pay
  rdf:type skos:Concept ;
  rdfs:isDefinedBy <http://data.europa.eu/a4g/ontology> ;
  rdfs:label "Organisation executing the payment"@en ;
  skos:inScheme epo:Function-taxonomy ;
  skos:prefLabel "Organisation executing the payment"@en ;
.
epo:Ext-urg
  rdf:type skos:Concept ;
  rdfs:isDefinedBy <http://data.europa.eu/a4g/ontology> ;
  rdfs:label "Extreme urgency brought about by events unforeseeable for the buyer"@en ;
  skos:inScheme <http://publications.europa.eu/resource/authority/Direct-award-justification> ;
  skos:prefLabel "Extreme urgency brought about by events unforeseeable for the buyer"@en ;
.
epo:FEB
  rdf:type skos:Concept ;
  rdfs:isDefinedBy <http://data.europa.eu/a4g/ontology> ;
  rdfs:label "February"@en ;
  skos:inScheme <http://publications.europa.eu/resource/authority/Timeperiods> ;
  skos:prefLabel "February"@en ;
.
epo:FRI
  rdf:type skos:Concept ;
  rdfs:isDefinedBy <http://data.europa.eu/a4g/ontology> ;
  rdfs:label "Friday"@en ;
  skos:inScheme <http://publications.europa.eu/resource/authority/Timeperiods> ;
  skos:prefLabel "Friday"@en ;
.
epo:Fa-mix
  rdf:type skos:Concept ;
  rdfs:isDefinedBy <http://data.europa.eu/a4g/ontology> ;
  rdfs:label "Framework agreement, partly without reopening and partly with reopening of competition"@en ;
  skos:inScheme epo:Framework-agreement ;
  skos:prefLabel "Framework agreement, partly without reopening and partly with reopening of competition"@en ;
.
epo:Fa-w-rc
  rdf:type skos:Concept ;
  rdfs:isDefinedBy <http://data.europa.eu/a4g/ontology> ;
  rdfs:label "Framework agreement, with reopening of competition"@en ;
  skos:inScheme epo:Framework-agreement ;
  skos:prefLabel "Framework agreement, with reopening of competition"@en ;
.
epo:Fa-wo-rc
  rdf:type skos:Concept ;
  rdfs:isDefinedBy <http://data.europa.eu/a4g/ontology> ;
  rdfs:label "Framework agreement, without reopening of competition"@en ;
  skos:inScheme epo:Framework-agreement ;
  skos:prefLabel "Framework agreement, without reopening of competition"@en ;
.
epo:Fair-comp
  rdf:type skos:Concept ;
  rdfs:isDefinedBy <http://data.europa.eu/a4g/ontology> ;
  rdfs:label "Fair competition"@en ;
  skos:inScheme <http://publications.europa.eu/resource/authority/Non-publication-justification> ;
  skos:prefLabel "Fair competition"@en ;
.
epo:FinancialAccount
  rdf:type owl:Class ;
  rdfs:comment """(To be discussed during eSubmission WG decision 28/11/2018)
"""@en ;
  rdfs:isDefinedBy <http://data.europa.eu/a4g/ontology> ;
  rdfs:label "Financial account"@en ;
  skos:definition """(To be discussed during eSubmission WG decision 28/11/2018)
"""@en ;
  skos:prefLabel "Financial account"@en ;
.
epo:FinancialOfferValue
  rdf:type owl:Class ;
  rdfs:comment """Monetary amount for which the tenderer commits to fulfil a given part of the tender.

Additional Information:

In the case of negotiated procedure the Financial Offer Value provided by the Tenderer is adapted according to the negotiations with the Buyer.

A value given for a group of lots may be different to the sum of the lots submitted individually (e.g. more advantageous).
Separate classes are added in the ontology for different value types (e.g. Procurement Value, Financial Official Value, other) for tracking back the provenance and enabling the individual and total values to be cross-checked.

WG Approval 28/05/2019"""@en ;
  rdfs:isDefinedBy <http://data.europa.eu/a4g/ontology> ;
  rdfs:label "Financial offer value"@en ;
  rdfs:subClassOf epo:Value ;
  owl:disjointWith epo:ProcurementValue ;
  skos:definition """Monetary amount for which the tenderer commits to fulfil a given part of the tender.

Additional Information:

In the case of negotiated procedure the Financial Offer Value provided by the Tenderer is adapted according to the negotiations with the Buyer.

A value given for a group of lots may be different to the sum of the lots submitted individually (e.g. more advantageous).
Separate classes are added in the ontology for different value types (e.g. Procurement Value, Financial Official Value, other) for tracking back the provenance and enabling the individual and total values to be cross-checked.

WG Approval 28/05/2019"""@en ;
  skos:prefLabel "Financial offer value"@en ;
.
epo:FinancialTenderDocument
  rdf:type owl:Class ;
  rdfs:comment """
"""@en ;
  rdfs:isDefinedBy <http://data.europa.eu/a4g/ontology> ;
  rdfs:label "Financial tender document"@en ;
  rdfs:subClassOf epo:TenderDocument ;
  owl:disjointWith epo:ESPDResponse ;
  owl:disjointWith epo:PreAwardCatalogueResponse ;
  owl:disjointWith epo:TechnicalTenderDocument ;
  skos:definition """
"""@en ;
  skos:prefLabel "Financial tender document"@en ;
.
epo:Fix-tot
  rdf:type skos:Concept ;
  rdfs:isDefinedBy <http://data.europa.eu/a4g/ontology> ;
  rdfs:label "Fixed (total)"@en ;
  skos:inScheme <http://publications.europa.eu/resource/authority/Number-fixed> ;
  skos:prefLabel "Fixed (total)"@en ;
.
epo:Fix-unit
  rdf:type skos:Concept ;
  rdfs:isDefinedBy <http://data.europa.eu/a4g/ontology> ;
  rdfs:label "Fixed (per unit)"@en ;
  skos:inScheme <http://publications.europa.eu/resource/authority/Number-fixed> ;
  skos:prefLabel "Fixed (per unit)"@en ;
.
epo:FollowupContractTerms
  rdf:type owl:Class ;
  rdfs:isDefinedBy <http://data.europa.eu/a4g/ontology> ;
  rdfs:label "Followup contract terms"@en ;
  skos:prefLabel "Followup contract terms"@en ;
.
epo:Form-type
  rdf:type skos:ConceptScheme ;
  rdfs:isDefinedBy <http://data.europa.eu/a4g/ontology> ;
  rdfs:label "Form-type"@en ;
  skos:prefLabel "Form-type" ;
.
epo:FormalOrganisation
  rdf:type owl:Class ;
  rdfs:comment """An Organization which is recognized in the world at large, in particular in legal jurisdictions, with associated rights and responsibilities. 

Additional information:
Examples include a corporation, charity, government or church.

Source: https://www.w3.org/TR/vocab-org/#class-formalorganization 

To be discussed further """@en ;
  rdfs:isDefinedBy <http://data.europa.eu/a4g/ontology> ;
  rdfs:label "Formal organisation"@en ;
  rdfs:subClassOf epo:Organisation ;
  rdfs:subClassOf org:FormalOrganization ;
  owl:disjointWith epo:RegisteredOrganisation ;
  skos:definition """An Organization which is recognized in the world at large, in particular in legal jurisdictions, with associated rights and responsibilities. 

Additional information:
Examples include a corporation, charity, government or church.

Source: https://www.w3.org/TR/vocab-org/#class-formalorganization 

To be discussed further """@en ;
  skos:prefLabel "Formal organisation"@en ;
.
epo:Framework-agreement
  rdf:type skos:ConceptScheme ;
  rdfs:isDefinedBy <http://data.europa.eu/a4g/ontology> ;
  rdfs:label "Framework-agreement"@en ;
  skos:prefLabel "Framework-agreement" ;
.
epo:FrameworkAgreement
  rdf:type owl:Class ;
  rdfs:comment """The initial contract resulting from the Framework Agreement.  

Additional Information:

The framework agreement contract is an agreement which the purpose is to establish the terms governing purchase contracts to be awarded during a given period.

WG Approval 09/01/2020"""@en ;
  rdfs:isDefinedBy <http://data.europa.eu/a4g/ontology> ;
  rdfs:label "Framework agreement"@en ;
  rdfs:subClassOf epo:Contract ;
  owl:disjointWith epo:PurchaseContract ;
  skos:definition """The initial contract resulting from the Framework Agreement.  

Additional Information:

The framework agreement contract is an agreement which the purpose is to establish the terms governing purchase contracts to be awarded during a given period.

WG Approval 09/01/2020"""@en ;
  skos:prefLabel "Framework agreement"@en ;
.
epo:FrameworkAgreementTechnique
  rdf:type owl:Class ;
  rdfs:comment """The terms governing contracts, reached between one more buyers and one or more economic operators during a given period.

(WG approval 05/12/2018)"""@en ;
  rdfs:isDefinedBy <http://data.europa.eu/a4g/ontology> ;
  rdfs:label "Framework agreement technique"@en ;
  rdfs:subClassOf epo:Technique ;
  owl:disjointWith epo:DynamicPurchaseSystemTechnique ;
  owl:disjointWith epo:EAuctionTechnique ;
  skos:definition """The terms governing contracts, reached between one more buyers and one or more economic operators during a given period.

(WG approval 05/12/2018)"""@en ;
  skos:prefLabel "Framework agreement technique"@en ;
.
epo:FrameworkAgreementTerms
  rdf:type owl:Class ;
  rdfs:comment """Reason for extending time limits.

Additional Information: in exceptional cases related, for example, to framework agreements that exceed the legal limits, these limits need to be justified.. (Four years in the case of the general procurement directive, seven years in the case of the defence directive, and eight years in the case of the sectoral directive.).

WG Approval 2019-19-02
"""@en ;
  rdfs:isDefinedBy <http://data.europa.eu/a4g/ontology> ;
  rdfs:label "Framework agreement terms"@en ;
  skos:definition """Reason for extending time limits.

Additional Information: in exceptional cases related, for example, to framework agreements that exceed the legal limits, these limits need to be justified.. (Four years in the case of the general procurement directive, seven years in the case of the defence directive, and eight years in the case of the sectoral directive.).

WG Approval 2019-19-02
"""@en ;
  skos:prefLabel "Framework agreement terms"@en ;
.
epo:Ful-soc-obj
  rdf:type skos:Concept ;
  rdfs:isDefinedBy <http://data.europa.eu/a4g/ontology> ;
  rdfs:label "Fulfillment of social objectives"@en ;
  skos:inScheme <http://publications.europa.eu/resource/authority/Strategic-procurement> ;
  skos:prefLabel "Fulfillment of social objectives"@en ;
.
epo:Function
  rdf:type owl:Class ;
  rdfs:comment """The specific task of an agent in a particular business process.

Additional Information
In the context of public procurement, ‘functions’ are tasks related to procurement in general or more specifically to the management or execution of concrete procurement procedures. 
Examples of functions in procurement can be organisations responsible for providing information on taxes in a specific region, organisation providing information concerning the general regulatory framework for employment protection and working conditions in a specific region, organisations providing information concerning the general regulatory framework for environmental protection, etc."""@en ;
  rdfs:isDefinedBy <http://data.europa.eu/a4g/ontology> ;
  rdfs:label "Function"@en ;
  skos:definition """The specific task of an agent in a particular business process.

Additional Information
In the context of public procurement, ‘functions’ are tasks related to procurement in general or more specifically to the management or execution of concrete procurement procedures. 
Examples of functions in procurement can be organisations responsible for providing information on taxes in a specific region, organisation providing information concerning the general regulatory framework for employment protection and working conditions in a specific region, organisations providing information concerning the general regulatory framework for environmental protection, etc."""@en ;
  skos:prefLabel "Function"@en ;
.
epo:Function-taxonomy
  rdf:type skos:ConceptScheme ;
  rdfs:isDefinedBy <http://data.europa.eu/a4g/ontology> ;
  rdfs:label "Function-taxonomy"@en ;
  skos:prefLabel "Function-taxonomy" ;
.
epo:Fund
  rdf:type owl:Class ;
  rdfs:comment """A financial resource used to support the procurement.

Additional Information:

In the context of EU, funds can be divided into programmes, actions and projects.

Examples of EU funds are: the European Structural and Investment Funds, European Social Fund (ESF), the Connecting Europe Facility (CEF) programme, or the ISA2 programme and its actions (e.g. Action 2016.05 European Public Procurement Initiative, which supports the eProcurement Ontology under sub-action 3).

Funds may change between the lot and the contract, for example in the case of an emergency crisis, a contract may be financed by a budget that was not foreseen in the call.

WG Approved 14/05/2019




"""@en ;
  rdfs:isDefinedBy <http://data.europa.eu/a4g/ontology> ;
  rdfs:label "Fund"@en ;
  skos:definition """A financial resource used to support the procurement.

Additional Information:

In the context of EU, funds can be divided into programmes, actions and projects.

Examples of EU funds are: the European Structural and Investment Funds, European Social Fund (ESF), the Connecting Europe Facility (CEF) programme, or the ISA2 programme and its actions (e.g. Action 2016.05 European Public Procurement Initiative, which supports the eProcurement Ontology under sub-action 3).

Funds may change between the lot and the contract, for example in the case of an emergency crisis, a contract may be financed by a budget that was not foreseen in the call.

WG Approved 14/05/2019




"""@en ;
  skos:prefLabel "Fund"@en ;
.
epo:Gen-pub
  rdf:type skos:Concept ;
  rdfs:isDefinedBy <http://data.europa.eu/a4g/ontology> ;
  rdfs:label "General public services"@en ;
  skos:inScheme <http://publications.europa.eu/resource/authority/Main-activity> ;
  skos:prefLabel "General public services"@en ;
.
epo:Gh-pro-tran-dis
  rdf:type skos:Concept ;
  rdfs:isDefinedBy <http://data.europa.eu/a4g/ontology> ;
  rdfs:label "Production, transport or distribution of gas or heat"@en ;
  skos:inScheme <http://publications.europa.eu/resource/authority/Main-activity> ;
  skos:prefLabel "Production, transport or distribution of gas or heat"@en ;
.
epo:GreenProcurement
  rdf:type owl:Class ;
  rdfs:comment """Approach whereby buyers seek to procure with a reduced environmental impact.

Additional Information:

The approach may apply to the complete life cycle. The reduced environmental impact is in comparison to goods, services and works with the same primary function that would otherwise be procured. 

Tightly related are article 68 - Life-cycle costing and article 67 - most economically advantageous tender (see GPP handbook) https://ec.europa.eu/environment/gpp/pdf/Buying-Green-Handbook-3rd-Edition.pdf
An instance of the class GreenProcurement is represented in eForms with the code \"env-imp\" defined in the codelist strategic-procurement.paragraphs) https://ec.europa.eu/environment/gpp/pdf/Buying-Green-Handbook-3rd-Edition.pdf"""@en ;
  rdfs:isDefinedBy <http://data.europa.eu/a4g/ontology> ;
  rdfs:label "Green procurement"@en ;
  rdfs:subClassOf epo:StrategicProcurement ;
  owl:disjointWith epo:InnovativeProcurement ;
  owl:disjointWith epo:SocialProcurement ;
  skos:definition """Approach whereby buyers seek to procure with a reduced environmental impact.

Additional Information:

The approach may apply to the complete life cycle. The reduced environmental impact is in comparison to goods, services and works with the same primary function that would otherwise be procured. 

Tightly related are article 68 - Life-cycle costing and article 67 - most economically advantageous tender (see GPP handbook) https://ec.europa.eu/environment/gpp/pdf/Buying-Green-Handbook-3rd-Edition.pdf
An instance of the class GreenProcurement is represented in eForms with the code \"env-imp\" defined in the codelist strategic-procurement.paragraphs) https://ec.europa.eu/environment/gpp/pdf/Buying-Green-Handbook-3rd-Edition.pdf"""@en ;
  skos:prefLabel "Green procurement"@en ;
.
epo:Group-lead
  rdf:type skos:Concept ;
  rdfs:isDefinedBy <http://data.europa.eu/a4g/ontology> ;
  rdfs:label "Group leader"@en ;
  skos:inScheme epo:Function-taxonomy ;
  skos:prefLabel "Group leader"@en ;
.
epo:HKG
  rdf:type skos:Concept ;
  rdfs:isDefinedBy <http://data.europa.eu/a4g/ontology> ;
  rdfs:label "Hong Kong"@en ;
  skos:inScheme <http://publications.europa.eu/resource/authority/Country> ;
  skos:prefLabel "Hong Kong"@en ;
.
epo:HOUR
  rdf:type skos:Concept ;
  rdfs:isDefinedBy <http://data.europa.eu/a4g/ontology> ;
  rdfs:label "(_S|Hour)(_P|Hours)"@en ;
  skos:inScheme <http://publications.europa.eu/resource/authority/Timeperiods> ;
  skos:prefLabel "(_S|Hour)(_P|Hours)"@en ;
.
epo:I03000000-1
  rdf:type skos:Concept ;
  rdfs:isDefinedBy <http://data.europa.eu/a4g/ontology> ;
  rdfs:label "Agricultural, farming, fishing, forestry and related products"@en ;
  skos:inScheme <http://publications.europa.eu/resource/authority/Cpv> ;
  skos:prefLabel "Agricultural, farming, fishing, forestry and related products"@en ;
.
epo:I03100000-2
  rdf:type skos:Concept ;
  rdfs:isDefinedBy <http://data.europa.eu/a4g/ontology> ;
  rdfs:label "Agricultural and horticultural products"@en ;
  skos:inScheme <http://publications.europa.eu/resource/authority/Cpv> ;
  skos:prefLabel "Agricultural and horticultural products"@en ;
.
epo:I03110000-5
  rdf:type skos:Concept ;
  rdfs:isDefinedBy <http://data.europa.eu/a4g/ontology> ;
  rdfs:label "Crops, products of market gardening and horticulture"@en ;
  skos:inScheme <http://publications.europa.eu/resource/authority/Cpv> ;
  skos:prefLabel "Crops, products of market gardening and horticulture"@en ;
.
epo:I03111000-2
  rdf:type skos:Concept ;
  rdfs:isDefinedBy <http://data.europa.eu/a4g/ontology> ;
  rdfs:label "Seeds"@en ;
  skos:inScheme <http://publications.europa.eu/resource/authority/Cpv> ;
  skos:prefLabel "Seeds"@en ;
.
epo:I03111100-3
  rdf:type skos:Concept ;
  rdfs:isDefinedBy <http://data.europa.eu/a4g/ontology> ;
  rdfs:label "Soya beans"@en ;
  skos:inScheme <http://publications.europa.eu/resource/authority/Cpv> ;
  skos:prefLabel "Soya beans"@en ;
.
epo:I31985R2137
  rdf:type skos:Concept ;
  rdfs:isDefinedBy <http://data.europa.eu/a4g/ontology> ;
  rdfs:label "{Regulation (EEC) No 2137/85}"@en ;
  skos:inScheme <http://publications.europa.eu/resource/authority/Legal-basis> ;
  skos:prefLabel "{Regulation (EEC) No 2137/85}"@en ;
.
epo:I31992L0013
  rdf:type skos:Concept ;
  rdfs:isDefinedBy <http://data.europa.eu/a4g/ontology> ;
  rdfs:label "Directive 92/13/EEC"@en ;
  skos:inScheme <http://publications.europa.eu/resource/authority/Legal-basis> ;
  skos:prefLabel "Directive 92/13/EEC"@en ;
.
epo:I31994D0001
  rdf:type skos:Concept ;
  rdfs:isDefinedBy <http://data.europa.eu/a4g/ontology> ;
  rdfs:label "Decision 94/1/EC, ECSC"@en ;
  skos:inScheme <http://publications.europa.eu/resource/authority/Legal-basis> ;
  skos:prefLabel "Decision 94/1/EC, ECSC"@en ;
.
epo:I31994D0800
  rdf:type skos:Concept ;
  rdfs:isDefinedBy <http://data.europa.eu/a4g/ontology> ;
  rdfs:label "Decision 94/800/EC"@en ;
  skos:inScheme <http://publications.europa.eu/resource/authority/Legal-basis> ;
  skos:prefLabel "Decision 94/800/EC"@en ;
.
epo:I32001R2157
  rdf:type skos:Concept ;
  rdfs:isDefinedBy <http://data.europa.eu/a4g/ontology> ;
  rdfs:label "{Regulation (EC) No 2157/2001}"@en ;
  skos:inScheme <http://publications.europa.eu/resource/authority/Legal-basis> ;
  skos:prefLabel "{Regulation (EC) No 2157/2001}"@en ;
.
epo:I32002D0309
  rdf:type skos:Concept ;
  rdfs:isDefinedBy <http://data.europa.eu/a4g/ontology> ;
  rdfs:label "Decision 2002/309/EC, Euratom"@en ;
  skos:inScheme <http://publications.europa.eu/resource/authority/Legal-basis> ;
  skos:prefLabel "Decision 2002/309/EC, Euratom"@en ;
.
epo:I32003R1435
  rdf:type skos:Concept ;
  rdfs:isDefinedBy <http://data.europa.eu/a4g/ontology> ;
  rdfs:label "{Regulation (EC) No 1435/2003}"@en ;
  skos:inScheme <http://publications.europa.eu/resource/authority/Legal-basis> ;
  skos:prefLabel "{Regulation (EC) No 1435/2003}"@en ;
.
epo:I32005D0015
  rdf:type skos:Concept ;
  rdfs:isDefinedBy <http://data.europa.eu/a4g/ontology> ;
  rdfs:label "Decision 2005/15/EC"@en ;
  skos:inScheme <http://publications.europa.eu/resource/authority/Legal-basis> ;
  skos:prefLabel "Decision 2005/15/EC"@en ;
.
epo:I32007L0066
  rdf:type skos:Concept ;
  rdfs:isDefinedBy <http://data.europa.eu/a4g/ontology> ;
  rdfs:label "Directive 2007/66/EC"@en ;
  skos:inScheme <http://publications.europa.eu/resource/authority/Legal-basis> ;
  skos:prefLabel "Directive 2007/66/EC"@en ;
.
epo:I32007R0718
  rdf:type skos:Concept ;
  rdfs:isDefinedBy <http://data.europa.eu/a4g/ontology> ;
  rdfs:label "{Regulation (EC) No 718/2007}"@en ;
  skos:inScheme <http://publications.europa.eu/resource/authority/Legal-basis> ;
  skos:prefLabel "{Regulation (EC) No 718/2007}"@en ;
.
epo:I32007R1370
  rdf:type skos:Concept ;
  rdfs:isDefinedBy <http://data.europa.eu/a4g/ontology> ;
  rdfs:label "{Regulation (EC) No 1370/2007}"@en ;
  skos:inScheme <http://publications.europa.eu/resource/authority/Legal-basis> ;
  skos:prefLabel "{Regulation (EC) No 1370/2007}"@en ;
.
epo:I32008R1008
  rdf:type skos:Concept ;
  rdfs:isDefinedBy <http://data.europa.eu/a4g/ontology> ;
  rdfs:label "{Regulation (EC) No 1008/2008}"@en ;
  skos:inScheme <http://publications.europa.eu/resource/authority/Legal-basis> ;
  skos:prefLabel "{Regulation (EC) No 1008/2008}"@en ;
.
epo:I32009L0081
  rdf:type skos:Concept ;
  rdfs:isDefinedBy <http://data.europa.eu/a4g/ontology> ;
  rdfs:label "Directive 2009/81/EC"@en ;
  skos:inScheme <http://publications.europa.eu/resource/authority/Legal-basis> ;
  skos:prefLabel "Directive 2009/81/EC"@en ;
.
epo:I32013L0016
  rdf:type skos:Concept ;
  rdfs:isDefinedBy <http://data.europa.eu/a4g/ontology> ;
  rdfs:label "Directive 2013/16/EU"@en ;
  skos:inScheme <http://publications.europa.eu/resource/authority/Legal-basis> ;
  skos:prefLabel "Directive 2013/16/EU"@en ;
.
epo:I32014D0115
  rdf:type skos:Concept ;
  rdfs:isDefinedBy <http://data.europa.eu/a4g/ontology> ;
  rdfs:label "Decision 2014/115/EU"@en ;
  skos:inScheme <http://publications.europa.eu/resource/authority/Legal-basis> ;
  skos:prefLabel "Decision 2014/115/EU"@en ;
.
epo:I32014D0691
  rdf:type skos:Concept ;
  rdfs:isDefinedBy <http://data.europa.eu/a4g/ontology> ;
  rdfs:label "Decision 2014/691/EU"@en ;
  skos:inScheme <http://publications.europa.eu/resource/authority/Legal-basis> ;
  skos:prefLabel "Decision 2014/691/EU"@en ;
.
epo:I32014L0023
  rdf:type skos:Concept ;
  rdfs:isDefinedBy <http://data.europa.eu/a4g/ontology> ;
  rdfs:label "Directive 2014/23/EU"@en ;
  skos:inScheme <http://publications.europa.eu/resource/authority/Legal-basis> ;
  skos:prefLabel "Directive 2014/23/EU"@en ;
.
epo:I32014L0024
  rdf:type skos:Concept ;
  rdfs:isDefinedBy <http://data.europa.eu/a4g/ontology> ;
  rdfs:label "Directive 2014/24/EU"@en ;
  skos:inScheme <http://publications.europa.eu/resource/authority/Legal-basis> ;
  skos:prefLabel "Directive 2014/24/EU"@en ;
.
epo:I32014L0025
  rdf:type skos:Concept ;
  rdfs:isDefinedBy <http://data.europa.eu/a4g/ontology> ;
  rdfs:label "Directive 2014/25/EU"@en ;
  skos:inScheme <http://publications.europa.eu/resource/authority/Legal-basis> ;
  skos:prefLabel "Directive 2014/25/EU"@en ;
.
epo:I32015R0323
  rdf:type skos:Concept ;
  rdfs:isDefinedBy <http://data.europa.eu/a4g/ontology> ;
  rdfs:label "{Regulation (EU) 2015/323}"@en ;
  skos:inScheme <http://publications.europa.eu/resource/authority/Legal-basis> ;
  skos:prefLabel "{Regulation (EU) 2015/323}"@en ;
.
epo:I32016D0002
  rdf:type skos:Concept ;
  rdfs:isDefinedBy <http://data.europa.eu/a4g/ontology> ;
  rdfs:label "{Decision (EU) 2016/245 (ECB/2016/2)}"@en ;
  skos:inScheme <http://publications.europa.eu/resource/authority/Legal-basis> ;
  skos:prefLabel "{Decision (EU) 2016/245 (ECB/2016/2)}"@en ;
.
epo:I32018R1046
  rdf:type skos:Concept ;
  rdfs:isDefinedBy <http://data.europa.eu/a4g/ontology> ;
  rdfs:label "{Regulation (EU, Euratom) 2018/1046}"@en ;
  skos:inScheme <http://publications.europa.eu/resource/authority/Legal-basis> ;
  skos:prefLabel "{Regulation (EU, Euratom) 2018/1046}"@en ;
.
epo:IOT
  rdf:type skos:Concept ;
  rdfs:isDefinedBy <http://data.europa.eu/a4g/ontology> ;
  rdfs:label "British Indian Ocean Territory"@en ;
  skos:inScheme <http://publications.europa.eu/resource/authority/Country> ;
  skos:prefLabel "British Indian Ocean Territory"@en ;
.
epo:IRI
  rdf:type rdfs:Datatype ;
  rdfs:isDefinedBy <http://data.europa.eu/a4g/ontology> ;
  rdfs:label "I r i"@en ;
  skos:prefLabel "I r i"@en ;
.
epo:Identifier
  rdf:type rdfs:Datatype ;
  rdf:type owl:Class ;
  rdfs:comment """A unique identifier of the instance of the concept.

Additional Information

For example, in the case of the Procurement Identifier, this could be the European Public Procurement Identifier, and/or any other identifier provided by the buyer, the service provider or any other stakeholder.

WG Approval 12/11/2019"""@en ;
  rdfs:isDefinedBy <http://data.europa.eu/a4g/ontology> ;
  rdfs:label "Identifier"@en ;
  rdfs:subClassOf <http://www.unece.org/cefact#Identifier> ;
  skos:definition """A unique identifier of the instance of the concept.

Additional Information

For example, in the case of the Procurement Identifier, this could be the European Public Procurement Identifier, and/or any other identifier provided by the buyer, the service provider or any other stakeholder.

WG Approval 12/11/2019"""@en ;
  skos:prefLabel "Identifier"@en ;
.
epo:Inc-urg-res
  rdf:type skos:Concept ;
  rdfs:isDefinedBy <http://data.europa.eu/a4g/ontology> ;
  rdfs:label "The periods for the restricted procedure and the negotiated procedure with prior publication of a contract notice are incompatible with the urgency resulting from a crisis"@en ;
  skos:inScheme <http://publications.europa.eu/resource/authority/Direct-award-justification> ;
  skos:prefLabel "The periods for the restricted procedure and the negotiated procedure with prior publication of a contract notice are incompatible with the urgency resulting from a crisis"@en ;
.
epo:Included
  rdf:type skos:Concept ;
  rdfs:isDefinedBy <http://data.europa.eu/a4g/ontology> ;
  rdfs:label "Accessibility criteria for persons with disabilities are included."@en ;
  skos:inScheme <http://publications.europa.eu/resource/authority/Accessibility> ;
  skos:prefLabel "Accessibility criteria for persons with disabilities are included."@en ;
.
epo:Indicator
  rdf:type rdfs:Datatype ;
  rdf:type owl:Class ;
  rdfs:isDefinedBy <http://data.europa.eu/a4g/ontology> ;
  rdfs:label "Indicator"@en ;
  rdfs:subClassOf <http://www.unece.org/cefact#Indicator> ;
  skos:prefLabel "Indicator"@en ;
.
epo:Indirect
  rdf:type skos:Concept ;
  rdfs:isDefinedBy <http://data.europa.eu/a4g/ontology> ;
  rdfs:label "Indirect"@en ;
  skos:inScheme epo:Communication-type ;
  skos:prefLabel "Indirect"@en ;
.
epo:Info-emp
  rdf:type skos:Concept ;
  rdfs:isDefinedBy <http://data.europa.eu/a4g/ontology> ;
  rdfs:label "Organisation providing information concerning the general regulatory framework for employment protection and working conditions applicable in the place where the contract is to be performed."@en ;
  skos:inScheme epo:Function-taxonomy ;
  skos:prefLabel "Organisation providing information concerning the general regulatory framework for employment protection and working conditions applicable in the place where the contract is to be performed."@en ;
.
epo:Info-envir
  rdf:type skos:Concept ;
  rdfs:isDefinedBy <http://data.europa.eu/a4g/ontology> ;
  rdfs:label "Organisation providing information concerning the general regulatory framework for environmental protection applicable in the place where the contract is to be performed."@en ;
  skos:inScheme epo:Function-taxonomy ;
  skos:prefLabel "Organisation providing information concerning the general regulatory framework for environmental protection applicable in the place where the contract is to be performed."@en ;
.
epo:Info-prov
  rdf:type skos:Concept ;
  rdfs:isDefinedBy <http://data.europa.eu/a4g/ontology> ;
  rdfs:label "Organisation providing additional information about the procurement procedure"@en ;
  skos:inScheme epo:Function-taxonomy ;
  skos:prefLabel "Organisation providing additional information about the procurement procedure"@en ;
.
epo:Info-tax
  rdf:type skos:Concept ;
  rdfs:isDefinedBy <http://data.europa.eu/a4g/ontology> ;
  rdfs:label "Organisation providing information concerning the general regulatory framework for taxes applicable in the place where the contract is to be performed."@en ;
  skos:inScheme epo:Function-taxonomy ;
  skos:prefLabel "Organisation providing information concerning the general regulatory framework for taxes applicable in the place where the contract is to be performed."@en ;
.
epo:Inn-pur
  rdf:type skos:Concept ;
  rdfs:isDefinedBy <http://data.europa.eu/a4g/ontology> ;
  rdfs:label "Innovative purchase"@en ;
  skos:inScheme <http://publications.europa.eu/resource/authority/Strategic-procurement> ;
  skos:prefLabel "Innovative purchase"@en ;
.
epo:Innovation
  rdf:type skos:Concept ;
  rdfs:isDefinedBy <http://data.europa.eu/a4g/ontology> ;
  rdfs:label "Innovation partnership"@en ;
  skos:inScheme <http://publications.europa.eu/resource/authority/Procurement-procedure-type> ;
  skos:prefLabel "Innovation partnership"@en ;
.
epo:InnovativeProcurement
  rdf:type owl:Class ;
  rdfs:comment """An instance of the class InnovativeProcurement is represented in eForms with the code \"inn-pur\" defined in the codelist strategic-procurement.

Research (21/01/2020):

Purchasing and early adoption of solutions which are not yet available on large scale commercial basis. 

Source: Adapted from the Digital Single Market's Policy on Public Procurement of Innovative Solutions. https://ec.europa.eu/digital-single-market/en/public-procurement-innovative-solutions

Additional Information: 
‘innovation’ means the implementation of a new or significantly improved product, service or process, including but not limited to production, building or construction processes, a new marketing method, or a new organisational method in business practices, workplace organisation or external relations inter alia with the purpose of helping to solve societal challenges or to support the Europe 2020 strategy for smart, sustainable and inclusive growth;
See: Directive 2014/24
Articles: 2, 26 (3), 31, 67 (2.a)

Question: 
Is  Pre-Commercial Procurement (PCP) another type of Strategic Procurement?"""@en ;
  rdfs:isDefinedBy <http://data.europa.eu/a4g/ontology> ;
  rdfs:label "Innovative procurement"@en ;
  rdfs:subClassOf epo:StrategicProcurement ;
  owl:disjointWith epo:GreenProcurement ;
  owl:disjointWith epo:SocialProcurement ;
  skos:definition """An instance of the class InnovativeProcurement is represented in eForms with the code \"inn-pur\" defined in the codelist strategic-procurement.

Research (21/01/2020):

Purchasing and early adoption of solutions which are not yet available on large scale commercial basis. 

Source: Adapted from the Digital Single Market's Policy on Public Procurement of Innovative Solutions. https://ec.europa.eu/digital-single-market/en/public-procurement-innovative-solutions

Additional Information: 
‘innovation’ means the implementation of a new or significantly improved product, service or process, including but not limited to production, building or construction processes, a new marketing method, or a new organisational method in business practices, workplace organisation or external relations inter alia with the purpose of helping to solve societal challenges or to support the Europe 2020 strategy for smart, sustainable and inclusive growth;
See: Directive 2014/24
Articles: 2, 26 (3), 31, 67 (2.a)

Question: 
Is  Pre-Commercial Procurement (PCP) another type of Strategic Procurement?"""@en ;
  skos:prefLabel "Innovative procurement"@en ;
.
epo:Ins-fund
  rdf:type skos:Concept ;
  rdfs:isDefinedBy <http://data.europa.eu/a4g/ontology> ;
  rdfs:label "Decision of the buyer, because of insufficient funds"@en ;
  skos:inScheme <http://publications.europa.eu/resource/authority/Non-award-justification> ;
  skos:prefLabel "Decision of the buyer, because of insufficient funds"@en ;
.
epo:Int-org
  rdf:type skos:Concept ;
  rdfs:isDefinedBy <http://data.europa.eu/a4g/ontology> ;
  rdfs:label "International organisation"@en ;
  skos:inScheme <http://publications.europa.eu/resource/authority/Buyer-legal-type> ;
  skos:prefLabel "International organisation"@en ;
.
epo:InvitationToTender
  rdf:type owl:Class ;
  rdfs:comment """
"""@en ;
  rdfs:isDefinedBy <http://data.europa.eu/a4g/ontology> ;
  rdfs:label "Invitation to tender"@en ;
  rdfs:subClassOf epo:ProcurementDocument ;
  owl:disjointWith epo:AdditionalDocument ;
  owl:disjointWith epo:CallForCompetition ;
  owl:disjointWith epo:ContractTemplate ;
  owl:disjointWith epo:DescriptiveDocument ;
  owl:disjointWith epo:DraftCV ;
  owl:disjointWith epo:ESPDRequest ;
  owl:disjointWith epo:PreAwardCatalogueRequest ;
  owl:disjointWith epo:TechnicalSpecifications ;
  skos:definition """
"""@en ;
  skos:prefLabel "Invitation to tender"@en ;
.
epo:Ipr-iss
  rdf:type skos:Concept ;
  rdfs:isDefinedBy <http://data.europa.eu/a4g/ontology> ;
  rdfs:label "Intellectual property right issues"@en ;
  skos:inScheme <http://publications.europa.eu/resource/authority/Communication-justification> ;
  skos:prefLabel "Intellectual property right issues"@en ;
.
epo:Item
  rdf:type owl:Class ;
  rdfs:isDefinedBy <http://data.europa.eu/a4g/ontology> ;
  rdfs:label "Item"@en ;
  skos:prefLabel "Item"@en ;
.
epo:JAN
  rdf:type skos:Concept ;
  rdfs:isDefinedBy <http://data.europa.eu/a4g/ontology> ;
  rdfs:label "January"@en ;
  skos:inScheme <http://publications.europa.eu/resource/authority/Timeperiods> ;
  skos:prefLabel "January"@en ;
.
epo:JOINT_VENTURE
  rdf:type skos:Concept ;
  rdfs:isDefinedBy <http://data.europa.eu/a4g/ontology> ;
  rdfs:label "Joint Venture"@en ;
  skos:inScheme epo:Eo-group-type ;
  skos:prefLabel "Joint Venture"@en ;
.
epo:JUL
  rdf:type skos:Concept ;
  rdfs:isDefinedBy <http://data.europa.eu/a4g/ontology> ;
  rdfs:label "July"@en ;
  skos:inScheme <http://publications.europa.eu/resource/authority/Timeperiods> ;
  skos:prefLabel "July"@en ;
.
epo:JUN
  rdf:type skos:Concept ;
  rdfs:isDefinedBy <http://data.europa.eu/a4g/ontology> ;
  rdfs:label "June"@en ;
  skos:inScheme <http://publications.europa.eu/resource/authority/Timeperiods> ;
  skos:prefLabel "June"@en ;
.
epo:JURY
  rdf:type skos:Concept ;
  rdfs:isDefinedBy <http://data.europa.eu/a4g/ontology> ;
  rdfs:label "J u r y"@en ;
  skos:inScheme epo:Evaluation-group-type ;
  skos:prefLabel "J u r y"@en ;
.
epo:KHM
  rdf:type skos:Concept ;
  rdfs:isDefinedBy <http://data.europa.eu/a4g/ontology> ;
  rdfs:label "Cambodia"@en ;
  skos:inScheme <http://publications.europa.eu/resource/authority/Country> ;
  skos:prefLabel "Cambodia"@en ;
.
epo:LA
  rdf:type skos:Concept ;
  rdfs:isDefinedBy <http://data.europa.eu/a4g/ontology> ;
  rdfs:label "Local Authority"@en ;
  skos:inScheme epo:Authority-type ;
  skos:prefLabel "Local Authority"@en ;
.
epo:LE
  rdf:type skos:Concept ;
  rdfs:isDefinedBy <http://data.europa.eu/a4g/ontology> ;
  rdfs:label "Lead Entity"@en ;
  skos:inScheme epo:Function-taxonomy ;
  skos:prefLabel "Lead Entity"@en ;
.
epo:La
  rdf:type skos:Concept ;
  rdfs:isDefinedBy <http://data.europa.eu/a4g/ontology> ;
  rdfs:label "Local authority"@en ;
  skos:inScheme <http://publications.europa.eu/resource/authority/Buyer-legal-type> ;
  skos:prefLabel "Local authority"@en ;
.
epo:Large
  rdf:type skos:Concept ;
  rdfs:isDefinedBy <http://data.europa.eu/a4g/ontology> ;
  rdfs:label "Large enterprise"@en ;
  skos:inScheme <http://publications.europa.eu/resource/authority/Economic-operator-size> ;
  skos:prefLabel "Large enterprise"@en ;
.
epo:Late-all
  rdf:type skos:Concept ;
  rdfs:isDefinedBy <http://data.europa.eu/a4g/ontology> ;
  rdfs:label "All missing tenderer-related documents can be submitted later"@en ;
  skos:inScheme <http://publications.europa.eu/resource/authority/Missing-info-submission> ;
  skos:prefLabel "All missing tenderer-related documents can be submitted later"@en ;
.
epo:Late-none
  rdf:type skos:Concept ;
  rdfs:isDefinedBy <http://data.europa.eu/a4g/ontology> ;
  rdfs:label "No documents can be submitted later"@en ;
  skos:inScheme <http://publications.europa.eu/resource/authority/Missing-info-submission> ;
  skos:prefLabel "No documents can be submitted later"@en ;
.
epo:Late-some
  rdf:type skos:Concept ;
  rdfs:isDefinedBy <http://data.europa.eu/a4g/ontology> ;
  rdfs:label "Some missing tenderer-related documents can be submitted later"@en ;
  skos:inScheme <http://publications.europa.eu/resource/authority/Missing-info-submission> ;
  skos:prefLabel "Some missing tenderer-related documents can be submitted later"@en ;
.
epo:Law-enf
  rdf:type skos:Concept ;
  rdfs:isDefinedBy <http://data.europa.eu/a4g/ontology> ;
  rdfs:label "Law enforcement"@en ;
  skos:inScheme <http://publications.europa.eu/resource/authority/Non-publication-justification> ;
  skos:prefLabel "Law enforcement"@en ;
.
epo:Legal-form-type
  rdf:type skos:ConceptScheme ;
  rdfs:isDefinedBy <http://data.europa.eu/a4g/ontology> ;
  rdfs:label "Legal-form-type"@en ;
  skos:prefLabel "Legal-form-type" ;
.
epo:Legal-regime
  rdf:type skos:ConceptScheme ;
  rdfs:isDefinedBy <http://data.europa.eu/a4g/ontology> ;
  rdfs:label "Legal-regime"@en ;
  skos:prefLabel "Legal-regime" ;
.
epo:Light-regime
  rdf:type skos:Concept ;
  rdfs:isDefinedBy <http://data.europa.eu/a4g/ontology> ;
  rdfs:label "Set of principles and rules for social and specific services"@en ;
  skos:inScheme epo:Legal-regime ;
  skos:prefLabel "Set of principles and rules for social and specific services"@en ;
.
epo:Lim-prov
  rdf:type skos:Concept ;
  rdfs:isDefinedBy <http://data.europa.eu/a4g/ontology> ;
  rdfs:label "Organisation providing more information on the time limits for review procedures"@en ;
  skos:inScheme epo:Function-taxonomy ;
  skos:prefLabel "Organisation providing more information on the time limits for review procedures"@en ;
.
epo:Location
  rdf:type owl:Class ;
  rdfs:comment """An identifiable geographic place. 

Source: ISO 19112"""@en ;
  rdfs:isDefinedBy <http://data.europa.eu/a4g/ontology> ;
  rdfs:label "Location"@en ;
  skos:definition """An identifiable geographic place. 

Source: ISO 19112"""@en ;
  skos:prefLabel "Location"@en ;
.
epo:LocationCoordinate
  rdf:type owl:Class ;
  rdfs:isDefinedBy <http://data.europa.eu/a4g/ontology> ;
  rdfs:label "Location coordinate"@en ;
  skos:prefLabel "Location coordinate"@en ;
.
epo:Lot
  rdf:type owl:Class ;
  rdfs:comment """A qualitative, quantitative or strategic subdivision of the goods, services or works to be procured, allowing the award of one or more contracts.

WG approval 12/09/2018"""@en ;
  rdfs:isDefinedBy <http://data.europa.eu/a4g/ontology> ;
  rdfs:label "Lot"@en ;
  skos:definition """A qualitative, quantitative or strategic subdivision of the goods, services or works to be procured, allowing the award of one or more contracts.

WG approval 12/09/2018"""@en ;
  skos:prefLabel "Lot"@en ;
.
epo:LotGroup
  rdf:type owl:Class ;
  rdfs:comment """Combination of several lots to conduct comparative assessment of the tenders.

Additional Information:

The comparative assessment may refer to the selection criteria, award and value that apply to several lots.

Pending of discussion with eForms



Member States may provide that, where more than one lot may be awarded to the same tenderer, contracting authorities may award contracts combining several or all lots where they have specified in the contract notice or in the invitation to confirm interest that they reserve the possibility of doing so and indicate the lots or groups of lots that may be combined."""@en ;
  rdfs:isDefinedBy <http://data.europa.eu/a4g/ontology> ;
  rdfs:label "Lot group"@en ;
  skos:definition """Combination of several lots to conduct comparative assessment of the tenders.

Additional Information:

The comparative assessment may refer to the selection criteria, award and value that apply to several lots.

Pending of discussion with eForms



Member States may provide that, where more than one lot may be awarded to the same tenderer, contracting authorities may award contracts combining several or all lots where they have specified in the contract notice or in the invitation to confirm interest that they reserve the possibility of doing so and indicate the lots or groups of lots that may be combined."""@en ;
  skos:prefLabel "Lot group"@en ;
.
epo:LotSpecification
  rdf:type owl:Class ;
  rdfs:isDefinedBy <http://data.europa.eu/a4g/ontology> ;
  rdfs:label "Lot specification"@en ;
  skos:prefLabel "Lot specification"@en ;
.
epo:MAC
  rdf:type skos:Concept ;
  rdfs:isDefinedBy <http://data.europa.eu/a4g/ontology> ;
  rdfs:label "Macao, SAR China"@en ;
  skos:inScheme <http://publications.europa.eu/resource/authority/Country> ;
  skos:prefLabel "Macao, SAR China"@en ;
.
epo:MAR
  rdf:type skos:Concept ;
  rdfs:isDefinedBy <http://data.europa.eu/a4g/ontology> ;
  rdfs:label "March"@en ;
  skos:inScheme <http://publications.europa.eu/resource/authority/Timeperiods> ;
  skos:prefLabel "March"@en ;
.
epo:MAY
  rdf:type skos:Concept ;
  rdfs:isDefinedBy <http://data.europa.eu/a4g/ontology> ;
  rdfs:label "May"@en ;
  skos:inScheme <http://publications.europa.eu/resource/authority/Timeperiods> ;
  skos:prefLabel "May"@en ;
.
epo:MG
  rdf:type skos:Concept ;
  rdfs:isDefinedBy <http://data.europa.eu/a4g/ontology> ;
  rdfs:label "Member of a Group"@en ;
  skos:inScheme epo:Function-taxonomy ;
  skos:prefLabel "Member of a Group"@en ;
.
epo:MIN
  rdf:type skos:Concept ;
  rdfs:isDefinedBy <http://data.europa.eu/a4g/ontology> ;
  rdfs:label "(_S|Minute)(_P|Minutes)"@en ;
  skos:inScheme <http://publications.europa.eu/resource/authority/Timeperiods> ;
  skos:prefLabel "(_S|Minute)(_P|Minutes)"@en ;
.
epo:MON
  rdf:type skos:Concept ;
  rdfs:isDefinedBy <http://data.europa.eu/a4g/ontology> ;
  rdfs:label "Monday"@en ;
  skos:inScheme <http://publications.europa.eu/resource/authority/Timeperiods> ;
  skos:prefLabel "Monday"@en ;
.
epo:MONTH
  rdf:type skos:Concept ;
  rdfs:isDefinedBy <http://data.europa.eu/a4g/ontology> ;
  rdfs:label "(_S|Month)(_P|Months)"@en ;
  skos:inScheme <http://publications.europa.eu/resource/authority/Timeperiods> ;
  skos:prefLabel "(_S|Month)(_P|Months)"@en ;
.
epo:Max-ten-pass
  rdf:type skos:Concept ;
  rdfs:isDefinedBy <http://data.europa.eu/a4g/ontology> ;
  rdfs:label "Maximum number of tenders passing"@en ;
  skos:inScheme <http://publications.europa.eu/resource/authority/Number-threshold> ;
  skos:prefLabel "Maximum number of tenders passing"@en ;
.
epo:Measure
  rdf:type rdfs:Datatype ;
  rdf:type owl:Class ;
  rdfs:isDefinedBy <http://data.europa.eu/a4g/ontology> ;
  rdfs:label "Measure"@en ;
  rdfs:subClassOf <http://www.unece.org/cefact#Measure> ;
  skos:prefLabel "Measure"@en ;
.
epo:Mediator
  rdf:type skos:Concept ;
  rdfs:isDefinedBy <http://data.europa.eu/a4g/ontology> ;
  rdfs:label "Mediator"@en ;
  skos:inScheme epo:Function-taxonomy ;
  skos:prefLabel "Mediator"@en ;
.
epo:Medium
  rdf:type skos:Concept ;
  rdfs:comment "An enterprise which employs between 50 to 250 persons and and whose annual turnover and/or annual balance sheet total is between EUR 10 to 43 million."@en ;
  rdfs:isDefinedBy <http://data.europa.eu/a4g/ontology> ;
  rdfs:label "Medium-sized-enterprise"@en ;
  skos:definition "An enterprise which employs between 50 to 250 persons and and whose annual turnover and/or annual balance sheet total is between EUR 10 to 43 million."@en ;
  skos:inScheme <http://publications.europa.eu/resource/authority/Economic-operator-size> ;
  skos:prefLabel "Medium-sized-enterprise"@en ;
.
epo:Micro
  rdf:type skos:Concept ;
  rdfs:comment "An enterprise which employs fewer than 10 persons and whose annual turnover and/or annual balance sheet total does not exceed EUR 2 million."@en ;
  rdfs:isDefinedBy <http://data.europa.eu/a4g/ontology> ;
  rdfs:label "Microenterprise"@en ;
  skos:definition "An enterprise which employs fewer than 10 persons and whose annual turnover and/or annual balance sheet total does not exceed EUR 2 million."@en ;
  skos:inScheme <http://publications.europa.eu/resource/authority/Economic-operator-size> ;
  skos:prefLabel "Microenterprise"@en ;
.
epo:Min-sco
  rdf:type skos:Concept ;
  rdfs:isDefinedBy <http://data.europa.eu/a4g/ontology> ;
  rdfs:label "Minimum score"@en ;
  skos:inScheme <http://publications.europa.eu/resource/authority/Number-threshold> ;
  skos:prefLabel "Minimum score"@en ;
.
epo:Mod-cir
  rdf:type skos:Concept ;
  rdfs:isDefinedBy <http://data.europa.eu/a4g/ontology> ;
  rdfs:label "Need for modifications because of circumstances which a diligent buyer could not predict.  "@en ;
  skos:inScheme <http://publications.europa.eu/resource/authority/Modification-justification> ;
  skos:prefLabel "Need for modifications because of circumstances which a diligent buyer could not predict.  "@en ;
.
epo:MultipleStageProcedureTerms
  rdf:type owl:Class ;
  rdfs:isDefinedBy <http://data.europa.eu/a4g/ontology> ;
  rdfs:label "Multiple stage procedure terms"@en ;
  skos:prefLabel "Multiple stage procedure terms"@en ;
.
epo:N-used
  rdf:type skos:Concept ;
  rdfs:isDefinedBy <http://data.europa.eu/a4g/ontology> ;
  rdfs:label "Not Used"@en ;
  skos:inScheme <http://publications.europa.eu/resource/authority/Usage> ;
  skos:prefLabel "Not Used"@en ;
.
epo:NO
  rdf:type skos:Concept ;
  rdfs:isDefinedBy <http://data.europa.eu/a4g/ontology> ;
  rdfs:label "Options are not used"@en ;
  skos:inScheme epo:Options ;
  skos:prefLabel "Options are not used"@en ;
.
epo:NOV
  rdf:type skos:Concept ;
  rdfs:isDefinedBy <http://data.europa.eu/a4g/ontology> ;
  rdfs:label "November"@en ;
  skos:inScheme <http://publications.europa.eu/resource/authority/Timeperiods> ;
  skos:prefLabel "November"@en ;
.
epo:Nace
  rdf:type skos:ConceptScheme ;
  rdfs:comment """Source: EU Vocabularies authority table \"<xref scope=\"external\" href=\"https://op.europa.eu/en/web/eu-vocabularies/at-dataset/-/resource/dataset/main-activity\"><foreign otherprops=\"#0000ff\"><u>Main Activity</u></foreign></xref>\" (https://op.europa.eu/en/web/eu-vocabularies/at-dataset/-/resource/dataset/main-activity).
"""@en ;
  rdfs:isDefinedBy <http://data.europa.eu/a4g/ontology> ;
  rdfs:label "Nace"@en ;
  skos:definition """Source: EU Vocabularies authority table \"<xref scope=\"external\" href=\"https://op.europa.eu/en/web/eu-vocabularies/at-dataset/-/resource/dataset/main-activity\"><foreign otherprops=\"#0000ff\"><u>Main Activity</u></foreign></xref>\" (https://op.europa.eu/en/web/eu-vocabularies/at-dataset/-/resource/dataset/main-activity).
"""@en ;
  skos:prefLabel "Nace" ;
.
epo:Name
  rdf:type owl:Class ;
  rdfs:isDefinedBy <http://data.europa.eu/a4g/ontology> ;
  rdfs:label "Name"@en ;
  rdfs:subClassOf epo:Text ;
  skos:prefLabel "Name"@en ;
.
epo:Neg-w-call
  rdf:type skos:Concept ;
  rdfs:isDefinedBy <http://data.europa.eu/a4g/ontology> ;
  rdfs:label "Negotiated with prior publication of a call for comeptition / competitive with negotiation"@en ;
  skos:inScheme <http://publications.europa.eu/resource/authority/Procurement-procedure-type> ;
  skos:prefLabel "Negotiated with prior publication of a call for comeptition / competitive with negotiation"@en ;
.
epo:Neg-wo-call
  rdf:type skos:Concept ;
  rdfs:isDefinedBy <http://data.europa.eu/a4g/ontology> ;
  rdfs:label "Negotiated without prior call for competition"@en ;
  skos:inScheme <http://publications.europa.eu/resource/authority/Procurement-procedure-type> ;
  skos:prefLabel "Negotiated without prior call for competition"@en ;
.
epo:No
  rdf:type skos:Concept ;
  rdfs:isDefinedBy <http://data.europa.eu/a4g/ontology> ;
  rdfs:label "No"@en ;
  skos:inScheme <http://publications.europa.eu/resource/authority/Applicability> ;
  skos:prefLabel "No"@en ;
.
epo:No-rece
  rdf:type skos:Concept ;
  rdfs:isDefinedBy <http://data.europa.eu/a4g/ontology> ;
  rdfs:label "No tenders, requests to participate or projects were received"@en ;
  skos:inScheme <http://publications.europa.eu/resource/authority/Non-award-justification> ;
  skos:prefLabel "No tenders, requests to participate or projects were received"@en ;
.
epo:No-reg-resp
  rdf:type skos:Concept ;
  rdfs:isDefinedBy <http://data.europa.eu/a4g/ontology> ;
  rdfs:label "No regular tenders, requests to participate, or applications acceptable under national provisions were received in response to a previous notice. Only those tenderers were included in the negotiations which have satisfied the selection criteria in the previous procedure."@en ;
  skos:inScheme <http://publications.europa.eu/resource/authority/Direct-award-justification> ;
  skos:prefLabel "No regular tenders, requests to participate, or applications acceptable under national provisions were received in response to a previous notice. Only those tenderers were included in the negotiations which have satisfied the selection criteria in the previous procedure."@en ;
.
epo:No-signed
  rdf:type skos:Concept ;
  rdfs:isDefinedBy <http://data.europa.eu/a4g/ontology> ;
  rdfs:label "The highest ranked tenderer(s) refused to sign the contract"@en ;
  skos:inScheme <http://publications.europa.eu/resource/authority/Non-award-justification> ;
  skos:prefLabel "The highest ranked tenderer(s) refused to sign the contract"@en ;
.
epo:No-suit-resp
  rdf:type skos:Concept ;
  rdfs:isDefinedBy <http://data.europa.eu/a4g/ontology> ;
  rdfs:label "No suitable tenders, requests to participate, or applications were received in response to a previous notice."@en ;
  skos:inScheme <http://publications.europa.eu/resource/authority/Direct-award-justification> ;
  skos:prefLabel "No suitable tenders, requests to participate, or applications were received in response to a previous notice."@en ;
.
epo:None
  rdf:type skos:Concept ;
  rdfs:isDefinedBy <http://data.europa.eu/a4g/ontology> ;
  rdfs:label "None"@en ;
  skos:inScheme epo:Framework-agreement ;
  skos:inScheme <http://publications.europa.eu/resource/authority/Dps-usage> ;
  skos:inScheme <http://publications.europa.eu/resource/authority/Strategic-procurement> ;
  skos:inScheme <http://publications.europa.eu/resource/authority/Subcontracting-indication> ;
  skos:prefLabel "None"@en ;
.
epo:Not-allowed
  rdf:type skos:Concept ;
  rdfs:isDefinedBy <http://data.europa.eu/a4g/ontology> ;
  rdfs:label "Not allowed"@en ;
  skos:inScheme <http://publications.europa.eu/resource/authority/Permission> ;
  skos:prefLabel "Not allowed"@en ;
.
epo:Not-inc-just
  rdf:type skos:Concept ;
  rdfs:isDefinedBy <http://data.europa.eu/a4g/ontology> ;
  rdfs:label "Accessibility criteria for persons with disabilities are not included with the following justification."@en ;
  skos:inScheme <http://publications.europa.eu/resource/authority/Accessibility> ;
  skos:prefLabel "Accessibility criteria for persons with disabilities are not included with the following justification."@en ;
.
epo:Not-inc-proc
  rdf:type skos:Concept ;
  rdfs:isDefinedBy <http://data.europa.eu/a4g/ontology> ;
  rdfs:label "Accessibility criteria for persons with disabilities are not included because the procurement is not intended for use by natural persons."@en ;
  skos:inScheme <http://publications.europa.eu/resource/authority/Accessibility> ;
  skos:prefLabel "Accessibility criteria for persons with disabilities are not included because the procurement is not intended for use by natural persons."@en ;
.
epo:Not-known
  rdf:type skos:Concept ;
  rdfs:isDefinedBy <http://data.europa.eu/a4g/ontology> ;
  rdfs:label "Not-known"@en ;
  skos:inScheme <http://publications.europa.eu/resource/authority/Applicability> ;
  skos:prefLabel "Not-known"@en ;
.
epo:Notice
  rdf:type owl:Class ;
  rdfs:comment """Document published by the buyer about market opportunities and results.

WG Approval 23/05/2019
"""@en ;
  rdfs:isDefinedBy <http://data.europa.eu/a4g/ontology> ;
  rdfs:label "Notice"@en ;
  rdfs:subClassOf epo:Document ;
  owl:disjointWith epo:Contract ;
  owl:disjointWith epo:ProcurementDocument ;
  owl:disjointWith epo:RequestForParticipation ;
  owl:disjointWith epo:TenderDocument ;
  skos:definition """Document published by the buyer about market opportunities and results.

WG Approval 23/05/2019
"""@en ;
  skos:prefLabel "Notice"@en ;
.
epo:Notice-corrigendum-justification
  rdf:type skos:ConceptScheme ;
  rdfs:isDefinedBy <http://data.europa.eu/a4g/ontology> ;
  rdfs:label "Notice-corrigendum-justification"@en ;
  skos:prefLabel "Notice-corrigendum-justification" ;
.
epo:Notification-phases-content-types
  rdf:type skos:ConceptScheme ;
  rdfs:isDefinedBy <http://data.europa.eu/a4g/ontology> ;
  rdfs:label "Notification-phases-content-types"@en ;
  skos:prefLabel "Notification-phases-content-types" ;
.
epo:Numeric
  rdf:type rdfs:Datatype ;
  rdf:type owl:Class ;
  rdfs:isDefinedBy <http://data.europa.eu/a4g/ontology> ;
  rdfs:label "Numeric"@en ;
  rdfs:subClassOf <http://www.unece.org/cefact#Numeric> ;
  owl:disjointWith epo:Percent ;
  skos:prefLabel "Numeric"@en ;
.
epo:Nyk
  rdf:type skos:Concept ;
  rdfs:comment "[] (eng | With regard to selection criterion used this can be used only in a PIN CFC / RTL)"@en ;
  rdfs:isDefinedBy <http://data.europa.eu/a4g/ontology> ;
  rdfs:label "Not yet known"@en ;
  skos:definition "[] (eng | With regard to selection criterion used this can be used only in a PIN CFC / RTL)"@en ;
  skos:inScheme <http://publications.europa.eu/resource/authority/Usage> ;
  skos:prefLabel "Not yet known"@en ;
.
epo:OCT
  rdf:type skos:Concept ;
  rdfs:isDefinedBy <http://data.europa.eu/a4g/ontology> ;
  rdfs:label "October"@en ;
  skos:inScheme <http://publications.europa.eu/resource/authority/Timeperiods> ;
  skos:prefLabel "October"@en ;
.
epo:OENRON
  rdf:type skos:Concept ;
  rdfs:isDefinedBy <http://data.europa.eu/a4g/ontology> ;
  rdfs:label "Other Entity (not relied upon)"@en ;
  skos:inScheme epo:Function-taxonomy ;
  skos:prefLabel "Other Entity (not relied upon)"@en ;
.
epo:OERON
  rdf:type skos:Concept ;
  rdfs:isDefinedBy <http://data.europa.eu/a4g/ontology> ;
  rdfs:label "Other Entity (relied upon)"@en ;
  skos:inScheme epo:Function-taxonomy ;
  skos:prefLabel "Other Entity (relied upon)"@en ;
.
epo:ON
  rdf:type skos:Concept ;
  rdfs:isDefinedBy <http://data.europa.eu/a4g/ontology> ;
  rdfs:label "Process the group always"@en ;
  skos:inScheme <http://data.europa.eu/m8g/Criterion-group-property-type> ;
  skos:prefLabel "Process the group always"@en ;
.
epo:ONFALSE
  rdf:type skos:Concept ;
  rdfs:isDefinedBy <http://data.europa.eu/a4g/ontology> ;
  rdfs:label "Process the group if the previous question was and INDICATOR answered with the value 'false'"@en ;
  skos:inScheme <http://data.europa.eu/m8g/Criterion-group-property-type> ;
  skos:prefLabel "Process the group if the previous question was and INDICATOR answered with the value 'false'"@en ;
.
epo:ONTRUE
  rdf:type skos:Concept ;
  rdfs:isDefinedBy <http://data.europa.eu/a4g/ontology> ;
  rdfs:label "Process the group if the previous question was and INDICATOR answered with the value 'true'"@en ;
  skos:inScheme <http://data.europa.eu/m8g/Criterion-group-property-type> ;
  skos:prefLabel "Process the group if the previous question was and INDICATOR answered with the value 'true'"@en ;
.
epo:OPEN
  rdf:type skos:Concept ;
  rdfs:isDefinedBy <http://data.europa.eu/a4g/ontology> ;
  rdfs:label "O p e n"@en ;
  skos:inScheme epo:Design-contest-type ;
  skos:prefLabel "O p e n"@en ;
.
epo:Offl-acc
  rdf:type skos:Concept ;
  rdfs:isDefinedBy <http://data.europa.eu/a4g/ontology> ;
  rdfs:label "Organisation providing offline access to the procurement documents"@en ;
  skos:inScheme epo:Function-taxonomy ;
  skos:prefLabel "Organisation providing offline access to the procurement documents"@en ;
.
epo:One-admis
  rdf:type skos:Concept ;
  rdfs:isDefinedBy <http://data.europa.eu/a4g/ontology> ;
  rdfs:label "Only one admissible tender, request to participate or project was received"@en ;
  skos:inScheme <http://publications.europa.eu/resource/authority/Non-award-justification> ;
  skos:prefLabel "Only one admissible tender, request to participate or project was received"@en ;
.
epo:Open
  rdf:type skos:Concept ;
  rdfs:isDefinedBy <http://data.europa.eu/a4g/ontology> ;
  rdfs:label "Open"@en ;
  skos:inScheme <http://publications.europa.eu/resource/authority/Procurement-procedure-type> ;
  skos:prefLabel "Open"@en ;
.
epo:Open-nw
  rdf:type skos:Concept ;
  rdfs:isDefinedBy <http://data.europa.eu/a4g/ontology> ;
  rdfs:label "The winner was not yet chosen, but the competition is still ongoing"@en ;
  skos:inScheme <http://publications.europa.eu/resource/authority/Winner-selection-status> ;
  skos:prefLabel "The winner was not yet chosen, but the competition is still ongoing"@en ;
.
epo:OpeningHoursSpecification
  rdf:type owl:Class ;
  rdfs:comment """A structured value providing information about the availability of the channel or a contact point. 

WG Approval 28/04/2020"""@en ;
  rdfs:isDefinedBy <http://data.europa.eu/a4g/ontology> ;
  rdfs:label "Opening hours specification"@en ;
  skos:definition """A structured value providing information about the availability of the channel or a contact point. 

WG Approval 28/04/2020"""@en ;
  skos:prefLabel "Opening hours specification"@en ;
.
epo:OpeningTerms
  rdf:type owl:Class ;
  rdfs:isDefinedBy <http://data.europa.eu/a4g/ontology> ;
  rdfs:label "Opening terms"@en ;
  skos:prefLabel "Opening terms"@en ;
.
epo:Options
  rdf:type skos:ConceptScheme ;
  rdfs:isDefinedBy <http://data.europa.eu/a4g/ontology> ;
  rdfs:label "Options"@en ;
  skos:prefLabel "Options" ;
.
epo:Ord-imp
  rdf:type skos:Concept ;
  rdfs:isDefinedBy <http://data.europa.eu/a4g/ontology> ;
  rdfs:label "Order of importance"@en ;
  skos:inScheme <http://publications.europa.eu/resource/authority/Number-weight> ;
  skos:prefLabel "Order of importance"@en ;
.
epo:Org-sub
  rdf:type skos:Concept ;
  rdfs:isDefinedBy <http://data.europa.eu/a4g/ontology> ;
  rdfs:label "Organisation awarding a contract subsidised by a contracting authority"@en ;
  skos:inScheme <http://publications.europa.eu/resource/authority/Buyer-legal-type> ;
  skos:prefLabel "Organisation awarding a contract subsidised by a contracting authority"@en ;
.
epo:Org-sub-cga
  rdf:type skos:Concept ;
  rdfs:isDefinedBy <http://data.europa.eu/a4g/ontology> ;
  rdfs:label "Organisation awarding a contract subsidised by a central government authority"@en ;
  skos:inScheme <http://publications.europa.eu/resource/authority/Buyer-legal-type> ;
  skos:prefLabel "Organisation awarding a contract subsidised by a central government authority"@en ;
.
epo:Org-sub-la
  rdf:type skos:Concept ;
  rdfs:isDefinedBy <http://data.europa.eu/a4g/ontology> ;
  rdfs:label "Organisation awarding a contract subsidised by a local authority"@en ;
  skos:inScheme <http://publications.europa.eu/resource/authority/Buyer-legal-type> ;
  skos:prefLabel "Organisation awarding a contract subsidised by a local authority"@en ;
.
epo:Org-sub-ra
  rdf:type skos:Concept ;
  rdfs:isDefinedBy <http://data.europa.eu/a4g/ontology> ;
  rdfs:label "Organisation awarding a contract subsidised by a regional authority"@en ;
  skos:inScheme <http://publications.europa.eu/resource/authority/Buyer-legal-type> ;
  skos:prefLabel "Organisation awarding a contract subsidised by a regional authority"@en ;
.
epo:Organisation
  rdf:type owl:Class ;
  rdfs:comment """A collection of people organized together into a community or other social, commercial or political structure. The group has some common purpose or reason for existence which goes beyond the set of people belonging to it and can act as an Agent. Organisations are often decomposable into hierarchical structures.

(WG approval 23/11/2018).
"""@en ;
  rdfs:isDefinedBy <http://data.europa.eu/a4g/ontology> ;
  rdfs:label "Organisation"@en ;
  rdfs:subClassOf epo:Agent ;
  rdfs:subClassOf org:Organization ;
  owl:disjointWith epo:Person ;
  owl:disjointWith epo:System ;
  owl:disjointWith org:FormalOrganization ;
  owl:disjointWith org:OrganizationalCollaboration ;
  owl:disjointWith org:OrganizationalUnit ;
  skos:definition """A collection of people organized together into a community or other social, commercial or political structure. The group has some common purpose or reason for existence which goes beyond the set of people belonging to it and can act as an Agent. Organisations are often decomposable into hierarchical structures.

(WG approval 23/11/2018).
"""@en ;
  skos:prefLabel "Organisation"@en ;
.
epo:Ori-not-canc
  rdf:type skos:Concept ;
  rdfs:isDefinedBy <http://data.europa.eu/a4g/ontology> ;
  rdfs:label "The original notice is cancelled"@en ;
  skos:inScheme epo:Notice-corrigendum-justification ;
  skos:prefLabel "The original notice is cancelled"@en ;
.
epo:Oth-mult
  rdf:type skos:Concept ;
  rdfs:isDefinedBy <http://data.europa.eu/a4g/ontology> ;
  rdfs:label "Other multiple stage procedure"@en ;
  skos:inScheme <http://publications.europa.eu/resource/authority/Procurement-procedure-type> ;
  skos:prefLabel "Other multiple stage procedure"@en ;
.
epo:Oth-pub-int
  rdf:type skos:Concept ;
  rdfs:isDefinedBy <http://data.europa.eu/a4g/ontology> ;
  rdfs:label "Other public interest"@en ;
  skos:inScheme <http://publications.europa.eu/resource/authority/Non-publication-justification> ;
  skos:prefLabel "Other public interest"@en ;
.
epo:Oth-single
  rdf:type skos:Concept ;
  rdfs:isDefinedBy <http://data.europa.eu/a4g/ontology> ;
  rdfs:label "Other single stage procedure"@en ;
  skos:inScheme <http://publications.europa.eu/resource/authority/Procurement-procedure-type> ;
  skos:prefLabel "Other single stage procedure"@en ;
.
epo:Other
  rdf:type skos:Concept ;
  rdfs:isDefinedBy <http://data.europa.eu/a4g/ontology> ;
  rdfs:label "Other"@en ;
  skos:inScheme <http://publications.europa.eu/resource/authority/Legal-basis> ;
  skos:inScheme <http://publications.europa.eu/resource/authority/Modification-justification> ;
  skos:inScheme <http://publications.europa.eu/resource/authority/Non-award-justification> ;
  skos:inScheme <http://publications.europa.eu/resource/authority/Selection-criterion> ;
  skos:prefLabel "Other"@en ;
.
epo:Other-righ-dir201423EU
  rdf:type skos:Concept ;
  rdfs:isDefinedBy <http://data.europa.eu/a4g/ontology> ;
  rdfs:label "The contract can be provided only by a particular economic operator because of protection of other exclusive rights, including intellectual property rights, other than those defined in Directive 2014/23/EU Art. 5(10)"@en ;
  skos:inScheme <http://publications.europa.eu/resource/authority/Direct-award-justification> ;
  skos:prefLabel "The contract can be provided only by a particular economic operator because of protection of other exclusive rights, including intellectual property rights, other than those defined in Directive 2014/23/EU Art. 5(10)"@en ;
.
epo:Other-serv-dir200981EC
  rdf:type skos:Concept ;
  rdfs:isDefinedBy <http://data.europa.eu/a4g/ontology> ;
  rdfs:label "The contract concerns research and development services other than those referred to in Directive 2009/81/EC Art. 13"@en ;
  skos:inScheme <http://publications.europa.eu/resource/authority/Direct-award-justification> ;
  skos:prefLabel "The contract concerns research and development services other than those referred to in Directive 2009/81/EC Art. 13"@en ;
.
epo:Out-dir
  rdf:type skos:Concept ;
  rdfs:isDefinedBy <http://data.europa.eu/a4g/ontology> ;
  rdfs:label "The procurement falls outside the scope of application of the directive"@en ;
  skos:inScheme <http://publications.europa.eu/resource/authority/Direct-award-justification> ;
  skos:prefLabel "The procurement falls outside the scope of application of the directive"@en ;
.
epo:PIN_REDUCE_TIME_LIMIT
  rdf:type skos:Concept ;
  rdfs:isDefinedBy <http://data.europa.eu/a4g/ontology> ;
  rdfs:label "Prior Information Notice to reduce time limits"@en ;
  skos:inScheme epo:Accelerated-procedure-justification-type ;
  skos:prefLabel "Prior Information Notice to reduce time limits"@en ;
.
epo:PLANNINGPIN
  rdf:type skos:Concept ;
  rdfs:isDefinedBy <http://data.europa.eu/a4g/ontology> ;
  rdfs:label "P l a n n i n g p i n"@en ;
  skos:inScheme epo:Notification-phases-content-types ;
  skos:prefLabel "P l a n n i n g p i n"@en ;
.
epo:PRICE
  rdf:type skos:Concept ;
  rdfs:isDefinedBy <http://data.europa.eu/a4g/ontology> ;
  rdfs:label "P r i c e"@en ;
  skos:inScheme epo:Award-dimension-parent-criterion-relation ;
  skos:prefLabel "P r i c e"@en ;
.
epo:PUBLIC
  rdf:type skos:Concept ;
  rdfs:isDefinedBy <http://data.europa.eu/a4g/ontology> ;
  rdfs:label "Information that can be disclose without any particular restriction."@en ;
  skos:inScheme <https://github.com/ESPD/ESPD-EDM/Confidentiality-level> ;
  skos:prefLabel "Information that can be disclose without any particular restriction."@en ;
.
epo:ParticipationCriterion
  rdf:type skos:Concept ;
  rdfs:isDefinedBy <http://data.europa.eu/a4g/ontology> ;
  rdfs:label "Participation criterion"@en ;
  skos:inScheme epo:E-evaluation-criterion-type ;
  skos:prefLabel "Participation criterion"@en ;
.
epo:Percent
  rdf:type rdfs:Datatype ;
  rdf:type owl:Class ;
  rdfs:isDefinedBy <http://data.europa.eu/a4g/ontology> ;
  rdfs:label "Percent"@en ;
  rdfs:subClassOf <http://www.unece.org/cefact#Numeric> ;
  owl:disjointWith epo:Numeric ;
  skos:prefLabel "Percent"@en ;
.
epo:Period
  rdf:type owl:Class ;
  rdfs:comment """A time interval or a duration.

(WG approval 28/04/2020)
"""@en ;
  rdfs:isDefinedBy <http://data.europa.eu/a4g/ontology> ;
  rdfs:label "Period"@en ;
  skos:definition """A time interval or a duration.

(WG approval 28/04/2020)
"""@en ;
  skos:prefLabel "Period"@en ;
.
epo:Person
  rdf:type owl:Class ;
  rdfs:comment """Individual who is able to carry out actions. 

WG Approval 28/04/2020
"""@en ;
  rdfs:isDefinedBy <http://data.europa.eu/a4g/ontology> ;
  rdfs:label "Person"@en ;
  rdfs:subClassOf epo:Agent ;
  rdfs:subClassOf foaf:Person ;
  owl:disjointWith epo:Organisation ;
  owl:disjointWith epo:System ;
  skos:definition """Individual who is able to carry out actions. 

WG Approval 28/04/2020
"""@en ;
  skos:prefLabel "Person"@en ;
.
epo:Phy-mod
  rdf:type skos:Concept ;
  rdfs:isDefinedBy <http://data.europa.eu/a4g/ontology> ;
  rdfs:label "Inclusion of a physical model"@en ;
  skos:inScheme <http://publications.europa.eu/resource/authority/Communication-justification> ;
  skos:prefLabel "Inclusion of a physical model"@en ;
.
epo:Plan
  rdf:type skos:Concept ;
  rdfs:isDefinedBy <http://data.europa.eu/a4g/ontology> ;
  rdfs:label "Planning"@en ;
  skos:inScheme epo:Form-type ;
  skos:prefLabel "Planning"@en ;
.
epo:PlannedProcurementPart
  rdf:type owl:Class ;
  rdfs:comment """A subdivision of a planned procurement that may later become one or more lots or a self-standing procedure. A lot or a procedure can also cover one or more parts of the planned procurement.

WG Approval 20/06/2019"""@en ;
  rdfs:isDefinedBy <http://data.europa.eu/a4g/ontology> ;
  rdfs:label "Planned procurement part"@en ;
  skos:definition """A subdivision of a planned procurement that may later become one or more lots or a self-standing procedure. A lot or a procedure can also cover one or more parts of the planned procurement.

WG Approval 20/06/2019"""@en ;
  skos:prefLabel "Planned procurement part"@en ;
.
epo:PositiveInteger
  rdf:type rdfs:Datatype ;
  rdfs:isDefinedBy <http://data.europa.eu/a4g/ontology> ;
  rdfs:label "Positive integer"@en ;
  skos:prefLabel "Positive integer"@en ;
.
epo:PreAwardCatalogueRequest
  rdf:type owl:Class ;
  rdfs:isDefinedBy <http://data.europa.eu/a4g/ontology> ;
  rdfs:label "Pre award catalogue request"@en ;
  rdfs:subClassOf epo:ProcurementDocument ;
  owl:disjointWith epo:AdditionalDocument ;
  owl:disjointWith epo:CallForCompetition ;
  owl:disjointWith epo:ContractTemplate ;
  owl:disjointWith epo:DescriptiveDocument ;
  owl:disjointWith epo:DraftCV ;
  owl:disjointWith epo:ESPDRequest ;
  owl:disjointWith epo:InvitationToTender ;
  owl:disjointWith epo:TechnicalSpecifications ;
  skos:prefLabel "Pre award catalogue request"@en ;
.
epo:PreAwardCatalogueResponse
  rdf:type owl:Class ;
  rdfs:isDefinedBy <http://data.europa.eu/a4g/ontology> ;
  rdfs:label "Pre award catalogue response"@en ;
  rdfs:subClassOf epo:TenderDocument ;
  owl:disjointWith epo:ESPDResponse ;
  owl:disjointWith epo:FinancialTenderDocument ;
  owl:disjointWith epo:TechnicalTenderDocument ;
  skos:prefLabel "Pre award catalogue response"@en ;
.
epo:Price
  rdf:type skos:Concept ;
  rdfs:isDefinedBy <http://data.europa.eu/a4g/ontology> ;
  rdfs:label "Price"@en ;
  skos:inScheme <http://publications.europa.eu/resource/authority/Award-criterion-type> ;
  skos:prefLabel "Price"@en ;
.
epo:PriorInformationNotice
  rdf:type owl:Class ;
  rdfs:comment "Notice which sets out the contracting authority's purchasing intentions. It is used by contracting authorities to provide suppliers with information about a procurement process. "@en ;
  rdfs:isDefinedBy <http://data.europa.eu/a4g/ontology> ;
  rdfs:label "Prior information notice"@en ;
  rdfs:subClassOf epo:Notice ;
  owl:disjointWith epo:CallForExpressionOfInterest ;
  owl:disjointWith epo:ContractAwardNotice ;
  owl:disjointWith epo:ContractModificationNotice ;
  owl:disjointWith epo:ContractNotice ;
  owl:disjointWith epo:VoluntaryEx-anteTransparencyNotice ;
  skos:definition "Notice which sets out the contracting authority's purchasing intentions. It is used by contracting authorities to provide suppliers with information about a procurement process. "@en ;
  skos:prefLabel "Prior information notice"@en ;
.
epo:Prize
  rdf:type owl:Class ;
  rdfs:isDefinedBy <http://data.europa.eu/a4g/ontology> ;
  rdfs:label "Prize"@en ;
  skos:prefLabel "Prize"@en ;
.
epo:Procedure
  rdf:type owl:Class ;
  rdfs:comment """A legally defined set of administrative activities conducted  to conclude one or more contracts.

Additional Information
The procedure is categorised in the law according to different rules determining whether the procedure is open, restricted, negotiated with or without  publicity, etc. (see Procedure Type).

WG Approval 20/08/2019
"""@en ;
  rdfs:isDefinedBy <http://data.europa.eu/a4g/ontology> ;
  rdfs:label "Procedure"@en ;
  skos:definition """A legally defined set of administrative activities conducted  to conclude one or more contracts.

Additional Information
The procedure is categorised in the law according to different rules determining whether the procedure is open, restricted, negotiated with or without  publicity, etc. (see Procedure Type).

WG Approval 20/08/2019
"""@en ;
  skos:prefLabel "Procedure"@en ;
.
epo:ProcedureTerms
  rdf:type owl:Class ;
  rdfs:comment """Conditions and stipulations defining particularities of the procedure.

(WG approval 23/11/2018)"""@en ;
  rdfs:isDefinedBy <http://data.europa.eu/a4g/ontology> ;
  rdfs:label "Procedure terms"@en ;
  skos:definition """Conditions and stipulations defining particularities of the procedure.

(WG approval 23/11/2018)"""@en ;
  skos:prefLabel "Procedure terms"@en ;
.
epo:Processor
  rdf:type skos:Concept ;
  rdfs:isDefinedBy <http://data.europa.eu/a4g/ontology> ;
  rdfs:label "Organisation processing tenders"@en ;
  skos:inScheme epo:Function-taxonomy ;
  skos:prefLabel "Organisation processing tenders"@en ;
.
epo:Procurement-regime-type
  rdf:type skos:ConceptScheme ;
  rdfs:isDefinedBy <http://data.europa.eu/a4g/ontology> ;
  rdfs:label "Procurement-regime-type"@en ;
  skos:prefLabel "Procurement-regime-type" ;
.
epo:ProcurementCriterion
  rdf:type owl:Class ;
  rdfs:comment """A criterion specific to Procurement.

Additional Information:

This Procurement Criterion can be only Exclusion Ground, Selection Criterion or Award Criterion. Each of these criteria can contain subcriteria (Criterion class).

WG Approval 23/04/2020"""@en ;
  rdfs:isDefinedBy <http://data.europa.eu/a4g/ontology> ;
  rdfs:label "Procurement criterion"@en ;
  rdfs:subClassOf <http://data.europa.eu/m8g/Criterion> ;
  skos:definition """A criterion specific to Procurement.

Additional Information:

This Procurement Criterion can be only Exclusion Ground, Selection Criterion or Award Criterion. Each of these criteria can contain subcriteria (Criterion class).

WG Approval 23/04/2020"""@en ;
  skos:prefLabel "Procurement criterion"@en ;
.
epo:ProcurementCriterionProperty
  rdf:type owl:Class ;
  rdfs:isDefinedBy <http://data.europa.eu/a4g/ontology> ;
  rdfs:label "Procurement criterion property"@en ;
  rdfs:subClassOf <http://data.europa.eu/m8g/Property> ;
  skos:prefLabel "Procurement criterion property"@en ;
.
epo:ProcurementDocument
  rdf:type owl:Class ;
  rdfs:comment """Document produced or referred to by the buyer to describe or determine elements of the procurement.

Additional information:

Procurement documents are to be accessible since the date of publication of the contract notice or the prior information notice when used as a call for competition.

Examples of procurement documents are technical specifications, the descriptive document, proposed conditions of contract, formats for the presentation of documents by candidates and tenderers, information on generally applicable obligations.

Other documents related to the procedure such as notices are not considered to be procurement documents.

WG Approval 23/05/2019 17:08:30"""@en ;
  rdfs:isDefinedBy <http://data.europa.eu/a4g/ontology> ;
  rdfs:label "Procurement document"@en ;
  rdfs:subClassOf epo:Document ;
  owl:disjointWith epo:Contract ;
  owl:disjointWith epo:Notice ;
  owl:disjointWith epo:RequestForParticipation ;
  owl:disjointWith epo:TenderDocument ;
  skos:definition """Document produced or referred to by the buyer to describe or determine elements of the procurement.

Additional information:

Procurement documents are to be accessible since the date of publication of the contract notice or the prior information notice when used as a call for competition.

Examples of procurement documents are technical specifications, the descriptive document, proposed conditions of contract, formats for the presentation of documents by candidates and tenderers, information on generally applicable obligations.

Other documents related to the procedure such as notices are not considered to be procurement documents.

WG Approval 23/05/2019 17:08:30"""@en ;
  skos:prefLabel "Procurement document"@en ;
.
epo:ProcurementServiceProvider
  rdf:type owl:Class ;
  rdfs:comment """Role of a public or private body which offers ancillary purchasing activities on the market.

Additional information

\"Ancillary purchasing activities\" means activities consisting in the provision of support to purchasing activities, in particular in the following forms:
(a) technical infrastructure enabling contracting authorities to award public contracts or to conclude framework agreements for works, supplies or services;
(b) advice on the conduct or design of public procurement procedures;
(c) preparation and management of procurement procedures on behalf and for the account of the contracting authority concerned;

Source: Directive 2014/24/EU, Article 2, paragraphs 17 and 15.

This would be equivalent to the concept of 'procuringEntity' in OCDS: 'The entity managing the procurement, which may be different from the buyer who is paying / using the items being procured'.

WG Approval 24/03/2020
"""@en ;
  rdfs:isDefinedBy <http://data.europa.eu/a4g/ontology> ;
  rdfs:label "Procurement service provider"@en ;
  rdfs:subClassOf epo:Role ;
  owl:disjointWith epo:Buyer ;
  owl:disjointWith epo:CentralPurchasingBody ;
  owl:disjointWith epo:EconomicOperator ;
  skos:definition """Role of a public or private body which offers ancillary purchasing activities on the market.

Additional information

\"Ancillary purchasing activities\" means activities consisting in the provision of support to purchasing activities, in particular in the following forms:
(a) technical infrastructure enabling contracting authorities to award public contracts or to conclude framework agreements for works, supplies or services;
(b) advice on the conduct or design of public procurement procedures;
(c) preparation and management of procurement procedures on behalf and for the account of the contracting authority concerned;

Source: Directive 2014/24/EU, Article 2, paragraphs 17 and 15.

This would be equivalent to the concept of 'procuringEntity' in OCDS: 'The entity managing the procurement, which may be different from the buyer who is paying / using the items being procured'.

WG Approval 24/03/2020
"""@en ;
  skos:prefLabel "Procurement service provider"@en ;
.
epo:ProcurementValue
  rdf:type owl:Class ;
  rdfs:comment """Monetary requirements established by the buyer related to a procurement.

Additional Information:

A value given for a group of lots may be different to the sum of the lots submitted individually (e.g. more advantageous).
Separate classes are added in the ontology for different value types (e.g. Procurement Value, Financial Official Value, other) for tracking back the provenance and enabling the individual and total values to be cross-checked.

WG Approval 28/05/2019"""@en ;
  rdfs:isDefinedBy <http://data.europa.eu/a4g/ontology> ;
  rdfs:label "Procurement value"@en ;
  rdfs:subClassOf epo:Value ;
  owl:disjointWith epo:FinancialOfferValue ;
  skos:definition """Monetary requirements established by the buyer related to a procurement.

Additional Information:

A value given for a group of lots may be different to the sum of the lots submitted individually (e.g. more advantageous).
Separate classes are added in the ontology for different value types (e.g. Procurement Value, Financial Official Value, other) for tracking back the provenance and enabling the individual and total values to be cross-checked.

WG Approval 28/05/2019"""@en ;
  skos:prefLabel "Procurement value"@en ;
.
epo:ProjectProcurement
  rdf:type owl:Class ;
  rdfs:comment """A set of linked procurement activities.

Additional Information:
Project Procurement can be explained as the grouping of several procurements. For example, when planning the construction of an airport several procurements can be foreseen, which may end up in different lots in one or more procedures: one aimed at the purchasing of tarmac for the runways, another for the contracting of catering services, another for the construction of the buildings, etc.. These procurements may be launched in different times (different years, for example).

WG 12/09/2018"""@en ;
  rdfs:isDefinedBy <http://data.europa.eu/a4g/ontology> ;
  rdfs:label "Project procurement"@en ;
  skos:definition """A set of linked procurement activities.

Additional Information:
Project Procurement can be explained as the grouping of several procurements. For example, when planning the construction of an airport several procurements can be foreseen, which may end up in different lots in one or more procedures: one aimed at the purchasing of tarmac for the runways, another for the contracting of catering services, another for the construction of the buildings, etc.. These procurements may be launched in different times (different years, for example).

WG 12/09/2018"""@en ;
  skos:prefLabel "Project procurement"@en ;
.
epo:Prop-subc-noblig
  rdf:type skos:Concept ;
  rdfs:isDefinedBy <http://data.europa.eu/a4g/ontology> ;
  rdfs:label "The proposed subcontractor(s) above any obligation to subcontract a minimum percentage of the contract"@en ;
  skos:inScheme <http://publications.europa.eu/resource/authority/Subcontracting-indication> ;
  skos:prefLabel "The proposed subcontractor(s) above any obligation to subcontract a minimum percentage of the contract"@en ;
.
epo:Prop-subc-oblig
  rdf:type skos:Concept ;
  rdfs:isDefinedBy <http://data.europa.eu/a4g/ontology> ;
  rdfs:label "The proposed subcontractor(s) necessary to fulfill the obligation to subcontract a minimum percentage of the contract"@en ;
  skos:inScheme <http://publications.europa.eu/resource/authority/Subcontracting-indication> ;
  skos:prefLabel "The proposed subcontractor(s) necessary to fulfill the obligation to subcontract a minimum percentage of the contract"@en ;
.
epo:Pub-info-post
  rdf:type skos:Concept ;
  rdfs:isDefinedBy <http://data.europa.eu/a4g/ontology> ;
  rdfs:label "Publication of information which was originally postponed for reasons of law enforcement, commercial interests of an economic operator, fair competition or other public interest"@en ;
  skos:inScheme epo:Notice-corrigendum-justification ;
  skos:prefLabel "Publication of information which was originally postponed for reasons of law enforcement, commercial interests of an economic operator, fair competition or other public interest"@en ;
.
epo:Pub-os
  rdf:type skos:Concept ;
  rdfs:isDefinedBy <http://data.europa.eu/a4g/ontology> ;
  rdfs:label "Public order and safety"@en ;
  skos:inScheme <http://publications.europa.eu/resource/authority/Main-activity> ;
  skos:prefLabel "Public order and safety"@en ;
.
epo:Pub-undert
  rdf:type skos:Concept ;
  rdfs:isDefinedBy <http://data.europa.eu/a4g/ontology> ;
  rdfs:label "Public undertaking"@en ;
  skos:inScheme <http://publications.europa.eu/resource/authority/Buyer-legal-type> ;
  skos:prefLabel "Public undertaking"@en ;
.
epo:Pub-undert-cga
  rdf:type skos:Concept ;
  rdfs:isDefinedBy <http://data.europa.eu/a4g/ontology> ;
  rdfs:label "Public undertaking, controlled by a central government authority"@en ;
  skos:inScheme <http://publications.europa.eu/resource/authority/Buyer-legal-type> ;
  skos:prefLabel "Public undertaking, controlled by a central government authority"@en ;
.
epo:Pub-undert-la
  rdf:type skos:Concept ;
  rdfs:isDefinedBy <http://data.europa.eu/a4g/ontology> ;
  rdfs:label "Public undertaking, controlled by a local authority"@en ;
  skos:inScheme <http://publications.europa.eu/resource/authority/Buyer-legal-type> ;
  skos:prefLabel "Public undertaking, controlled by a local authority"@en ;
.
epo:Pub-undert-ra
  rdf:type skos:Concept ;
  rdfs:isDefinedBy <http://data.europa.eu/a4g/ontology> ;
  rdfs:label "Public undertaking, controlled by a regional authority"@en ;
  skos:inScheme <http://publications.europa.eu/resource/authority/Buyer-legal-type> ;
  skos:prefLabel "Public undertaking, controlled by a regional authority"@en ;
.
epo:PublicOrganisation
  rdf:type owl:Class ;
  rdfs:comment """A body governed by public law:
- (a) established for the specific purpose of meeting needs in the general interest
- (b) having legal personality; 
- (c) financed, for the most part by the State, or regional or local authorities. 

Additional information: 
Examples of Public Organisations are municipality, international public body, ministry, others.

WG Approval 28/04/2020"""@en ;
  rdfs:isDefinedBy <http://data.europa.eu/a4g/ontology> ;
  rdfs:label "Public organisation"@en ;
  rdfs:subClassOf epo:FormalOrganisation ;
  owl:disjointWith epo:RegisteredOrganisation ;
  skos:definition """A body governed by public law:
- (a) established for the specific purpose of meeting needs in the general interest
- (b) having legal personality; 
- (c) financed, for the most part by the State, or regional or local authorities. 

Additional information: 
Examples of Public Organisations are municipality, international public body, ministry, others.

WG Approval 28/04/2020"""@en ;
  skos:prefLabel "Public organisation"@en ;
.
epo:PublicationProvision
  rdf:type owl:Class ;
  rdfs:comment """Information about fields not intended for publication. 


Additional Information:
The non-published information may become available at a later date and may differ from one element to another within a given document.

Examples of fields that may not be immediately published are Winner, Tender and Procedure Lot Result, etc., e.g. for security reasons.

WG Approval 16/05/2019




"""@en ;
  rdfs:isDefinedBy <http://data.europa.eu/a4g/ontology> ;
  rdfs:label "Publication provision"@en ;
  skos:definition """Information about fields not intended for publication. 


Additional Information:
The non-published information may become available at a later date and may differ from one element to another within a given document.

Examples of fields that may not be immediately published are Winner, Tender and Procedure Lot Result, etc., e.g. for security reasons.

WG Approval 16/05/2019




"""@en ;
  skos:prefLabel "Publication provision"@en ;
.
epo:Pur-liq-insol
  rdf:type skos:Concept ;
  rdfs:isDefinedBy <http://data.europa.eu/a4g/ontology> ;
  rdfs:label "Purchase on particularly advantageous terms from the liquidator in an insolvency procedure, an arrangement with creditors or a similar procedure under national laws and regulations"@en ;
  skos:inScheme <http://publications.europa.eu/resource/authority/Direct-award-justification> ;
  skos:prefLabel "Purchase on particularly advantageous terms from the liquidator in an insolvency procedure, an arrangement with creditors or a similar procedure under national laws and regulations"@en ;
.
epo:Pur-ope-wind
  rdf:type skos:Concept ;
  rdfs:isDefinedBy <http://data.europa.eu/a4g/ontology> ;
  rdfs:label "Purchase on particularly advantageous terms from an economic operator which is definitely winding up its business activities"@en ;
  skos:inScheme <http://publications.europa.eu/resource/authority/Direct-award-justification> ;
  skos:prefLabel "Purchase on particularly advantageous terms from an economic operator which is definitely winding up its business activities"@en ;
.
epo:PurchaseContract
  rdf:type owl:Class ;
  rdfs:comment "A contract resulting from a Dynamic Purchasing System or Framework Agreement Contract."@en ;
  rdfs:isDefinedBy <http://data.europa.eu/a4g/ontology> ;
  rdfs:label "Purchase contract"@en ;
  rdfs:subClassOf epo:Contract ;
  owl:disjointWith epo:FrameworkAgreement ;
  skos:definition "A contract resulting from a Dynamic Purchasing System or Framework Agreement Contract."@en ;
  skos:prefLabel "Purchase contract"@en ;
.
epo:Purpose
  rdf:type owl:Class ;
  rdfs:comment """The description of the objectives related to a procurement. 

Additional information:

The description of the objectives includes the subject matter and quantities.


The quantification of the objectives related to a procurement.

To be re-reviewed by the WG the soonest.

(WG to be discussed, this was pointed out on the 09/04/2019 14:38:25 WG Meeting)

The old definition read as follows:

The description of the objectives related to a procurement.

(WG approval 05/12/2018)
"""@en ;
  rdfs:isDefinedBy <http://data.europa.eu/a4g/ontology> ;
  rdfs:label "Purpose"@en ;
  skos:definition """The description of the objectives related to a procurement. 

Additional information:

The description of the objectives includes the subject matter and quantities.


The quantification of the objectives related to a procurement.

To be re-reviewed by the WG the soonest.

(WG to be discussed, this was pointed out on the 09/04/2019 14:38:25 WG Meeting)

The old definition read as follows:

The description of the objectives related to a procurement.

(WG approval 05/12/2018)
"""@en ;
  skos:prefLabel "Purpose"@en ;
.
epo:QUALITY
  rdf:type skos:Concept ;
  rdfs:isDefinedBy <http://data.europa.eu/a4g/ontology> ;
  rdfs:label "Q u a l i t y"@en ;
  skos:inScheme epo:Award-dimension-parent-criterion-relation ;
  skos:prefLabel "Q u a l i t y"@en ;
.
epo:QUARTER
  rdf:type skos:Concept ;
  rdfs:isDefinedBy <http://data.europa.eu/a4g/ontology> ;
  rdfs:label "Quarter"@en ;
  skos:inScheme <http://publications.europa.eu/resource/authority/Timeperiods> ;
  skos:prefLabel "Quarter"@en ;
.
epo:QualificationSystem
  rdf:type owl:Class ;
  rdfs:isDefinedBy <http://data.europa.eu/a4g/ontology> ;
  rdfs:label "Qualification system"@en ;
  skos:prefLabel "Qualification system"@en ;
.
epo:Quality
  rdf:type skos:Concept ;
  rdfs:isDefinedBy <http://data.europa.eu/a4g/ontology> ;
  rdfs:label "Quality"@en ;
  skos:inScheme <http://publications.europa.eu/resource/authority/Award-criterion-type> ;
  skos:prefLabel "Quality"@en ;
.
epo:Quantity
  rdf:type rdfs:Datatype ;
  rdf:type owl:Class ;
  rdfs:isDefinedBy <http://data.europa.eu/a4g/ontology> ;
  rdfs:label "Quantity"@en ;
  rdfs:subClassOf <http://www.unece.org/cefact#Quantity> ;
  skos:prefLabel "Quantity"@en ;
.
epo:RA
  rdf:type skos:Concept ;
  rdfs:isDefinedBy <http://data.europa.eu/a4g/ontology> ;
  rdfs:label "Regional Authority"@en ;
  skos:inScheme epo:Authority-type ;
  skos:prefLabel "Regional Authority"@en ;
.
epo:REGULAR_BOARD
  rdf:type skos:Concept ;
  rdfs:isDefinedBy <http://data.europa.eu/a4g/ontology> ;
  rdfs:label "R e g u l a r_ b o a r d"@en ;
  skos:inScheme epo:Evaluation-group-type ;
  skos:prefLabel "R e g u l a r_ b o a r d"@en ;
.
epo:REQUEST_FOR_CLARIFICATION
  rdf:type skos:Concept ;
  rdfs:isDefinedBy <http://data.europa.eu/a4g/ontology> ;
  rdfs:label "R e q u e s t_ f o r_ c l a r i f i c a t i o n"@en ;
  skos:inScheme epo:Submission-document-type ;
  skos:prefLabel "R e q u e s t_ f o r_ c l a r i f i c a t i o n"@en ;
.
epo:REQUEST_FOR_PARTICIPATION
  rdf:type skos:Concept ;
  rdfs:isDefinedBy <http://data.europa.eu/a4g/ontology> ;
  rdfs:label "R e q u e s t_ f o r_ p a r t i c i p a t i o n"@en ;
  skos:inScheme epo:Submission-document-type ;
  skos:prefLabel "R e q u e s t_ f o r_ p a r t i c i p a t i o n"@en ;
.
epo:RESTRICTED
  rdf:type skos:Concept ;
  rdfs:isDefinedBy <http://data.europa.eu/a4g/ontology> ;
  rdfs:label "Information and material the unauthorised disclosure of which could be disadvantageous to the interests of the European Union, of one or more of the Member States or of one or more parties participating in a Procedure."@en ;
  rdfs:label "R e s t r i c t e d"@en ;
  skos:inScheme epo:Design-contest-type ;
  skos:inScheme <https://github.com/ESPD/ESPD-EDM/Confidentiality-level> ;
  skos:prefLabel "Information and material the unauthorised disclosure of which could be disadvantageous to the interests of the European Union, of one or more of the Member States or of one or more parties participating in a Procedure."@en ;
  skos:prefLabel "R e s t r i c t e d"@en ;
.
epo:RESULTCAN
  rdf:type skos:Concept ;
  rdfs:isDefinedBy <http://data.europa.eu/a4g/ontology> ;
  rdfs:label "R e s u l t c a n"@en ;
  skos:inScheme epo:Notification-phases-content-types ;
  skos:prefLabel "R e s u l t c a n"@en ;
.
epo:Ra
  rdf:type skos:Concept ;
  rdfs:isDefinedBy <http://data.europa.eu/a4g/ontology> ;
  rdfs:label "Regional authority"@en ;
  skos:inScheme <http://publications.europa.eu/resource/authority/Buyer-legal-type> ;
  skos:prefLabel "Regional authority"@en ;
.
epo:Recepient
  rdf:type skos:Concept ;
  rdfs:isDefinedBy <http://data.europa.eu/a4g/ontology> ;
  rdfs:label "Organisation receiving tenders"@en ;
  skos:inScheme epo:Function-taxonomy ;
  skos:prefLabel "Organisation receiving tenders"@en ;
.
epo:Red-env-imp
  rdf:type skos:Concept ;
  rdfs:isDefinedBy <http://data.europa.eu/a4g/ontology> ;
  rdfs:label "Reduction of environmental impacts"@en ;
  skos:inScheme <http://publications.europa.eu/resource/authority/Strategic-procurement> ;
  skos:prefLabel "Reduction of environmental impacts"@en ;
.
epo:RegisteredOrganisation
  rdf:type owl:Class ;
  rdfs:comment """An organization that gains legal entity status by the act of registration cf. org:FormalOrganization 
"""@en ;
  rdfs:isDefinedBy <http://data.europa.eu/a4g/ontology> ;
  rdfs:label "Registered organisation"@en ;
  rdfs:subClassOf epo:FormalOrganisation ;
  rdfs:subClassOf org:FormalOrganization ;
  owl:disjointWith epo:FormalOrganisation ;
  owl:disjointWith epo:PublicOrganisation ;
  skos:definition """An organization that gains legal entity status by the act of registration cf. org:FormalOrganization 
"""@en ;
  skos:prefLabel "Registered organisation"@en ;
.
epo:Rep-ext-dir
  rdf:type skos:Concept ;
  rdfs:isDefinedBy <http://data.europa.eu/a4g/ontology> ;
  rdfs:label "Partial replacement or extension of existing supplies or installations by the original supplier ordered under the strict conditions stated in the Directive"@en ;
  skos:inScheme <http://publications.europa.eu/resource/authority/Direct-award-justification> ;
  skos:prefLabel "Partial replacement or extension of existing supplies or installations by the original supplier ordered under the strict conditions stated in the Directive"@en ;
.
epo:Rep-work-dir
  rdf:type skos:Concept ;
  rdfs:isDefinedBy <http://data.europa.eu/a4g/ontology> ;
  rdfs:label "New works or services, constituting a repetition of existing works or services and ordered in accordance with the strict conditions stated in the Directive"@en ;
  skos:inScheme <http://publications.europa.eu/resource/authority/Direct-award-justification> ;
  skos:prefLabel "New works or services, constituting a repetition of existing works or services and ordered in accordance with the strict conditions stated in the Directive"@en ;
.
epo:Req-proc
  rdf:type skos:Concept ;
  rdfs:isDefinedBy <http://data.europa.eu/a4g/ontology> ;
  rdfs:label "Organisation processing requests to participate"@en ;
  skos:inScheme epo:Function-taxonomy ;
  skos:prefLabel "Organisation processing requests to participate"@en ;
.
epo:Req-recep
  rdf:type skos:Concept ;
  rdfs:isDefinedBy <http://data.europa.eu/a4g/ontology> ;
  rdfs:label "Organisation receiving requests to participate"@en ;
  skos:inScheme epo:Function-taxonomy ;
  skos:prefLabel "Organisation receiving requests to participate"@en ;
.
epo:RequestForParticipation
  rdf:type owl:Class ;
  rdfs:isDefinedBy <http://data.europa.eu/a4g/ontology> ;
  rdfs:label "Request for participation"@en ;
  rdfs:subClassOf epo:Document ;
  owl:disjointWith epo:Contract ;
  owl:disjointWith epo:Notice ;
  owl:disjointWith epo:ProcurementDocument ;
  owl:disjointWith epo:TenderDocument ;
  skos:prefLabel "Request for participation"@en ;
.
epo:Required
  rdf:type skos:Concept ;
  rdfs:isDefinedBy <http://data.europa.eu/a4g/ontology> ;
  rdfs:label "Required"@en ;
  skos:inScheme <http://publications.europa.eu/resource/authority/Permission> ;
  skos:prefLabel "Required"@en ;
.
epo:Res-exp-stu-dev
  rdf:type skos:Concept ;
  rdfs:isDefinedBy <http://data.europa.eu/a4g/ontology> ;
  rdfs:label "Purpose of the contract is purely research, experiment, study or development under the conditions stated in the Directive"@en ;
  skos:inScheme <http://publications.europa.eu/resource/authority/Direct-award-justification> ;
  skos:prefLabel "Purpose of the contract is purely research, experiment, study or development under the conditions stated in the Directive"@en ;
.
epo:Res-pub-ser-rel
  rdf:type skos:Concept ;
  rdfs:isDefinedBy <http://data.europa.eu/a4g/ontology> ;
  rdfs:label "Participation is reserved to organisations pursuing a public service mission and fulfilling other relevant conditions in the legislation."@en ;
  skos:inScheme <http://publications.europa.eu/resource/authority/Reserved-procurement> ;
  skos:prefLabel "Participation is reserved to organisations pursuing a public service mission and fulfilling other relevant conditions in the legislation."@en ;
.
epo:Res-she-ws
  rdf:type skos:Concept ;
  rdfs:isDefinedBy <http://data.europa.eu/a4g/ontology> ;
  rdfs:label "Participation is reserved to sheltered workshops and economic operators aiming at the social and professional integration of disabled or disadvantaged persons."@en ;
  skos:inScheme <http://publications.europa.eu/resource/authority/Reserved-procurement> ;
  skos:prefLabel "Participation is reserved to sheltered workshops and economic operators aiming at the social and professional integration of disabled or disadvantaged persons."@en ;
.
epo:ResourceElement
  rdf:type owl:Class ;
  rdfs:comment """Reference to a semantic building block necessary to describe a specific concept. 

Addtional Information:

A building block may be a basic core component (e.g. Receipt Deadline, a property of type DateTime, in the class Submission Terms) or an aggregate component (e.g. Submission Terms, a class in the ontology).

WG Approval 23/05/2019"""@en ;
  rdfs:isDefinedBy <http://data.europa.eu/a4g/ontology> ;
  rdfs:label "Resource element"@en ;
  skos:definition """Reference to a semantic building block necessary to describe a specific concept. 

Addtional Information:

A building block may be a basic core component (e.g. Receipt Deadline, a property of type DateTime, in the class Submission Terms) or an aggregate component (e.g. Submission Terms, a class in the ontology).

WG Approval 23/05/2019"""@en ;
  skos:prefLabel "Resource element"@en ;
.
epo:Restricted
  rdf:type skos:Concept ;
  rdfs:isDefinedBy <http://data.europa.eu/a4g/ontology> ;
  rdfs:label "Restricted"@en ;
  skos:inScheme <http://publications.europa.eu/resource/authority/Procurement-procedure-type> ;
  skos:prefLabel "Restricted"@en ;
.
epo:Result
  rdf:type skos:Concept ;
  rdfs:isDefinedBy <http://data.europa.eu/a4g/ontology> ;
  rdfs:label "Result"@en ;
  skos:inScheme epo:Form-type ;
  skos:prefLabel "Result"@en ;
.
epo:Rev-body
  rdf:type skos:Concept ;
  rdfs:isDefinedBy <http://data.europa.eu/a4g/ontology> ;
  rdfs:label "Decision of a review body or another judicial body"@en ;
  skos:inScheme <http://publications.europa.eu/resource/authority/Non-award-justification> ;
  skos:prefLabel "Decision of a review body or another judicial body"@en ;
.
epo:Rev-buyer
  rdf:type skos:Concept ;
  rdfs:isDefinedBy <http://data.europa.eu/a4g/ontology> ;
  rdfs:label "Decision of the buyer following a tenderer's request to review the award"@en ;
  skos:inScheme <http://publications.europa.eu/resource/authority/Non-award-justification> ;
  skos:prefLabel "Decision of the buyer following a tenderer's request to review the award"@en ;
.
epo:ReviewTerms
  rdf:type owl:Class ;
  rdfs:comment """Conditions and stipulations defining particularities of the review.

(WG approval 23/11/2018)
"""@en ;
  rdfs:isDefinedBy <http://data.europa.eu/a4g/ontology> ;
  rdfs:label "Review terms"@en ;
  skos:definition """Conditions and stipulations defining particularities of the review.

(WG approval 23/11/2018)
"""@en ;
  skos:prefLabel "Review terms"@en ;
.
epo:Reviewer
  rdf:type skos:Concept ;
  rdfs:isDefinedBy <http://data.europa.eu/a4g/ontology> ;
  rdfs:label "Reviewer"@en ;
  skos:inScheme epo:Function-taxonomy ;
  skos:prefLabel "Reviewer"@en ;
.
epo:Role
  rdf:type owl:Class ;
  rdfs:comment """A part played by an agent in a particular business process.
<foreign otherprops=\"#333333\">
</foreign>Additional information
In ePO, the 'business processes' related to procurement can be 'purchasing', 'tendering', 'evaluating', 'awarding', 'ordering', 'invoicing', etc. 

The concept of 'role' is different from the concept of 'function'. However, functions can be carried out by procurement-related roles and other domain-related agents. Please refer to the class 'Function' to see the difference.
"""@en ;
  rdfs:isDefinedBy <http://data.europa.eu/a4g/ontology> ;
  rdfs:label "Role"@en ;
  skos:definition """A part played by an agent in a particular business process.
<foreign otherprops=\"#333333\">
</foreign>Additional information
In ePO, the 'business processes' related to procurement can be 'purchasing', 'tendering', 'evaluating', 'awarding', 'ordering', 'invoicing', etc. 

The concept of 'role' is different from the concept of 'function'. However, functions can be carried out by procurement-related roles and other domain-related agents. Please refer to the class 'Function' to see the difference.
"""@en ;
  skos:prefLabel "Role"@en ;
.
epo:SAT
  rdf:type skos:Concept ;
  rdfs:isDefinedBy <http://data.europa.eu/a4g/ontology> ;
  rdfs:label "Saturday"@en ;
  skos:inScheme <http://publications.europa.eu/resource/authority/Timeperiods> ;
  skos:prefLabel "Saturday"@en ;
.
epo:SC
  rdf:type skos:Concept ;
  rdfs:isDefinedBy <http://data.europa.eu/a4g/ontology> ;
  rdfs:label "Sole Contractor"@en ;
  skos:inScheme epo:Function-taxonomy ;
  skos:prefLabel "Sole Contractor"@en ;
.
epo:SCA
  rdf:type skos:Concept ;
  rdfs:isDefinedBy <http://data.europa.eu/a4g/ontology> ;
  rdfs:label "Subcentral Government Authority"@en ;
  skos:inScheme epo:Authority-type ;
  skos:prefLabel "Subcentral Government Authority"@en ;
.
epo:SEC
  rdf:type skos:Concept ;
  rdfs:isDefinedBy <http://data.europa.eu/a4g/ontology> ;
  rdfs:label "(_S|Second)(_P|Seconds)"@en ;
  skos:inScheme <http://publications.europa.eu/resource/authority/Timeperiods> ;
  skos:prefLabel "(_S|Second)(_P|Seconds)"@en ;
.
epo:SECRET
  rdf:type skos:Concept ;
  rdfs:isDefinedBy <http://data.europa.eu/a4g/ontology> ;
  rdfs:label "Information and material the unauthorised disclosure of which could seriously harm the essential interests of the European Union, of one or more of the Member States or of one or more parties participating in a Procedure."@en ;
  skos:inScheme <https://github.com/ESPD/ESPD-EDM/Confidentiality-level> ;
  skos:prefLabel "Information and material the unauthorised disclosure of which could seriously harm the essential interests of the European Union, of one or more of the Member States or of one or more parties participating in a Procedure."@en ;
.
epo:SEP
  rdf:type skos:Concept ;
  rdfs:isDefinedBy <http://data.europa.eu/a4g/ontology> ;
  rdfs:label "September"@en ;
  skos:inScheme <http://publications.europa.eu/resource/authority/Timeperiods> ;
  skos:prefLabel "September"@en ;
.
epo:SOCIAL_SPECIFIC_SERVICES
  rdf:type skos:Concept ;
  rdfs:isDefinedBy <http://data.europa.eu/a4g/ontology> ;
  rdfs:label "Social an other specific services"@en ;
  skos:inScheme epo:Procurement-regime-type ;
  skos:prefLabel "Social an other specific services"@en ;
.
epo:SPRING
  rdf:type skos:Concept ;
  rdfs:isDefinedBy <http://data.europa.eu/a4g/ontology> ;
  rdfs:label "Spring"@en ;
  skos:inScheme <http://publications.europa.eu/resource/authority/Timeperiods> ;
  skos:prefLabel "Spring"@en ;
.
epo:ST
  rdf:type skos:Concept ;
  rdfs:isDefinedBy <http://data.europa.eu/a4g/ontology> ;
  rdfs:label "Sole Tenderer"@en ;
  skos:inScheme epo:Function-taxonomy ;
  skos:prefLabel "Sole Tenderer"@en ;
.
epo:STATE_OF_URGENCY
  rdf:type skos:Concept ;
  rdfs:isDefinedBy <http://data.europa.eu/a4g/ontology> ;
  rdfs:label "State of Urgency"@en ;
  skos:inScheme epo:Accelerated-procedure-justification-type ;
  skos:prefLabel "State of Urgency"@en ;
.
epo:SUBCONTRACTOR
  rdf:type skos:Concept ;
  rdfs:isDefinedBy <http://data.europa.eu/a4g/ontology> ;
  rdfs:label "S u b c o n t r a c t o r"@en ;
  skos:inScheme epo:Security-clearance-address ;
  skos:prefLabel "S u b c o n t r a c t o r"@en ;
.
epo:SUMMER
  rdf:type skos:Concept ;
  rdfs:isDefinedBy <http://data.europa.eu/a4g/ontology> ;
  rdfs:label "Summer"@en ;
  skos:inScheme <http://publications.europa.eu/resource/authority/Timeperiods> ;
  skos:prefLabel "Summer"@en ;
.
epo:SUN
  rdf:type skos:Concept ;
  rdfs:isDefinedBy <http://data.europa.eu/a4g/ontology> ;
  rdfs:label "Sunday"@en ;
  skos:inScheme <http://publications.europa.eu/resource/authority/Timeperiods> ;
  skos:prefLabel "Sunday"@en ;
.
epo:Security-clearance-address
  rdf:type skos:ConceptScheme ;
  rdfs:comment "We cannot have direct properties pointing at descendant roles of the class Agent, because at the notification time many of them do not exist yet."@en ;
  rdfs:isDefinedBy <http://data.europa.eu/a4g/ontology> ;
  rdfs:label "Security-clearance-address"@en ;
  skos:definition "We cannot have direct properties pointing at descendant roles of the class Agent, because at the notification time many of them do not exist yet."@en ;
  skos:prefLabel "Security-clearance-address" ;
.
epo:SecurityClearanceTerms
  rdf:type owl:Class ;
  rdfs:comment """Status requested to individuals allowing them access to classified information (state or organisational secrets) or to restricted areas, after completion of a thorough background check.

WG Approval 2015-02-26
"""@en ;
  rdfs:isDefinedBy <http://data.europa.eu/a4g/ontology> ;
  rdfs:label "Security clearance terms"@en ;
  skos:definition """Status requested to individuals allowing them access to classified information (state or organisational secrets) or to restricted areas, after completion of a thorough background check.

WG Approval 2015-02-26
"""@en ;
  skos:prefLabel "Security clearance terms"@en ;
.
epo:Selec-w
  rdf:type skos:Concept ;
  rdfs:isDefinedBy <http://data.europa.eu/a4g/ontology> ;
  rdfs:label "The winner was chosen"@en ;
  skos:inScheme <http://publications.europa.eu/resource/authority/Winner-selection-status> ;
  skos:prefLabel "The winner was chosen"@en ;
.
epo:SelectionCriterion
  rdf:type owl:Class ;
  rdf:type skos:Concept ;
  rdfs:comment """Describes a capacity requirement that the economic operator needs to fulfill to participate in the procedure.

WG approval 31/10/2018"""@en ;
  rdfs:isDefinedBy <http://data.europa.eu/a4g/ontology> ;
  rdfs:label "Selection criterion"@en ;
  rdfs:subClassOf epo:ProcurementCriterion ;
  owl:disjointWith epo:AwardCriterion ;
  owl:disjointWith epo:ExclusionGround ;
  skos:definition """Describes a capacity requirement that the economic operator needs to fulfill to participate in the procedure.

WG approval 31/10/2018"""@en ;
  skos:inScheme epo:E-evaluation-criterion-type ;
  skos:prefLabel "Selection criterion"@en ;
.
epo:Sen-info
  rdf:type skos:Concept ;
  rdfs:isDefinedBy <http://data.europa.eu/a4g/ontology> ;
  rdfs:label "Protection of particularly sensitive information"@en ;
  skos:inScheme <http://publications.europa.eu/resource/authority/Communication-justification> ;
  skos:prefLabel "Protection of particularly sensitive information"@en ;
.
epo:Services
  rdf:type skos:Concept ;
  rdfs:isDefinedBy <http://data.europa.eu/a4g/ontology> ;
  rdfs:label "Services"@en ;
  skos:inScheme <http://publications.europa.eu/resource/authority/Contract-nature> ;
  skos:prefLabel "Services"@en ;
.
epo:Share-subc
  rdf:type skos:Concept ;
  rdfs:isDefinedBy <http://data.europa.eu/a4g/ontology> ;
  rdfs:label "The share of the contract that the tenderer intends to subcontract"@en ;
  skos:inScheme <http://publications.europa.eu/resource/authority/Subcontracting-indication> ;
  skos:prefLabel "The share of the contract that the tenderer intends to subcontract"@en ;
.
epo:Signatory
  rdf:type skos:Concept ;
  rdfs:isDefinedBy <http://data.europa.eu/a4g/ontology> ;
  rdfs:label "Organisation signing the contract"@en ;
  skos:inScheme epo:Function-taxonomy ;
  skos:prefLabel "Organisation signing the contract"@en ;
.
epo:Size
  rdf:type skos:ConceptScheme ;
  rdfs:isDefinedBy <http://data.europa.eu/a4g/ontology> ;
  rdfs:label "Size"@en ;
  skos:prefLabel "Size" ;
.
epo:Small
  rdf:type skos:Concept ;
  rdfs:comment "Fewer than 50 persons and whose annual turnover and/or annual balance sheet total does not exceed EUR 10 million."@en ;
  rdfs:isDefinedBy <http://data.europa.eu/a4g/ontology> ;
  rdfs:label "Small enterprise"@en ;
  skos:definition "Fewer than 50 persons and whose annual turnover and/or annual balance sheet total does not exceed EUR 10 million."@en ;
  skos:inScheme <http://publications.europa.eu/resource/authority/Economic-operator-size> ;
  skos:prefLabel "Small enterprise"@en ;
.
epo:Sme
  rdf:type skos:Concept ;
  rdfs:isDefinedBy <http://data.europa.eu/a4g/ontology> ;
  rdfs:label "Micro, small, or medium"@en ;
  skos:inScheme <http://publications.europa.eu/resource/authority/Economic-operator-size> ;
  skos:prefLabel "Micro, small, or medium"@en ;
.
epo:SocialProcurement
  rdf:type owl:Class ;
  rdfs:comment """An instance of the class SocialProcurement  is represented in eForms with the code \"soc-obj\" defined in the codelist strategic-procurement.


Research (21/01/2020): 
Socially responsible public procurement (SRPP):

‘SRPP’ means procurement operations that take into account one or more of the following social considerations: employment opportunities, decent work, compliance with social and labour rights, social inclusion (including persons with disabilities), equal opportunities, accessibility design for all, taking account of sustainability criteria, including ethical trade issues and wider voluntary compliance with corporate social responsibility (CSR), while observing the principles enshrined in the Treaty for the European Union (TFEU) and the Procurement Directives. 
Source: Buying Social - A Guide to Taking Account of Social Considerations in Public Procurement (Publications Office of the European Union, 2011) https://op.europa.eu/en/publication-detail/-/publication/cb70c481-0e29-4040-9be2-c408cddf081f/language-en
See Article 18 and Annex X Directive 2014/24."""@en ;
  rdfs:isDefinedBy <http://data.europa.eu/a4g/ontology> ;
  rdfs:label "Social procurement"@en ;
  rdfs:subClassOf epo:StrategicProcurement ;
  owl:disjointWith epo:GreenProcurement ;
  owl:disjointWith epo:InnovativeProcurement ;
  skos:definition """An instance of the class SocialProcurement  is represented in eForms with the code \"soc-obj\" defined in the codelist strategic-procurement.


Research (21/01/2020): 
Socially responsible public procurement (SRPP):

‘SRPP’ means procurement operations that take into account one or more of the following social considerations: employment opportunities, decent work, compliance with social and labour rights, social inclusion (including persons with disabilities), equal opportunities, accessibility design for all, taking account of sustainability criteria, including ethical trade issues and wider voluntary compliance with corporate social responsibility (CSR), while observing the principles enshrined in the Treaty for the European Union (TFEU) and the Procurement Directives. 
Source: Buying Social - A Guide to Taking Account of Social Considerations in Public Procurement (Publications Office of the European Union, 2011) https://op.europa.eu/en/publication-detail/-/publication/cb70c481-0e29-4040-9be2-c408cddf081f/language-en
See Article 18 and Annex X Directive 2014/24."""@en ;
  skos:prefLabel "Social procurement"@en ;
.
epo:Sp-of-eq
  rdf:type skos:Concept ;
  rdfs:isDefinedBy <http://data.europa.eu/a4g/ontology> ;
  rdfs:label "Buyer would need specialised office equipment"@en ;
  skos:inScheme <http://publications.europa.eu/resource/authority/Communication-justification> ;
  skos:prefLabel "Buyer would need specialised office equipment"@en ;
.
epo:Spec-rights-entity
  rdf:type skos:Concept ;
  rdfs:isDefinedBy <http://data.europa.eu/a4g/ontology> ;
  rdfs:label "Entity with special or exclusive rights"@en ;
  skos:inScheme <http://publications.europa.eu/resource/authority/Buyer-legal-type> ;
  skos:prefLabel "Entity with special or exclusive rights"@en ;
.
epo:Standard
  rdf:type skos:Concept ;
  rdfs:isDefinedBy <http://data.europa.eu/a4g/ontology> ;
  rdfs:label "Set of principles and rules for procedures in general"@en ;
  skos:inScheme epo:Legal-regime ;
  skos:prefLabel "Set of principles and rules for procedures in general"@en ;
.
epo:StatisticalInformation
  rdf:type owl:Class ;
  rdfs:comment """Statistical data on the procedure and the lot. 

Additional Information

At the present time Procurement Procedures are not fully electronic. At a later date, information on the tenders received could be inferred by the data in the eProcurement system.
Therefore this class is temporal and should cease to exist in fully electronic procurement.
The need for its presence responds also to the alignment with the Regulation (EU) 2019/1780 (eForms).

Attention will have to be paid in the future to possible inconsistencies derived from data placed in other classes and data held in the Statistical Information class; e.g. the TenderEvaluation class (see eEvaluation diagram) has the attribute admissibileTender indicator, which in case of being false, may enter in contradiction with the highest or lowest tender value for that very same inadmissible tender.

WG Approval 12/12/2019
"""@en ;
  rdfs:isDefinedBy <http://data.europa.eu/a4g/ontology> ;
  rdfs:label "Statistical information"@en ;
  skos:definition """Statistical data on the procedure and the lot. 

Additional Information

At the present time Procurement Procedures are not fully electronic. At a later date, information on the tenders received could be inferred by the data in the eProcurement system.
Therefore this class is temporal and should cease to exist in fully electronic procurement.
The need for its presence responds also to the alignment with the Regulation (EU) 2019/1780 (eForms).

Attention will have to be paid in the future to possible inconsistencies derived from data placed in other classes and data held in the Statistical Information class; e.g. the TenderEvaluation class (see eEvaluation diagram) has the attribute admissibileTender indicator, which in case of being false, may enter in contradiction with the highest or lowest tender value for that very same inadmissible tender.

WG Approval 12/12/2019
"""@en ;
  skos:prefLabel "Statistical information"@en ;
.
epo:StrategicProcurement
  rdf:type owl:Class ;
  rdfs:comment """Public procurement that contributes to achieving pressing policy goals.

Additional Information:
Specific strategic goals could be, for example, environmental protection, innovation, job creation and the development of small and medium enterprises.

Based on https://legalinstruments.oecd.org/en/instruments/OECD-LEGAL-0411 (see paragraph on \"background information\".

WG Approval 10/03/2020"""@en ;
  rdfs:isDefinedBy <http://data.europa.eu/a4g/ontology> ;
  rdfs:label "Strategic procurement"@en ;
  skos:definition """Public procurement that contributes to achieving pressing policy goals.

Additional Information:
Specific strategic goals could be, for example, environmental protection, innovation, job creation and the development of small and medium enterprises.

Based on https://legalinstruments.oecd.org/en/instruments/OECD-LEGAL-0411 (see paragraph on \"background information\".

WG Approval 10/03/2020"""@en ;
  skos:prefLabel "Strategic procurement"@en ;
.
epo:Subcontract
  rdf:type owl:Class ;
  rdfs:comment """A contract between a contractor of an original contract and another economic operator to fulfil the original contract.

WG Approval 07/05/2019"""@en ;
  rdfs:isDefinedBy <http://data.europa.eu/a4g/ontology> ;
  rdfs:label "Subcontract"@en ;
  skos:definition """A contract between a contractor of an original contract and another economic operator to fulfil the original contract.

WG Approval 07/05/2019"""@en ;
  skos:prefLabel "Subcontract"@en ;
.
epo:SubcontractTerms
  rdf:type owl:Class ;
  rdfs:comment "A concept to describe the main information regarding the share of parts of the contract to third parties."@en ;
  rdfs:isDefinedBy <http://data.europa.eu/a4g/ontology> ;
  rdfs:label "Subcontract terms"@en ;
  skos:definition "A concept to describe the main information regarding the share of parts of the contract to third parties."@en ;
  skos:prefLabel "Subcontract terms"@en ;
.
epo:Subcontractor
  rdf:type owl:Class ;
  rdfs:comment """An individual or a business that has an agreement to perform part or all of the obligations of another contractor's contract. 

Additional information

For some procedures, the subcontractor signs as well the contract between the buyer and the contractor.

At tendering time, entities relied upon by the economic operators can be subcontractors or not. 

When modelling ESPD we well analyse whether we need or not a role named \"relied upon\"."""@en ;
  rdfs:isDefinedBy <http://data.europa.eu/a4g/ontology> ;
  rdfs:label "Subcontractor"@en ;
  rdfs:subClassOf epo:EconomicOperator ;
  owl:disjointWith epo:Tenderer ;
  skos:definition """An individual or a business that has an agreement to perform part or all of the obligations of another contractor's contract. 

Additional information

For some procedures, the subcontractor signs as well the contract between the buyer and the contractor.

At tendering time, entities relied upon by the economic operators can be subcontractors or not. 

When modelling ESPD we well analyse whether we need or not a role named \"relied upon\"."""@en ;
  skos:prefLabel "Subcontractor"@en ;
.
epo:Subj-subc-noblig
  rdf:type skos:Concept ;
  rdfs:isDefinedBy <http://data.europa.eu/a4g/ontology> ;
  rdfs:label "The subject-matter of the subcontract(s) above any obligation to subcontract a minimum percentage of the contract"@en ;
  skos:inScheme <http://publications.europa.eu/resource/authority/Subcontracting-indication> ;
  skos:prefLabel "The subject-matter of the subcontract(s) above any obligation to subcontract a minimum percentage of the contract"@en ;
.
epo:Subj-subc-oblig
  rdf:type skos:Concept ;
  rdfs:isDefinedBy <http://data.europa.eu/a4g/ontology> ;
  rdfs:label "The subject-matter of the subcontract(s) necessary to fulfill the obligation to subcontract a minimum percentage of the contract"@en ;
  skos:inScheme <http://publications.europa.eu/resource/authority/Subcontracting-indication> ;
  skos:prefLabel "The subject-matter of the subcontract(s) necessary to fulfill the obligation to subcontract a minimum percentage of the contract"@en ;
.
epo:Submission-document-type
  rdf:type skos:ConceptScheme ;
  rdfs:comment """The period during which tenders submitted for this procurement procedure must remain valid.

(Pending to review by the WG)
"""@en ;
  rdfs:isDefinedBy <http://data.europa.eu/a4g/ontology> ;
  rdfs:label "Submission-document-type"@en ;
  skos:definition """The period during which tenders submitted for this procurement procedure must remain valid.

(Pending to review by the WG)
"""@en ;
  skos:prefLabel "Submission-document-type" ;
.
epo:SubmissionTerms
  rdf:type owl:Class ;
  rdfs:comment """Conditions and stipulations defining particularities of submitting tenders.

WG Approval 03/10/2019 """@en ;
  rdfs:isDefinedBy <http://data.europa.eu/a4g/ontology> ;
  rdfs:label "Submission terms"@en ;
  skos:definition """Conditions and stipulations defining particularities of submitting tenders.

WG Approval 03/10/2019 """@en ;
  skos:prefLabel "Submission terms"@en ;
.
epo:Sui-act
  rdf:type skos:Concept ;
  rdfs:isDefinedBy <http://data.europa.eu/a4g/ontology> ;
  rdfs:label "Suitability to pursue the professional activity"@en ;
  skos:inScheme <http://publications.europa.eu/resource/authority/Selection-criterion> ;
  skos:prefLabel "Suitability to pursue the professional activity"@en ;
.
epo:Supp-comm-mark
  rdf:type skos:Concept ;
  rdfs:isDefinedBy <http://data.europa.eu/a4g/ontology> ;
  rdfs:label "Procurement of supplies quoted and purchased on a commodity market"@en ;
  skos:inScheme <http://publications.europa.eu/resource/authority/Direct-award-justification> ;
  skos:prefLabel "Procurement of supplies quoted and purchased on a commodity market"@en ;
.
epo:Supplies
  rdf:type skos:Concept ;
  rdfs:isDefinedBy <http://data.europa.eu/a4g/ontology> ;
  rdfs:label "Supplies"@en ;
  skos:inScheme <http://publications.europa.eu/resource/authority/Contract-nature> ;
  skos:prefLabel "Supplies"@en ;
.
epo:System
  rdf:type owl:Class ;
  rdfs:comment """Software application used for performing procurement activities. 

WG Approval 28/04/2020

"""@en ;
  rdfs:isDefinedBy <http://data.europa.eu/a4g/ontology> ;
  rdfs:label "System"@en ;
  rdfs:subClassOf epo:Agent ;
  owl:disjointWith epo:Organisation ;
  owl:disjointWith epo:Person ;
  skos:definition """Software application used for performing procurement activities. 

WG Approval 28/04/2020

"""@en ;
  skos:prefLabel "System"@en ;
.
epo:TCD
  rdf:type skos:Concept ;
  rdfs:isDefinedBy <http://data.europa.eu/a4g/ontology> ;
  rdfs:label "Chad"@en ;
  skos:inScheme <http://publications.europa.eu/resource/authority/Country> ;
  skos:prefLabel "Chad"@en ;
.
epo:TENDER
  rdf:type skos:Concept ;
  rdfs:isDefinedBy <http://data.europa.eu/a4g/ontology> ;
  rdfs:label "T e n d e r"@en ;
  skos:inScheme epo:Submission-document-type ;
  skos:prefLabel "T e n d e r"@en ;
.
epo:TENDERER
  rdf:type skos:Concept ;
  rdfs:isDefinedBy <http://data.europa.eu/a4g/ontology> ;
  rdfs:label "T e n d e r e r"@en ;
  skos:inScheme epo:Security-clearance-address ;
  skos:prefLabel "T e n d e r e r"@en ;
.
epo:THU
  rdf:type skos:Concept ;
  rdfs:isDefinedBy <http://data.europa.eu/a4g/ontology> ;
  rdfs:label "Thursday"@en ;
  skos:inScheme <http://publications.europa.eu/resource/authority/Timeperiods> ;
  skos:prefLabel "Thursday"@en ;
.
epo:TOP_SECRET
  rdf:type skos:Concept ;
  rdfs:isDefinedBy <http://data.europa.eu/a4g/ontology> ;
  rdfs:label "Information and material the unauthorised disclosure of which could cause exceptionally grave prejudice to the essential interests of the European Union, of one or more of the Member States  or of one or more parties participating in a Procedure."@en ;
  skos:inScheme <https://github.com/ESPD/ESPD-EDM/Confidentiality-level> ;
  skos:prefLabel "Information and material the unauthorised disclosure of which could cause exceptionally grave prejudice to the essential interests of the European Union, of one or more of the Member States  or of one or more parties participating in a Procedure."@en ;
.
epo:TUE
  rdf:type skos:Concept ;
  rdfs:isDefinedBy <http://data.europa.eu/a4g/ontology> ;
  rdfs:label "Tuesday"@en ;
  skos:inScheme <http://publications.europa.eu/resource/authority/Timeperiods> ;
  skos:prefLabel "Tuesday"@en ;
.
epo:Tch-per-error
  rdf:type skos:Concept ;
  rdfs:isDefinedBy <http://data.europa.eu/a4g/ontology> ;
  rdfs:label "Decision of the buyer, not following a tenderer's request to review the award, because of technical or procedural errors"@en ;
  skos:inScheme <http://publications.europa.eu/resource/authority/Non-award-justification> ;
  skos:prefLabel "Decision of the buyer, not following a tenderer's request to review the award, because of technical or procedural errors"@en ;
.
epo:Tdf-non-av
  rdf:type skos:Concept ;
  rdfs:isDefinedBy <http://data.europa.eu/a4g/ontology> ;
  rdfs:label "Tools, devices, or file formats not generally available"@en ;
  skos:inScheme <http://publications.europa.eu/resource/authority/Communication-justification> ;
  skos:prefLabel "Tools, devices, or file formats not generally available"@en ;
.
epo:TechnicalSpecifications
  rdf:type owl:Class ;
  rdfs:isDefinedBy <http://data.europa.eu/a4g/ontology> ;
  rdfs:label "Technical specifications"@en ;
  rdfs:subClassOf epo:ProcurementDocument ;
  owl:disjointWith epo:AdditionalDocument ;
  owl:disjointWith epo:CallForCompetition ;
  owl:disjointWith epo:ContractTemplate ;
  owl:disjointWith epo:DescriptiveDocument ;
  owl:disjointWith epo:DraftCV ;
  owl:disjointWith epo:ESPDRequest ;
  owl:disjointWith epo:InvitationToTender ;
  owl:disjointWith epo:PreAwardCatalogueRequest ;
  skos:prefLabel "Technical specifications"@en ;
.
epo:TechnicalTenderDocument
  rdf:type owl:Class ;
  rdfs:isDefinedBy <http://data.europa.eu/a4g/ontology> ;
  rdfs:label "Technical tender document"@en ;
  rdfs:subClassOf epo:TenderDocument ;
  owl:disjointWith epo:ESPDResponse ;
  owl:disjointWith epo:FinancialTenderDocument ;
  owl:disjointWith epo:PreAwardCatalogueResponse ;
  skos:prefLabel "Technical tender document"@en ;
.
epo:Technique
  rdf:type owl:Class ;
  rdfs:comment """Methods used for conducting procurement procedure.

Addtional information:

Several techniques can be combined in one single procurement procedure (e.g. eAuction can be carried out in a Framework Agreement or DPS).

WG Approval 19/09/2019 
"""@en ;
  rdfs:isDefinedBy <http://data.europa.eu/a4g/ontology> ;
  rdfs:label "Technique"@en ;
  skos:definition """Methods used for conducting procurement procedure.

Addtional information:

Several techniques can be combined in one single procurement procedure (e.g. eAuction can be carried out in a Framework Agreement or DPS).

WG Approval 19/09/2019 
"""@en ;
  skos:prefLabel "Technique"@en ;
.
epo:Temp-adv
  rdf:type skos:Concept ;
  rdfs:isDefinedBy <http://data.europa.eu/a4g/ontology> ;
  rdfs:label "Bargain purchase taking advantage of a particularly advantageous opportunity available for a very short time at a price considerably lower than market prices"@en ;
  skos:inScheme <http://publications.europa.eu/resource/authority/Direct-award-justification> ;
  skos:prefLabel "Bargain purchase taking advantage of a particularly advantageous opportunity available for a very short time at a price considerably lower than market prices"@en ;
.
epo:Tender
  rdf:type owl:Class ;
  rdfs:comment """Information submitted by the economic operator to specify its offer regarding one or more lots or the whole procedure, in response to the call for tender.

(WG approval 07/11/2018)
"""@en ;
  rdfs:isDefinedBy <http://data.europa.eu/a4g/ontology> ;
  rdfs:label "Tender"@en ;
  skos:definition """Information submitted by the economic operator to specify its offer regarding one or more lots or the whole procedure, in response to the call for tender.

(WG approval 07/11/2018)
"""@en ;
  skos:prefLabel "Tender"@en ;
.
epo:TenderDocument
  rdf:type owl:Class ;
  rdfs:comment """Document provided by a candidate or tenderer.
Additional information:

In the case of a candidate the documents are intended to express interest in the procedure. Examples are Expression of Interest, an ESPD Response, etc.
In the case of a tenderer the documents provide the information requested by the buyer. Examples are the ESPD Response, the Technical Tender Document, the Financial Tender Document, the Pre-award Catalogue Response, etc.

WG Approval 23/05/2019"""@en ;
  rdfs:isDefinedBy <http://data.europa.eu/a4g/ontology> ;
  rdfs:label "Tender document"@en ;
  rdfs:subClassOf epo:Document ;
  owl:disjointWith epo:Contract ;
  owl:disjointWith epo:Notice ;
  owl:disjointWith epo:ProcurementDocument ;
  owl:disjointWith epo:RequestForParticipation ;
  skos:definition """Document provided by a candidate or tenderer.
Additional information:

In the case of a candidate the documents are intended to express interest in the procedure. Examples are Expression of Interest, an ESPD Response, etc.
In the case of a tenderer the documents provide the information requested by the buyer. Examples are the ESPD Response, the Technical Tender Document, the Financial Tender Document, the Pre-award Catalogue Response, etc.

WG Approval 23/05/2019"""@en ;
  skos:prefLabel "Tender document"@en ;
.
epo:TenderEvaluation
  rdf:type owl:Class ;
  rdfs:isDefinedBy <http://data.europa.eu/a4g/ontology> ;
  rdfs:label "Tender evaluation"@en ;
  skos:prefLabel "Tender evaluation"@en ;
.
epo:TenderLot
  rdf:type owl:Class ;
  rdfs:comment """Part of the tender that applies to the related lot.

Additional Information: 

See also the definitions of Tender and Lot for a complete understanding.



"""@en ;
  rdfs:isDefinedBy <http://data.europa.eu/a4g/ontology> ;
  rdfs:label "Tender lot"@en ;
  skos:definition """Part of the tender that applies to the related lot.

Additional Information: 

See also the definitions of Tender and Lot for a complete understanding.



"""@en ;
  skos:prefLabel "Tender lot"@en ;
.
epo:TenderLotEvaluationRank
  rdf:type owl:Class ;
  rdfs:comment """The position of the Tender Lot in relation to other Tender Lots (i.e. first, second, third, etc.).

Additional information: This is specially the case of design contests, some framework agreements with multiple winners (e.g. cascades) or innovation partnerships.

In multi-staged procedures this may be used for ranking the Tender Lots to be evaluated for further stages.

WG Approval 19/12/2019

"""@en ;
  rdfs:isDefinedBy <http://data.europa.eu/a4g/ontology> ;
  rdfs:label "Tender lot evaluation rank"@en ;
  skos:definition """The position of the Tender Lot in relation to other Tender Lots (i.e. first, second, third, etc.).

Additional information: This is specially the case of design contests, some framework agreements with multiple winners (e.g. cascades) or innovation partnerships.

In multi-staged procedures this may be used for ranking the Tender Lots to be evaluated for further stages.

WG Approval 19/12/2019

"""@en ;
  skos:prefLabel "Tender lot evaluation rank"@en ;
.
epo:Tenderer
  rdf:type owl:Class ;
  rdfs:comment """An economic operator that has submitted a tender.

WG approval 07/11/2018"""@en ;
  rdfs:isDefinedBy <http://data.europa.eu/a4g/ontology> ;
  rdfs:label "Tenderer"@en ;
  rdfs:subClassOf epo:EconomicOperator ;
  owl:disjointWith epo:Subcontractor ;
  skos:definition """An economic operator that has submitted a tender.

WG approval 07/11/2018"""@en ;
  skos:prefLabel "Tenderer"@en ;
.
epo:Text
  rdf:type rdfs:Datatype ;
  rdf:type owl:Class ;
  rdfs:isDefinedBy <http://data.europa.eu/a4g/ontology> ;
  rdfs:label "Text"@en ;
  rdfs:subClassOf <http://www.unece.org/cefact#Text> ;
  skos:prefLabel "Text"@en ;
.
epo:Time
  rdf:type rdfs:Datatype ;
  rdfs:isDefinedBy <http://data.europa.eu/a4g/ontology> ;
  rdfs:label "Time"@en ;
  skos:prefLabel "Time"@en ;
.
epo:TitleIIIOfDirective200981EC
  rdf:type skos:Concept ;
  rdfs:isDefinedBy <http://data.europa.eu/a4g/ontology> ;
  rdfs:label "Title i i i of directive200981 e c"@en ;
  skos:inScheme <http://publications.europa.eu/resource/authority/Subcontracting-obligation> ;
  skos:prefLabel "Title i i i of directive200981 e c"@en ;
.
epo:Tp-abil
  rdf:type skos:Concept ;
  rdfs:isDefinedBy <http://data.europa.eu/a4g/ontology> ;
  rdfs:label "Technical and professional ability"@en ;
  skos:inScheme <http://publications.europa.eu/resource/authority/Selection-criterion> ;
  skos:prefLabel "Technical and professional ability"@en ;
.
epo:UNDERTAKING
  rdf:type skos:Concept ;
  rdfs:isDefinedBy <http://data.europa.eu/a4g/ontology> ;
  rdfs:label "Undertaking"@en ;
  skos:inScheme epo:Eo-group-type ;
  skos:prefLabel "Undertaking"@en ;
.
epo:UNKNOWN
  rdf:type skos:Concept ;
  rdfs:isDefinedBy <http://data.europa.eu/a4g/ontology> ;
  rdfs:label "Unknown"@en ;
  skos:inScheme <http://publications.europa.eu/resource/authority/Timeperiods> ;
  skos:prefLabel "Unknown"@en ;
.
epo:UNLIMITED
  rdf:type skos:Concept ;
  rdfs:isDefinedBy <http://data.europa.eu/a4g/ontology> ;
  rdfs:label "Unlimited"@en ;
  skos:inScheme <http://publications.europa.eu/resource/authority/Timeperiods> ;
  skos:prefLabel "Unlimited"@en ;
.
epo:URI
  rdf:type rdfs:Datatype ;
  rdfs:isDefinedBy <http://data.europa.eu/a4g/ontology> ;
  rdfs:label "U r i"@en ;
  skos:prefLabel "U r i"@en ;
.
epo:Uniq-art-work
  rdf:type skos:Concept ;
  rdfs:isDefinedBy <http://data.europa.eu/a4g/ontology> ;
  rdfs:label "The contract can be provided only by a particular economic operator because of creation or acquisition of a unique work of art or artistic performance"@en ;
  skos:inScheme <http://publications.europa.eu/resource/authority/Direct-award-justification> ;
  skos:prefLabel "The contract can be provided only by a particular economic operator because of creation or acquisition of a unique work of art or artistic performance"@en ;
.
epo:Unit-code
  rdf:type skos:ConceptScheme ;
  rdfs:isDefinedBy <http://data.europa.eu/a4g/ontology> ;
  rdfs:label "Unit-code"@en ;
  skos:prefLabel "Unit-code" ;
.
epo:Up-add-info
  rdf:type skos:Concept ;
  rdfs:isDefinedBy <http://data.europa.eu/a4g/ontology> ;
  rdfs:label "Updated or additional information"@en ;
  skos:inScheme epo:Notice-corrigendum-justification ;
  skos:prefLabel "Updated or additional information"@en ;
.
epo:Used
  rdf:type skos:Concept ;
  rdfs:isDefinedBy <http://data.europa.eu/a4g/ontology> ;
  rdfs:label "Used"@en ;
  skos:inScheme <http://publications.europa.eu/resource/authority/Usage> ;
  skos:prefLabel "Used"@en ;
.
epo:VGB
  rdf:type skos:Concept ;
  rdfs:isDefinedBy <http://data.europa.eu/a4g/ontology> ;
  rdfs:label "British Virgin Islands"@en ;
  skos:inScheme <http://publications.europa.eu/resource/authority/Country> ;
  skos:prefLabel "British Virgin Islands"@en ;
.
epo:Value
  rdf:type owl:Class ;
  rdfs:isDefinedBy <http://data.europa.eu/a4g/ontology> ;
  rdfs:label "Value"@en ;
  skos:prefLabel "Value"@en ;
.
epo:VoluntaryEx-anteTransparencyNotice
  rdf:type owl:Class ;
  rdfs:comment """A notice informing of the intention to award  a contract without prior publication of a contract notice.
 
Additional Information:
 
For European notices above the threshold
 
\"A means of advertising the intention to award the contract without opening it up to formal competition. A contracting authority may decide that a contract does not require prior publication through a contract notice in the O.J.E.U. A reason for this decision may be that the contract meets the exceptional conditions described in Article 31 of Directive 2004/18/EC. In a recent V.E.A.T notice the reason was listed as “extreme urgency brought about by events unforeseeable by the contracting entity and in accordance with the strict conditions stated in the Directive” .
\"Voluntary Ex-Ante Transparency Notice\" (VEAT) where a contracting authority deems that a contract does not require prior publication of a contract notice in the European Journal (OJEU). This may apply, for example, if the contract meets the exceptional conditions justifying direct award of contracts.
 
<b>This definition is still to be worked on.</b>"""@en ;
  rdfs:isDefinedBy <http://data.europa.eu/a4g/ontology> ;
  rdfs:label "Voluntary ex-ante transparency notice"@en ;
  rdfs:subClassOf epo:Notice ;
  owl:disjointWith epo:CallForExpressionOfInterest ;
  owl:disjointWith epo:ContractAwardNotice ;
  owl:disjointWith epo:ContractModificationNotice ;
  owl:disjointWith epo:ContractNotice ;
  owl:disjointWith epo:PriorInformationNotice ;
  skos:definition """A notice informing of the intention to award  a contract without prior publication of a contract notice.
 
Additional Information:
 
For European notices above the threshold
 
\"A means of advertising the intention to award the contract without opening it up to formal competition. A contracting authority may decide that a contract does not require prior publication through a contract notice in the O.J.E.U. A reason for this decision may be that the contract meets the exceptional conditions described in Article 31 of Directive 2004/18/EC. In a recent V.E.A.T notice the reason was listed as “extreme urgency brought about by events unforeseeable by the contracting entity and in accordance with the strict conditions stated in the Directive” .
\"Voluntary Ex-Ante Transparency Notice\" (VEAT) where a contracting authority deems that a contract does not require prior publication of a contract notice in the European Journal (OJEU). This may apply, for example, if the contract meets the exceptional conditions justifying direct award of contracts.
 
<b>This definition is still to be worked on.</b>"""@en ;
  skos:prefLabel "Voluntary ex-ante transparency notice"@en ;
.
epo:WED
  rdf:type skos:Concept ;
  rdfs:isDefinedBy <http://data.europa.eu/a4g/ontology> ;
  rdfs:label "Wednesday"@en ;
  skos:inScheme <http://publications.europa.eu/resource/authority/Timeperiods> ;
  skos:prefLabel "Wednesday"@en ;
.
epo:WEEK
  rdf:type skos:Concept ;
  rdfs:isDefinedBy <http://data.europa.eu/a4g/ontology> ;
  rdfs:label "Week"@en ;
  skos:inScheme <http://publications.europa.eu/resource/authority/Timeperiods> ;
  skos:prefLabel "Week"@en ;
.
epo:WINNER
  rdf:type skos:Concept ;
  rdfs:isDefinedBy <http://data.europa.eu/a4g/ontology> ;
  rdfs:label "W i n n e r"@en ;
  skos:inScheme epo:Security-clearance-address ;
  skos:prefLabel "W i n n e r"@en ;
.
epo:WINTER
  rdf:type skos:Concept ;
  rdfs:isDefinedBy <http://data.europa.eu/a4g/ontology> ;
  rdfs:label "Winter"@en ;
  skos:inScheme <http://publications.europa.eu/resource/authority/Timeperiods> ;
  skos:prefLabel "Winter"@en ;
.
epo:WORKING_DAY
  rdf:type skos:Concept ;
  rdfs:isDefinedBy <http://data.europa.eu/a4g/ontology> ;
  rdfs:label "Working Day"@en ;
  skos:inScheme <http://publications.europa.eu/resource/authority/Timeperiods> ;
  skos:prefLabel "Working Day"@en ;
.
epo:Wei-dec-exa
  rdf:type skos:Concept ;
  rdfs:isDefinedBy <http://data.europa.eu/a4g/ontology> ;
  rdfs:label "Weight (decimal, exact)"@en ;
  skos:inScheme <http://publications.europa.eu/resource/authority/Number-weight> ;
  skos:prefLabel "Weight (decimal, exact)"@en ;
.
epo:Wei-dec-mid
  rdf:type skos:Concept ;
  rdfs:isDefinedBy <http://data.europa.eu/a4g/ontology> ;
  rdfs:label "Weight (decimal, middle of a range)"@en ;
  skos:inScheme <http://publications.europa.eu/resource/authority/Number-weight> ;
  skos:prefLabel "Weight (decimal, middle of a range)"@en ;
.
epo:Wei-per-exa
  rdf:type skos:Concept ;
  rdfs:isDefinedBy <http://data.europa.eu/a4g/ontology> ;
  rdfs:label "Weight (percentage, exact)"@en ;
  skos:inScheme <http://publications.europa.eu/resource/authority/Number-weight> ;
  skos:prefLabel "Weight (percentage, exact)"@en ;
.
epo:Wei-per-mid
  rdf:type skos:Concept ;
  rdfs:isDefinedBy <http://data.europa.eu/a4g/ontology> ;
  rdfs:label "Weight (percentage, middle of a range)"@en ;
  skos:inScheme <http://publications.europa.eu/resource/authority/Number-weight> ;
  skos:prefLabel "Weight (percentage, middle of a range)"@en ;
.
epo:Wei-poi-exa
  rdf:type skos:Concept ;
  rdfs:isDefinedBy <http://data.europa.eu/a4g/ontology> ;
  rdfs:label "Weight (points, exact)"@en ;
  skos:inScheme <http://publications.europa.eu/resource/authority/Number-weight> ;
  skos:prefLabel "Weight (points, exact)"@en ;
.
epo:Wei-poi-mid
  rdf:type skos:Concept ;
  rdfs:isDefinedBy <http://data.europa.eu/a4g/ontology> ;
  rdfs:label "Weight (points, middle of a range)"@en ;
  skos:inScheme <http://publications.europa.eu/resource/authority/Number-weight> ;
  skos:prefLabel "Weight (points, middle of a range)"@en ;
.
epo:Winner
  rdf:type owl:Class ;
  rdfs:comment """The tenderer to whom the contract is awarded.

(WG approval 20/11/2018)"""@en ;
  rdfs:isDefinedBy <http://data.europa.eu/a4g/ontology> ;
  rdfs:label "Winner"@en ;
  rdfs:subClassOf epo:Tenderer ;
  skos:definition """The tenderer to whom the contract is awarded.

(WG approval 20/11/2018)"""@en ;
  skos:prefLabel "Winner"@en ;
.
epo:Works
  rdf:type skos:Concept ;
  rdfs:isDefinedBy <http://data.europa.eu/a4g/ontology> ;
  rdfs:label "Works"@en ;
  skos:inScheme <http://publications.europa.eu/resource/authority/Contract-nature> ;
  skos:prefLabel "Works"@en ;
.
epo:YEAR
  rdf:type skos:Concept ;
  rdfs:isDefinedBy <http://data.europa.eu/a4g/ontology> ;
  rdfs:label "(_S|Year)(_P|Years)"@en ;
  skos:inScheme <http://publications.europa.eu/resource/authority/Timeperiods> ;
  skos:prefLabel "(_S|Year)(_P|Years)"@en ;
.
epo:YEAR_HALF
  rdf:type skos:Concept ;
  rdfs:isDefinedBy <http://data.europa.eu/a4g/ontology> ;
  rdfs:label "Half year"@en ;
  skos:inScheme <http://publications.europa.eu/resource/authority/Timeperiods> ;
  skos:prefLabel "Half year"@en ;
.
epo:YES
  rdf:type skos:Concept ;
  rdfs:isDefinedBy <http://data.europa.eu/a4g/ontology> ;
  rdfs:label "Options are used"@en ;
  skos:inScheme epo:Options ;
  skos:prefLabel "Options are used"@en ;
.
epo:Yes
  rdf:type skos:Concept ;
  rdfs:isDefinedBy <http://data.europa.eu/a4g/ontology> ;
  rdfs:label "Yes"@en ;
  skos:inScheme <http://publications.europa.eu/resource/authority/Applicability> ;
  skos:prefLabel "Yes"@en ;
.
epo:acceptsProposalOf
  rdf:type owl:ObjectProperty ;
  rdfs:isDefinedBy <http://data.europa.eu/a4g/ontology> ;
  rdfs:label "Accepts proposal of"@en ;
  skos:prefLabel "Accepts proposal of"@en ;
.
epo:accessMarketThrough
  rdf:type owl:ObjectProperty ;
  rdfs:isDefinedBy <http://data.europa.eu/a4g/ontology> ;
  rdfs:label "Access market through"@en ;
  skos:prefLabel "Access market through"@en ;
.
epo:actsAs
  rdf:type owl:ObjectProperty ;
  rdfs:isDefinedBy <http://data.europa.eu/a4g/ontology> ;
  rdfs:label "Acts as"@en ;
  skos:prefLabel "Acts as"@en ;
.
epo:actsOnBehalfOf
  rdf:type owl:ObjectProperty ;
  rdfs:isDefinedBy <http://data.europa.eu/a4g/ontology> ;
  rdfs:label "Acts on behalf of"@en ;
  skos:prefLabel "Acts on behalf of"@en ;
.
epo:additionalClassifications
  rdf:type owl:ObjectProperty ;
  rdfs:isDefinedBy <http://data.europa.eu/a4g/ontology> ;
  rdfs:label "Additional classifications"@en ;
  skos:prefLabel "Additional classifications"@en ;
.
epo:appliesTo
  rdf:type owl:ObjectProperty ;
  rdfs:comment """Identifier of one or more lots within the procedure to which this submission terms refer.

WG Approval 07/03/2019 16:29:39

"""@en ;
  rdfs:comment """The Contracting Authority uses this property to precise the Lots for which a concrete requirement (expressed as Procurement Criterion Property) is applicable to.

WG Approval 05/09/2019 """@en ;
  rdfs:isDefinedBy <http://data.europa.eu/a4g/ontology> ;
  rdfs:label "Applies to"@en ;
  skos:definition """Identifier of one or more lots within the procedure to which this submission terms refer.

WG Approval 07/03/2019 16:29:39

"""@en ;
  skos:definition """The Contracting Authority uses this property to precise the Lots for which a concrete requirement (expressed as Procurement Criterion Property) is applicable to.

WG Approval 05/09/2019 """@en ;
  skos:prefLabel "Applies to"@en ;
.
epo:appliesToFollowupContractTerms
  rdf:type owl:ObjectProperty ;
  rdfs:isDefinedBy <http://data.europa.eu/a4g/ontology> ;
  rdfs:label "Applies to followup contract terms"@en ;
  skos:prefLabel "Applies to followup contract terms"@en ;
.
epo:apply
  rdf:type owl:ObjectProperty ;
  rdfs:isDefinedBy <http://data.europa.eu/a4g/ontology> ;
  rdfs:label "Apply"@en ;
  skos:prefLabel "Apply"@en ;
.
epo:applyTo
  rdf:type owl:ObjectProperty ;
  rdfs:isDefinedBy <http://data.europa.eu/a4g/ontology> ;
  rdfs:label "Apply to"@en ;
  skos:prefLabel "Apply to"@en ;
.
epo:appointedBy
  rdf:type owl:ObjectProperty ;
  rdfs:isDefinedBy <http://data.europa.eu/a4g/ontology> ;
  rdfs:label "Appointed by"@en ;
  skos:prefLabel "Appointed by"@en ;
.
epo:appoints
  rdf:type owl:ObjectProperty ;
  rdfs:isDefinedBy <http://data.europa.eu/a4g/ontology> ;
  rdfs:label "Appoints"@en ;
  skos:prefLabel "Appoints"@en ;
.
epo:assesses
  rdf:type owl:ObjectProperty ;
  rdfs:isDefinedBy <http://data.europa.eu/a4g/ontology> ;
  rdfs:label "Assesses"@en ;
  skos:prefLabel "Assesses"@en ;
.
epo:attaches
  rdf:type owl:ObjectProperty ;
  rdfs:isDefinedBy <http://data.europa.eu/a4g/ontology> ;
  rdfs:label "Attaches"@en ;
  skos:prefLabel "Attaches"@en ;
.
epo:belongsTo
  rdf:type owl:ObjectProperty ;
  rdfs:isDefinedBy <http://data.europa.eu/a4g/ontology> ;
  rdfs:label "Belongs to"@en ;
  skos:prefLabel "Belongs to"@en ;
.
epo:changeRefersToInstance
  rdf:type owl:ObjectProperty ;
  rdfs:isDefinedBy <http://data.europa.eu/a4g/ontology> ;
  rdfs:label "Change refers to instance"@en ;
  skos:prefLabel "Change refers to instance"@en ;
.
epo:combineLotsInto
  rdf:type owl:ObjectProperty ;
  rdfs:isDefinedBy <http://data.europa.eu/a4g/ontology> ;
  rdfs:label "Combine lots into"@en ;
  skos:prefLabel "Combine lots into"@en ;
.
epo:comeFrom
  rdf:type owl:ObjectProperty ;
  rdfs:isDefinedBy <http://data.europa.eu/a4g/ontology> ;
  rdfs:label "Come from"@en ;
  skos:prefLabel "Come from"@en ;
.
epo:concludes
  rdf:type owl:ObjectProperty ;
  rdfs:isDefinedBy <http://data.europa.eu/a4g/ontology> ;
  rdfs:label "Concludes"@en ;
  skos:prefLabel "Concludes"@en ;
.
epo:contributesToImplement
  rdf:type owl:ObjectProperty ;
  rdfs:isDefinedBy <http://data.europa.eu/a4g/ontology> ;
  rdfs:label "Contributes to implement"@en ;
  skos:prefLabel "Contributes to implement"@en ;
.
epo:creationOfCallForExpressionOfInterest
  rdf:type owl:ObjectProperty ;
  rdfs:isDefinedBy <http://data.europa.eu/a4g/ontology> ;
  rdfs:label "Creation of call for expression of interest"@en ;
  skos:prefLabel "Creation of call for expression of interest"@en ;
.
epo:creator
  rdf:type owl:ObjectProperty ;
  rdfs:isDefinedBy <http://data.europa.eu/a4g/ontology> ;
  rdfs:label "Creator"@en ;
  skos:prefLabel "Creator"@en ;
.
epo:defines
  rdf:type owl:ObjectProperty ;
  rdfs:isDefinedBy <http://data.europa.eu/a4g/ontology> ;
  rdfs:label "Defines"@en ;
  skos:prefLabel "Defines"@en ;
.
epo:eCataloguePermission
  rdf:type owl:ObjectProperty ;
  rdfs:comment """The extent to which electronic catalogues may be used in tenders.

WG Approval 03/10/2019"""@en ;
  rdfs:isDefinedBy <http://data.europa.eu/a4g/ontology> ;
  rdfs:label "E catalogue permission"@en ;
  skos:definition """The extent to which electronic catalogues may be used in tenders.

WG Approval 03/10/2019"""@en ;
  skos:prefLabel "E catalogue permission"@en ;
.
epo:eInvoicing
  rdf:type rdf:Property ;
  rdfs:comment """Electronic means will be used for invoicing in the post-award process.

WG Approval 12/09/2019
"""@en ;
  rdfs:isDefinedBy <http://data.europa.eu/a4g/ontology> ;
  rdfs:label "E invoicing"@en ;
  skos:definition """Electronic means will be used for invoicing in the post-award process.

WG Approval 12/09/2019
"""@en ;
  skos:prefLabel "E invoicing"@en ;
.
epo:eOrdering
  rdf:type rdf:Property ;
  rdfs:comment """Electronic means will be used for requesting and purchasing in the post-award process.

WG Approval 12/09/2019

"""@en ;
  rdfs:isDefinedBy <http://data.europa.eu/a4g/ontology> ;
  rdfs:label "E ordering"@en ;
  skos:definition """Electronic means will be used for requesting and purchasing in the post-award process.

WG Approval 12/09/2019

"""@en ;
  skos:prefLabel "E ordering"@en ;
.
epo:ePayment
  rdf:type rdf:Property ;
  rdfs:comment """
"""@en ;
  rdfs:isDefinedBy <http://data.europa.eu/a4g/ontology> ;
  rdfs:label "E payment"@en ;
  skos:definition """
"""@en ;
  skos:prefLabel "E payment"@en ;
.
epo:eSubmissionPermission
  rdf:type owl:ObjectProperty ;
  rdfs:comment """The requirements as to what extent electronic submission is allowed.

WG Approval 03/10/2019"""@en ;
  rdfs:isDefinedBy <http://data.europa.eu/a4g/ontology> ;
  rdfs:label "E submission permission"@en ;
  skos:definition """The requirements as to what extent electronic submission is allowed.

WG Approval 03/10/2019"""@en ;
  skos:prefLabel "E submission permission"@en ;
.
epo:eSubmissioneSignature
  rdf:type owl:ObjectProperty ;
  rdfs:comment """The tender is required to be signed electronically.

Additional Information: 

Signature can be defined as \"data in electronic form which is attached to or logically associated with other data in electronic form and which is used by the signatory to sign. 
For more details on the meaning and uses of electronic signature you may consult different authoritative sources, a relevant one being for instance the Regulation (EU) 910/2014 on electronic identification and trust services for electronic transactions in the internal market.

WG Approval 12/03/2019"""@en ;
  rdfs:isDefinedBy <http://data.europa.eu/a4g/ontology> ;
  rdfs:label "E submissione signature"@en ;
  skos:definition """The tender is required to be signed electronically.

Additional Information: 

Signature can be defined as \"data in electronic form which is attached to or logically associated with other data in electronic form and which is used by the signatory to sign. 
For more details on the meaning and uses of electronic signature you may consult different authoritative sources, a relevant one being for instance the Regulation (EU) 910/2014 on electronic identification and trust services for electronic transactions in the internal market.

WG Approval 12/03/2019"""@en ;
  skos:prefLabel "E submissione signature"@en ;
.
epo:epoElectronicTendersLot
  rdf:type owl:DatatypeProperty ;
  rdfs:comment "Tenders received digitally."@en ;
  rdfs:isDefinedBy <http://data.europa.eu/a4g/ontology> ;
  rdfs:label "Epo electronic tenders lot"@en ;
  skos:definition "Tenders received digitally."@en ;
  skos:prefLabel "Epo electronic tenders lot"@en ;
.
epo:epohasLegalFormType
  rdf:type owl:ObjectProperty ;
  rdfs:isDefinedBy <http://data.europa.eu/a4g/ontology> ;
  rdfs:label "Epohas legal form type"@en ;
  skos:prefLabel "Epohas legal form type"@en ;
.
epo:evaluates
  rdf:type owl:ObjectProperty ;
  rdfs:isDefinedBy <http://data.europa.eu/a4g/ontology> ;
  rdfs:label "Evaluates"@en ;
  skos:prefLabel "Evaluates"@en ;
.
epo:evaluationOf
  rdf:type owl:ObjectProperty ;
  rdfs:isDefinedBy <http://data.europa.eu/a4g/ontology> ;
  rdfs:label "Evaluation of"@en ;
  skos:prefLabel "Evaluation of"@en ;
.
epo:excecutes
  rdf:type owl:ObjectProperty ;
  rdfs:isDefinedBy <http://data.europa.eu/a4g/ontology> ;
  rdfs:label "Excecutes"@en ;
  skos:prefLabel "Excecutes"@en ;
.
epo:foreseesPlannedProcurementPart
  rdf:type owl:ObjectProperty ;
  rdfs:isDefinedBy <http://data.europa.eu/a4g/ontology> ;
  rdfs:label "Foresees planned procurement part"@en ;
  skos:prefLabel "Foresees planned procurement part"@en ;
.
epo:fulfillsRequirement
  rdf:type owl:ObjectProperty ;
  rdfs:isDefinedBy <http://data.europa.eu/a4g/ontology> ;
  rdfs:label "Fulfills requirement"@en ;
  skos:prefLabel "Fulfills requirement"@en ;
.
epo:funds
  rdf:type owl:ObjectProperty ;
  rdfs:comment """Funds may change between the lot and the contract, for example in the case of an emergency crisis, a contract may be financed by a budget that was not foreseen in the call.
"""@en ;
  rdfs:isDefinedBy <http://data.europa.eu/a4g/ontology> ;
  rdfs:label "Funds"@en ;
  skos:definition """Funds may change between the lot and the contract, for example in the case of an emergency crisis, a contract may be financed by a budget that was not foreseen in the call.
"""@en ;
  skos:prefLabel "Funds"@en ;
.
epo:groups
  rdf:type owl:ObjectProperty ;
  rdfs:isDefinedBy <http://data.europa.eu/a4g/ontology> ;
  rdfs:label "Groups"@en ;
  skos:prefLabel "Groups"@en ;
.
epo:has
  rdf:type owl:ObjectProperty ;
  rdfs:comment """The value offered by the Tenderer for a Lot.

Additional Information:

This value is normally the one awarded for a winning Tender Lot. In case of negotiated procedures the original financial value may be reviewed and the offer updated.
"""@en ;
  rdfs:isDefinedBy <http://data.europa.eu/a4g/ontology> ;
  rdfs:label "Has"@en ;
  skos:definition """The value offered by the Tenderer for a Lot.

Additional Information:

This value is normally the one awarded for a winning Tender Lot. In case of negotiated procedures the original financial value may be reviewed and the offer updated.
"""@en ;
  skos:prefLabel "Has"@en ;
.
epo:hasAbnormallyLowTendersLot
  rdf:type owl:DatatypeProperty ;
  rdfs:comment """Tenders received that were found irregular and non-acceptable due to an abnormally low price or cost.
"""@en ;
  rdfs:isDefinedBy <http://data.europa.eu/a4g/ontology> ;
  rdfs:label "Abnormally low tenders lot"@en ;
  skos:definition """Tenders received that were found irregular and non-acceptable due to an abnormally low price or cost.
"""@en ;
  skos:prefLabel "Abnormally low tenders lot"@en ;
.
epo:hasAccelerated
  rdf:type rdf:Property ;
  rdfs:comment """Statement about  the fact that the procedure will be reduced due to a state of urgency.

Additional Information

This modifies the time limit for the receipt of requests to participate or the receipt of tenders.

WG Approval 20/08/2019
"""@en ;
  rdfs:isDefinedBy <http://data.europa.eu/a4g/ontology> ;
  rdfs:label "Accelerated"@en ;
  skos:definition """Statement about  the fact that the procedure will be reduced due to a state of urgency.

Additional Information

This modifies the time limit for the receipt of requests to participate or the receipt of tenders.

WG Approval 20/08/2019
"""@en ;
  skos:prefLabel "Accelerated"@en ;
.
epo:hasAcceleratedJustification
  rdf:type owl:ObjectProperty ;
  rdfs:isDefinedBy <http://data.europa.eu/a4g/ontology> ;
  rdfs:label "Has accelerated justification"@en ;
  skos:prefLabel "Has accelerated justification"@en ;
.
epo:hasAcceleratedProcedureJustification
  rdf:type owl:DatatypeProperty ;
  rdfs:comment """The reasons why an accelerated procedure is required.

Additional Information:
A procedure is accelerated to cover needs of extraordinary circumstances ie earthquake relief.

WG Approval 5/11/2019
"""@en ;
  rdfs:isDefinedBy <http://data.europa.eu/a4g/ontology> ;
  rdfs:label "Accelerated procedure justification"@en ;
  skos:definition """The reasons why an accelerated procedure is required.

Additional Information:
A procedure is accelerated to cover needs of extraordinary circumstances ie earthquake relief.

WG Approval 5/11/2019
"""@en ;
  skos:prefLabel "Accelerated procedure justification"@en ;
.
epo:hasAccessibilityCriteria
  rdf:type owl:ObjectProperty ;
  rdfs:isDefinedBy <http://data.europa.eu/a4g/ontology> ;
  rdfs:label "Accessibility criteria"@en ;
  skos:prefLabel "Accessibility criteria"@en ;
.
epo:hasAccountFormat
  rdf:type owl:ObjectProperty ;
  rdfs:isDefinedBy <http://data.europa.eu/a4g/ontology> ;
  rdfs:label "Account format"@en ;
  skos:prefLabel "Account format"@en ;
.
epo:hasAccountType
  rdf:type owl:ObjectProperty ;
  rdfs:isDefinedBy <http://data.europa.eu/a4g/ontology> ;
  rdfs:label "Account type"@en ;
  skos:prefLabel "Account type"@en ;
.
epo:hasActivityDescription
  rdf:type owl:DatatypeProperty ;
  rdfs:comment """In the ePO ontology a taxonomy with all activities, based on different classifications (COFOG, UTILITIES, NACE), will be provided. In ePO this field is to be used exclusively to complement the definition attached to the MainActivityCode.

However, in eForms there is the code \"other\" to cover undefined activities. For mapping to this eForms feature one could also use this property.
"""@en ;
  rdfs:isDefinedBy <http://data.europa.eu/a4g/ontology> ;
  rdfs:label "Activity description"@en ;
  skos:definition """In the ePO ontology a taxonomy with all activities, based on different classifications (COFOG, UTILITIES, NACE), will be provided. In ePO this field is to be used exclusively to complement the definition attached to the MainActivityCode.

However, in eForms there is the code \"other\" to cover undefined activities. For mapping to this eForms feature one could also use this property.
"""@en ;
  skos:prefLabel "Activity description"@en ;
.
epo:hasAdditionalClassification
  rdf:type owl:ObjectProperty ;
  rdfs:isDefinedBy <http://data.europa.eu/a4g/ontology> ;
  rdfs:label "Additional classification"@en ;
  skos:prefLabel "Additional classification"@en ;
.
epo:hasAdditionalContractNature
  rdf:type owl:ObjectProperty ;
  rdfs:isDefinedBy <http://data.europa.eu/a4g/ontology> ;
  rdfs:label "Additional contract nature"@en ;
  rdfs:label "Has additional contract nature"@en ;
  skos:prefLabel "Additional contract nature"@en ;
  skos:prefLabel "Has additional contract nature"@en ;
.
epo:hasAdditionalInformation
  rdf:type owl:DatatypeProperty ;
  rdfs:comment """Supplementary data about the instance of the concept.

Additional Information

For example, information about the Lot not specified elsewhere in the Notice.

WG Approval 15/10/2019"""@en ;
  rdfs:comment """Supplementary data about the instance of the concept.

WG Approval 30/09/2019

(The property epo:hasAdditionalInformation is equivalent to cagv:hasDescription)"""@en ;
  rdfs:isDefinedBy <http://data.europa.eu/a4g/ontology> ;
  rdfs:label "Additional information"@en ;
  skos:definition """Supplementary data about the instance of the concept.

Additional Information

For example, information about the Lot not specified elsewhere in the Notice.

WG Approval 15/10/2019"""@en ;
  skos:definition """Supplementary data about the instance of the concept.

WG Approval 30/09/2019

(The property epo:hasAdditionalInformation is equivalent to cagv:hasDescription)"""@en ;
  skos:prefLabel "Additional information"@en ;
.
epo:hasAdditionalInformationDeadline
  rdf:type rdf:Property ;
  rdf:type owl:DatatypeProperty ;
  rdfs:comment """The time limit for requesting further information.

WG Approval 03/10/2019"""@en ;
  rdfs:isDefinedBy <http://data.europa.eu/a4g/ontology> ;
  rdfs:label "Additional information deadline"@en ;
  skos:definition """The time limit for requesting further information.

WG Approval 03/10/2019"""@en ;
  skos:prefLabel "Additional information deadline"@en ;
.
epo:hasAdditionalStreetName
  rdf:type owl:DatatypeProperty ;
  rdfs:isDefinedBy <http://data.europa.eu/a4g/ontology> ;
  rdfs:label "Additional street name"@en ;
  skos:prefLabel "Additional street name"@en ;
.
epo:hasAddressType
  rdf:type owl:ObjectProperty ;
  rdfs:isDefinedBy <http://data.europa.eu/a4g/ontology> ;
  rdfs:label "Address type"@en ;
  skos:prefLabel "Address type"@en ;
.
epo:hasAdmissibleTender
  rdf:type rdf:Property ;
  rdfs:comment """A tender shall be considered admissible where it has been submitted by a tenderer, who has not been excluded and who meets the selection criteria, and when it is in conformity with the technical specifications without being irregular (e.g. received late, having an abnormally low price or cost) or unacceptable or unsuitable. 

To be discussed

(This definition comes from BT-710 in eForms)
"""@en ;
  rdfs:isDefinedBy <http://data.europa.eu/a4g/ontology> ;
  rdfs:label "Admissible tender"@en ;
  skos:definition """A tender shall be considered admissible where it has been submitted by a tenderer, who has not been excluded and who meets the selection criteria, and when it is in conformity with the technical specifications without being irregular (e.g. received late, having an abnormally low price or cost) or unacceptable or unsuitable. 

To be discussed

(This definition comes from BT-710 in eForms)
"""@en ;
  skos:prefLabel "Admissible tender"@en ;
.
epo:hasAlias
  rdf:type owl:ObjectProperty ;
  rdfs:isDefinedBy <http://data.europa.eu/a4g/ontology> ;
  rdfs:label "Has alias"@en ;
  skos:prefLabel "Has alias"@en ;
.
epo:hasAliasName
  rdf:type owl:DatatypeProperty ;
  rdfs:isDefinedBy <http://data.europa.eu/a4g/ontology> ;
  rdfs:label "Alias name"@en ;
  skos:prefLabel "Alias name"@en ;
.
epo:hasAlternativeName
  rdf:type owl:DatatypeProperty ;
  rdfs:isDefinedBy <http://data.europa.eu/a4g/ontology> ;
  rdfs:label "Alternative name"@en ;
  skos:prefLabel "Alternative name"@en ;
.
epo:hasAltitude
  rdf:type owl:ObjectProperty ;
  rdfs:isDefinedBy <http://data.europa.eu/a4g/ontology> ;
  rdfs:label "Altitude"@en ;
  skos:prefLabel "Altitude"@en ;
.
epo:hasApplied
  rdf:type owl:ObjectProperty ;
  rdfs:isDefinedBy <http://data.europa.eu/a4g/ontology> ;
  rdfs:label "Has applied"@en ;
  skos:prefLabel "Has applied"@en ;
.
epo:hasAvailabilityDate
  rdf:type owl:DatatypeProperty ;
  rdfs:isDefinedBy <http://data.europa.eu/a4g/ontology> ;
  rdfs:label "Availability date"@en ;
  skos:prefLabel "Availability date"@en ;
.
epo:hasAvailabilityRestriction
  rdf:type owl:ObjectProperty ;
  rdfs:isDefinedBy <http://data.europa.eu/a4g/ontology> ;
  rdfs:label "Has availability restriction"@en ;
  skos:prefLabel "Has availability restriction"@en ;
.
epo:hasAvailabilityTime
  rdf:type rdf:Property ;
  rdfs:isDefinedBy <http://data.europa.eu/a4g/ontology> ;
  rdfs:label "Availability time"@en ;
  skos:prefLabel "Availability time"@en ;
.
epo:hasAvaliabilityRestriction
  rdf:type owl:ObjectProperty ;
  rdfs:isDefinedBy <http://data.europa.eu/a4g/ontology> ;
  rdfs:label "Has avaliability restriction"@en ;
  skos:prefLabel "Has avaliability restriction"@en ;
.
epo:hasAwardCriteriaEvaluationFormula
  rdf:type owl:DatatypeProperty ;
  rdfs:comment """Based on the Award Dimension Type code list

Let's say we have 5 different quality award criteria

QUALITY

1st - e.g. please describe how you'll make this machine (WEIGHT 20%)
2nd - describe the workflow used to manufacture the machine (WEIGHT 25%)
3rd - describe the materials used for each component of the machine (WEIGHT 10%)
4th - describe the quality control measures (WEIGHT 5%)
5th - describe how the manufacturing dead-lines (WEIGHT 40%)

PRICE CRITERIA
(list of criteria related to price)

COST CRITERIA
(list of criteria related to cost)

Overall award criteria Weight 20% Price, 60% Quality, 20% Cost"""@en ;
  rdfs:isDefinedBy <http://data.europa.eu/a4g/ontology> ;
  rdfs:label "Award criteria evaluation formula"@en ;
  skos:definition """Based on the Award Dimension Type code list

Let's say we have 5 different quality award criteria

QUALITY

1st - e.g. please describe how you'll make this machine (WEIGHT 20%)
2nd - describe the workflow used to manufacture the machine (WEIGHT 25%)
3rd - describe the materials used for each component of the machine (WEIGHT 10%)
4th - describe the quality control measures (WEIGHT 5%)
5th - describe how the manufacturing dead-lines (WEIGHT 40%)

PRICE CRITERIA
(list of criteria related to price)

COST CRITERIA
(list of criteria related to cost)

Overall award criteria Weight 20% Price, 60% Quality, 20% Cost"""@en ;
  skos:prefLabel "Award criteria evaluation formula"@en ;
.
epo:hasAwardCriterionType
  rdf:type owl:ObjectProperty ;
  rdfs:isDefinedBy <http://data.europa.eu/a4g/ontology> ;
  rdfs:label "Award criterion type"@en ;
  skos:prefLabel "Award criterion type"@en ;
.
epo:hasAwardDateScheduled
  rdf:type owl:DatatypeProperty ;
  rdfs:isDefinedBy <http://data.europa.eu/a4g/ontology> ;
  rdfs:label "Award date scheduled"@en ;
  skos:prefLabel "Award date scheduled"@en ;
.
epo:hasAwardDecisionDate
  rdf:type owl:DatatypeProperty ;
  rdfs:comment """The official date of the award decision.

WG Approval 09/01/2020"""@en ;
  rdfs:isDefinedBy <http://data.europa.eu/a4g/ontology> ;
  rdfs:label "Award decision date"@en ;
  skos:definition """The official date of the award decision.

WG Approval 09/01/2020"""@en ;
  skos:prefLabel "Award decision date"@en ;
.
epo:hasAwardStatus
  rdf:type owl:ObjectProperty ;
  rdfs:comment """Indicates whether the lot is awarded, not awarded or still open.

 
WG Approval 03/12/2019"""@en ;
  rdfs:isDefinedBy <http://data.europa.eu/a4g/ontology> ;
  rdfs:label "Award status"@en ;
  rdfs:label "Has award status"@en ;
  skos:definition """Indicates whether the lot is awarded, not awarded or still open.

 
WG Approval 03/12/2019"""@en ;
  skos:prefLabel "Award status"@en ;
  skos:prefLabel "Has award status"@en ;
.
epo:hasAwardedEstimatedValue
  rdf:type owl:ObjectProperty ;
  rdfs:comment """The estimated value that can be spent as provided by the Award Decision.

<u>Additional Information</u>:
This property is used for framework agreements and dynamic purchasing systems. 
Different cases of awarded values may refer to a lot, the global value of the procedure, or of a combinatorial value of a group of lots.

WG Approval 12/12/2019

"""@en ;
  rdfs:isDefinedBy <http://data.europa.eu/a4g/ontology> ;
  rdfs:label "Has awarded estimated value"@en ;
  skos:definition """The estimated value that can be spent as provided by the Award Decision.

<u>Additional Information</u>:
This property is used for framework agreements and dynamic purchasing systems. 
Different cases of awarded values may refer to a lot, the global value of the procedure, or of a combinatorial value of a group of lots.

WG Approval 12/12/2019

"""@en ;
  skos:prefLabel "Has awarded estimated value"@en ;
.
epo:hasAwardedMaximumValue
  rdf:type owl:ObjectProperty ;
  rdfs:comment """The maximum value that can be spent as provided by the Award Decision.

<u>Additional Information</u>:
This property is used for framework agreements and dynamic purchasing systems. 
Different cases of awarded values may refer to a lot, the global value of the procedure, or of a combinatorial value of a group of lots.

WG Approval 12/12/2019
"""@en ;
  rdfs:isDefinedBy <http://data.europa.eu/a4g/ontology> ;
  rdfs:label "Has awarded maximum value"@en ;
  skos:definition """The maximum value that can be spent as provided by the Award Decision.

<u>Additional Information</u>:
This property is used for framework agreements and dynamic purchasing systems. 
Different cases of awarded values may refer to a lot, the global value of the procedure, or of a combinatorial value of a group of lots.

WG Approval 12/12/2019
"""@en ;
  skos:prefLabel "Has awarded maximum value"@en ;
.
epo:hasAwardedValue
  rdf:type owl:ObjectProperty ;
  rdfs:comment """The value of the procurement provided by the Award Decision.

Additional Information:
Different cases of awarded values may refer to a lot, the global value of the procedure, or of a combinatorial value of a group of lots.

In the case of framework agreements and dynamic purchasing systems this refers to the maximum awarded value.

WG Approval 10/12/2019"""@en ;
  rdfs:isDefinedBy <http://data.europa.eu/a4g/ontology> ;
  rdfs:label "Has awarded value"@en ;
  skos:definition """The value of the procurement provided by the Award Decision.

Additional Information:
Different cases of awarded values may refer to a lot, the global value of the procedure, or of a combinatorial value of a group of lots.

In the case of framework agreements and dynamic purchasing systems this refers to the maximum awarded value.

WG Approval 10/12/2019"""@en ;
  skos:prefLabel "Has awarded value"@en ;
.
epo:hasBeneficialOwner
  rdf:type owl:ObjectProperty ;
  rdfs:comment """Any natural person(s) who ultimately owns or controls the organisation and/or the natural person(s) on whose behalf a transaction or activity is being conducted.

"""@en ;
  rdfs:isDefinedBy <http://data.europa.eu/a4g/ontology> ;
  rdfs:label "Has beneficial owner"@en ;
  skos:definition """Any natural person(s) who ultimately owns or controls the organisation and/or the natural person(s) on whose behalf a transaction or activity is being conducted.

"""@en ;
  skos:prefLabel "Has beneficial owner"@en ;
.
epo:hasBeneficialOwnerNationality
  rdf:type owl:ObjectProperty ;
  rdfs:comment """The nationality of any natural person(s) who ultimately owns or controls the economic operator and/or the natural person(s) on whose behalf a transaction or activity is being conducted.

<u>Additional information</u>: 

Directive (EU) 2015/849 details specific types of owners:  
<ul>
 <li>corporate entities;</li>
</ul>
<ul>
 <li>trusts;</li>
 <li>legal entities.</li>
</ul>

For procurement above the european thresholds the complete definition from article 3 paragraph 6 of this Directive should be taken into consideration.

See http://data.europa.eu/eli/dir/2015/849/oj 

WG Approval 21/11/2019"""@en ;
  rdfs:isDefinedBy <http://data.europa.eu/a4g/ontology> ;
  rdfs:label "Beneficial owner nationality"@en ;
  rdfs:label "Has beneficial owner nationality"@en ;
  skos:definition """The nationality of any natural person(s) who ultimately owns or controls the economic operator and/or the natural person(s) on whose behalf a transaction or activity is being conducted.

<u>Additional information</u>: 

Directive (EU) 2015/849 details specific types of owners:  
<ul>
 <li>corporate entities;</li>
</ul>
<ul>
 <li>trusts;</li>
 <li>legal entities.</li>
</ul>

For procurement above the european thresholds the complete definition from article 3 paragraph 6 of this Directive should be taken into consideration.

See http://data.europa.eu/eli/dir/2015/849/oj 

WG Approval 21/11/2019"""@en ;
  skos:prefLabel "Beneficial owner nationality"@en ;
  skos:prefLabel "Has beneficial owner nationality"@en ;
.
epo:hasBirthFamilyName
  rdf:type owl:DatatypeProperty ;
  rdfs:isDefinedBy <http://data.europa.eu/a4g/ontology> ;
  rdfs:label "Birth family name"@en ;
  skos:prefLabel "Birth family name"@en ;
.
epo:hasBlockName
  rdf:type owl:DatatypeProperty ;
  rdfs:isDefinedBy <http://data.europa.eu/a4g/ontology> ;
  rdfs:label "Block name"@en ;
  skos:prefLabel "Block name"@en ;
.
epo:hasBroadPlaceOfPerformance
  rdf:type owl:ObjectProperty ;
  rdfs:comment """Geopolitical zone where the contract can be executed.

Additional Information

Used for setting restrictions that cannot be established with one country code or a geographical zone identifier (like NUTS), because they have a broader scope (geographical, economic, political, other)."""@en ;
  rdfs:isDefinedBy <http://data.europa.eu/a4g/ontology> ;
  rdfs:label "Broad place of performance"@en ;
  rdfs:label "Has broad place of performance"@en ;
  skos:definition """Geopolitical zone where the contract can be executed.

Additional Information

Used for setting restrictions that cannot be established with one country code or a geographical zone identifier (like NUTS), because they have a broader scope (geographical, economic, political, other)."""@en ;
  skos:prefLabel "Broad place of performance"@en ;
  skos:prefLabel "Has broad place of performance"@en ;
.
epo:hasBuildingName
  rdf:type owl:DatatypeProperty ;
  rdfs:isDefinedBy <http://data.europa.eu/a4g/ontology> ;
  rdfs:label "Building name"@en ;
  skos:prefLabel "Building name"@en ;
.
epo:hasBuildingNumber
  rdf:type owl:DatatypeProperty ;
  rdfs:isDefinedBy <http://data.europa.eu/a4g/ontology> ;
  rdfs:label "Building number"@en ;
  skos:prefLabel "Building number"@en ;
.
epo:hasBuyerCoverage
  rdf:type owl:DatatypeProperty ;
  rdfs:comment """Buyers that can use the Framework Agreement not mentioned by name.

Additional Information: 
For example,  \"all hospitals in the Tuscany region

WG Approval 2019-05-06"""@en ;
  rdfs:isDefinedBy <http://data.europa.eu/a4g/ontology> ;
  rdfs:label "Buyer coverage"@en ;
  skos:definition """Buyers that can use the Framework Agreement not mentioned by name.

Additional Information: 
For example,  \"all hospitals in the Tuscany region

WG Approval 2019-05-06"""@en ;
  skos:prefLabel "Buyer coverage"@en ;
.
epo:hasBuyerLegalType
  rdf:type owl:ObjectProperty ;
  rdfs:isDefinedBy <http://data.europa.eu/a4g/ontology> ;
  rdfs:label "Buyer legal type"@en ;
  rdfs:label "Has buyer legal type"@en ;
  skos:prefLabel "Buyer legal type"@en ;
  skos:prefLabel "Has buyer legal type"@en ;
.
epo:hasBuyerLegalTypeDescription
  rdf:type owl:DatatypeProperty ;
  rdfs:isDefinedBy <http://data.europa.eu/a4g/ontology> ;
  rdfs:label "Buyer legal type description"@en ;
  skos:prefLabel "Buyer legal type description"@en ;
.
epo:hasBuyers
  rdf:type owl:ObjectProperty ;
  rdfs:isDefinedBy <http://data.europa.eu/a4g/ontology> ;
  rdfs:label "Has buyers"@en ;
  skos:prefLabel "Has buyers"@en ;
.
epo:hasCalculationMethod
  rdf:type owl:DatatypeProperty ;
  rdfs:comment """Formula for obtaining values.

Additional Information:
The possible values are monetary values, ranking scores, criterion weighting.

WG Approval 25/05/2018"""@en ;
  rdfs:isDefinedBy <http://data.europa.eu/a4g/ontology> ;
  rdfs:label "Calculation method"@en ;
  skos:definition """Formula for obtaining values.

Additional Information:
The possible values are monetary values, ranking scores, criterion weighting.

WG Approval 25/05/2018"""@en ;
  skos:prefLabel "Calculation method"@en ;
.
epo:hasChangeReason
  rdf:type owl:ObjectProperty ;
  rdfs:comment """The motives for the change.

WG 5/11/2019"""@en ;
  rdfs:isDefinedBy <http://data.europa.eu/a4g/ontology> ;
  rdfs:label "Change reason"@en ;
  rdfs:label "Has change reason"@en ;
  skos:definition """The motives for the change.

WG 5/11/2019"""@en ;
  skos:prefLabel "Change reason"@en ;
  skos:prefLabel "Has change reason"@en ;
.
epo:hasChanged
  rdf:type owl:ObjectProperty ;
  rdfs:isDefinedBy <http://data.europa.eu/a4g/ontology> ;
  rdfs:label "Has changed"@en ;
  skos:prefLabel "Has changed"@en ;
.
epo:hasChangedElement
  rdf:type owl:ObjectProperty ;
  rdfs:isDefinedBy <http://data.europa.eu/a4g/ontology> ;
  rdfs:label "Has changed element"@en ;
  skos:prefLabel "Has changed element"@en ;
.
epo:hasChoiceJustification
  rdf:type owl:DatatypeProperty ;
  rdfs:isDefinedBy <http://data.europa.eu/a4g/ontology> ;
  rdfs:label "Choice justification"@en ;
  skos:prefLabel "Choice justification"@en ;
.
epo:hasCityName
  rdf:type owl:DatatypeProperty ;
  rdfs:isDefinedBy <http://data.europa.eu/a4g/ontology> ;
  rdfs:label "City name"@en ;
  skos:prefLabel "City name"@en ;
.
epo:hasCitySubdivisionName
  rdf:type owl:DatatypeProperty ;
  rdfs:isDefinedBy <http://data.europa.eu/a4g/ontology> ;
  rdfs:label "City subdivision name"@en ;
  skos:prefLabel "City subdivision name"@en ;
.
epo:hasClarificationsAvailableVia
  rdf:type owl:ObjectProperty ;
  rdfs:isDefinedBy <http://data.europa.eu/a4g/ontology> ;
  rdfs:label "Has clarifications available via"@en ;
  skos:prefLabel "Has clarifications available via"@en ;
.
epo:hasClassification
  rdf:type owl:ObjectProperty ;
  rdfs:isDefinedBy <http://data.europa.eu/a4g/ontology> ;
  rdfs:label "Classification"@en ;
  skos:prefLabel "Classification"@en ;
.
epo:hasCleanVehicles
  rdf:type owl:DatatypeProperty ;
  rdfs:isDefinedBy <http://data.europa.eu/a4g/ontology> ;
  rdfs:label "Clean vehicles"@en ;
  skos:prefLabel "Clean vehicles"@en ;
.
epo:hasCommunicationType
  rdf:type owl:ObjectProperty ;
  rdfs:isDefinedBy <http://data.europa.eu/a4g/ontology> ;
  rdfs:label "Communication type"@en ;
  rdfs:label "Has communication type"@en ;
  skos:prefLabel "Communication type"@en ;
  skos:prefLabel "Has communication type"@en ;
.
epo:hasCompetitionTermination
  rdf:type rdf:Property ;
  rdfs:comment """No further contracts will be awarded in this competition. This field can be used even if no contracts are awarded in the contract award notice.

Additional Information: 

PIN for Competition and DPS, for example, are cases where the termination needs to be signaled.
In the case of DPS this specifies the closure of the DPS. 
"""@en ;
  rdfs:isDefinedBy <http://data.europa.eu/a4g/ontology> ;
  rdfs:label "Competition termination"@en ;
  skos:definition """No further contracts will be awarded in this competition. This field can be used even if no contracts are awarded in the contract award notice.

Additional Information: 

PIN for Competition and DPS, for example, are cases where the termination needs to be signaled.
In the case of DPS this specifies the closure of the DPS. 
"""@en ;
  skos:prefLabel "Competition termination"@en ;
.
epo:hasContactPersonRole
  rdf:type owl:ObjectProperty ;
  rdfs:isDefinedBy <http://data.europa.eu/a4g/ontology> ;
  rdfs:label "Has contact person role"@en ;
  skos:prefLabel "Has contact person role"@en ;
.
epo:hasContractConclusionDate
  rdf:type owl:DatatypeProperty ;
  rdfs:comment """The date the contract was signed by the last signatory party.

<u>Additional Information:</u>
In exceptional cases contracts may be concluded without signature and therefore another date may be used. The date of contract conclusion is always later than the end of any standstill period.
This concept is not to be confused with the date of completion/end of the contract.

WG Approval 09/01/2020"""@en ;
  rdfs:isDefinedBy <http://data.europa.eu/a4g/ontology> ;
  rdfs:label "Contract conclusion date"@en ;
  skos:definition """The date the contract was signed by the last signatory party.

<u>Additional Information:</u>
In exceptional cases contracts may be concluded without signature and therefore another date may be used. The date of contract conclusion is always later than the end of any standstill period.
This concept is not to be confused with the date of completion/end of the contract.

WG Approval 09/01/2020"""@en ;
  skos:prefLabel "Contract conclusion date"@en ;
.
epo:hasContractEstimatedDuration
  rdf:type owl:ObjectProperty ;
  rdfs:comment """The estimated date when the contract is to be started.

Additional Information

When the Lot uses a Technique the contract estimated duration applies to the Technique.

"""@en ;
  rdfs:isDefinedBy <http://data.europa.eu/a4g/ontology> ;
  rdfs:label "Has contract estimated duration"@en ;
  skos:definition """The estimated date when the contract is to be started.

Additional Information

When the Lot uses a Technique the contract estimated duration applies to the Technique.

"""@en ;
  skos:prefLabel "Has contract estimated duration"@en ;
.
epo:hasContractModficationJustification
  rdf:type owl:ObjectProperty ;
  rdfs:isDefinedBy <http://data.europa.eu/a4g/ontology> ;
  rdfs:label "Has contract modfication justification"@en ;
  skos:prefLabel "Has contract modfication justification"@en ;
.
epo:hasContractNatureType
  rdf:type owl:ObjectProperty ;
  rdfs:isDefinedBy <http://data.europa.eu/a4g/ontology> ;
  rdfs:label "Contract nature type"@en ;
  rdfs:label "Has contract nature type"@en ;
  skos:prefLabel "Contract nature type"@en ;
  skos:prefLabel "Has contract nature type"@en ;
.
epo:hasContractPurpose
  rdf:type owl:ObjectProperty ;
  rdfs:isDefinedBy <http://data.europa.eu/a4g/ontology> ;
  rdfs:label "Has contract purpose"@en ;
  skos:prefLabel "Has contract purpose"@en ;
.
epo:hasContractingEntity
  rdf:type rdf:Property ;
  rdfs:comment """Role of entities, which:

(a) are contracting authorities or public undertakings and which pursue one of the activities referred to in Articles 8 to 14 of the Directive 2014/25/EU.

(b) when they are not contracting authorities or public undertakings, have as one of their activities any of the activities referred to in Articles 8 to 14, or any combination thereof and operate on the basis of special or exclusive rights granted by a competent authority of a Member State.

Additional Information

The indicator is needed in order to discriminate between those contracts where the Contracting Entity acts as a Contracting Authority undergoing the limits and the rules of Directive 24 and those where it acts as a  Contracting Entity, with certain relaxed constraints.
For example, the Contracting Entities have different thresholds for the application of Directive 24 if compared with Contracting Authorities.

WG Approval 28/04/2020
"""@en ;
  rdfs:isDefinedBy <http://data.europa.eu/a4g/ontology> ;
  rdfs:label "Contracting entity"@en ;
  skos:definition """Role of entities, which:

(a) are contracting authorities or public undertakings and which pursue one of the activities referred to in Articles 8 to 14 of the Directive 2014/25/EU.

(b) when they are not contracting authorities or public undertakings, have as one of their activities any of the activities referred to in Articles 8 to 14, or any combination thereof and operate on the basis of special or exclusive rights granted by a competent authority of a Member State.

Additional Information

The indicator is needed in order to discriminate between those contracts where the Contracting Entity acts as a Contracting Authority undergoing the limits and the rules of Directive 24 and those where it acts as a  Contracting Entity, with certain relaxed constraints.
For example, the Contracting Entities have different thresholds for the application of Directive 24 if compared with Contracting Authorities.

WG Approval 28/04/2020
"""@en ;
  skos:prefLabel "Contracting entity"@en ;
.
epo:hasContractorLegalFormRequirement
  rdf:type rdf:Property ;
  rdfs:comment """A specific legal entity must be taken up by a tenderer composed of a group of economic operators once it has been awarded a contract.

Additional information: this may be applied in the case of groups (e.g. a consortium) where the requirement is that they have to formalise the relationship of the group members as a legal entity itself once the contract is awarded.

WG Approval 2019-01-29
"""@en ;
  rdfs:isDefinedBy <http://data.europa.eu/a4g/ontology> ;
  rdfs:label "Contractor legal form requirement"@en ;
  skos:definition """A specific legal entity must be taken up by a tenderer composed of a group of economic operators once it has been awarded a contract.

Additional information: this may be applied in the case of groups (e.g. a consortium) where the requirement is that they have to formalise the relationship of the group members as a legal entity itself once the contract is awarded.

WG Approval 2019-01-29
"""@en ;
  skos:prefLabel "Contractor legal form requirement"@en ;
.
epo:hasContractorLegalFormRequirementDescription
  rdf:type owl:DatatypeProperty ;
  rdfs:comment "A constraint concerning the legal form that must be adopted by a tenderer composed of a group of economic operators once it has been awarded a contract."@en ;
  rdfs:isDefinedBy <http://data.europa.eu/a4g/ontology> ;
  rdfs:label "Contractor legal form requirement description"@en ;
  skos:definition "A constraint concerning the legal form that must be adopted by a tenderer composed of a group of economic operators once it has been awarded a contract."@en ;
  skos:prefLabel "Contractor legal form requirement description"@en ;
.
epo:hasCoordinateSystem
  rdf:type owl:ObjectProperty ;
  rdfs:isDefinedBy <http://data.europa.eu/a4g/ontology> ;
  rdfs:label "Coordinate system"@en ;
  skos:prefLabel "Coordinate system"@en ;
.
epo:hasCountry
  rdf:type owl:ObjectProperty ;
  rdfs:comment """A country is one of the political units which the world is divided into, covering a particular area of land.

(WG approval 8/06/2018)"""@en ;
  rdfs:isDefinedBy <http://data.europa.eu/a4g/ontology> ;
  rdfs:label "Country"@en ;
  rdfs:label "Has country"@en ;
  skos:definition """A country is one of the political units which the world is divided into, covering a particular area of land.

(WG approval 8/06/2018)"""@en ;
  skos:prefLabel "Country"@en ;
  skos:prefLabel "Has country"@en ;
.
epo:hasCountryCode
  rdf:type owl:ObjectProperty ;
  rdfs:isDefinedBy <http://data.europa.eu/a4g/ontology> ;
  rdfs:label "Country code"@en ;
  rdfs:label "Has country code"@en ;
  skos:prefLabel "Country code"@en ;
  skos:prefLabel "Has country code"@en ;
.
epo:hasCountryOfBirth
  rdf:type owl:ObjectProperty ;
  rdfs:isDefinedBy <http://data.europa.eu/a4g/ontology> ;
  rdfs:label "Has country of birth"@en ;
  skos:prefLabel "Has country of birth"@en ;
.
epo:hasCountryOfOrigin
  rdf:type owl:ObjectProperty ;
  rdfs:comment """The source country of the product or service.

<u>Additional Information:</u>
<u>
</u>The country of origin can be provided by  the buyer as a requirement or by the tenderer information of the item to be provided.

WG Approval 07/01/2020"""@en ;
  rdfs:isDefinedBy <http://data.europa.eu/a4g/ontology> ;
  rdfs:label "Country of origin"@en ;
  rdfs:label "Has country of origin"@en ;
  skos:definition """The source country of the product or service.

<u>Additional Information:</u>
<u>
</u>The country of origin can be provided by  the buyer as a requirement or by the tenderer information of the item to be provided.

WG Approval 07/01/2020"""@en ;
  skos:prefLabel "Country of origin"@en ;
  skos:prefLabel "Has country of origin"@en ;
.
epo:hasCountrySubentity
  rdf:type owl:DatatypeProperty ;
  rdfs:isDefinedBy <http://data.europa.eu/a4g/ontology> ;
  rdfs:label "Country subentity"@en ;
  skos:prefLabel "Country subentity"@en ;
.
epo:hasCountrySubentityCode
  rdf:type owl:ObjectProperty ;
  rdfs:isDefinedBy <http://data.europa.eu/a4g/ontology> ;
  rdfs:label "Country subentity code"@en ;
  rdfs:label "Has country subentity code"@en ;
  skos:prefLabel "Country subentity code"@en ;
  skos:prefLabel "Has country subentity code"@en ;
.
epo:hasCurrency
  rdf:type owl:ObjectProperty ;
  rdfs:isDefinedBy <http://data.europa.eu/a4g/ontology> ;
  rdfs:label "Currency"@en ;
  rdfs:label "Has currency"@en ;
  skos:prefLabel "Currency"@en ;
  skos:prefLabel "Has currency"@en ;
.
epo:hasCurrencyType
  rdf:type owl:ObjectProperty ;
  rdfs:isDefinedBy <http://data.europa.eu/a4g/ontology> ;
  rdfs:label "Currency type"@en ;
  rdfs:label "Has currency type"@en ;
  skos:prefLabel "Currency type"@en ;
  skos:prefLabel "Has currency type"@en ;
.
epo:hasDPSScopeType
  rdf:type owl:ObjectProperty ;
  rdfs:isDefinedBy <http://data.europa.eu/a4g/ontology> ;
  rdfs:label "D p s scope type"@en ;
  skos:prefLabel "D p s scope type"@en ;
.
epo:hasDPSTermination
  rdf:type rdf:Property ;
  rdfs:comment """End of the Dynamic Purchase System (DPS). 

Additional Information: This property can be used in the contract award notice even if no contracts are awarded . 

WG Approval 22/11/2019"""@en ;
  rdfs:isDefinedBy <http://data.europa.eu/a4g/ontology> ;
  rdfs:label "D p s termination"@en ;
  skos:definition """End of the Dynamic Purchase System (DPS). 

Additional Information: This property can be used in the contract award notice even if no contracts are awarded . 

WG Approval 22/11/2019"""@en ;
  skos:prefLabel "D p s termination"@en ;
.
epo:hasDPSUsage
  rdf:type owl:ObjectProperty ;
  rdfs:isDefinedBy <http://data.europa.eu/a4g/ontology> ;
  rdfs:label "D p s usage"@en ;
  rdfs:label "Has d p s usage"@en ;
  skos:prefLabel "D p s usage"@en ;
  skos:prefLabel "Has d p s usage"@en ;
.
epo:hasDateOfBirth
  rdf:type owl:DatatypeProperty ;
  rdfs:isDefinedBy <http://data.europa.eu/a4g/ontology> ;
  rdfs:label "Date of birth"@en ;
  skos:prefLabel "Date of birth"@en ;
.
epo:hasDateOfDeath
  rdf:type owl:DatatypeProperty ;
  rdfs:isDefinedBy <http://data.europa.eu/a4g/ontology> ;
  rdfs:label "Date of death"@en ;
  skos:prefLabel "Date of death"@en ;
.
epo:hasDateTime
  rdf:type owl:DatatypeProperty ;
  rdfs:comment """The date and time of the change

WG Approval 5/11/2019
"""@en ;
  rdfs:isDefinedBy <http://data.europa.eu/a4g/ontology> ;
  rdfs:label "Date time"@en ;
  skos:definition """The date and time of the change

WG Approval 5/11/2019
"""@en ;
  skos:prefLabel "Date time"@en ;
.
epo:hasDeadline
  rdf:type owl:DatatypeProperty ;
  rdfs:comment """The deadline by which the security clearance must be submitted to the buyer.

WG Approval 12/09/2019

"""@en ;
  rdfs:isDefinedBy <http://data.europa.eu/a4g/ontology> ;
  rdfs:label "Deadline"@en ;
  skos:definition """The deadline by which the security clearance must be submitted to the buyer.

WG Approval 12/09/2019

"""@en ;
  skos:prefLabel "Deadline"@en ;
.
epo:hasDefaultContactPoint
  rdf:type owl:ObjectProperty ;
  rdfs:comment "To be discussed 30/04/2020"@en ;
  rdfs:isDefinedBy <http://data.europa.eu/a4g/ontology> ;
  rdfs:label "Has default contact point"@en ;
  skos:definition "To be discussed 30/04/2020"@en ;
  skos:prefLabel "Has default contact point"@en ;
.
epo:hasDepartment
  rdf:type owl:DatatypeProperty ;
  rdfs:isDefinedBy <http://data.europa.eu/a4g/ontology> ;
  rdfs:label "Department"@en ;
  skos:prefLabel "Department"@en ;
.
epo:hasDescription
  rdf:type rdf:Property ;
  rdf:type owl:DatatypeProperty ;
  rdfs:comment "A description of this period, expressed as text."@en ;
  rdfs:comment """A narrative text explaining the content of an instance of the class.

WG Decision 17/09/2019 """@en ;
  rdfs:comment """Additional information about the security clearance (e.g. which level of security clearance is required, which team members must have it, whether it is necessary already for accessing the procurement documents or only for contract execution).

WG Approval 12/09/2019
"""@en ;
  rdfs:comment """An explanatory text about this context. 

 WG Approval 5/11/2019"""@en ;
  rdfs:comment """Information about the change.

Additional Information

Used, for example, to explain the main reason for the change in a document compared to the original document.

WG Approval 17/10/2019"""@en ;
  rdfs:comment """Self-explanatory text about a concept.

"""@en ;
  rdfs:comment """Self-explanatory text about a concept.

WG Approval 08/05/2019"""@en ;
  rdfs:comment """Self-explanatory text about a concept.

WG Approval 23/04/2020"""@en ;
  rdfs:comment """Self-explanatory text about a concept.
"""@en ;
  rdfs:comment """Self-explanatory text about the instance of the concept.

WG Approval 30/09/2019"""@en ;
  rdfs:isDefinedBy <http://data.europa.eu/a4g/ontology> ;
  rdfs:label "Description"@en ;
  skos:definition "A description of this period, expressed as text."@en ;
  skos:definition """A narrative text explaining the content of an instance of the class.

WG Decision 17/09/2019 """@en ;
  skos:definition """Additional information about the security clearance (e.g. which level of security clearance is required, which team members must have it, whether it is necessary already for accessing the procurement documents or only for contract execution).

WG Approval 12/09/2019
"""@en ;
  skos:definition """An explanatory text about this context. 

 WG Approval 5/11/2019"""@en ;
  skos:definition """Information about the change.

Additional Information

Used, for example, to explain the main reason for the change in a document compared to the original document.

WG Approval 17/10/2019"""@en ;
  skos:definition """Self-explanatory text about a concept.

"""@en ;
  skos:definition """Self-explanatory text about a concept.

WG Approval 08/05/2019"""@en ;
  skos:definition """Self-explanatory text about a concept.

WG Approval 23/04/2020"""@en ;
  skos:definition """Self-explanatory text about a concept.
"""@en ;
  skos:definition """Self-explanatory text about the instance of the concept.

WG Approval 30/09/2019"""@en ;
  skos:prefLabel "Description"@en ;
.
epo:hasDescriptionCode
  rdf:type rdf:Property ;
  rdfs:comment """A code to inform about a lapse of time that cannot be expressed by means of a start data and end date or duration measure. 

Additional information
For example, unlimited, unknown, etc.

WG Approval 1/08/2019"""@en ;
  rdfs:isDefinedBy <http://data.europa.eu/a4g/ontology> ;
  rdfs:label "Description code"@en ;
  skos:definition """A code to inform about a lapse of time that cannot be expressed by means of a start data and end date or duration measure. 

Additional information
For example, unlimited, unknown, etc.

WG Approval 1/08/2019"""@en ;
  skos:prefLabel "Description code"@en ;
.
epo:hasDesignContestType
  rdf:type owl:ObjectProperty ;
  rdfs:isDefinedBy <http://data.europa.eu/a4g/ontology> ;
  rdfs:label "Design contest type"@en ;
  rdfs:label "Has design contest type"@en ;
  skos:prefLabel "Design contest type"@en ;
  skos:prefLabel "Has design contest type"@en ;
.
epo:hasDispatchDate
  rdf:type owl:DatatypeProperty ;
  rdfs:comment "Date of transmission of a record to an organisation."@en ;
  rdfs:isDefinedBy <http://data.europa.eu/a4g/ontology> ;
  rdfs:label "Dispatch date"@en ;
  skos:definition "Date of transmission of a record to an organisation."@en ;
  skos:prefLabel "Dispatch date"@en ;
.
epo:hasDistrict
  rdf:type owl:DatatypeProperty ;
  rdfs:isDefinedBy <http://data.europa.eu/a4g/ontology> ;
  rdfs:label "District"@en ;
  skos:prefLabel "District"@en ;
.
epo:hasDownloadURL
  rdf:type owl:ObjectProperty ;
  rdfs:isDefinedBy <http://data.europa.eu/a4g/ontology> ;
  rdfs:label "Has download u r l"@en ;
  skos:prefLabel "Has download u r l"@en ;
.
epo:hasDuration
  rdf:type owl:ObjectProperty ;
  rdfs:isDefinedBy <http://data.europa.eu/a4g/ontology> ;
  rdfs:label "Has duration"@en ;
  skos:prefLabel "Has duration"@en ;
.
epo:hasDurationEvaluationPeriod
  rdf:type owl:ObjectProperty ;
  rdfs:isDefinedBy <http://data.europa.eu/a4g/ontology> ;
  rdfs:label "Has duration evaluation period"@en ;
  skos:prefLabel "Has duration evaluation period"@en ;
.
epo:hasDurationExtensionJustification
  rdf:type owl:DatatypeProperty ;
  rdfs:comment """The justification for exceptional cases when the duration of the framework agreement exceeds the legal limits. 

Additional Information

Four years in the case of the general procurement Directive, seven years in the case of the defence Directive, and eight years in the case of the sectoral Directive.

WG Approval 26/09/2019"""@en ;
  rdfs:isDefinedBy <http://data.europa.eu/a4g/ontology> ;
  rdfs:label "Duration extension justification"@en ;
  skos:definition """The justification for exceptional cases when the duration of the framework agreement exceeds the legal limits. 

Additional Information

Four years in the case of the general procurement Directive, seven years in the case of the defence Directive, and eight years in the case of the sectoral Directive.

WG Approval 26/09/2019"""@en ;
  skos:prefLabel "Duration extension justification"@en ;
.
epo:hasDurationMeasure
  rdf:type owl:ObjectProperty ;
  rdfs:comment """The duration of this period, expressed as an ISO 8601 code. See also the ccts:Measure data type in the ePO package \"ccts\".
"""@en ;
  rdfs:isDefinedBy <http://data.europa.eu/a4g/ontology> ;
  rdfs:label "Duration measure"@en ;
  skos:definition """The duration of this period, expressed as an ISO 8601 code. See also the ccts:Measure data type in the ePO package \"ccts\".
"""@en ;
  skos:prefLabel "Duration measure"@en ;
.
epo:hasECataloguePermissions
  rdf:type owl:ObjectProperty ;
  rdfs:isDefinedBy <http://data.europa.eu/a4g/ontology> ;
  rdfs:label "Has e catalogue permissions"@en ;
  skos:prefLabel "Has e catalogue permissions"@en ;
.
epo:hasEEARecievedTenderLots
  rdf:type owl:DatatypeProperty ;
  rdfs:comment """The amount of tenders received from economic operators in other EEA countries other than the country of the buyer.

WG Approval 12/12/2019"""@en ;
  rdfs:isDefinedBy <http://data.europa.eu/a4g/ontology> ;
  rdfs:label "E e a recieved tender lots"@en ;
  skos:definition """The amount of tenders received from economic operators in other EEA countries other than the country of the buyer.

WG Approval 12/12/2019"""@en ;
  skos:prefLabel "E e a recieved tender lots"@en ;
.
epo:hasEOGroupType
  rdf:type owl:ObjectProperty ;
  rdfs:isDefinedBy <http://data.europa.eu/a4g/ontology> ;
  rdfs:label "E o group type"@en ;
  rdfs:label "Has e o group type"@en ;
  skos:prefLabel "E o group type"@en ;
  skos:prefLabel "Has e o group type"@en ;
.
epo:hasEOSizeType
  rdf:type owl:ObjectProperty ;
  rdfs:isDefinedBy <http://data.europa.eu/a4g/ontology> ;
  rdfs:label "E o size type"@en ;
  skos:prefLabel "E o size type"@en ;
.
epo:hasEOsHavingInterestIn
  rdf:type owl:ObjectProperty ;
  rdfs:isDefinedBy <http://data.europa.eu/a4g/ontology> ;
  rdfs:label "Has e os having interest in"@en ;
  skos:prefLabel "Has e os having interest in"@en ;
.
epo:hasEconomicOperatorSize
  rdf:type owl:ObjectProperty ;
  rdfs:isDefinedBy <http://data.europa.eu/a4g/ontology> ;
  rdfs:label "Has economic operator size"@en ;
  skos:prefLabel "Has economic operator size"@en ;
.
epo:hasElectronicSubmission
  rdf:type rdf:Property ;
  rdfs:comment "Transmission of tenders is possible by electronic means of communication. "@en ;
  rdfs:isDefinedBy <http://data.europa.eu/a4g/ontology> ;
  rdfs:label "Electronic submission"@en ;
  skos:definition "Transmission of tenders is possible by electronic means of communication. "@en ;
  skos:prefLabel "Electronic submission"@en ;
.
epo:hasElementIRI
  rdf:type rdf:Property ;
  rdfs:comment "The Element may identify any type of elements, including documents, e.g. a Procurement Document that has changed."@en ;
  rdfs:isDefinedBy <http://data.europa.eu/a4g/ontology> ;
  rdfs:label "Element i r i"@en ;
  skos:definition "The Element may identify any type of elements, including documents, e.g. a Procurement Document that has changed."@en ;
  skos:prefLabel "Element i r i"@en ;
.
epo:hasEmail
  rdf:type rdf:Property ;
  rdfs:comment "The eMail address used to reach a person or an organisation."@en ;
  rdfs:isDefinedBy <http://data.europa.eu/a4g/ontology> ;
  rdfs:label "Email"@en ;
  skos:definition "The eMail address used to reach a person or an organisation."@en ;
  skos:prefLabel "Email"@en ;
.
epo:hasEndDate
  rdf:type owl:DatatypeProperty ;
  rdfs:comment "The date on which this period ends."@en ;
  rdfs:isDefinedBy <http://data.europa.eu/a4g/ontology> ;
  rdfs:label "End date"@en ;
  skos:definition "The date on which this period ends."@en ;
  skos:prefLabel "End date"@en ;
.
epo:hasEndTime
  rdf:type rdf:Property ;
  rdfs:comment "The time at which this period ends."@en ;
  rdfs:isDefinedBy <http://data.europa.eu/a4g/ontology> ;
  rdfs:label "End time"@en ;
  skos:definition "The time at which this period ends."@en ;
  skos:prefLabel "End time"@en ;
.
epo:hasEndpoint
  rdf:type rdf:Property ;
  rdfs:isDefinedBy <http://data.europa.eu/a4g/ontology> ;
  rdfs:label "Endpoint"@en ;
  skos:prefLabel "Endpoint"@en ;
.
epo:hasEntryintoForceDate
  rdf:type owl:DatatypeProperty ;
  rdfs:comment """The date on which the contract enters into force.

Additional information: 

This is generally the date on which the fulfillment of the contract begins.

WG approval 05/11/2019"""@en ;
  rdfs:isDefinedBy <http://data.europa.eu/a4g/ontology> ;
  rdfs:label "Entryinto force date"@en ;
  skos:definition """The date on which the contract enters into force.

Additional information: 

This is generally the date on which the fulfillment of the contract begins.

WG approval 05/11/2019"""@en ;
  skos:prefLabel "Entryinto force date"@en ;
.
epo:hasEstimatedBuyerConcessionRevenue
  rdf:type owl:ObjectProperty ;
  rdfs:comment """The expected payments made by the buyer to the economic operator awarded the concession that are not directly related to the use of the concession.

<u>Additional Information:</u>
For example the public buyer pays a yearly fee to provide a ticketing solution to the public.  The fee the public pays for every ticket sold through the solution is not included in this estimation but in the estimation of the user concession revenue.

WG Approval 07/01/2020"""@en ;
  rdfs:isDefinedBy <http://data.europa.eu/a4g/ontology> ;
  rdfs:label "Has estimated buyer concession revenue"@en ;
  skos:definition """The expected payments made by the buyer to the economic operator awarded the concession that are not directly related to the use of the concession.

<u>Additional Information:</u>
For example the public buyer pays a yearly fee to provide a ticketing solution to the public.  The fee the public pays for every ticket sold through the solution is not included in this estimation but in the estimation of the user concession revenue.

WG Approval 07/01/2020"""@en ;
  skos:prefLabel "Has estimated buyer concession revenue"@en ;
.
epo:hasEstimatedContractNoticePublicationDate
  rdf:type owl:DatatypeProperty ;
  rdfs:isDefinedBy <http://data.europa.eu/a4g/ontology> ;
  rdfs:label "Estimated contract notice publication date"@en ;
  skos:prefLabel "Estimated contract notice publication date"@en ;
.
epo:hasEstimatedDuration
  rdf:type owl:ObjectProperty ;
  rdfs:isDefinedBy <http://data.europa.eu/a4g/ontology> ;
  rdfs:label "Has estimated duration"@en ;
  skos:prefLabel "Has estimated duration"@en ;
.
epo:hasEstimatedInvitationToExpressInterestDate
  rdf:type owl:DatatypeProperty ;
  rdfs:comment """The estimated date of dispatch of the invitations to confirm interest.
"""@en ;
  rdfs:isDefinedBy <http://data.europa.eu/a4g/ontology> ;
  rdfs:label "Estimated invitation to express interest date"@en ;
  skos:definition """The estimated date of dispatch of the invitations to confirm interest.
"""@en ;
  skos:prefLabel "Estimated invitation to express interest date"@en ;
.
epo:hasEstimatedInvitationToTenderDate
  rdf:type owl:DatatypeProperty ;
  rdfs:comment """The estimated date of dispatch of the invitations to submit tenders in two (or more) stage procedures.

WG Approval 01/10/2019"""@en ;
  rdfs:isDefinedBy <http://data.europa.eu/a4g/ontology> ;
  rdfs:label "Estimated invitation to tender date"@en ;
  skos:definition """The estimated date of dispatch of the invitations to submit tenders in two (or more) stage procedures.

WG Approval 01/10/2019"""@en ;
  skos:prefLabel "Estimated invitation to tender date"@en ;
.
epo:hasEstimatedShare
  rdf:type rdf:Property ;
  rdfs:comment """The estimated proportion foreseen to be subcontracted.

WG Approval 07/01/2020"""@en ;
  rdfs:isDefinedBy <http://data.europa.eu/a4g/ontology> ;
  rdfs:label "Estimated share"@en ;
  skos:definition """The estimated proportion foreseen to be subcontracted.

WG Approval 07/01/2020"""@en ;
  skos:prefLabel "Estimated share"@en ;
.
epo:hasEstimatedTenderInvitationDate
  rdf:type owl:DatatypeProperty ;
  rdfs:isDefinedBy <http://data.europa.eu/a4g/ontology> ;
  rdfs:label "Estimated tender invitation date"@en ;
  skos:prefLabel "Estimated tender invitation date"@en ;
.
epo:hasEstimatedUserConcessionRevenue
  rdf:type owl:ObjectProperty ;
  rdfs:comment """The estimated revenue coming from the use of the concession.

Additional Information:
Revenues are for example fees and fines. For example, the fees and fines coming from the cars using a motorway."""@en ;
  rdfs:isDefinedBy <http://data.europa.eu/a4g/ontology> ;
  rdfs:label "Has estimated user concession revenue"@en ;
  skos:definition """The estimated revenue coming from the use of the concession.

Additional Information:
Revenues are for example fees and fines. For example, the fees and fines coming from the cars using a motorway."""@en ;
  skos:prefLabel "Has estimated user concession revenue"@en ;
.
epo:hasEstimatedValue
  rdf:type owl:ObjectProperty ;
  rdfs:comment """A forecast of the value of the procurement before competition.

Additional Information
Different cases of estimated values may refer to a lot, the global value of the procedure, or of a combinatorial value of a group of lots.
The forecast is calculated by the buyer and covers all revenues  whether coming from the buyer or third parties.
See for example recital (19), Article 5 of Directive 2014/24/EU and other articles from the rest of Directives about procurement.

In the case of framework agreements and dynamic purchasing systems this refers to the maximum estimated value.
<b>
</b><b>WG Approval 05/12/2019</b>
"""@en ;
  rdfs:comment """A forecast of the value of the procurement before competition.

Additional Information
Different cases of estimated values may refer to a lot, the global value of the procedure, or of a combinatorial value of a group of lots.
The forecast is calculated by the buyer and covers all revenues  whether coming from the buyer or third parties.
See for example recital (19), Article 5 of Directive 2014/24/EU and other articles from the rest of Directives about procurement.

In the case of lots or groups of lots using framework agreements and dynamic purchasing systems this refers to the maximum estimated value.
<b>
</b><b>WG Approval 05/12/2019</b>"""@en ;
  rdfs:comment """The estimated value of the part of the contract to be subcontracted.

WG Approval 08/05/2019
"""@en ;
  rdfs:isDefinedBy <http://data.europa.eu/a4g/ontology> ;
  rdfs:label "Has estimated value"@en ;
  skos:definition """A forecast of the value of the procurement before competition.

Additional Information
Different cases of estimated values may refer to a lot, the global value of the procedure, or of a combinatorial value of a group of lots.
The forecast is calculated by the buyer and covers all revenues  whether coming from the buyer or third parties.
See for example recital (19), Article 5 of Directive 2014/24/EU and other articles from the rest of Directives about procurement.

In the case of framework agreements and dynamic purchasing systems this refers to the maximum estimated value.
<b>
</b><b>WG Approval 05/12/2019</b>
"""@en ;
  skos:definition """A forecast of the value of the procurement before competition.

Additional Information
Different cases of estimated values may refer to a lot, the global value of the procedure, or of a combinatorial value of a group of lots.
The forecast is calculated by the buyer and covers all revenues  whether coming from the buyer or third parties.
See for example recital (19), Article 5 of Directive 2014/24/EU and other articles from the rest of Directives about procurement.

In the case of lots or groups of lots using framework agreements and dynamic purchasing systems this refers to the maximum estimated value.
<b>
</b><b>WG Approval 05/12/2019</b>"""@en ;
  skos:definition """The estimated value of the part of the contract to be subcontracted.

WG Approval 08/05/2019
"""@en ;
  skos:prefLabel "Has estimated value"@en ;
.
epo:hasEvaluationGroupType
  rdf:type owl:ObjectProperty ;
  rdfs:isDefinedBy <http://data.europa.eu/a4g/ontology> ;
  rdfs:label "Evaluation group type"@en ;
  rdfs:label "Has evaluation group type"@en ;
  skos:prefLabel "Evaluation group type"@en ;
  skos:prefLabel "Has evaluation group type"@en ;
.
epo:hasExclusionGorundApplicability
  rdf:type owl:ObjectProperty ;
  rdfs:isDefinedBy <http://data.europa.eu/a4g/ontology> ;
  rdfs:label "Has exclusion gorund applicability"@en ;
  skos:prefLabel "Has exclusion gorund applicability"@en ;
.
epo:hasExclusionGroundApplicability
  rdf:type owl:ObjectProperty ;
  rdfs:isDefinedBy <http://data.europa.eu/a4g/ontology> ;
  rdfs:label "Exclusion ground applicability"@en ;
  skos:prefLabel "Exclusion ground applicability"@en ;
.
epo:hasExclusionGroundType
  rdf:type owl:ObjectProperty ;
  rdfs:isDefinedBy <http://data.europa.eu/a4g/ontology> ;
  rdfs:label "Has exclusion ground type"@en ;
  skos:prefLabel "Has exclusion ground type"@en ;
.
epo:hasFamilyName
  rdf:type owl:DatatypeProperty ;
  rdfs:isDefinedBy <http://data.europa.eu/a4g/ontology> ;
  rdfs:label "Family name"@en ;
  skos:prefLabel "Family name"@en ;
.
epo:hasFax
  rdf:type owl:DatatypeProperty ;
  rdfs:comment "The fax number used to reach a person or an organisation."@en ;
  rdfs:isDefinedBy <http://data.europa.eu/a4g/ontology> ;
  rdfs:label "Fax"@en ;
  skos:definition "The fax number used to reach a person or an organisation."@en ;
  skos:prefLabel "Fax"@en ;
.
epo:hasFinalRanking
  rdf:type owl:DatatypeProperty ;
  rdfs:comment """If there's no first stage then there is only a final stage.

"""@en ;
  rdfs:isDefinedBy <http://data.europa.eu/a4g/ontology> ;
  rdfs:label "Final ranking"@en ;
  skos:definition """If there's no first stage then there is only a final stage.

"""@en ;
  skos:prefLabel "Final ranking"@en ;
.
epo:hasFixedValue
  rdf:type owl:DatatypeProperty ;
  rdfs:comment """The overall criteria of one single type that will be evaluated. 

Additional information:  

For instance quality, cost and price  are award criteria. One dimension would be quality with its own weight and threshold that maybe calculated on the basis of the individual criteria.

WG decision 05/11/2019  """@en ;
  rdfs:isDefinedBy <http://data.europa.eu/a4g/ontology> ;
  rdfs:label "Fixed value"@en ;
  skos:definition """The overall criteria of one single type that will be evaluated. 

Additional information:  

For instance quality, cost and price  are award criteria. One dimension would be quality with its own weight and threshold that maybe calculated on the basis of the individual criteria.

WG decision 05/11/2019  """@en ;
  skos:prefLabel "Fixed value"@en ;
.
epo:hasFixedValueType
  rdf:type owl:ObjectProperty ;
  rdfs:comment """The method to interpret the fixed value as pertaining to a total or unit.

WG Approval 17/09/2019"""@en ;
  rdfs:isDefinedBy <http://data.europa.eu/a4g/ontology> ;
  rdfs:label "Fixed value type"@en ;
  rdfs:label "Has fixed value type"@en ;
  skos:definition """The method to interpret the fixed value as pertaining to a total or unit.

WG Approval 17/09/2019"""@en ;
  skos:prefLabel "Fixed value type"@en ;
  skos:prefLabel "Has fixed value type"@en ;
.
epo:hasFloor
  rdf:type owl:DatatypeProperty ;
  rdfs:isDefinedBy <http://data.europa.eu/a4g/ontology> ;
  rdfs:label "Floor"@en ;
  skos:prefLabel "Floor"@en ;
.
epo:hasFollow-upContract
  rdf:type rdf:Property ;
  rdfs:comment """Any subsequent service contract will be awarded to the winner or, in the case of a design contest, winners.

WG Approval 29/08/2019 """@en ;
  rdfs:isDefinedBy <http://data.europa.eu/a4g/ontology> ;
  rdfs:label "Follow-up contract"@en ;
  skos:definition """Any subsequent service contract will be awarded to the winner or, in the case of a design contest, winners.

WG Approval 29/08/2019 """@en ;
  skos:prefLabel "Follow-up contract"@en ;
.
epo:hasFollow-upContractInformation
  rdf:type owl:DatatypeProperty ;
  rdfs:comment """Further information about follow-up contracts, prizes and payments (for example non-monetary prizes, payments given for participation).

WG Approval 03/09/2019"""@en ;
  rdfs:isDefinedBy <http://data.europa.eu/a4g/ontology> ;
  rdfs:label "Follow-up contract information"@en ;
  skos:definition """Further information about follow-up contracts, prizes and payments (for example non-monetary prizes, payments given for participation).

WG Approval 03/09/2019"""@en ;
  skos:prefLabel "Follow-up contract information"@en ;
.
epo:hasFormType
  rdf:type owl:ObjectProperty ;
  rdfs:isDefinedBy <http://data.europa.eu/a4g/ontology> ;
  rdfs:label "Form type"@en ;
  rdfs:label "Has form type"@en ;
  skos:prefLabel "Form type"@en ;
  skos:prefLabel "Has form type"@en ;
.
epo:hasFormalLocation
  rdf:type owl:ObjectProperty ;
  rdfs:isDefinedBy <http://data.europa.eu/a4g/ontology> ;
  rdfs:label "Has formal location"@en ;
  skos:prefLabel "Has formal location"@en ;
.
epo:hasFormalName
  rdf:type owl:ObjectProperty ;
  rdfs:isDefinedBy <http://data.europa.eu/a4g/ontology> ;
  rdfs:label "Has formal name"@en ;
  skos:prefLabel "Has formal name"@en ;
.
epo:hasFormula
  rdf:type owl:DatatypeProperty ;
  rdfs:isDefinedBy <http://data.europa.eu/a4g/ontology> ;
  rdfs:label "Formula"@en ;
  skos:prefLabel "Formula"@en ;
.
epo:hasFrameworkAgreementType
  rdf:type owl:ObjectProperty ;
  rdfs:comment """The form of framework agreement used in a procurement procedure.

Addition information:

A concept to distinguish the different types of framework agreement, which are: 
1. Framework agreement without reopening of competition,
2. Framework agreement with reopening of competition, or 
3. Framework agreement partly without reopening of competition.

WG Approval 19/09/2019 

"""@en ;
  rdfs:isDefinedBy <http://data.europa.eu/a4g/ontology> ;
  rdfs:label "Framework agreement type"@en ;
  rdfs:label "Has framework agreement type"@en ;
  skos:definition """The form of framework agreement used in a procurement procedure.

Addition information:

A concept to distinguish the different types of framework agreement, which are: 
1. Framework agreement without reopening of competition,
2. Framework agreement with reopening of competition, or 
3. Framework agreement partly without reopening of competition.

WG Approval 19/09/2019 

"""@en ;
  skos:prefLabel "Framework agreement type"@en ;
  skos:prefLabel "Has framework agreement type"@en ;
.
epo:hasFreeE-Access
  rdf:type rdf:Property ;
  rdfs:comment "Indicates whether the procurement documents are electronically available for unrestricted and full direct access, free of charge."@en ;
  rdfs:isDefinedBy <http://data.europa.eu/a4g/ontology> ;
  rdfs:label "Free e- access"@en ;
  skos:definition "Indicates whether the procurement documents are electronically available for unrestricted and full direct access, free of charge."@en ;
  skos:prefLabel "Free e- access"@en ;
.
epo:hasFulfillsRequirement
  rdf:type owl:ObjectProperty ;
  rdfs:isDefinedBy <http://data.europa.eu/a4g/ontology> ;
  rdfs:label "Fulfills requirement"@en ;
  skos:prefLabel "Fulfills requirement"@en ;
.
epo:hasFullName
  rdf:type owl:DatatypeProperty ;
  rdfs:isDefinedBy <http://data.europa.eu/a4g/ontology> ;
  rdfs:label "Full name"@en ;
  skos:prefLabel "Full name"@en ;
.
epo:hasFunctionType
  rdf:type owl:ObjectProperty ;
  rdfs:comment """

"""@en ;
  rdfs:isDefinedBy <http://data.europa.eu/a4g/ontology> ;
  rdfs:label "Function type"@en ;
  rdfs:label "Has function type"@en ;
  skos:definition """

"""@en ;
  skos:prefLabel "Function type"@en ;
  skos:prefLabel "Has function type"@en ;
.
epo:hasGPAUsage
  rdf:type rdf:Property ;
  rdfs:comment """Specifies whether the Agreement on Government Procurement (GPA) applies.

Additional information: 
The GPA aims to establish a multilateral framework of balanced rights and obligations relating to public contracts with a view to achieving the liberalization and expansion of world trade.

WG Approval 15/10/2019

"""@en ;
  rdfs:isDefinedBy <http://data.europa.eu/a4g/ontology> ;
  rdfs:label "G p a usage"@en ;
  skos:definition """Specifies whether the Agreement on Government Procurement (GPA) applies.

Additional information: 
The GPA aims to establish a multilateral framework of balanced rights and obligations relating to public contracts with a view to achieving the liberalization and expansion of world trade.

WG Approval 15/10/2019

"""@en ;
  skos:prefLabel "G p a usage"@en ;
.
epo:hasGeneralEmploymentCommunicationMeans
  rdf:type owl:ObjectProperty ;
  rdfs:comment """The electronic means used to obtain the information concerning the general regulatory framework for environmental protection applicable in the place where the contract is to be performed.

WG Approval 21/03/2019 16:11:58"""@en ;
  rdfs:isDefinedBy <http://data.europa.eu/a4g/ontology> ;
  rdfs:label "Has general employment communication means"@en ;
  skos:definition """The electronic means used to obtain the information concerning the general regulatory framework for environmental protection applicable in the place where the contract is to be performed.

WG Approval 21/03/2019 16:11:58"""@en ;
  skos:prefLabel "Has general employment communication means"@en ;
.
epo:hasGeneralEnvironmentCommunicationMeans
  rdf:type owl:ObjectProperty ;
  rdfs:comment """The electronic means used to obtain the information concerning the general regulatory framework for employment protection and working conditions applicable in the place where the contract is to be performed.

WG Approval 21/03/2019 16:12:34"""@en ;
  rdfs:isDefinedBy <http://data.europa.eu/a4g/ontology> ;
  rdfs:label "Has general environment communication means"@en ;
  skos:definition """The electronic means used to obtain the information concerning the general regulatory framework for employment protection and working conditions applicable in the place where the contract is to be performed.

WG Approval 21/03/2019 16:12:34"""@en ;
  skos:prefLabel "Has general environment communication means"@en ;
.
epo:hasGeneralTaxCommunicationMeans
  rdf:type owl:ObjectProperty ;
  rdfs:comment """The electronic means used to obtain the information concerning the general regulatory framework for taxes applicable in the place where the contract is to be performed.

WG Approval 21/03/2019 16:11:30"""@en ;
  rdfs:isDefinedBy <http://data.europa.eu/a4g/ontology> ;
  rdfs:label "Has general tax communication means"@en ;
  skos:definition """The electronic means used to obtain the information concerning the general regulatory framework for taxes applicable in the place where the contract is to be performed.

WG Approval 21/03/2019 16:11:30"""@en ;
  skos:prefLabel "Has general tax communication means"@en ;
.
epo:hasGivenName
  rdf:type owl:DatatypeProperty ;
  rdfs:isDefinedBy <http://data.europa.eu/a4g/ontology> ;
  rdfs:label "Given name"@en ;
  skos:prefLabel "Given name"@en ;
.
epo:hasGroupLotEvaluationMethod
  rdf:type owl:DatatypeProperty ;
  rdfs:comment """Description of how lots and groups of lots are evaluated against one another in the procedure.



"""@en ;
  rdfs:isDefinedBy <http://data.europa.eu/a4g/ontology> ;
  rdfs:label "Group lot evaluation method"@en ;
  skos:definition """Description of how lots and groups of lots are evaluated against one another in the procedure.



"""@en ;
  skos:prefLabel "Group lot evaluation method"@en ;
.
epo:hasHighestReceivedTenderLotValue
  rdf:type owl:ObjectProperty ;
  rdfs:comment """Amount of the Tender with the highest value.

Additional Information
The value must correspond to an admissible tender. For example, tenders compliant with the procurement document requirements, not having an abnormally low price or cost, etc. 


WG Approval 12/12/2019

"""@en ;
  rdfs:isDefinedBy <http://data.europa.eu/a4g/ontology> ;
  rdfs:label "Highest received tender lot value"@en ;
  skos:definition """Amount of the Tender with the highest value.

Additional Information
The value must correspond to an admissible tender. For example, tenders compliant with the procurement document requirements, not having an abnormally low price or cost, etc. 


WG Approval 12/12/2019

"""@en ;
  skos:prefLabel "Highest received tender lot value"@en ;
.
epo:hasID
  rdf:type rdf:Property ;
  rdf:type owl:ObjectProperty ;
  rdfs:comment "<foreign otherprops=\"#ff0000\">A unique identification for the Procedure.</foreign>"@en ;
  rdfs:comment "A character string to identify and distinguish uniquely, one instance of an object in an identification scheme from all other objects in the same scheme together with relevant supplementary information."@en ;
  rdfs:comment """A unique identifier of the instance of the concept.

Additional Information

For example, in the case of the Procurement Identifier, this could be the European Public Procurement Identifier, and/or any other identifier provided by the buyer, the service provider or any other stakeholder.

WG Approval 12/11/2019
<foreign otherprops=\"#ff0000\">
</foreign><foreign otherprops=\"#ff0000\">
</foreign>"""@en ;
  rdfs:comment "Identifies the criterion unambiguously and uniquely across all  procurement procedures.."@en ;
  rdfs:isDefinedBy <http://data.europa.eu/a4g/ontology> ;
  rdfs:label "Has i d"@en ;
  rdfs:label "I d"@en ;
  skos:definition "<foreign otherprops=\"#ff0000\">A unique identification for the Procedure.</foreign>"@en ;
  skos:definition "A character string to identify and distinguish uniquely, one instance of an object in an identification scheme from all other objects in the same scheme together with relevant supplementary information."@en ;
  skos:definition """A unique identifier of the instance of the concept.

Additional Information

For example, in the case of the Procurement Identifier, this could be the European Public Procurement Identifier, and/or any other identifier provided by the buyer, the service provider or any other stakeholder.

WG Approval 12/11/2019
<foreign otherprops=\"#ff0000\">
</foreign><foreign otherprops=\"#ff0000\">
</foreign>"""@en ;
  skos:definition "Identifies the criterion unambiguously and uniquely across all  procurement procedures.."@en ;
  skos:prefLabel "Has i d"@en ;
  skos:prefLabel "I d"@en ;
.
epo:hasInadmissibleTendersLot
  rdf:type owl:DatatypeProperty ;
  rdfs:comment """Tenders received that cannot be awarded  due to non-compliance to procurement document requirements or having an abnormally low price or cost.

<u>Additional Information: </u>
Non-compliance with a Procurement Document requirements include exclusion grounds, selection criteria and submission deadline, etc.

WG Approval 12/12/2019"""@en ;
  rdfs:isDefinedBy <http://data.europa.eu/a4g/ontology> ;
  rdfs:label "Inadmissible tenders lot"@en ;
  skos:definition """Tenders received that cannot be awarded  due to non-compliance to procurement document requirements or having an abnormally low price or cost.

<u>Additional Information: </u>
Non-compliance with a Procurement Document requirements include exclusion grounds, selection criteria and submission deadline, etc.

WG Approval 12/12/2019"""@en ;
  skos:prefLabel "Inadmissible tenders lot"@en ;
.
epo:hasInhouseMail
  rdf:type owl:DatatypeProperty ;
  rdfs:isDefinedBy <http://data.europa.eu/a4g/ontology> ;
  rdfs:label "Inhouse mail"@en ;
  skos:prefLabel "Inhouse mail"@en ;
.
epo:hasInternetAddress
  rdf:type rdf:Property ;
  rdfs:comment """The website of the organisation.
"""@en ;
  rdfs:isDefinedBy <http://data.europa.eu/a4g/ontology> ;
  rdfs:label "Internet address"@en ;
  skos:definition """The website of the organisation.
"""@en ;
  skos:prefLabel "Internet address"@en ;
.
epo:hasInterval
  rdf:type owl:ObjectProperty ;
  rdfs:isDefinedBy <http://data.europa.eu/a4g/ontology> ;
  rdfs:label "Has interval"@en ;
  skos:prefLabel "Has interval"@en ;
.
epo:hasIsAbnormallyLow
  rdf:type rdf:Property ;
  rdfs:comment "A tender that is judged abnormally low based on technically, economically or legally unsound assumptions or practices."@en ;
  rdfs:isDefinedBy <http://data.europa.eu/a4g/ontology> ;
  rdfs:label "Is abnormally low"@en ;
  skos:definition "A tender that is judged abnormally low based on technically, economically or legally unsound assumptions or practices."@en ;
  skos:prefLabel "Is abnormally low"@en ;
.
epo:hasIsAbnormallyLowJustification
  rdf:type owl:DatatypeProperty ;
  rdfs:isDefinedBy <http://data.europa.eu/a4g/ontology> ;
  rdfs:label "Is abnormally low justification"@en ;
  skos:prefLabel "Is abnormally low justification"@en ;
.
epo:hasJuryDecisionBinding
  rdf:type rdf:Property ;
  rdfs:comment "Indicates whether the procuring entity is bound to apply the decision of the jury."@en ;
  rdfs:isDefinedBy <http://data.europa.eu/a4g/ontology> ;
  rdfs:label "Jury decision binding"@en ;
  skos:definition "Indicates whether the procuring entity is bound to apply the decision of the jury."@en ;
  skos:prefLabel "Jury decision binding"@en ;
.
epo:hasJustification
  rdf:type owl:DatatypeProperty ;
  rdfs:comment """An explanation about the reasons for using the concept. 




WG Approval 5/11/2019
"""@en ;
  rdfs:comment """An explanation about the reasons for using the concept. 

WG Approval 5/11/2019"""@en ;
  rdfs:isDefinedBy <http://data.europa.eu/a4g/ontology> ;
  rdfs:label "Justification"@en ;
  skos:definition """An explanation about the reasons for using the concept. 




WG Approval 5/11/2019
"""@en ;
  skos:definition """An explanation about the reasons for using the concept. 

WG Approval 5/11/2019"""@en ;
  skos:prefLabel "Justification"@en ;
.
epo:hasJustificationType
  rdf:type owl:ObjectProperty ;
  rdfs:isDefinedBy <http://data.europa.eu/a4g/ontology> ;
  rdfs:label "Has justification type"@en ;
  rdfs:label "Justification type"@en ;
  skos:prefLabel "Has justification type"@en ;
  skos:prefLabel "Justification type"@en ;
.
epo:hasLateTendererInformation
  rdf:type owl:ObjectProperty ;
  rdfs:comment """Whether tenderer-related information can be supplemented even after the submission deadline.

WG Approval 10/10/2019"""@en ;
  rdfs:isDefinedBy <http://data.europa.eu/a4g/ontology> ;
  rdfs:label "Has late tenderer information"@en ;
  rdfs:label "Late tenderer information"@en ;
  skos:definition """Whether tenderer-related information can be supplemented even after the submission deadline.

WG Approval 10/10/2019"""@en ;
  skos:prefLabel "Has late tenderer information"@en ;
  skos:prefLabel "Late tenderer information"@en ;
.
epo:hasLateTendererInformationDescription
  rdf:type owl:DatatypeProperty ;
  rdfs:isDefinedBy <http://data.europa.eu/a4g/ontology> ;
  rdfs:label "Late tenderer information description"@en ;
  skos:prefLabel "Late tenderer information description"@en ;
.
epo:hasLatitudeDegrees
  rdf:type owl:ObjectProperty ;
  rdfs:isDefinedBy <http://data.europa.eu/a4g/ontology> ;
  rdfs:label "Latitude degrees"@en ;
  skos:prefLabel "Latitude degrees"@en ;
.
epo:hasLatitudeDirection
  rdf:type owl:ObjectProperty ;
  rdfs:isDefinedBy <http://data.europa.eu/a4g/ontology> ;
  rdfs:label "Latitude direction"@en ;
  skos:prefLabel "Latitude direction"@en ;
.
epo:hasLatitudeMinutes
  rdf:type owl:ObjectProperty ;
  rdfs:isDefinedBy <http://data.europa.eu/a4g/ontology> ;
  rdfs:label "Latitude minutes"@en ;
  skos:prefLabel "Latitude minutes"@en ;
.
epo:hasLegalBasis
  rdf:type owl:ObjectProperty ;
  rdfs:isDefinedBy <http://data.europa.eu/a4g/ontology> ;
  rdfs:label "Legal basis"@en ;
  skos:prefLabel "Legal basis"@en ;
.
epo:hasLegalBasisID
  rdf:type rdf:Property ;
  rdf:type owl:ObjectProperty ;
  rdfs:isDefinedBy <http://data.europa.eu/a4g/ontology> ;
  rdfs:label "Has legal basis i d"@en ;
  rdfs:label "Legal basis i d"@en ;
  skos:prefLabel "Has legal basis i d"@en ;
  skos:prefLabel "Legal basis i d"@en ;
.
epo:hasLegalFormType
  rdf:type owl:ObjectProperty ;
  rdfs:comment """Identity that a organisation legally assumes taking into account its ownership and the responsibility that its owners have in legal terms.

Examples: Limited Liability Company; GBHM;  SLU; Cooperativa; Société Anonime; etc."""@en ;
  rdfs:isDefinedBy <http://data.europa.eu/a4g/ontology> ;
  rdfs:label "Has legal form type"@en ;
  rdfs:label "Legal form type"@en ;
  skos:definition """Identity that a organisation legally assumes taking into account its ownership and the responsibility that its owners have in legal terms.

Examples: Limited Liability Company; GBHM;  SLU; Cooperativa; Société Anonime; etc."""@en ;
  skos:prefLabel "Has legal form type"@en ;
  skos:prefLabel "Legal form type"@en ;
.
epo:hasLegalLocation
  rdf:type owl:ObjectProperty ;
  rdfs:isDefinedBy <http://data.europa.eu/a4g/ontology> ;
  rdfs:label "Has legal location"@en ;
  skos:prefLabel "Has legal location"@en ;
.
epo:hasLegalName
  rdf:type rdf:Property ;
  rdfs:isDefinedBy <http://data.europa.eu/a4g/ontology> ;
  rdfs:label "Legal name"@en ;
  skos:prefLabel "Legal name"@en ;
.
epo:hasLegalRegime
  rdf:type owl:ObjectProperty ;
  rdfs:isDefinedBy <http://data.europa.eu/a4g/ontology> ;
  rdfs:label "Legal regime"@en ;
  skos:prefLabel "Legal regime"@en ;
.
epo:hasLimitationDescription
  rdf:type owl:DatatypeProperty ;
  rdfs:comment """Self-explanatory text about a concept.
"""@en ;
  rdfs:isDefinedBy <http://data.europa.eu/a4g/ontology> ;
  rdfs:label "Limitation description"@en ;
  skos:definition """Self-explanatory text about a concept.
"""@en ;
  skos:prefLabel "Limitation description"@en ;
.
epo:hasListedCompany
  rdf:type rdf:Property ;
  rdfs:comment """Public companies listed on a stock exchange and subject to disclosure requirements (either by stock exchange
 rules or through law or enforceable means), which impose requirements to ensure adequate transparency of 
beneficial ownership. 

<u>Additional Information:</u>

In eForms this indicator is used when the nationality of beneficial owner is not provided because the Economic Operator is registered in a regulated market that is subject to disclosure requirements consistent with Union law or subject to equivalent international standards which ensure adequate transparency of ownership information. 

WG Approval 21/11/2019"""@en ;
  rdfs:isDefinedBy <http://data.europa.eu/a4g/ontology> ;
  rdfs:label "Listed company"@en ;
  skos:definition """Public companies listed on a stock exchange and subject to disclosure requirements (either by stock exchange
 rules or through law or enforceable means), which impose requirements to ensure adequate transparency of 
beneficial ownership. 

<u>Additional Information:</u>

In eForms this indicator is used when the nationality of beneficial owner is not provided because the Economic Operator is registered in a regulated market that is subject to disclosure requirements consistent with Union law or subject to equivalent international standards which ensure adequate transparency of ownership information. 

WG Approval 21/11/2019"""@en ;
  skos:prefLabel "Listed company"@en ;
.
epo:hasLocation
  rdf:type owl:ObjectProperty ;
  rdfs:isDefinedBy <http://data.europa.eu/a4g/ontology> ;
  rdfs:label "Has location"@en ;
  skos:prefLabel "Has location"@en ;
.
epo:hasLongitudeDegrees
  rdf:type owl:ObjectProperty ;
  rdfs:isDefinedBy <http://data.europa.eu/a4g/ontology> ;
  rdfs:label "Longitude degrees"@en ;
  skos:prefLabel "Longitude degrees"@en ;
.
epo:hasLongitudeDirection
  rdf:type owl:ObjectProperty ;
  rdfs:isDefinedBy <http://data.europa.eu/a4g/ontology> ;
  rdfs:label "Longitude direction"@en ;
  skos:prefLabel "Longitude direction"@en ;
.
epo:hasLongitudeMinutes
  rdf:type owl:ObjectProperty ;
  rdfs:isDefinedBy <http://data.europa.eu/a4g/ontology> ;
  rdfs:label "Longitude minutes"@en ;
  skos:prefLabel "Longitude minutes"@en ;
.
epo:hasLotAwardLimit
  rdf:type owl:DatatypeProperty ;
  rdfs:comment """The total number of lots for which contract(s) can be awarded to one tenderer.

(WG Approval 12/12/2018)"""@en ;
  rdfs:isDefinedBy <http://data.europa.eu/a4g/ontology> ;
  rdfs:label "Lot award limit"@en ;
  skos:definition """The total number of lots for which contract(s) can be awarded to one tenderer.

(WG Approval 12/12/2018)"""@en ;
  skos:prefLabel "Lot award limit"@en ;
.
epo:hasLotMinimumSubmission
  rdf:type owl:DatatypeProperty ;
  rdfs:comment """The minimum number of lots for which one tenderer must submit tenders. 

Additional Information

This can be used to state that a tenderer has to submit the maximum number of lots announced in the contract notice (i.e. in this case the Lot Minimum Submission would equal to the Lot Submission Limit).

"""@en ;
  rdfs:isDefinedBy <http://data.europa.eu/a4g/ontology> ;
  rdfs:label "Lot minimum submission"@en ;
  skos:definition """The minimum number of lots for which one tenderer must submit tenders. 

Additional Information

This can be used to state that a tenderer has to submit the maximum number of lots announced in the contract notice (i.e. in this case the Lot Minimum Submission would equal to the Lot Submission Limit).

"""@en ;
  skos:prefLabel "Lot minimum submission"@en ;
.
epo:hasLotSubmissionLimit
  rdf:type owl:DatatypeProperty ;
  rdfs:comment """The total number of lots for which one tenderer can submit tenders.

(WG approval 12/12/2018)

"""@en ;
  rdfs:isDefinedBy <http://data.europa.eu/a4g/ontology> ;
  rdfs:label "Lot submission limit"@en ;
  skos:definition """The total number of lots for which one tenderer can submit tenders.

(WG approval 12/12/2018)

"""@en ;
  skos:prefLabel "Lot submission limit"@en ;
.
epo:hasLowestReceivedTenderLotValue
  rdf:type owl:ObjectProperty ;
  rdfs:comment """Amount of the Tender with the lowest value.

Additional Information
The value must correspond to an admissible tender. For example, tenders compliant with the procurement document requirements, not having an abnormally low price or cost, etc. 

WG Approval 12/12/2019
"""@en ;
  rdfs:isDefinedBy <http://data.europa.eu/a4g/ontology> ;
  rdfs:label "Lowest received tender lot value"@en ;
  skos:definition """Amount of the Tender with the lowest value.

Additional Information
The value must correspond to an admissible tender. For example, tenders compliant with the procurement document requirements, not having an abnormally low price or cost, etc. 

WG Approval 12/12/2019
"""@en ;
  skos:prefLabel "Lowest received tender lot value"@en ;
.
epo:hasMainActivity
  rdf:type owl:ObjectProperty ;
  rdfs:isDefinedBy <http://data.europa.eu/a4g/ontology> ;
  rdfs:label "Has main activity"@en ;
  skos:prefLabel "Has main activity"@en ;
.
epo:hasMainActivityType
  rdf:type owl:ObjectProperty ;
  rdfs:isDefinedBy <http://data.europa.eu/a4g/ontology> ;
  rdfs:label "Has main activity type"@en ;
  rdfs:label "Main activity type"@en ;
  skos:prefLabel "Has main activity type"@en ;
  skos:prefLabel "Main activity type"@en ;
.
epo:hasMainClassification
  rdf:type owl:ObjectProperty ;
  rdfs:isDefinedBy <http://data.europa.eu/a4g/ontology> ;
  rdfs:label "Has main classification"@en ;
  rdfs:label "Main classification"@en ;
  skos:prefLabel "Has main classification"@en ;
  skos:prefLabel "Main classification"@en ;
.
epo:hasMainFeatures
  rdf:type owl:DatatypeProperty ;
  rdfs:comment """Main features of the procedure and information about where the full rules for the procedure can be found. 

Additional Information

This information should be given when the procedure is not one of those mentioned in the procurement directives. This can be the case for example for concessions, for social and other specific services, and in case of voluntary publication of procurement procedures below the EU procurement thresholds."""@en ;
  rdfs:isDefinedBy <http://data.europa.eu/a4g/ontology> ;
  rdfs:label "Main features"@en ;
  skos:definition """Main features of the procedure and information about where the full rules for the procedure can be found. 

Additional Information

This information should be given when the procedure is not one of those mentioned in the procurement directives. This can be the case for example for concessions, for social and other specific services, and in case of voluntary publication of procurement procedures below the EU procurement thresholds."""@en ;
  skos:prefLabel "Main features"@en ;
.
epo:hasMarkAttention
  rdf:type owl:DatatypeProperty ;
  rdfs:isDefinedBy <http://data.europa.eu/a4g/ontology> ;
  rdfs:label "Mark attention"@en ;
  skos:prefLabel "Mark attention"@en ;
.
epo:hasMarkCare
  rdf:type owl:DatatypeProperty ;
  rdfs:isDefinedBy <http://data.europa.eu/a4g/ontology> ;
  rdfs:label "Mark care"@en ;
  skos:prefLabel "Mark care"@en ;
.
epo:hasMaximumAmount
  rdf:type owl:ObjectProperty ;
  rdfs:comment """The highest amount which can be spent within a procurement over its whole duration.

WG Approval 11/10/2019"""@en ;
  rdfs:isDefinedBy <http://data.europa.eu/a4g/ontology> ;
  rdfs:label "Maximum amount"@en ;
  skos:definition """The highest amount which can be spent within a procurement over its whole duration.

WG Approval 11/10/2019"""@en ;
  skos:prefLabel "Maximum amount"@en ;
.
epo:hasMaximumCandidates
  rdf:type rdf:Property ;
  rdfs:isDefinedBy <http://data.europa.eu/a4g/ontology> ;
  rdfs:label "Maximum candidates"@en ;
  skos:prefLabel "Maximum candidates"@en ;
.
epo:hasMaximumNumberOfAwardedTenderers
  rdf:type owl:ObjectProperty ;
  rdfs:comment """Maximum number of tenderers who may be awarded a contract within the framework agreement.

Additional Information: the number is a positive integer.

WG Approval 2019-02-05
"""@en ;
  rdfs:isDefinedBy <http://data.europa.eu/a4g/ontology> ;
  rdfs:label "Maximum number of awarded tenderers"@en ;
  skos:definition """Maximum number of tenderers who may be awarded a contract within the framework agreement.

Additional Information: the number is a positive integer.

WG Approval 2019-02-05
"""@en ;
  skos:prefLabel "Maximum number of awarded tenderers"@en ;
.
epo:hasMaximumNumberOfCandidates
  rdf:type owl:DatatypeProperty ;
  rdfs:comment """Maximum number of candidates to be invited for the second stage of the procedure.

WG Approval 22/08/2019"""@en ;
  rdfs:isDefinedBy <http://data.europa.eu/a4g/ontology> ;
  rdfs:label "Maximum number of candidates"@en ;
  skos:definition """Maximum number of candidates to be invited for the second stage of the procedure.

WG Approval 22/08/2019"""@en ;
  skos:prefLabel "Maximum number of candidates"@en ;
.
epo:hasMaximumNumberOfLotsToBeAwarded
  rdf:type owl:DatatypeProperty ;
  rdfs:comment """The maximum number of lots for which contract(s) can be awarded to one tenderer.

WG Approval 22/08/2019"""@en ;
  rdfs:isDefinedBy <http://data.europa.eu/a4g/ontology> ;
  rdfs:label "Maximum number of lots to be awarded"@en ;
  skos:definition """The maximum number of lots for which contract(s) can be awarded to one tenderer.

WG Approval 22/08/2019"""@en ;
  skos:prefLabel "Maximum number of lots to be awarded"@en ;
.
epo:hasMaximumNumberOfRenewals
  rdf:type owl:DatatypeProperty ;
  rdfs:comment """The maximum number of times the contract can be renewed. 

Additional Information

By renewing, the buyer reserves the right (i.e. not an obligation) to renew the contract (i.e. extend its duration) without a new procurement procedure. 
For example, a contract may be valid for one year and the buyer may keep a possibility to renew it (e.g. once, twice) for another three months, if he is content with the services he received.

PLEASE REVIEW THIS DEFINITION AGAIN WITH THE WORKING GROUP. It was originally taken from eForms.
"""@en ;
  rdfs:isDefinedBy <http://data.europa.eu/a4g/ontology> ;
  rdfs:label "Maximum number of renewals"@en ;
  skos:definition """The maximum number of times the contract can be renewed. 

Additional Information

By renewing, the buyer reserves the right (i.e. not an obligation) to renew the contract (i.e. extend its duration) without a new procurement procedure. 
For example, a contract may be valid for one year and the buyer may keep a possibility to renew it (e.g. once, twice) for another three months, if he is content with the services he received.

PLEASE REVIEW THIS DEFINITION AGAIN WITH THE WORKING GROUP. It was originally taken from eForms.
"""@en ;
  skos:prefLabel "Maximum number of renewals"@en ;
.
epo:hasMaximumShare
  rdf:type rdf:Property ;
  rdfs:comment """The maximum proportion of something to be distributed.

Additional Information:
In the case of subcontracting the share may refer to the proportion of works, services or supplies being subcontracted.

WG Approval 17/09/2019 

"""@en ;
  rdfs:isDefinedBy <http://data.europa.eu/a4g/ontology> ;
  rdfs:label "Maximum share"@en ;
  skos:definition """The maximum proportion of something to be distributed.

Additional Information:
In the case of subcontracting the share may refer to the proportion of works, services or supplies being subcontracted.

WG Approval 17/09/2019 

"""@en ;
  skos:prefLabel "Maximum share"@en ;
.
epo:hasMeansOfCommunication
  rdf:type owl:ObjectProperty ;
  rdfs:isDefinedBy <http://data.europa.eu/a4g/ontology> ;
  rdfs:label "Has means of communication"@en ;
  skos:prefLabel "Has means of communication"@en ;
.
epo:hasMediumTendersPerLot
  rdf:type owl:DatatypeProperty ;
  rdfs:comment """Tenders from medium-sized enterprise.

<u>Additional Information:</u>

See Commission Recommendation 2003/361/EC.
"""@en ;
  rdfs:isDefinedBy <http://data.europa.eu/a4g/ontology> ;
  rdfs:label "Medium tenders per lot"@en ;
  skos:definition """Tenders from medium-sized enterprise.

<u>Additional Information:</u>

See Commission Recommendation 2003/361/EC.
"""@en ;
  skos:prefLabel "Medium tenders per lot"@en ;
.
epo:hasMinimumAmount
  rdf:type owl:ObjectProperty ;
  rdfs:isDefinedBy <http://data.europa.eu/a4g/ontology> ;
  rdfs:label "Minimum amount"@en ;
  skos:prefLabel "Minimum amount"@en ;
.
epo:hasMinimumNumberOfCandidates
  rdf:type owl:DatatypeProperty ;
  rdfs:comment """Minimum number of candidates to be invited for the second stage of the procedure.

WG Approval 22/08/2019 """@en ;
  rdfs:isDefinedBy <http://data.europa.eu/a4g/ontology> ;
  rdfs:label "Minimum number of candidates"@en ;
  skos:definition """Minimum number of candidates to be invited for the second stage of the procedure.

WG Approval 22/08/2019 """@en ;
  skos:prefLabel "Minimum number of candidates"@en ;
.
epo:hasMinimumShare
  rdf:type rdf:Property ;
  rdfs:comment """The minimum proportion of something to be distributed.

Additional Information:
In the case of subcontracting the share may refer to the proportion of works, services or supplies being subcontracted.

WG Approval 17/09/2019"""@en ;
  rdfs:isDefinedBy <http://data.europa.eu/a4g/ontology> ;
  rdfs:label "Minimum share"@en ;
  skos:definition """The minimum proportion of something to be distributed.

Additional Information:
In the case of subcontracting the share may refer to the proportion of works, services or supplies being subcontracted.

WG Approval 17/09/2019"""@en ;
  skos:prefLabel "Minimum share"@en ;
.
epo:hasMinimumShareSubjectMatter
  rdf:type owl:DatatypeProperty ;
  rdfs:isDefinedBy <http://data.europa.eu/a4g/ontology> ;
  rdfs:label "Minimum share subject matter"@en ;
  skos:prefLabel "Minimum share subject matter"@en ;
.
epo:hasMinimumSubcontractorsProposedObligation
  rdf:type rdf:Property ;
  rdfs:isDefinedBy <http://data.europa.eu/a4g/ontology> ;
  rdfs:label "Minimum subcontractors proposed obligation"@en ;
  skos:prefLabel "Minimum subcontractors proposed obligation"@en ;
.
epo:hasModificationReason
  rdf:type owl:ObjectProperty ;
  rdfs:isDefinedBy <http://data.europa.eu/a4g/ontology> ;
  rdfs:label "Modification reason"@en ;
  skos:prefLabel "Modification reason"@en ;
.
epo:hasMultipleTenders
  rdf:type rdf:Property ;
  rdfs:comment """Tenderers may submit more than one competing tenders.

WG Approval 10/10/2019


"""@en ;
  rdfs:isDefinedBy <http://data.europa.eu/a4g/ontology> ;
  rdfs:label "Multiple tenders"@en ;
  skos:definition """Tenderers may submit more than one competing tenders.

WG Approval 10/10/2019


"""@en ;
  skos:prefLabel "Multiple tenders"@en ;
.
epo:hasName
  rdf:type owl:DatatypeProperty ;
  rdfs:comment """A short text representing an instance of the class.

WG Approval 17/09/2019

"""@en ;
  rdfs:isDefinedBy <http://data.europa.eu/a4g/ontology> ;
  rdfs:label "Name"@en ;
  skos:definition """A short text representing an instance of the class.

WG Approval 17/09/2019

"""@en ;
  skos:prefLabel "Name"@en ;
.
epo:hasNationality
  rdf:type owl:ObjectProperty ;
  rdfs:isDefinedBy <http://data.europa.eu/a4g/ontology> ;
  rdfs:label "Has nationality"@en ;
  rdfs:label "Nationality"@en ;
  skos:prefLabel "Has nationality"@en ;
  skos:prefLabel "Nationality"@en ;
.
epo:hasNoNegotiationNecessary
  rdf:type rdf:Property ;
  rdfs:comment """The buyer reserves the right to award the contract on the basis of the initial tenders without any further negotiations.

Additional information:
See Article 29(4) of Directive 2014/24/EU. 
"""@en ;
  rdfs:isDefinedBy <http://data.europa.eu/a4g/ontology> ;
  rdfs:label "No negotiation necessary"@en ;
  skos:definition """The buyer reserves the right to award the contract on the basis of the initial tenders without any further negotiations.

Additional information:
See Article 29(4) of Directive 2014/24/EU. 
"""@en ;
  skos:prefLabel "No negotiation necessary"@en ;
.
epo:hasNoResultReason
  rdf:type owl:DatatypeProperty ;
  rdfs:comment "Justification why the contract has and will not have a winner."@en ;
  rdfs:isDefinedBy <http://data.europa.eu/a4g/ontology> ;
  rdfs:label "No result reason"@en ;
  skos:definition "Justification why the contract has and will not have a winner."@en ;
  skos:prefLabel "No result reason"@en ;
.
epo:hasNonAccessibilityCriteriaJustification
  rdf:type owl:DatatypeProperty ;
  rdfs:comment """Reason for not applying accessibility criteria.

WG Approval 05/03/2019"""@en ;
  rdfs:isDefinedBy <http://data.europa.eu/a4g/ontology> ;
  rdfs:label "Non accessibility criteria justification"@en ;
  skos:definition """Reason for not applying accessibility criteria.

WG Approval 05/03/2019"""@en ;
  skos:prefLabel "Non accessibility criteria justification"@en ;
.
epo:hasNonAwardJustification
  rdf:type owl:ObjectProperty ;
  rdfs:isDefinedBy <http://data.europa.eu/a4g/ontology> ;
  rdfs:label "Has non award justification"@en ;
  rdfs:label "Non award justification"@en ;
  skos:prefLabel "Has non award justification"@en ;
  skos:prefLabel "Non award justification"@en ;
.
epo:hasNonElectronicSubmissionDescription
  rdf:type owl:DatatypeProperty ;
  rdfs:comment """Textual explanation of how non-electronic tenders are to be presented.

WG Approval 03/10/2019 

"""@en ;
  rdfs:isDefinedBy <http://data.europa.eu/a4g/ontology> ;
  rdfs:label "Non electronic submission description"@en ;
  skos:definition """Textual explanation of how non-electronic tenders are to be presented.

WG Approval 03/10/2019 

"""@en ;
  skos:prefLabel "Non electronic submission description"@en ;
.
epo:hasNonElectronicSubmissionJustification
  rdf:type owl:ObjectProperty ;
  rdfs:comment "Basis for physical submission of tenders."@en ;
  rdfs:comment """Reason for not accepting electronic tenders.

WG Approval 03/10/2019 
"""@en ;
  rdfs:isDefinedBy <http://data.europa.eu/a4g/ontology> ;
  rdfs:label "Has non electronic submission justification"@en ;
  rdfs:label "Non electronic submission justification"@en ;
  skos:definition "Basis for physical submission of tenders."@en ;
  skos:definition """Reason for not accepting electronic tenders.

WG Approval 03/10/2019 
"""@en ;
  skos:prefLabel "Has non electronic submission justification"@en ;
  skos:prefLabel "Non electronic submission justification"@en ;
.
epo:hasNonPublicationJustification
  rdf:type owl:ObjectProperty ;
  rdfs:isDefinedBy <http://data.europa.eu/a4g/ontology> ;
  rdfs:label "Has non publication justification"@en ;
  rdfs:label "Non publication justification"@en ;
  skos:prefLabel "Has non publication justification"@en ;
  skos:prefLabel "Non publication justification"@en ;
.
epo:hasNonPublicationJustificationDescription
  rdf:type owl:DatatypeProperty ;
  rdfs:isDefinedBy <http://data.europa.eu/a4g/ontology> ;
  rdfs:label "Non publication justification description"@en ;
  skos:prefLabel "Non publication justification description"@en ;
.
epo:hasNonPublishedElement
  rdf:type owl:ObjectProperty ;
  rdfs:comment "For example, elements in the Contract Award Notice that are published at a later date."@en ;
  rdfs:isDefinedBy <http://data.europa.eu/a4g/ontology> ;
  rdfs:label "Has non published element"@en ;
  skos:definition "For example, elements in the Contract Award Notice that are published at a later date."@en ;
  skos:prefLabel "Has non published element"@en ;
.
epo:hasNotificationPhasesType
  rdf:type owl:ObjectProperty ;
  rdfs:isDefinedBy <http://data.europa.eu/a4g/ontology> ;
  rdfs:label "Has notification phases type"@en ;
  rdfs:label "Notification phases type"@en ;
  skos:prefLabel "Has notification phases type"@en ;
  skos:prefLabel "Notification phases type"@en ;
.
epo:hasNumberAwardedContract
  rdf:type owl:DatatypeProperty ;
  rdfs:isDefinedBy <http://data.europa.eu/a4g/ontology> ;
  rdfs:label "Number awarded contract"@en ;
  skos:prefLabel "Number awarded contract"@en ;
.
epo:hasOfficialLanguage
  rdf:type owl:ObjectProperty ;
  rdfs:comment """The language(s) in which the instances of the given concepts are officially available. These linguistic versions are equally legally valid.

WG Approval 03/10/2019"""@en ;
  rdfs:isDefinedBy <http://data.europa.eu/a4g/ontology> ;
  rdfs:label "Has official language"@en ;
  rdfs:label "Official language"@en ;
  skos:definition """The language(s) in which the instances of the given concepts are officially available. These linguistic versions are equally legally valid.

WG Approval 03/10/2019"""@en ;
  skos:prefLabel "Has official language"@en ;
  skos:prefLabel "Official language"@en ;
.
epo:hasOpeningDateTime
  rdf:type rdf:Property ;
  rdfs:comment """Date and time for the opening of tenders.

WG Approval 12/03/2019

"""@en ;
  rdfs:isDefinedBy <http://data.europa.eu/a4g/ontology> ;
  rdfs:label "Opening date time"@en ;
  skos:definition """Date and time for the opening of tenders.

WG Approval 12/03/2019

"""@en ;
  skos:prefLabel "Opening date time"@en ;
.
epo:hasOpeningDescription
  rdf:type owl:DatatypeProperty ;
  rdfs:comment """Further information about the opening of tenders. 

Additional Information
For example, who may participate in the opening and whether any authorization is needed.

WG Approval 12/03/2019"""@en ;
  rdfs:isDefinedBy <http://data.europa.eu/a4g/ontology> ;
  rdfs:label "Opening description"@en ;
  skos:definition """Further information about the opening of tenders. 

Additional Information
For example, who may participate in the opening and whether any authorization is needed.

WG Approval 12/03/2019"""@en ;
  skos:prefLabel "Opening description"@en ;
.
epo:hasOpeningPlace
  rdf:type owl:ObjectProperty ;
  rdfs:comment """he place where the tenders will be publicly opened.

WG Approval 10-10-2019"""@en ;
  rdfs:isDefinedBy <http://data.europa.eu/a4g/ontology> ;
  rdfs:label "Has opening place"@en ;
  skos:definition """he place where the tenders will be publicly opened.

WG Approval 10-10-2019"""@en ;
  skos:prefLabel "Has opening place"@en ;
.
epo:hasOptionPermissions
  rdf:type owl:ObjectProperty ;
  rdfs:comment """
"""@en ;
  rdfs:isDefinedBy <http://data.europa.eu/a4g/ontology> ;
  rdfs:label "Has option permissions"@en ;
  skos:definition """
"""@en ;
  skos:prefLabel "Has option permissions"@en ;
.
epo:hasOptions
  rdf:type owl:ObjectProperty ;
  rdfs:comment """The buyer reserves the right (not an obligation) for additional purchases from the contractor (while the contract is valid).

WG Approval 09/04/2019 14:45:05


The old definition we had in ePO reads as follows (and never was approved by the WG:

\"Statement by the Procuring Entity about whether it may apply modifications to the procurement procedure that would alter the overall nature of the contract or the framework agreement.\"
"""@en ;
  rdfs:isDefinedBy <http://data.europa.eu/a4g/ontology> ;
  rdfs:label "Has options"@en ;
  rdfs:label "Options"@en ;
  skos:definition """The buyer reserves the right (not an obligation) for additional purchases from the contractor (while the contract is valid).

WG Approval 09/04/2019 14:45:05


The old definition we had in ePO reads as follows (and never was approved by the WG:

\"Statement by the Procuring Entity about whether it may apply modifications to the procurement procedure that would alter the overall nature of the contract or the framework agreement.\"
"""@en ;
  skos:prefLabel "Has options"@en ;
  skos:prefLabel "Options"@en ;
.
epo:hasOptionsDescription
  rdf:type owl:DatatypeProperty ;
  rdfs:comment """The motivation and details about additional purchases that the buyer may undertake while the contract is valid.

WG Approval 09/04/2019 """@en ;
  rdfs:isDefinedBy <http://data.europa.eu/a4g/ontology> ;
  rdfs:label "Options description"@en ;
  skos:definition """The motivation and details about additional purchases that the buyer may undertake while the contract is valid.

WG Approval 09/04/2019 """@en ;
  skos:prefLabel "Options description"@en ;
.
epo:hasOptionsPermisisions
  rdf:type owl:ObjectProperty ;
  rdfs:isDefinedBy <http://data.europa.eu/a4g/ontology> ;
  rdfs:label "Options permisisions"@en ;
  skos:prefLabel "Options permisisions"@en ;
.
epo:hasOtherCharges
  rdf:type owl:ObjectProperty ;
  rdfs:isDefinedBy <http://data.europa.eu/a4g/ontology> ;
  rdfs:label "Other charges"@en ;
  skos:prefLabel "Other charges"@en ;
.
epo:hasOverallAmount
  rdf:type owl:ObjectProperty ;
  rdfs:comment """In the case of a procurement procedure it includes options and renewals.
"""@en ;
  rdfs:isDefinedBy <http://data.europa.eu/a4g/ontology> ;
  rdfs:label "Overall amount"@en ;
  skos:definition """In the case of a procurement procedure it includes options and renewals.
"""@en ;
  skos:prefLabel "Overall amount"@en ;
.
epo:hasOverallCostAwardCriteriaPonderation
  rdf:type owl:DatatypeProperty ;
  rdfs:isDefinedBy <http://data.europa.eu/a4g/ontology> ;
  rdfs:label "Overall cost award criteria ponderation"@en ;
  skos:prefLabel "Overall cost award criteria ponderation"@en ;
.
epo:hasOverallMaximumValue
  rdf:type owl:ObjectProperty ;
  rdfs:comment """Establishes the maximum value for the Framework Agreement, either for the lots specified in the Framework Agreement Lots or for all the lots of the procedure.

"""@en ;
  rdfs:isDefinedBy <http://data.europa.eu/a4g/ontology> ;
  rdfs:label "Has overall maximum value"@en ;
  skos:definition """Establishes the maximum value for the Framework Agreement, either for the lots specified in the Framework Agreement Lots or for all the lots of the procedure.

"""@en ;
  skos:prefLabel "Has overall maximum value"@en ;
.
epo:hasOverallPriceAwardCriteriaPonderation
  rdf:type owl:DatatypeProperty ;
  rdfs:isDefinedBy <http://data.europa.eu/a4g/ontology> ;
  rdfs:label "Overall price award criteria ponderation"@en ;
  skos:prefLabel "Overall price award criteria ponderation"@en ;
.
epo:hasOverallPurpose
  rdf:type owl:ObjectProperty ;
  rdfs:isDefinedBy <http://data.europa.eu/a4g/ontology> ;
  rdfs:label "Has overall purpose"@en ;
  skos:prefLabel "Has overall purpose"@en ;
.
epo:hasOverallQualityAwardCriteriaPonderation
  rdf:type owl:DatatypeProperty ;
  rdfs:isDefinedBy <http://data.europa.eu/a4g/ontology> ;
  rdfs:label "Overall quality award criteria ponderation"@en ;
  skos:prefLabel "Overall quality award criteria ponderation"@en ;
.
epo:hasParticipationEvaluationPeriod
  rdf:type owl:ObjectProperty ;
  rdfs:comment """Deadline for CA to finalise the assessment of request to participate in a DPS.

Pending of approval

See Art. 34.5. first subparagraph

"""@en ;
  rdfs:isDefinedBy <http://data.europa.eu/a4g/ontology> ;
  rdfs:label "Has participation evaluation period"@en ;
  skos:definition """Deadline for CA to finalise the assessment of request to participate in a DPS.

Pending of approval

See Art. 34.5. first subparagraph

"""@en ;
  skos:prefLabel "Has participation evaluation period"@en ;
.
epo:hasParticipationPayment
  rdf:type rdf:Property ;
  rdfs:isDefinedBy <http://data.europa.eu/a4g/ontology> ;
  rdfs:label "Participation payment"@en ;
  skos:prefLabel "Participation payment"@en ;
.
epo:hasPatronimicName
  rdf:type owl:DatatypeProperty ;
  rdfs:isDefinedBy <http://data.europa.eu/a4g/ontology> ;
  rdfs:label "Patronimic name"@en ;
  skos:prefLabel "Patronimic name"@en ;
.
epo:hasPaymentArrangements
  rdf:type owl:DatatypeProperty ;
  rdfs:comment """Information about financial clauses that will govern some economic aspects of the execution of the contract.

Additional Information: These clauses usually refer to financial and payment provisions.

This type of information should be structured instead of a free text in order to reuse it an ideal world. Unfortunately this is an information that in the real life no one is willing to provide pro-actively.

WG Pending of discussion with eForms"""@en ;
  rdfs:isDefinedBy <http://data.europa.eu/a4g/ontology> ;
  rdfs:label "Payment arrangements"@en ;
  skos:definition """Information about financial clauses that will govern some economic aspects of the execution of the contract.

Additional Information: These clauses usually refer to financial and payment provisions.

This type of information should be structured instead of a free text in order to reuse it an ideal world. Unfortunately this is an information that in the real life no one is willing to provide pro-actively.

WG Pending of discussion with eForms"""@en ;
  skos:prefLabel "Payment arrangements"@en ;
.
epo:hasPaymentNote
  rdf:type owl:DatatypeProperty ;
  rdfs:isDefinedBy <http://data.europa.eu/a4g/ontology> ;
  rdfs:label "Payment note"@en ;
  skos:prefLabel "Payment note"@en ;
.
epo:hasPercentageEvaluated
  rdf:type owl:ObjectProperty ;
  rdfs:isDefinedBy <http://data.europa.eu/a4g/ontology> ;
  rdfs:label "Percentage evaluated"@en ;
  skos:prefLabel "Percentage evaluated"@en ;
.
epo:hasPercentageOfEvaluation
  rdf:type owl:ObjectProperty ;
  rdfs:isDefinedBy <http://data.europa.eu/a4g/ontology> ;
  rdfs:label "Percentage of evaluation"@en ;
  skos:prefLabel "Percentage of evaluation"@en ;
.
epo:hasPerformanceConditions
  rdf:type owl:DatatypeProperty ;
  rdfs:comment """The particular conditions and additional information related to the execution of the contract.

Additional Information: 

For example, specific information about the place of performance, intermediary deliverables, compensation for damages, intellectual property rights.

WG approval 15-01-2019"""@en ;
  rdfs:isDefinedBy <http://data.europa.eu/a4g/ontology> ;
  rdfs:label "Performance conditions"@en ;
  skos:definition """The particular conditions and additional information related to the execution of the contract.

Additional Information: 

For example, specific information about the place of performance, intermediary deliverables, compensation for damages, intellectual property rights.

WG approval 15-01-2019"""@en ;
  skos:prefLabel "Performance conditions"@en ;
.
epo:hasPerformingStafQualificationInformation
  rdf:type owl:ObjectProperty ;
  rdfs:isDefinedBy <http://data.europa.eu/a4g/ontology> ;
  rdfs:label "Performing staf qualification information"@en ;
  skos:prefLabel "Performing staf qualification information"@en ;
.
epo:hasPlaceOfPerformanceAdditionalInformation
  rdf:type owl:DatatypeProperty ;
  rdfs:comment """Further details on the location of the execution of the contract.

WG Approval 30/07/2019"""@en ;
  rdfs:isDefinedBy <http://data.europa.eu/a4g/ontology> ;
  rdfs:label "Place of performance additional information"@en ;
  skos:definition """Further details on the location of the execution of the contract.

WG Approval 30/07/2019"""@en ;
  skos:prefLabel "Place of performance additional information"@en ;
.
epo:hasPlannedPeriod
  rdf:type owl:ObjectProperty ;
  rdfs:isDefinedBy <http://data.europa.eu/a4g/ontology> ;
  rdfs:label "Has planned period"@en ;
  skos:prefLabel "Has planned period"@en ;
.
epo:hasPlotIdentification
  rdf:type owl:DatatypeProperty ;
  rdfs:isDefinedBy <http://data.europa.eu/a4g/ontology> ;
  rdfs:label "Plot identification"@en ;
  skos:prefLabel "Plot identification"@en ;
.
epo:hasPostalAddress
  rdf:type owl:ObjectProperty ;
  rdfs:isDefinedBy <http://data.europa.eu/a4g/ontology> ;
  rdfs:label "Has postal address"@en ;
  skos:prefLabel "Has postal address"@en ;
.
epo:hasPostalZone
  rdf:type owl:DatatypeProperty ;
  rdfs:isDefinedBy <http://data.europa.eu/a4g/ontology> ;
  rdfs:label "Postal zone"@en ;
  skos:prefLabel "Postal zone"@en ;
.
epo:hasPostbox
  rdf:type owl:DatatypeProperty ;
  rdfs:isDefinedBy <http://data.europa.eu/a4g/ontology> ;
  rdfs:label "Postbox"@en ;
  skos:prefLabel "Postbox"@en ;
.
epo:hasPreferredPublicationDate
  rdf:type owl:DatatypeProperty ;
  rdfs:isDefinedBy <http://data.europa.eu/a4g/ontology> ;
  rdfs:label "Preferred publication date"@en ;
  skos:prefLabel "Preferred publication date"@en ;
.
epo:hasPreviousPublication
  rdf:type owl:ObjectProperty ;
  rdfs:isDefinedBy <http://data.europa.eu/a4g/ontology> ;
  rdfs:label "Has previous publication"@en ;
  skos:prefLabel "Has previous publication"@en ;
.
epo:hasPrizeRank
  rdf:type owl:DatatypeProperty ;
  rdfs:comment """The position of the prize (e.g. first place, second place) in a design contest list of prizes.

WG Approval 29/08/2019 
"""@en ;
  rdfs:isDefinedBy <http://data.europa.eu/a4g/ontology> ;
  rdfs:label "Prize rank"@en ;
  skos:definition """The position of the prize (e.g. first place, second place) in a design contest list of prizes.

WG Approval 29/08/2019 
"""@en ;
  skos:prefLabel "Prize rank"@en ;
.
epo:hasPrizeValue
  rdf:type owl:ObjectProperty ;
  rdfs:comment """The monetary value of a prize, if any, for the winner (or runners-up) of the design contest.

WG Approval 29/08/2019"""@en ;
  rdfs:isDefinedBy <http://data.europa.eu/a4g/ontology> ;
  rdfs:label "Prize value"@en ;
  skos:definition """The monetary value of a prize, if any, for the winner (or runners-up) of the design contest.

WG Approval 29/08/2019"""@en ;
  skos:prefLabel "Prize value"@en ;
.
epo:hasProcedureType
  rdf:type owl:ObjectProperty ;
  rdfs:isDefinedBy <http://data.europa.eu/a4g/ontology> ;
  rdfs:label "Has procedure type"@en ;
  rdfs:label "Procedure type"@en ;
  skos:prefLabel "Has procedure type"@en ;
  skos:prefLabel "Procedure type"@en ;
.
epo:hasProcurementCriterionApplicability
  rdf:type owl:ObjectProperty ;
  rdfs:isDefinedBy <http://data.europa.eu/a4g/ontology> ;
  rdfs:label "Has procurement criterion applicability"@en ;
  skos:prefLabel "Has procurement criterion applicability"@en ;
.
epo:hasProcurementDocumentsChanged
  rdf:type rdf:Property ;
  rdfs:comment """One or more procurement documents have been changed.

WG Approval 05/11/2019"""@en ;
  rdfs:isDefinedBy <http://data.europa.eu/a4g/ontology> ;
  rdfs:label "Procurement documents changed"@en ;
  skos:definition """One or more procurement documents have been changed.

WG Approval 05/11/2019"""@en ;
  skos:prefLabel "Procurement documents changed"@en ;
.
epo:hasProcurementDocumentsMadeAvailableVia
  rdf:type owl:ObjectProperty ;
  rdfs:isDefinedBy <http://data.europa.eu/a4g/ontology> ;
  rdfs:label "Has procurement documents made available via"@en ;
  skos:prefLabel "Has procurement documents made available via"@en ;
.
epo:hasProcurementRegime
  rdf:type owl:ObjectProperty ;
  rdfs:isDefinedBy <http://data.europa.eu/a4g/ontology> ;
  rdfs:label "Has procurement regime"@en ;
  skos:prefLabel "Has procurement regime"@en ;
.
epo:hasProcurementValue
  rdf:type owl:ObjectProperty ;
  rdfs:comment "At contract time, this procurement value may be different from the Procurement Value of a Lot or a Procedure that was announced."@en ;
  rdfs:isDefinedBy <http://data.europa.eu/a4g/ontology> ;
  rdfs:label "Has procurement value"@en ;
  skos:definition "At contract time, this procurement value may be different from the Procurement Value of a Lot or a Procedure that was announced."@en ;
  skos:prefLabel "Has procurement value"@en ;
.
epo:hasPublicationDate
  rdf:type owl:DatatypeProperty ;
  rdfs:comment """The date when a record is made publicly available.

(WG approval 01/06/2018)"""@en ;
  rdfs:isDefinedBy <http://data.europa.eu/a4g/ontology> ;
  rdfs:label "Publication date"@en ;
  skos:definition """The date when a record is made publicly available.

(WG approval 01/06/2018)"""@en ;
  skos:prefLabel "Publication date"@en ;
.
epo:hasPurpose
  rdf:type owl:ObjectProperty ;
  rdfs:isDefinedBy <http://data.europa.eu/a4g/ontology> ;
  rdfs:label "Has purpose"@en ;
  skos:prefLabel "Has purpose"@en ;
.
epo:hasQualified
  rdf:type owl:ObjectProperty ;
  rdfs:isDefinedBy <http://data.europa.eu/a4g/ontology> ;
  rdfs:label "Has qualified"@en ;
  skos:prefLabel "Has qualified"@en ;
.
epo:hasQuestionsMadeAvailableVia
  rdf:type owl:ObjectProperty ;
  rdfs:isDefinedBy <http://data.europa.eu/a4g/ontology> ;
  rdfs:label "Has questions made available via"@en ;
  skos:prefLabel "Has questions made available via"@en ;
.
epo:hasRankingInFirstStage
  rdf:type owl:DatatypeProperty ;
  rdfs:isDefinedBy <http://data.europa.eu/a4g/ontology> ;
  rdfs:label "Ranking in first stage"@en ;
  skos:prefLabel "Ranking in first stage"@en ;
.
epo:hasReason
  rdf:type owl:DatatypeProperty ;
  rdfs:comment """Code explaining the change.

WG Approval 5/11/2019"""@en ;
  rdfs:isDefinedBy <http://data.europa.eu/a4g/ontology> ;
  rdfs:label "Reason"@en ;
  skos:definition """Code explaining the change.

WG Approval 5/11/2019"""@en ;
  skos:prefLabel "Reason"@en ;
.
epo:hasReceiptExpressionsDeadline
  rdf:type rdf:Property ;
  rdfs:comment """Time limit for receipt of expressions of interest.


Pending of review by the WG

"""@en ;
  rdfs:isDefinedBy <http://data.europa.eu/a4g/ontology> ;
  rdfs:label "Receipt expressions deadline"@en ;
  skos:definition """Time limit for receipt of expressions of interest.


Pending of review by the WG

"""@en ;
  skos:prefLabel "Receipt expressions deadline"@en ;
.
epo:hasReceivedMicroTenderLots
  rdf:type owl:DatatypeProperty ;
  rdfs:comment """The amount of tenders received from a micro enterprise.

<u>Additional Information:</u>

See Commission Recommendation 2003/361/EC.

WG Approval 12/12/2019"""@en ;
  rdfs:isDefinedBy <http://data.europa.eu/a4g/ontology> ;
  rdfs:label "Received micro tender lots"@en ;
  skos:definition """The amount of tenders received from a micro enterprise.

<u>Additional Information:</u>

See Commission Recommendation 2003/361/EC.

WG Approval 12/12/2019"""@en ;
  skos:prefLabel "Received micro tender lots"@en ;
.
epo:hasReceivedNON-EEATenderLots
  rdf:type owl:DatatypeProperty ;
  rdfs:comment """The amount of tenders received from economic operators in non-EEA countries. 

WG Approval 12/12/2019 15:20:36"""@en ;
  rdfs:isDefinedBy <http://data.europa.eu/a4g/ontology> ;
  rdfs:label "Received n o n- e e a tender lots"@en ;
  skos:definition """The amount of tenders received from economic operators in non-EEA countries. 

WG Approval 12/12/2019 15:20:36"""@en ;
  skos:prefLabel "Received n o n- e e a tender lots"@en ;
.
epo:hasReceivedParticipationRequestsPerLot
  rdf:type owl:DatatypeProperty ;
  rdfs:comment """The amount of applications to participate from economic operators.

WG Approval 12/12/2019"""@en ;
  rdfs:isDefinedBy <http://data.europa.eu/a4g/ontology> ;
  rdfs:label "Received participation requests per lot"@en ;
  skos:definition """The amount of applications to participate from economic operators.

WG Approval 12/12/2019"""@en ;
  skos:prefLabel "Received participation requests per lot"@en ;
.
epo:hasReceivedReviewRequestsPerLot
  rdf:type owl:DatatypeProperty ;
  rdfs:comment """The number of economic operators that requested the buyer to review any of its decisions (e.g. the technical specifications, award decision), as set out in Art. 1(5) of Directive 89/665/EEC and Directive 92/13/EEC.

WG Approval 11/04/2019"""@en ;
  rdfs:isDefinedBy <http://data.europa.eu/a4g/ontology> ;
  rdfs:label "Received review requests per lot"@en ;
  skos:definition """The number of economic operators that requested the buyer to review any of its decisions (e.g. the technical specifications, award decision), as set out in Art. 1(5) of Directive 89/665/EEC and Directive 92/13/EEC.

WG Approval 11/04/2019"""@en ;
  skos:prefLabel "Received review requests per lot"@en ;
.
epo:hasReceivedSMETenderLots
  rdf:type owl:DatatypeProperty ;
  rdfs:comment """The amount of tenders received from micro, small and medium-sized enterprises.

<u>Additional Information:</u>

See Commission Recommendation 2003/361/EC. 
The ReceivedSMETenderLots is used when the size of the company is not exactly knokn.

WG Approval 05/03/2020
"""@en ;
  rdfs:isDefinedBy <http://data.europa.eu/a4g/ontology> ;
  rdfs:label "Received s m e tender lots"@en ;
  skos:definition """The amount of tenders received from micro, small and medium-sized enterprises.

<u>Additional Information:</u>

See Commission Recommendation 2003/361/EC. 
The ReceivedSMETenderLots is used when the size of the company is not exactly knokn.

WG Approval 05/03/2020
"""@en ;
  skos:prefLabel "Received s m e tender lots"@en ;
.
epo:hasReceivedSmallTenderLots
  rdf:type owl:DatatypeProperty ;
  rdfs:comment """Tenders from small enterprise.

<u>Additional Information:</u>

See Commission Recommendation 2003/361/EC.

"""@en ;
  rdfs:isDefinedBy <http://data.europa.eu/a4g/ontology> ;
  rdfs:label "Received small tender lots"@en ;
  skos:definition """Tenders from small enterprise.

<u>Additional Information:</u>

See Commission Recommendation 2003/361/EC.

"""@en ;
  skos:prefLabel "Received small tender lots"@en ;
.
epo:hasReceptionDate
  rdf:type owl:DatatypeProperty ;
  rdfs:comment "Date of reception of a record by an organisation."@en ;
  rdfs:isDefinedBy <http://data.europa.eu/a4g/ontology> ;
  rdfs:label "Reception date"@en ;
  skos:definition "Date of reception of a record by an organisation."@en ;
  skos:prefLabel "Reception date"@en ;
.
epo:hasRecurrence
  rdf:type rdf:Property ;
  rdfs:comment """The Procurement being notified is likely to be included in another procedure in the foreseeable future. 

Additional Information:

For example, a regularly re-tendered municipal service. This does not include awarding multiple contracts within a single qualification system, framework agreement, or a dynamic purchasing system.

"""@en ;
  rdfs:isDefinedBy <http://data.europa.eu/a4g/ontology> ;
  rdfs:label "Recurrence"@en ;
  skos:definition """The Procurement being notified is likely to be included in another procedure in the foreseeable future. 

Additional Information:

For example, a regularly re-tendered municipal service. This does not include awarding multiple contracts within a single qualification system, framework agreement, or a dynamic purchasing system.

"""@en ;
  skos:prefLabel "Recurrence"@en ;
.
epo:hasRecurrenceDescription
  rdf:type owl:DatatypeProperty ;
  rdfs:comment """Any additional information about the recurrence of the Procurement.
 
Additional Information:
For example estimated timing of the Procedure.


(WG approval 2019-01-16)"""@en ;
  rdfs:isDefinedBy <http://data.europa.eu/a4g/ontology> ;
  rdfs:label "Recurrence description"@en ;
  skos:definition """Any additional information about the recurrence of the Procurement.
 
Additional Information:
For example estimated timing of the Procedure.


(WG approval 2019-01-16)"""@en ;
  skos:prefLabel "Recurrence description"@en ;
.
epo:hasRegion
  rdf:type owl:DatatypeProperty ;
  rdfs:isDefinedBy <http://data.europa.eu/a4g/ontology> ;
  rdfs:label "Region"@en ;
  skos:prefLabel "Region"@en ;
.
epo:hasRegisteredLocation
  rdf:type owl:ObjectProperty ;
  rdfs:isDefinedBy <http://data.europa.eu/a4g/ontology> ;
  rdfs:label "Has registered location"@en ;
  skos:prefLabel "Has registered location"@en ;
.
epo:hasRenewalDescription
  rdf:type owl:DatatypeProperty ;
  rdfs:comment """Any other information about the renewal(s).

WG approval 16/04/2019 """@en ;
  rdfs:isDefinedBy <http://data.europa.eu/a4g/ontology> ;
  rdfs:label "Renewal description"@en ;
  skos:definition """Any other information about the renewal(s).

WG approval 16/04/2019 """@en ;
  skos:prefLabel "Renewal description"@en ;
.
epo:hasRenewalIndicator
  rdf:type rdf:Property ;
  rdfs:isDefinedBy <http://data.europa.eu/a4g/ontology> ;
  rdfs:label "Renewal indicator"@en ;
  skos:prefLabel "Renewal indicator"@en ;
.
epo:hasRequestForParticipationDeadline
  rdf:type rdf:Property ;
  rdfs:comment """The time limit for receipt of requests to participate in a procedure.

Additional Information

This is also applicable for the procedures in a Dynamic Purchase System, whereby the economic operator requests to be qualified for the system.

WG Approval 10/10/2019"""@en ;
  rdfs:isDefinedBy <http://data.europa.eu/a4g/ontology> ;
  rdfs:label "Request for participation deadline"@en ;
  skos:definition """The time limit for receipt of requests to participate in a procedure.

Additional Information

This is also applicable for the procedures in a Dynamic Purchase System, whereby the economic operator requests to be qualified for the system.

WG Approval 10/10/2019"""@en ;
  skos:prefLabel "Request for participation deadline"@en ;
.
epo:hasReservedExecution
  rdf:type owl:ObjectProperty ;
  rdfs:comment """<foreign otherprops=\"#24292e\">The execution of the contract is restricted to the framework of sheltered employment programmes</foreign>.

WG Approval 12/09/2019




"""@en ;
  rdfs:isDefinedBy <http://data.europa.eu/a4g/ontology> ;
  rdfs:label "Has reserved execution"@en ;
  rdfs:label "Reserved execution"@en ;
  skos:definition """<foreign otherprops=\"#24292e\">The execution of the contract is restricted to the framework of sheltered employment programmes</foreign>.

WG Approval 12/09/2019




"""@en ;
  skos:prefLabel "Has reserved execution"@en ;
  skos:prefLabel "Reserved execution"@en ;
.
epo:hasReservedProcurement
  rdf:type owl:ObjectProperty ;
  rdfs:isDefinedBy <http://data.europa.eu/a4g/ontology> ;
  rdfs:label "Has reserved procurement"@en ;
  rdfs:label "Reserved procurement"@en ;
  skos:prefLabel "Has reserved procurement"@en ;
  skos:prefLabel "Reserved procurement"@en ;
.
epo:hasRestrictedAccessAddress
  rdf:type owl:ObjectProperty ;
  rdfs:comment "The internet address with information on accessing the restricted (part of the) procurement documents."@en ;
  rdfs:isDefinedBy <http://data.europa.eu/a4g/ontology> ;
  rdfs:label "Has restricted access address"@en ;
  skos:definition "The internet address with information on accessing the restricted (part of the) procurement documents."@en ;
  skos:prefLabel "Has restricted access address"@en ;
.
epo:hasRestrictedCommunicationsJustification
  rdf:type owl:ObjectProperty ;
  rdfs:isDefinedBy <http://data.europa.eu/a4g/ontology> ;
  rdfs:label "Restricted communications justification"@en ;
  skos:prefLabel "Restricted communications justification"@en ;
.
epo:hasRestrictedProcurementDocumentsMadeAvailableVia
  rdf:type owl:ObjectProperty ;
  rdfs:isDefinedBy <http://data.europa.eu/a4g/ontology> ;
  rdfs:label "Has restricted procurement documents made available via"@en ;
  skos:prefLabel "Has restricted procurement documents made available via"@en ;
.
epo:hasReviewDeadline
  rdf:type rdf:Property ;
  rdfs:isDefinedBy <http://data.europa.eu/a4g/ontology> ;
  rdfs:label "Review deadline"@en ;
  skos:prefLabel "Review deadline"@en ;
.
epo:hasReviewDeadlineInformation
  rdf:type owl:DatatypeProperty ;
  rdfs:comment """The description of the time limits for review procedures.

WG Approval 01/10/2019
"""@en ;
  rdfs:isDefinedBy <http://data.europa.eu/a4g/ontology> ;
  rdfs:label "Review deadline information"@en ;
  skos:definition """The description of the time limits for review procedures.

WG Approval 01/10/2019
"""@en ;
  skos:prefLabel "Review deadline information"@en ;
.
epo:hasReviewProcedure
  rdf:type owl:DatatypeProperty ;
  rdfs:isDefinedBy <http://data.europa.eu/a4g/ontology> ;
  rdfs:label "Review procedure"@en ;
  skos:prefLabel "Review procedure"@en ;
.
epo:hasRoom
  rdf:type owl:DatatypeProperty ;
  rdfs:isDefinedBy <http://data.europa.eu/a4g/ontology> ;
  rdfs:label "Room"@en ;
  skos:prefLabel "Room"@en ;
.
epo:hasRulesSetBy
  rdf:type owl:ObjectProperty ;
  rdfs:isDefinedBy <http://data.europa.eu/a4g/ontology> ;
  rdfs:label "Has rules set by"@en ;
  skos:prefLabel "Has rules set by"@en ;
.
epo:hasSMESuitable
  rdf:type rdf:Property ;
  rdfs:comment """The Lot is suitable for small and medium enterprises (SMEs).


Additional Information

This allows the buyer to make emphasis on the fact that the procedure has been designed having SMEs in mind. This indicator is also to be reflected in the selection criteria.

For example, number of employees and turnover are applicable to the definition of an SME.

WG Approval 15/10/2019"""@en ;
  rdfs:isDefinedBy <http://data.europa.eu/a4g/ontology> ;
  rdfs:label "S m e suitable"@en ;
  skos:definition """The Lot is suitable for small and medium enterprises (SMEs).


Additional Information

This allows the buyer to make emphasis on the fact that the procedure has been designed having SMEs in mind. This indicator is also to be reflected in the selection criteria.

For example, number of employees and turnover are applicable to the definition of an SME.

WG Approval 15/10/2019"""@en ;
  skos:prefLabel "S m e suitable"@en ;
.
epo:hasScore
  rdf:type owl:DatatypeProperty ;
  rdfs:isDefinedBy <http://data.europa.eu/a4g/ontology> ;
  rdfs:label "Score"@en ;
  skos:prefLabel "Score"@en ;
.
epo:hasSecondStage
  rdf:type owl:ObjectProperty ;
  rdfs:isDefinedBy <http://data.europa.eu/a4g/ontology> ;
  rdfs:label "Has second stage"@en ;
  skos:prefLabel "Has second stage"@en ;
.
epo:hasSelectionCriterionApplicability
  rdf:type owl:ObjectProperty ;
  rdfs:isDefinedBy <http://data.europa.eu/a4g/ontology> ;
  rdfs:label "Has selection criterion applicability"@en ;
  rdfs:label "Selection criterion applicability"@en ;
  skos:prefLabel "Has selection criterion applicability"@en ;
  skos:prefLabel "Selection criterion applicability"@en ;
.
epo:hasSelectionCriterionType
  rdf:type owl:ObjectProperty ;
  rdfs:isDefinedBy <http://data.europa.eu/a4g/ontology> ;
  rdfs:label "Has selection criterion type"@en ;
  rdfs:label "Selection criterion type"@en ;
  skos:prefLabel "Has selection criterion type"@en ;
  skos:prefLabel "Selection criterion type"@en ;
.
epo:hasShelteredEmploymentUsage
  rdf:type owl:ObjectProperty ;
  rdfs:isDefinedBy <http://data.europa.eu/a4g/ontology> ;
  rdfs:label "Has sheltered employment usage"@en ;
  skos:prefLabel "Has sheltered employment usage"@en ;
.
epo:hasShownInterest
  rdf:type owl:ObjectProperty ;
  rdfs:isDefinedBy <http://data.europa.eu/a4g/ontology> ;
  rdfs:label "Has shown interest"@en ;
  skos:prefLabel "Has shown interest"@en ;
.
epo:hasSize
  rdf:type owl:ObjectProperty ;
  rdfs:isDefinedBy <http://data.europa.eu/a4g/ontology> ;
  rdfs:label "Has size"@en ;
  rdfs:label "Size"@en ;
  skos:prefLabel "Has size"@en ;
  skos:prefLabel "Size"@en ;
.
epo:hasSomeProcurementDocumentsRestrctedJustification
  rdf:type owl:DatatypeProperty ;
  rdfs:isDefinedBy <http://data.europa.eu/a4g/ontology> ;
  rdfs:label "Some procurement documents restrcted justification"@en ;
  skos:prefLabel "Some procurement documents restrcted justification"@en ;
.
epo:hasSomeProcurementDocumentsRestricted
  rdf:type rdf:Property ;
  rdfs:comment """The access to certain procurement documents is restricted.

WG Approval 10/10/2019"""@en ;
  rdfs:isDefinedBy <http://data.europa.eu/a4g/ontology> ;
  rdfs:label "Some procurement documents restricted"@en ;
  skos:definition """The access to certain procurement documents is restricted.

WG Approval 10/10/2019"""@en ;
  skos:prefLabel "Some procurement documents restricted"@en ;
.
epo:hasSpecificPlaceOfPerformance
  rdf:type owl:ObjectProperty ;
  rdfs:isDefinedBy <http://data.europa.eu/a4g/ontology> ;
  rdfs:label "Has specific place of performance"@en ;
  skos:prefLabel "Has specific place of performance"@en ;
.
epo:hasStartDate
  rdf:type rdf:Property ;
  rdfs:comment "The date on which this period begins."@en ;
  rdfs:isDefinedBy <http://data.europa.eu/a4g/ontology> ;
  rdfs:label "Start date"@en ;
  skos:definition "The date on which this period begins."@en ;
  skos:prefLabel "Start date"@en ;
.
epo:hasStartTime
  rdf:type rdf:Property ;
  rdfs:comment "The time at which this period begins."@en ;
  rdfs:isDefinedBy <http://data.europa.eu/a4g/ontology> ;
  rdfs:label "Start time"@en ;
  skos:definition "The time at which this period begins."@en ;
  skos:prefLabel "Start time"@en ;
.
epo:hasStrategicProcurementDescription
  rdf:type owl:DatatypeProperty ;
  rdfs:comment """Self-explanatory text about a concept.
"""@en ;
  rdfs:isDefinedBy <http://data.europa.eu/a4g/ontology> ;
  rdfs:label "Strategic procurement description"@en ;
  skos:definition """Self-explanatory text about a concept.
"""@en ;
  skos:prefLabel "Strategic procurement description"@en ;
.
epo:hasStrategicProcurementType
  rdf:type owl:ObjectProperty ;
  rdfs:isDefinedBy <http://data.europa.eu/a4g/ontology> ;
  rdfs:label "Has strategic procurement type"@en ;
  skos:prefLabel "Has strategic procurement type"@en ;
.
epo:hasStreetName
  rdf:type owl:DatatypeProperty ;
  rdfs:isDefinedBy <http://data.europa.eu/a4g/ontology> ;
  rdfs:label "Street name"@en ;
  skos:prefLabel "Street name"@en ;
.
epo:hasSubcontracted
  rdf:type owl:ObjectProperty ;
  rdfs:isDefinedBy <http://data.europa.eu/a4g/ontology> ;
  rdfs:label "Has subcontracted"@en ;
  skos:prefLabel "Has subcontracted"@en ;
.
epo:hasSubcontracting
  rdf:type owl:ObjectProperty ;
  rdfs:isDefinedBy <http://data.europa.eu/a4g/ontology> ;
  rdfs:label "Subcontracting"@en ;
  skos:prefLabel "Subcontracting"@en ;
.
epo:hasSubcontractingApplicability
  rdf:type owl:ObjectProperty ;
  rdfs:isDefinedBy <http://data.europa.eu/a4g/ontology> ;
  rdfs:label "Has subcontracting applicability"@en ;
  skos:prefLabel "Has subcontracting applicability"@en ;
.
epo:hasSubcontractingInvolved
  rdf:type rdf:Property ;
  rdfs:comment """List of Subcontractors and the subject matter they cover are required.

Additional Information: 
The tenderer will ned to supply this information in the tender.

WG Approval 28/02/2019"""@en ;
  rdfs:isDefinedBy <http://data.europa.eu/a4g/ontology> ;
  rdfs:label "Subcontracting involved"@en ;
  skos:definition """List of Subcontractors and the subject matter they cover are required.

Additional Information: 
The tenderer will ned to supply this information in the tender.

WG Approval 28/02/2019"""@en ;
  skos:prefLabel "Subcontracting involved"@en ;
.
epo:hasSubcontractingObligation
  rdf:type owl:ObjectProperty ;
  rdfs:isDefinedBy <http://data.europa.eu/a4g/ontology> ;
  rdfs:label "Has subcontracting obligation"@en ;
  rdfs:label "Subcontracting obligation"@en ;
  skos:prefLabel "Has subcontracting obligation"@en ;
  skos:prefLabel "Subcontracting obligation"@en ;
.
epo:hasSubcontractingUsage
  rdf:type owl:ObjectProperty ;
  rdfs:comment """Whether subcontracting will be used or not (or not known yet).

WG Approval 08/05/2019
"""@en ;
  rdfs:isDefinedBy <http://data.europa.eu/a4g/ontology> ;
  rdfs:label "Has subcontracting usage"@en ;
  rdfs:label "Subcontracting usage"@en ;
  skos:definition """Whether subcontracting will be used or not (or not known yet).

WG Approval 08/05/2019
"""@en ;
  skos:prefLabel "Has subcontracting usage"@en ;
  skos:prefLabel "Subcontracting usage"@en ;
.
epo:hasSubcontractorsProposedAboveObligation
  rdf:type rdf:Property ;
  rdfs:isDefinedBy <http://data.europa.eu/a4g/ontology> ;
  rdfs:label "Subcontractors proposed above obligation"@en ;
  skos:prefLabel "Subcontractors proposed above obligation"@en ;
.
epo:hasSubcriterionType
  rdf:type owl:ObjectProperty ;
  rdfs:isDefinedBy <http://data.europa.eu/a4g/ontology> ;
  rdfs:label "Has subcriterion type"@en ;
  skos:prefLabel "Has subcriterion type"@en ;
.
epo:hasSubmissionDocumentType
  rdf:type owl:ObjectProperty ;
  rdfs:isDefinedBy <http://data.europa.eu/a4g/ontology> ;
  rdfs:label "Has submission document type"@en ;
  rdfs:label "Submission document type"@en ;
  skos:prefLabel "Has submission document type"@en ;
  skos:prefLabel "Submission document type"@en ;
.
epo:hasSuccessiveReduction
  rdf:type rdf:Property ;
  rdfs:comment """The number of solutions or tenders will be reduced in iterative evaluations for multiple staged procedures.

Additional information:
This refers to multiple-stage procedures (included two-stage procedures, at least). Open Procedures can be seen as one-stage procedures.
WG Approval 22/08/2019 """@en ;
  rdfs:isDefinedBy <http://data.europa.eu/a4g/ontology> ;
  rdfs:label "Successive reduction"@en ;
  skos:definition """The number of solutions or tenders will be reduced in iterative evaluations for multiple staged procedures.

Additional information:
This refers to multiple-stage procedures (included two-stage procedures, at least). Open Procedures can be seen as one-stage procedures.
WG Approval 22/08/2019 """@en ;
  skos:prefLabel "Successive reduction"@en ;
.
epo:hasTaxIdentifier
  rdf:type owl:ObjectProperty ;
  rdfs:isDefinedBy <http://data.europa.eu/a4g/ontology> ;
  rdfs:label "Tax identifier"@en ;
  skos:prefLabel "Tax identifier"@en ;
.
epo:hasTaxIncludedIndicator
  rdf:type rdf:Property ;
  rdfs:isDefinedBy <http://data.europa.eu/a4g/ontology> ;
  rdfs:label "Tax included indicator"@en ;
  skos:prefLabel "Tax included indicator"@en ;
.
epo:hasTelephone
  rdf:type owl:DatatypeProperty ;
  rdfs:comment """The telephone number used to reach a person or an organisation.
"""@en ;
  rdfs:isDefinedBy <http://data.europa.eu/a4g/ontology> ;
  rdfs:label "Telephone"@en ;
  skos:definition """The telephone number used to reach a person or an organisation.
"""@en ;
  skos:prefLabel "Telephone"@en ;
.
epo:hasTenderEvaluationTerms
  rdf:type owl:ObjectProperty ;
  rdfs:isDefinedBy <http://data.europa.eu/a4g/ontology> ;
  rdfs:label "Has tender evaluation terms"@en ;
  skos:prefLabel "Has tender evaluation terms"@en ;
.
epo:hasTenderGuaranteeDescription
  rdf:type owl:DatatypeProperty ;
  rdfs:comment """Information on the Tender Guarantee Required from the tenderer when submitting a tender. 

Additional Information
This information may include the amount and the way of delivering of the guarantee.

WG Approval 10/10/2019"""@en ;
  rdfs:isDefinedBy <http://data.europa.eu/a4g/ontology> ;
  rdfs:label "Tender guarantee description"@en ;
  skos:definition """Information on the Tender Guarantee Required from the tenderer when submitting a tender. 

Additional Information
This information may include the amount and the way of delivering of the guarantee.

WG Approval 10/10/2019"""@en ;
  skos:prefLabel "Tender guarantee description"@en ;
.
epo:hasTenderGuaranteeRequired
  rdf:type rdf:Property ;
  rdfs:comment """The tender must include a financial commitment to be used in case of default.

Additional Information:
1. The financial commitment may be retained by the buyer in the case the tenderer withdraws the tender before the award of the contract or does not sign the contract.
2. Usual modalities are bonds, cheques, loans, other.

WG Approval 10/10/2019
"""@en ;
  rdfs:isDefinedBy <http://data.europa.eu/a4g/ontology> ;
  rdfs:label "Tender guarantee required"@en ;
  skos:definition """The tender must include a financial commitment to be used in case of default.

Additional Information:
1. The financial commitment may be retained by the buyer in the case the tenderer withdraws the tender before the award of the contract or does not sign the contract.
2. Usual modalities are bonds, cheques, loans, other.

WG Approval 10/10/2019
"""@en ;
  skos:prefLabel "Tender guarantee required"@en ;
.
epo:hasTenderLanguage
  rdf:type owl:ObjectProperty ;
  rdfs:comment """Language in which the tender is to be expressed. 

WG Approval 03/10/2019 """@en ;
  rdfs:isDefinedBy <http://data.europa.eu/a4g/ontology> ;
  rdfs:label "Has tender language"@en ;
  rdfs:label "Tender language"@en ;
  skos:definition """Language in which the tender is to be expressed. 

WG Approval 03/10/2019 """@en ;
  skos:prefLabel "Has tender language"@en ;
  skos:prefLabel "Tender language"@en ;
.
epo:hasTenderReceiptDeadLine
  rdf:type rdf:Property ;
  rdfs:isDefinedBy <http://data.europa.eu/a4g/ontology> ;
  rdfs:label "Tender receipt dead line"@en ;
  skos:prefLabel "Tender receipt dead line"@en ;
.
epo:hasTenderReceiptDeadline
  rdf:type rdf:Property ;
  rdfs:comment """The deadline for receiving tenders.

Additional Information
This is the  deadline by which the buyer must receive the tenders and is not the time at which the economic operator sends its tender.

WG Approval 10/10/2019"""@en ;
  rdfs:isDefinedBy <http://data.europa.eu/a4g/ontology> ;
  rdfs:label "Tender receipt deadline"@en ;
  skos:definition """The deadline for receiving tenders.

Additional Information
This is the  deadline by which the buyer must receive the tenders and is not the time at which the economic operator sends its tender.

WG Approval 10/10/2019"""@en ;
  skos:prefLabel "Tender receipt deadline"@en ;
.
epo:hasTenderSubcontractingInformation
  rdf:type owl:ObjectProperty ;
  rdfs:comment """The information about subcontracting that must be indicated in the tender.

WG  Approval 10/10/2019"""@en ;
  rdfs:isDefinedBy <http://data.europa.eu/a4g/ontology> ;
  rdfs:label "Has tender subcontracting information"@en ;
  rdfs:label "Tender subcontracting information"@en ;
  skos:definition """The information about subcontracting that must be indicated in the tender.

WG  Approval 10/10/2019"""@en ;
  skos:prefLabel "Has tender subcontracting information"@en ;
  skos:prefLabel "Tender subcontracting information"@en ;
.
epo:hasTenderSubmissionCommunicationMeans
  rdf:type owl:ObjectProperty ;
  rdfs:isDefinedBy <http://data.europa.eu/a4g/ontology> ;
  rdfs:label "Has tender submission communication means"@en ;
  skos:prefLabel "Has tender submission communication means"@en ;
.
epo:hasTenderValidityDeadline
  rdf:type rdf:Property ;
  rdfs:comment """The period, from the tender submission deadline, for which tenders must remain valid.

WG Approval 10-10-2019"""@en ;
  rdfs:isDefinedBy <http://data.europa.eu/a4g/ontology> ;
  rdfs:label "Tender validity deadline"@en ;
  skos:definition """The period, from the tender submission deadline, for which tenders must remain valid.

WG Approval 10-10-2019"""@en ;
  skos:prefLabel "Tender validity deadline"@en ;
.
epo:hasTendersReceivedPerLot
  rdf:type owl:DatatypeProperty ;
  rdfs:comment """The total amount of tenders received.

WG Approval 12/12/2019"""@en ;
  rdfs:isDefinedBy <http://data.europa.eu/a4g/ontology> ;
  rdfs:label "Tenders received per lot"@en ;
  skos:definition """The total amount of tenders received.

WG Approval 12/12/2019"""@en ;
  skos:prefLabel "Tenders received per lot"@en ;
.
epo:hasText
  rdf:type owl:DatatypeProperty ;
  rdfs:isDefinedBy <http://data.europa.eu/a4g/ontology> ;
  rdfs:label "Text"@en ;
  skos:prefLabel "Text"@en ;
.
epo:hasThresholdType
  rdf:type owl:ObjectProperty ;
  rdfs:comment """The method to interpret the threshold value as minimum or a maximum.

WG Approval 17/09/2019 """@en ;
  rdfs:comment """The type of threshold for a Selection Criterion.

Additional Information

For example, a minimum score or a maximum number of tenders with the highest score passing.
"""@en ;
  rdfs:isDefinedBy <http://data.europa.eu/a4g/ontology> ;
  rdfs:label "Has threshold type"@en ;
  rdfs:label "Threshold type"@en ;
  skos:definition """The method to interpret the threshold value as minimum or a maximum.

WG Approval 17/09/2019 """@en ;
  skos:definition """The type of threshold for a Selection Criterion.

Additional Information

For example, a minimum score or a maximum number of tenders with the highest score passing.
"""@en ;
  skos:prefLabel "Has threshold type"@en ;
  skos:prefLabel "Threshold type"@en ;
.
epo:hasThresholdValue
  rdf:type owl:DatatypeProperty ;
  rdfs:isDefinedBy <http://data.europa.eu/a4g/ontology> ;
  rdfs:label "Threshold value"@en ;
  skos:prefLabel "Threshold value"@en ;
.
epo:hasTimePeriods
  rdf:type owl:ObjectProperty ;
  rdfs:isDefinedBy <http://data.europa.eu/a4g/ontology> ;
  rdfs:label "Has time periods"@en ;
  skos:prefLabel "Has time periods"@en ;
.
epo:hasTimezoneOffset
  rdf:type owl:DatatypeProperty ;
  rdfs:isDefinedBy <http://data.europa.eu/a4g/ontology> ;
  rdfs:label "Timezone offset"@en ;
  skos:prefLabel "Timezone offset"@en ;
.
epo:hasTitle
  rdf:type owl:DatatypeProperty ;
  rdfs:comment """A short self-descriptive name of the instance of the concept.

Additional Information:

For example, the title of a planned part that may become a procedure or a lot in the future; the title of a contract, etc.

(WG Approval 11-11-2019)
"""@en ;
  rdfs:comment """A short self-descriptive name of the instance of the concept.

Additional Information:

For example, the title of a planned part that may become a procedure or a lot in the future; the title of a contract, etc.

(WG Approval 11-11-2019)"""@en ;
  rdfs:isDefinedBy <http://data.europa.eu/a4g/ontology> ;
  rdfs:label "Title"@en ;
  skos:definition """A short self-descriptive name of the instance of the concept.

Additional Information:

For example, the title of a planned part that may become a procedure or a lot in the future; the title of a contract, etc.

(WG Approval 11-11-2019)
"""@en ;
  skos:definition """A short self-descriptive name of the instance of the concept.

Additional Information:

For example, the title of a planned part that may become a procedure or a lot in the future; the title of a contract, etc.

(WG Approval 11-11-2019)"""@en ;
  skos:prefLabel "Title"@en ;
.
epo:hasTotalAmountWithoutVAT
  rdf:type owl:ObjectProperty ;
  rdfs:isDefinedBy <http://data.europa.eu/a4g/ontology> ;
  rdfs:label "Total amount without v a t"@en ;
  skos:prefLabel "Total amount without v a t"@en ;
.
epo:hasTotalFrameworkValue
  rdf:type owl:ObjectProperty ;
  rdfs:comment """The maximum value which can be spent through all the framework agreements announced in this notice, including options and renewals of contracts.

Additional information:

The value provided is a threshold value that implicity means that it cannot be exceeded however it may not be reached during the execution of a contract.

The Framework Agreements in a CAN are to be traced back and added to provide this value. The path to get the value of an individual Framework Agreement is:

CAN isA Notice,
CAN notifiesAwardResult AwardDecision,
AwardDecision refersTo Lot,
Lot uses Technique, 
FrameworkAgreement isA Technique,
FrameworkAgreement hasAwardedValue ProcurementValue .

WG Approval 03/12/2019

"""@en ;
  rdfs:isDefinedBy <http://data.europa.eu/a4g/ontology> ;
  rdfs:label "Has total framework value"@en ;
  skos:definition """The maximum value which can be spent through all the framework agreements announced in this notice, including options and renewals of contracts.

Additional information:

The value provided is a threshold value that implicity means that it cannot be exceeded however it may not be reached during the execution of a contract.

The Framework Agreements in a CAN are to be traced back and added to provide this value. The path to get the value of an individual Framework Agreement is:

CAN isA Notice,
CAN notifiesAwardResult AwardDecision,
AwardDecision refersTo Lot,
Lot uses Technique, 
FrameworkAgreement isA Technique,
FrameworkAgreement hasAwardedValue ProcurementValue .

WG Approval 03/12/2019

"""@en ;
  skos:prefLabel "Has total framework value"@en ;
.
epo:hasTotalMagnitudeQuantity
  rdf:type owl:ObjectProperty ;
  rdfs:comment """The number of units required.

Additional Information

The quantity needs to go along with the unit. In the ePO we use the ISO 15000-5 UN/CEFACT CCTS QuantityType for quantities, which uses the attribute \"unitCode\" to specify what the quantity is about.
For example, 3 months; 131 printers; 1,000 tones; etc.


"""@en ;
  rdfs:isDefinedBy <http://data.europa.eu/a4g/ontology> ;
  rdfs:label "Total magnitude quantity"@en ;
  skos:definition """The number of units required.

Additional Information

The quantity needs to go along with the unit. In the ePO we use the ISO 15000-5 UN/CEFACT CCTS QuantityType for quantities, which uses the attribute \"unitCode\" to specify what the quantity is about.
For example, 3 months; 131 printers; 1,000 tones; etc.


"""@en ;
  skos:prefLabel "Total magnitude quantity"@en ;
.
epo:hasTotalVATAmount
  rdf:type owl:ObjectProperty ;
  rdfs:isDefinedBy <http://data.europa.eu/a4g/ontology> ;
  rdfs:label "Total v a t amount"@en ;
  skos:prefLabel "Total v a t amount"@en ;
.
epo:hasTotalValue
  rdf:type owl:ObjectProperty ;
  rdfs:comment """The value of all lots awarded for this notice, including options and renewals. 

Additional information:
The values of the individual Lots awarded under a framework agreement and mentioned in this notice are included.

The values of the individual lots announced in a CAN are to be traced back and added to provide this value.

The path to get the value of an individual Lot is:

CAN isA Notice ,
CAN notifiesAwardResult AwardDecision ,
AwardDecision refersTo Lot ,
hasAwardedValue ProcurementValue .

WG Approval 03/12/2019
"""@en ;
  rdfs:isDefinedBy <http://data.europa.eu/a4g/ontology> ;
  rdfs:label "Has total value"@en ;
  skos:definition """The value of all lots awarded for this notice, including options and renewals. 

Additional information:
The values of the individual Lots awarded under a framework agreement and mentioned in this notice are included.

The values of the individual lots announced in a CAN are to be traced back and added to provide this value.

The path to get the value of an individual Lot is:

CAN isA Notice ,
CAN notifiesAwardResult AwardDecision ,
AwardDecision refersTo Lot ,
hasAwardedValue ProcurementValue .

WG Approval 03/12/2019
"""@en ;
  skos:prefLabel "Has total value"@en ;
.
epo:hasTotalVehicles
  rdf:type owl:DatatypeProperty ;
  rdfs:isDefinedBy <http://data.europa.eu/a4g/ontology> ;
  rdfs:label "Total vehicles"@en ;
  skos:prefLabel "Total vehicles"@en ;
.
epo:hasType
  rdf:type rdf:Property ;
  rdfs:comment """The categorisation of the set of activities of the procedure according to the Law. 

Additional Information
For example \"Open Procedure\", \"Restricted\", \"Negotiated without Publicity\", etc. (see code list \"procurement-procedure-type\"

WG Approval 20/08/2019
"""@en ;
  rdfs:comment """The property Type can be used to identify the namespace and class of the Agent.

This may be useful for XML implementations of the Model, where software applications need to know the type of the Agent in order to identify the particular Agent sub-class properties. But could also create a consistency problem consisting in specifying an IRI for one type of Agent whilst the actual individual of Agent is a different one.

One way of resolving this inconsistency would be cross-checking by externalised means the requested IRI ID against the actual type of class (via shapes, Schematron, etc.).

For more details on IRIs, check the Request For Comments website: https://tools.ietf.org/html/rfc3987

Examples of IRIs:

<foreign otherprops=\"#993300\">https://github.com/semiceu/cagv/2.0.0/xml/CV-Agent#Organisation</foreign>
<foreign otherprops=\"#993300\">
</foreign><foreign otherprops=\"#993300\">https://github.com/semiceu/cagv/2.0.0/xml/CV-Agent#NaturalPerson</foreign>
<foreign otherprops=\"#993300\">
</foreign><foreign otherprops=\"#993300\">https://github.com/semiceu/cagv/2.0.0/xml/CV-Agent#System</foreign>

An example of inconsistency:

cagv:Agent.ID = 986454b6-22af-4894-9a3d-f201d236b88c
cagv:Agent.Type = <foreign otherprops=\"#993300\">https://github.com/semiceu/cagv/2.0.0/xml/CV-Agent#ORganisation</foreign>
cagv:NaturalPerson.ID = 986454b6-22af-4894-9a3d-f201d236b88c


"""@en ;
  rdfs:isDefinedBy <http://data.europa.eu/a4g/ontology> ;
  rdfs:label "Type"@en ;
  skos:definition """The categorisation of the set of activities of the procedure according to the Law. 

Additional Information
For example \"Open Procedure\", \"Restricted\", \"Negotiated without Publicity\", etc. (see code list \"procurement-procedure-type\"

WG Approval 20/08/2019
"""@en ;
  skos:definition """The property Type can be used to identify the namespace and class of the Agent.

This may be useful for XML implementations of the Model, where software applications need to know the type of the Agent in order to identify the particular Agent sub-class properties. But could also create a consistency problem consisting in specifying an IRI for one type of Agent whilst the actual individual of Agent is a different one.

One way of resolving this inconsistency would be cross-checking by externalised means the requested IRI ID against the actual type of class (via shapes, Schematron, etc.).

For more details on IRIs, check the Request For Comments website: https://tools.ietf.org/html/rfc3987

Examples of IRIs:

<foreign otherprops=\"#993300\">https://github.com/semiceu/cagv/2.0.0/xml/CV-Agent#Organisation</foreign>
<foreign otherprops=\"#993300\">
</foreign><foreign otherprops=\"#993300\">https://github.com/semiceu/cagv/2.0.0/xml/CV-Agent#NaturalPerson</foreign>
<foreign otherprops=\"#993300\">
</foreign><foreign otherprops=\"#993300\">https://github.com/semiceu/cagv/2.0.0/xml/CV-Agent#System</foreign>

An example of inconsistency:

cagv:Agent.ID = 986454b6-22af-4894-9a3d-f201d236b88c
cagv:Agent.Type = <foreign otherprops=\"#993300\">https://github.com/semiceu/cagv/2.0.0/xml/CV-Agent#ORganisation</foreign>
cagv:NaturalPerson.ID = 986454b6-22af-4894-9a3d-f201d236b88c


"""@en ;
  skos:prefLabel "Type"@en ;
.
epo:hasURL
  rdf:type rdf:Property ;
  rdfs:comment """The identifier of a resource.

Additional Information

For example:

1. The URL of the system from where to access the procurement documents;
2. The URL of the system for the submission of tender documents;
3. The URL of the system from where to download a tool to communicate with the Buyer;
4. The URL of the system used by a Technique to allow Economic Operators to exchange information with the Buyer (e.g. eAuction and DPS Systems)
5. The URL of the system used to exchange information between Buyer and EO for questions and clarifications;

WG Approval 30/09/2019


"""@en ;
  rdfs:comment """The identifier of a resource.

Additional Information

For example:

1. The URL of the system from where to access the procurement documents;
2. The URL of the system for the submission of tender documents;
3. The URL of the system from where to download a tool to communicate with the Buyer;
4. The URL of the system used by a Technique to allow Economic Operators to exchange information with the Buyer (e.g. eAuction and DPS Systems)
5. The URL of the system used to exchange information between Buyer and EO for questions and clarifications;

WG Approval 30/09/2019

"""@en ;
  rdfs:isDefinedBy <http://data.europa.eu/a4g/ontology> ;
  rdfs:label "U r l"@en ;
  skos:definition """The identifier of a resource.

Additional Information

For example:

1. The URL of the system from where to access the procurement documents;
2. The URL of the system for the submission of tender documents;
3. The URL of the system from where to download a tool to communicate with the Buyer;
4. The URL of the system used by a Technique to allow Economic Operators to exchange information with the Buyer (e.g. eAuction and DPS Systems)
5. The URL of the system used to exchange information between Buyer and EO for questions and clarifications;

WG Approval 30/09/2019


"""@en ;
  skos:definition """The identifier of a resource.

Additional Information

For example:

1. The URL of the system from where to access the procurement documents;
2. The URL of the system for the submission of tender documents;
3. The URL of the system from where to download a tool to communicate with the Buyer;
4. The URL of the system used by a Technique to allow Economic Operators to exchange information with the Buyer (e.g. eAuction and DPS Systems)
5. The URL of the system used to exchange information between Buyer and EO for questions and clarifications;

WG Approval 30/09/2019

"""@en ;
  skos:prefLabel "U r l"@en ;
.
epo:hasUUID
  rdf:type owl:ObjectProperty ;
  rdfs:isDefinedBy <http://data.europa.eu/a4g/ontology> ;
  rdfs:label "U u i d"@en ;
  skos:prefLabel "U u i d"@en ;
.
epo:hasUnit
  rdf:type owl:ObjectProperty ;
  rdfs:isDefinedBy <http://data.europa.eu/a4g/ontology> ;
  rdfs:label "Has unit"@en ;
  rdfs:label "Unit"@en ;
  skos:prefLabel "Has unit"@en ;
  skos:prefLabel "Unit"@en ;
.
epo:hasUnofficialLanguage
  rdf:type owl:ObjectProperty ;
  rdfs:comment """The language translation(s) in which the instances of the given concepts are available. These linguistic versions are not an official translation, they are provided only for information.

WG Approval 03/10/2019"""@en ;
  rdfs:comment """The language(s) in which the instances of the given concepts are also available in the following languages. These versions are not an official translation, they are provided only for information.

WG Approval 03/10/2019"""@en ;
  rdfs:isDefinedBy <http://data.europa.eu/a4g/ontology> ;
  rdfs:label "Has unofficial language"@en ;
  rdfs:label "Unofficial language"@en ;
  skos:definition """The language translation(s) in which the instances of the given concepts are available. These linguistic versions are not an official translation, they are provided only for information.

WG Approval 03/10/2019"""@en ;
  skos:definition """The language(s) in which the instances of the given concepts are also available in the following languages. These versions are not an official translation, they are provided only for information.

WG Approval 03/10/2019"""@en ;
  skos:prefLabel "Has unofficial language"@en ;
  skos:prefLabel "Unofficial language"@en ;
.
epo:hasUnverifiedTenderLot
  rdf:type owl:DatatypeProperty ;
  rdfs:comment """Tenders received for which there non-award acceptability has not been evaluated
.

<u>Additional information

:</u>

Non-award acceptability includes non-compliance to procurement document requirements (ie exclusion grounds, selection criterion)."""@en ;
  rdfs:isDefinedBy <http://data.europa.eu/a4g/ontology> ;
  rdfs:label "Unverified tender lot"@en ;
  skos:definition """Tenders received for which there non-award acceptability has not been evaluated
.

<u>Additional information

:</u>

Non-award acceptability includes non-compliance to procurement document requirements (ie exclusion grounds, selection criterion)."""@en ;
  skos:prefLabel "Unverified tender lot"@en ;
.
epo:hasUsedForCandidateRestriction
  rdf:type rdf:Property ;
  rdfs:isDefinedBy <http://data.europa.eu/a4g/ontology> ;
  rdfs:label "Used for candidate restriction"@en ;
  skos:prefLabel "Used for candidate restriction"@en ;
.
epo:hasValidityPeriod
  rdf:type owl:ObjectProperty ;
  rdfs:isDefinedBy <http://data.europa.eu/a4g/ontology> ;
  rdfs:label "Has validity period"@en ;
  skos:prefLabel "Has validity period"@en ;
.
epo:hasVariant
  rdf:type rdf:Property ;
  rdfs:comment """Alternative solution to fulfil the buyer's needs as opposed to solutions indicated in the procurement documents.

Additional Information:

The permission to offer variants is only allowed if specified in a Contract Notice or a Prior Information Notice that used as a means for calling for a competition.
The buyer lays out minimum requirements in the procurement documents that must be respected by tenderers submitting variants.

WG Approval 29/05/2019

"""@en ;
  rdfs:isDefinedBy <http://data.europa.eu/a4g/ontology> ;
  rdfs:label "Variant"@en ;
  skos:definition """Alternative solution to fulfil the buyer's needs as opposed to solutions indicated in the procurement documents.

Additional Information:

The permission to offer variants is only allowed if specified in a Contract Notice or a Prior Information Notice that used as a means for calling for a competition.
The buyer lays out minimum requirements in the procurement documents that must be respected by tenderers submitting variants.

WG Approval 29/05/2019

"""@en ;
  skos:prefLabel "Variant"@en ;
.
epo:hasVariantPermissions
  rdf:type owl:ObjectProperty ;
  rdfs:isDefinedBy <http://data.europa.eu/a4g/ontology> ;
  rdfs:label "Has variant permissions"@en ;
  skos:prefLabel "Has variant permissions"@en ;
.
epo:hasVariantsPermission
  rdf:type owl:ObjectProperty ;
  rdfs:comment """The obligation or possibility for tenderers to submit variants or not.

Additional Information:

Variants are alternative ways to fulfil the buyer's needs as opposed to solutions indicated in the procurement documents.

eForms: Whether tenderers are required, allowed or forbidden to submit tenders which fulfil the buyer's needs differently than as proposed in the procurement documents. 

Additional Information:

Further conditions for submitting variant tenders are in the procurement documents.
"""@en ;
  rdfs:isDefinedBy <http://data.europa.eu/a4g/ontology> ;
  rdfs:label "Variants permission"@en ;
  skos:definition """The obligation or possibility for tenderers to submit variants or not.

Additional Information:

Variants are alternative ways to fulfil the buyer's needs as opposed to solutions indicated in the procurement documents.

eForms: Whether tenderers are required, allowed or forbidden to submit tenders which fulfil the buyer's needs differently than as proposed in the procurement documents. 

Additional Information:

Further conditions for submitting variant tenders are in the procurement documents.
"""@en ;
  skos:prefLabel "Variants permission"@en ;
.
epo:hasVirtualTenderOpeningAddress
  rdf:type owl:ObjectProperty ;
  rdfs:isDefinedBy <http://data.europa.eu/a4g/ontology> ;
  rdfs:label "Has virtual tender opening address"@en ;
  skos:prefLabel "Has virtual tender opening address"@en ;
.
epo:hasWeightValue
  rdf:type owl:DatatypeProperty ;
  rdfs:comment """Relative importance assigned to a given criterion.

Additional Information: This is modeled as a Quantity because quantities have an attribute named unitCode, which allows to explain what the numeric value is about. In the case of Award Criteria this unitCode could use the Code List defined by eForms defining different types of evaluation award criteria, e.g. 
A rule should nevertheless be imposed: these Quantities should be of the form x.y, where x &lt; 0  so they can be used to represent percentages).

(WG approval 15/06/2018
reviewed on 23-01-2019)"""@en ;
  rdfs:isDefinedBy <http://data.europa.eu/a4g/ontology> ;
  rdfs:label "Weight value"@en ;
  skos:definition """Relative importance assigned to a given criterion.

Additional Information: This is modeled as a Quantity because quantities have an attribute named unitCode, which allows to explain what the numeric value is about. In the case of Award Criteria this unitCode could use the Code List defined by eForms defining different types of evaluation award criteria, e.g. 
A rule should nevertheless be imposed: these Quantities should be of the form x.y, where x &lt; 0  so they can be used to represent percentages).

(WG approval 15/06/2018
reviewed on 23-01-2019)"""@en ;
  skos:prefLabel "Weight value"@en ;
.
epo:hasWeightValueType
  rdf:type owl:ObjectProperty ;
  rdfs:comment """The method to interpret the value as a numerical coefficient expressing the relative importance of the item. 

WG Approval 17/09/2019 """@en ;
  rdfs:isDefinedBy <http://data.europa.eu/a4g/ontology> ;
  rdfs:label "Has weight value type"@en ;
  rdfs:label "Weight value type"@en ;
  skos:definition """The method to interpret the value as a numerical coefficient expressing the relative importance of the item. 

WG Approval 17/09/2019 """@en ;
  skos:prefLabel "Has weight value type"@en ;
  skos:prefLabel "Weight value type"@en ;
.
epo:hasWeightingJustification
  rdf:type owl:DatatypeProperty ;
  rdfs:comment """Explanation about why the actual weighting model is chosen. 

Additional information: 
In eNotification: This property is specifically used to describe why the order of importance is used over another weighting model.
In ESPD: This is used to explain other complex models of weighting for transparency reasons. 

WG Approval 19/09/2019 """@en ;
  rdfs:isDefinedBy <http://data.europa.eu/a4g/ontology> ;
  rdfs:label "Weighting justification"@en ;
  skos:definition """Explanation about why the actual weighting model is chosen. 

Additional information: 
In eNotification: This property is specifically used to describe why the order of importance is used over another weighting model.
In ESPD: This is used to explain other complex models of weighting for transparency reasons. 

WG Approval 19/09/2019 """@en ;
  skos:prefLabel "Weighting justification"@en ;
.
epo:hasWeigthingJustification
  rdf:type owl:DatatypeProperty ;
  rdfs:isDefinedBy <http://data.europa.eu/a4g/ontology> ;
  rdfs:label "Weigthing justification"@en ;
  skos:prefLabel "Weigthing justification"@en ;
.
epo:hasWinnerRank
  rdf:type owl:DatatypeProperty ;
  rdfs:comment """The position of the winner, i.e. whether the economic operator ended up first, second, third, etc.

Additional information: This is specially the case of design contests, some framework agreements with multiple winners (e.g. cascades) or innovation partnerships.

WG Approval 25/04/2019
"""@en ;
  rdfs:isDefinedBy <http://data.europa.eu/a4g/ontology> ;
  rdfs:label "Winner rank"@en ;
  skos:definition """The position of the winner, i.e. whether the economic operator ended up first, second, third, etc.

Additional information: This is specially the case of design contests, some framework agreements with multiple winners (e.g. cascades) or innovation partnerships.

WG Approval 25/04/2019
"""@en ;
  skos:prefLabel "Winner rank"@en ;
.
epo:hasWinning
  rdf:type owl:ObjectProperty ;
  rdfs:isDefinedBy <http://data.europa.eu/a4g/ontology> ;
  rdfs:label "Has winning"@en ;
  skos:prefLabel "Has winning"@en ;
.
epo:hasZeroEmissionVehicles
  rdf:type owl:DatatypeProperty ;
  rdfs:isDefinedBy <http://data.europa.eu/a4g/ontology> ;
  rdfs:label "Zero emission vehicles"@en ;
  skos:prefLabel "Zero emission vehicles"@en ;
.
epo:haseSubmissionPermission
  rdf:type owl:ObjectProperty ;
  rdfs:isDefinedBy <http://data.europa.eu/a4g/ontology> ;
  rdfs:label "Hase submission permission"@en ;
  skos:prefLabel "Hase submission permission"@en ;
.
epo:includes
  rdf:type owl:ObjectProperty ;
  rdfs:isDefinedBy <http://data.europa.eu/a4g/ontology> ;
  rdfs:label "Includes"@en ;
  skos:prefLabel "Includes"@en ;
.
epo:includesAccessibilityCriteria
  rdf:type owl:ObjectProperty ;
  rdfs:isDefinedBy <http://data.europa.eu/a4g/ontology> ;
  rdfs:label "Includes accessibility criteria"@en ;
  skos:prefLabel "Includes accessibility criteria"@en ;
.
epo:involvesOverallStrategicProcurement
  rdf:type owl:ObjectProperty ;
  rdfs:isDefinedBy <http://data.europa.eu/a4g/ontology> ;
  rdfs:label "Involves overall strategic procurement"@en ;
  skos:prefLabel "Involves overall strategic procurement"@en ;
.
epo:isAbout
  rdf:type owl:ObjectProperty ;
  rdfs:isDefinedBy <http://data.europa.eu/a4g/ontology> ;
  rdfs:label "Is about"@en ;
  skos:prefLabel "Is about"@en ;
.
epo:isApplicableToSecurityClearanceAddress
  rdf:type owl:ObjectProperty ;
  rdfs:isDefinedBy <http://data.europa.eu/a4g/ontology> ;
  rdfs:label "Is applicable to security clearance address"@en ;
  skos:prefLabel "Is applicable to security clearance address"@en ;
.
epo:isAppliedTo
  rdf:type owl:ObjectProperty ;
  rdfs:isDefinedBy <http://data.europa.eu/a4g/ontology> ;
  rdfs:label "Is applied to"@en ;
  skos:prefLabel "Is applied to"@en ;
.
epo:isAssessedIn
  rdf:type owl:ObjectProperty ;
  rdfs:isDefinedBy <http://data.europa.eu/a4g/ontology> ;
  rdfs:label "Is assessed in"@en ;
  skos:prefLabel "Is assessed in"@en ;
.
epo:isAssignedForEvaluationOf
  rdf:type owl:ObjectProperty ;
  rdfs:isDefinedBy <http://data.europa.eu/a4g/ontology> ;
  rdfs:label "Is assigned for evaluation of"@en ;
  skos:prefLabel "Is assigned for evaluation of"@en ;
.
epo:isAttachedIn
  rdf:type owl:ObjectProperty ;
  rdfs:isDefinedBy <http://data.europa.eu/a4g/ontology> ;
  rdfs:label "Is attached in"@en ;
  skos:prefLabel "Is attached in"@en ;
.
epo:isAvailableVia
  rdf:type owl:ObjectProperty ;
  rdfs:isDefinedBy <http://data.europa.eu/a4g/ontology> ;
  rdfs:label "Is available via"@en ;
  skos:prefLabel "Is available via"@en ;
.
epo:isAwardedTo
  rdf:type owl:ObjectProperty ;
  rdfs:isDefinedBy <http://data.europa.eu/a4g/ontology> ;
  rdfs:label "Is awarded to"@en ;
  skos:prefLabel "Is awarded to"@en ;
.
epo:isBasedOn
  rdf:type owl:ObjectProperty ;
  rdfs:isDefinedBy <http://data.europa.eu/a4g/ontology> ;
  rdfs:label "Is based on"@en ;
  skos:prefLabel "Is based on"@en ;
.
epo:isBeneficialOwnerOf
  rdf:type owl:ObjectProperty ;
  rdfs:comment """Any natural person(s) who ultimately owns or controls the organisation and/or the natural person(s) on whose behalf a transaction or activity is being conducted.

"""@en ;
  rdfs:isDefinedBy <http://data.europa.eu/a4g/ontology> ;
  rdfs:label "Is beneficial owner of"@en ;
  skos:definition """Any natural person(s) who ultimately owns or controls the organisation and/or the natural person(s) on whose behalf a transaction or activity is being conducted.

"""@en ;
  skos:prefLabel "Is beneficial owner of"@en ;
.
epo:isComposedOf
  rdf:type owl:ObjectProperty ;
  rdfs:isDefinedBy <http://data.europa.eu/a4g/ontology> ;
  rdfs:label "Is composed of"@en ;
  skos:prefLabel "Is composed of"@en ;
.
epo:isConcludedBy
  rdf:type owl:ObjectProperty ;
  rdfs:isDefinedBy <http://data.europa.eu/a4g/ontology> ;
  rdfs:label "Is concluded by"@en ;
  skos:prefLabel "Is concluded by"@en ;
.
epo:isCreatedBy
  rdf:type owl:ObjectProperty ;
  rdfs:isDefinedBy <http://data.europa.eu/a4g/ontology> ;
  rdfs:label "Is created by"@en ;
  skos:prefLabel "Is created by"@en ;
.
epo:isExecutedBy
  rdf:type owl:ObjectProperty ;
  rdfs:isDefinedBy <http://data.europa.eu/a4g/ontology> ;
  rdfs:label "Is executed by"@en ;
  skos:prefLabel "Is executed by"@en ;
.
epo:isForeseenInProjectProcurement
  rdf:type owl:ObjectProperty ;
  rdfs:isDefinedBy <http://data.europa.eu/a4g/ontology> ;
  rdfs:label "Is foreseen in project procurement"@en ;
  skos:prefLabel "Is foreseen in project procurement"@en ;
.
epo:isFundedBy
  rdf:type owl:ObjectProperty ;
  rdfs:comment """Funds may change between the lot and the contract, for example in the case of an emergency crisis, a contract may be financed by a budget that was not foreseen in the call.
"""@en ;
  rdfs:comment "Funds may change between the lot and the contract, for example in the case of an emergency crisis, a contract may be financed by a budget that was not foreseen in the call."@en ;
  rdfs:isDefinedBy <http://data.europa.eu/a4g/ontology> ;
  rdfs:label "Is funded by"@en ;
  skos:definition """Funds may change between the lot and the contract, for example in the case of an emergency crisis, a contract may be financed by a budget that was not foreseen in the call.
"""@en ;
  skos:definition "Funds may change between the lot and the contract, for example in the case of an emergency crisis, a contract may be financed by a budget that was not foreseen in the call."@en ;
  skos:prefLabel "Is funded by"@en ;
.
epo:isFundedWith
  rdf:type owl:ObjectProperty ;
  rdfs:isDefinedBy <http://data.europa.eu/a4g/ontology> ;
  rdfs:label "Is funded with"@en ;
  skos:prefLabel "Is funded with"@en ;
.
epo:isGroupedIn
  rdf:type owl:ObjectProperty ;
  rdfs:isDefinedBy <http://data.europa.eu/a4g/ontology> ;
  rdfs:label "Is grouped in"@en ;
  skos:prefLabel "Is grouped in"@en ;
.
epo:isIncludedIn
  rdf:type owl:ObjectProperty ;
  rdfs:isDefinedBy <http://data.europa.eu/a4g/ontology> ;
  rdfs:label "Is included in"@en ;
  skos:prefLabel "Is included in"@en ;
.
epo:isMadeAvailableUnder
  rdf:type owl:ObjectProperty ;
  rdfs:isDefinedBy <http://data.europa.eu/a4g/ontology> ;
  rdfs:label "Is made available under"@en ;
  skos:prefLabel "Is made available under"@en ;
.
epo:isMadeAvailableVia
  rdf:type owl:ObjectProperty ;
  rdfs:isDefinedBy <http://data.europa.eu/a4g/ontology> ;
  rdfs:label "Is made available via"@en ;
  skos:prefLabel "Is made available via"@en ;
.
epo:isNotifiedIn
  rdf:type owl:ObjectProperty ;
  rdfs:isDefinedBy <http://data.europa.eu/a4g/ontology> ;
  rdfs:label "Is notified in"@en ;
  skos:prefLabel "Is notified in"@en ;
.
epo:isNotifiedThrough
  rdf:type owl:ObjectProperty ;
  rdfs:comment "[only CN or PIN]"@en ;
  rdfs:isDefinedBy <http://data.europa.eu/a4g/ontology> ;
  rdfs:label "Is notified through"@en ;
  skos:prefLabel "Is notified through"@en ;
  skos:scopeNote "[only CN or PIN]"@en ;
.
epo:isOrganisedIn
  rdf:type owl:ObjectProperty ;
  rdfs:comment """

Additional Information
This property allows to obtain the estimated value of both a group of lots used in a Framework Agreement and the estimated value of each individual lot; which helps to compare the difference between the estimated value of the group against the addition of each lot estimated value.

"""@en ;
  rdfs:isDefinedBy <http://data.europa.eu/a4g/ontology> ;
  rdfs:label "Is organised in"@en ;
  skos:definition """

Additional Information
This property allows to obtain the estimated value of both a group of lots used in a Framework Agreement and the estimated value of each individual lot; which helps to compare the difference between the estimated value of the group against the addition of each lot estimated value.

"""@en ;
  skos:prefLabel "Is organised in"@en ;
.
epo:isOwnBy
  rdf:type owl:ObjectProperty ;
  rdfs:isDefinedBy <http://data.europa.eu/a4g/ontology> ;
  rdfs:label "Is own by"@en ;
  skos:prefLabel "Is own by"@en ;
.
epo:isPersonOfContact
  rdf:type owl:ObjectProperty ;
  rdfs:isDefinedBy <http://data.europa.eu/a4g/ontology> ;
  rdfs:label "Is person of contact"@en ;
  skos:prefLabel "Is person of contact"@en ;
.
epo:isPlannedBy
  rdf:type owl:ObjectProperty ;
  rdfs:isDefinedBy <http://data.europa.eu/a4g/ontology> ;
  rdfs:label "Is planned by"@en ;
  skos:prefLabel "Is planned by"@en ;
.
epo:isQualifiedBy
  rdf:type owl:ObjectProperty ;
  rdfs:isDefinedBy <http://data.europa.eu/a4g/ontology> ;
  rdfs:label "Is qualified by"@en ;
  skos:prefLabel "Is qualified by"@en ;
.
epo:isReferedByA
  rdf:type owl:ObjectProperty ;
  rdfs:isDefinedBy <http://data.europa.eu/a4g/ontology> ;
  rdfs:label "Is refered by a"@en ;
  skos:prefLabel "Is refered by a"@en ;
.
epo:isReferredToBy
  rdf:type owl:ObjectProperty ;
  rdfs:isDefinedBy <http://data.europa.eu/a4g/ontology> ;
  rdfs:label "Is referred to by"@en ;
  skos:prefLabel "Is referred to by"@en ;
.
epo:isReferredToIn
  rdf:type owl:ObjectProperty ;
  rdfs:comment """The Contracting Authority uses this property to precise the Lots for which a concrete requirement (expressed as Procurement Criterion Property) is applicable to.

WG Approval 05/09/2019 """@en ;
  rdfs:isDefinedBy <http://data.europa.eu/a4g/ontology> ;
  rdfs:label "Is referred to in"@en ;
  skos:definition """The Contracting Authority uses this property to precise the Lots for which a concrete requirement (expressed as Procurement Criterion Property) is applicable to.

WG Approval 05/09/2019 """@en ;
  skos:prefLabel "Is referred to in"@en ;
.
epo:isRelatedTo
  rdf:type owl:ObjectProperty ;
  rdfs:isDefinedBy <http://data.europa.eu/a4g/ontology> ;
  rdfs:label "Is related to"@en ;
  skos:prefLabel "Is related to"@en ;
.
epo:isResponsibleFor
  rdf:type owl:ObjectProperty ;
  rdfs:isDefinedBy <http://data.europa.eu/a4g/ontology> ;
  rdfs:label "Is responsible for"@en ;
  skos:prefLabel "Is responsible for"@en ;
.
epo:isResponsiblityOf
  rdf:type owl:ObjectProperty ;
  rdfs:isDefinedBy <http://data.europa.eu/a4g/ontology> ;
  rdfs:label "Is responsiblity of"@en ;
  skos:prefLabel "Is responsiblity of"@en ;
.
epo:isRoleOf
  rdf:type owl:ObjectProperty ;
  rdfs:comment """
"""@en ;
  rdfs:isDefinedBy <http://data.europa.eu/a4g/ontology> ;
  rdfs:label "Is role of"@en ;
  skos:definition """
"""@en ;
  skos:prefLabel "Is role of"@en ;
.
epo:isRoleOfBusiness
  rdf:type owl:ObjectProperty ;
  rdfs:isDefinedBy <http://data.europa.eu/a4g/ontology> ;
  rdfs:label "Is role of business"@en ;
  skos:prefLabel "Is role of business"@en ;
.
epo:isSignatoryPartyOf
  rdf:type owl:ObjectProperty ;
  rdfs:isDefinedBy <http://data.europa.eu/a4g/ontology> ;
  rdfs:label "Is signatory party of"@en ;
  skos:prefLabel "Is signatory party of"@en ;
.
epo:isSignedBy
  rdf:type owl:ObjectProperty ;
  rdfs:isDefinedBy <http://data.europa.eu/a4g/ontology> ;
  rdfs:label "Is signed by"@en ;
  skos:prefLabel "Is signed by"@en ;
.
epo:isSpecifiedIn
  rdf:type owl:ObjectProperty ;
  rdfs:isDefinedBy <http://data.europa.eu/a4g/ontology> ;
  rdfs:label "Is specified in"@en ;
  skos:prefLabel "Is specified in"@en ;
.
epo:isSubmittedBy
  rdf:type owl:ObjectProperty ;
  rdfs:comment """The transmitter of documents. 

Additional Information

An example of transmitters are TeD eSenders, which are usually either the Buyer or a Service Provider acting on behalf of the Buyer, qualified by the Publication Office of the European Union.

"""@en ;
  rdfs:isDefinedBy <http://data.europa.eu/a4g/ontology> ;
  rdfs:label "Is submitted by"@en ;
  skos:definition """The transmitter of documents. 

Additional Information

An example of transmitters are TeD eSenders, which are usually either the Buyer or a Service Provider acting on behalf of the Buyer, qualified by the Publication Office of the European Union.

"""@en ;
  skos:prefLabel "Is submitted by"@en ;
.
epo:isToBeProvidedWithin
  rdf:type owl:ObjectProperty ;
  rdfs:isDefinedBy <http://data.europa.eu/a4g/ontology> ;
  rdfs:label "Is to be provided within"@en ;
  skos:prefLabel "Is to be provided within"@en ;
.
epo:isUsedIn
  rdf:type owl:ObjectProperty ;
  rdfs:isDefinedBy <http://data.europa.eu/a4g/ontology> ;
  rdfs:label "Is used in"@en ;
  skos:prefLabel "Is used in"@en ;
.
epo:isUsedToAward
  rdf:type owl:ObjectProperty ;
  rdfs:isDefinedBy <http://data.europa.eu/a4g/ontology> ;
  rdfs:label "Is used to award"@en ;
  skos:prefLabel "Is used to award"@en ;
.
epo:issues
  rdf:type owl:ObjectProperty ;
  rdfs:isDefinedBy <http://data.europa.eu/a4g/ontology> ;
  rdfs:label "Issues"@en ;
  skos:prefLabel "Issues"@en ;
.
epo:leadsTo
  rdf:type owl:ObjectProperty ;
  rdfs:isDefinedBy <http://data.europa.eu/a4g/ontology> ;
  rdfs:label "Leads to"@en ;
  skos:prefLabel "Leads to"@en ;
.
epo:makesDecsion
  rdf:type owl:ObjectProperty ;
  rdfs:comment "This decision may be made based on the evaluation results issued by the evaluation board."@en ;
  rdfs:isDefinedBy <http://data.europa.eu/a4g/ontology> ;
  rdfs:label "Makes decsion"@en ;
  skos:prefLabel "Makes decsion"@en ;
  skos:scopeNote "This decision may be made based on the evaluation results issued by the evaluation board."@en ;
.
epo:manages
  rdf:type owl:ObjectProperty ;
  rdfs:isDefinedBy <http://data.europa.eu/a4g/ontology> ;
  rdfs:label "Manages"@en ;
  skos:prefLabel "Manages"@en ;
.
epo:modifies
  rdf:type owl:ObjectProperty ;
  rdfs:isDefinedBy <http://data.europa.eu/a4g/ontology> ;
  rdfs:label "Modifies"@en ;
  skos:prefLabel "Modifies"@en ;
.
epo:notifies
  rdf:type owl:ObjectProperty ;
  rdfs:isDefinedBy <http://data.europa.eu/a4g/ontology> ;
  rdfs:label "Notifies"@en ;
  skos:prefLabel "Notifies"@en ;
.
epo:notifiesAwardResult
  rdf:type owl:ObjectProperty ;
  rdfs:isDefinedBy <http://data.europa.eu/a4g/ontology> ;
  rdfs:label "Notifies award result"@en ;
  skos:prefLabel "Notifies award result"@en ;
.
epo:owns
  rdf:type owl:ObjectProperty ;
  rdfs:isDefinedBy <http://data.europa.eu/a4g/ontology> ;
  rdfs:label "Owns"@en ;
  skos:prefLabel "Owns"@en ;
.
epo:performsEvaluation
  rdf:type owl:ObjectProperty ;
  rdfs:isDefinedBy <http://data.europa.eu/a4g/ontology> ;
  rdfs:label "Performs evaluation"@en ;
  skos:prefLabel "Performs evaluation"@en ;
.
epo:plans
  rdf:type owl:ObjectProperty ;
  rdfs:isDefinedBy <http://data.europa.eu/a4g/ontology> ;
  rdfs:label "Plans"@en ;
  skos:prefLabel "Plans"@en ;
.
epo:playsRole
  rdf:type owl:ObjectProperty ;
  rdfs:comment """
"""@en ;
  rdfs:isDefinedBy <http://data.europa.eu/a4g/ontology> ;
  rdfs:label "Plays role"@en ;
  skos:definition """
"""@en ;
  skos:prefLabel "Plays role"@en ;
.
epo:preceeds
  rdf:type owl:ObjectProperty ;
  rdfs:isDefinedBy <http://data.europa.eu/a4g/ontology> ;
  rdfs:label "Preceeds"@en ;
  skos:prefLabel "Preceeds"@en ;
.
epo:proposes
  rdf:type owl:ObjectProperty ;
  rdfs:comment """The 0 cardinality of this relation between Evaluation Result and Candidate Short List caters for cases such as Dynamic Purchasing Systems (DPS) and reopening of competition (in Framework Agreements) where the Candidate Short List is generated based on the selected candidates (DPS) and from the winners of a Framework Agreement. 

In those cases there is no need for the candidates to go through a new selection process."""@en ;
  rdfs:isDefinedBy <http://data.europa.eu/a4g/ontology> ;
  rdfs:label "Proposes"@en ;
  skos:definition """The 0 cardinality of this relation between Evaluation Result and Candidate Short List caters for cases such as Dynamic Purchasing Systems (DPS) and reopening of competition (in Framework Agreements) where the Candidate Short List is generated based on the selected candidates (DPS) and from the winners of a Framework Agreement. 

In those cases there is no need for the candidates to go through a new selection process."""@en ;
  skos:prefLabel "Proposes"@en ;
.
epo:proposesSubcontractor
  rdf:type owl:ObjectProperty ;
  rdfs:isDefinedBy <http://data.europa.eu/a4g/ontology> ;
  rdfs:label "Proposes subcontractor"@en ;
  skos:prefLabel "Proposes subcontractor"@en ;
.
epo:providesAdditionalInformation
  rdf:type owl:ObjectProperty ;
  rdfs:isDefinedBy <http://data.europa.eu/a4g/ontology> ;
  rdfs:label "Provides additional information"@en ;
  skos:prefLabel "Provides additional information"@en ;
.
epo:providesInformationFor
  rdf:type owl:ObjectProperty ;
  rdfs:isDefinedBy <http://data.europa.eu/a4g/ontology> ;
  rdfs:label "Provides information for"@en ;
  skos:prefLabel "Provides information for"@en ;
.
epo:qualificationCriteria
  rdf:type owl:ObjectProperty ;
  rdfs:isDefinedBy <http://data.europa.eu/a4g/ontology> ;
  rdfs:label "Qualification criteria"@en ;
  skos:prefLabel "Qualification criteria"@en ;
.
epo:ranks
  rdf:type owl:ObjectProperty ;
  rdfs:isDefinedBy <http://data.europa.eu/a4g/ontology> ;
  rdfs:label "Ranks"@en ;
  skos:prefLabel "Ranks"@en ;
.
epo:ranksTenders
  rdf:type owl:ObjectProperty ;
  rdfs:comment "Procurement procedures may need to rank the evaluated tenders."@en ;
  rdfs:isDefinedBy <http://data.europa.eu/a4g/ontology> ;
  rdfs:label "Ranks tenders"@en ;
  skos:definition "Procurement procedures may need to rank the evaluated tenders."@en ;
  skos:prefLabel "Ranks tenders"@en ;
.
epo:refersTo
  rdf:type owl:ObjectProperty ;
  rdfs:isDefinedBy <http://data.europa.eu/a4g/ontology> ;
  rdfs:label "Refers to"@en ;
  skos:prefLabel "Refers to"@en ;
.
epo:refersToADifferent
  rdf:type owl:ObjectProperty ;
  rdfs:isDefinedBy <http://data.europa.eu/a4g/ontology> ;
  rdfs:label "Refers to a different"@en ;
  skos:prefLabel "Refers to a different"@en ;
.
epo:refersToAwardResult
  rdf:type owl:ObjectProperty ;
  rdfs:isDefinedBy <http://data.europa.eu/a4g/ontology> ;
  rdfs:label "Refers to award result"@en ;
  skos:prefLabel "Refers to award result"@en ;
.
epo:refersToPrevious
  rdf:type owl:ObjectProperty ;
  rdfs:isDefinedBy <http://data.europa.eu/a4g/ontology> ;
  rdfs:label "Refers to previous"@en ;
  skos:prefLabel "Refers to previous"@en ;
.
epo:refersToPreviousProcedureLots
  rdf:type owl:ObjectProperty ;
  rdfs:comment """Reference to one or more Lots in a previous procedure.

Additional Information:
In the case of Direct Award Terms, this property points to a previous Procedure justifying the use of Direct Award without a prior publication.

WG Approval 22/11/2019 14:33:55"""@en ;
  rdfs:isDefinedBy <http://data.europa.eu/a4g/ontology> ;
  rdfs:label "Refers to previous procedure lots"@en ;
  skos:definition """Reference to one or more Lots in a previous procedure.

Additional Information:
In the case of Direct Award Terms, this property points to a previous Procedure justifying the use of Direct Award without a prior publication.

WG Approval 22/11/2019 14:33:55"""@en ;
  skos:prefLabel "Refers to previous procedure lots"@en ;
.
epo:refersToSignatory
  rdf:type owl:ObjectProperty ;
  rdfs:isDefinedBy <http://data.europa.eu/a4g/ontology> ;
  rdfs:label "Refers to signatory"@en ;
  skos:prefLabel "Refers to signatory"@en ;
.
epo:relatesTo
  rdf:type owl:ObjectProperty ;
  rdfs:comment """Associated to. 

Additional information: 

In the case of a Planning form this subproperty notifies is used. 

In the case of Competition form this subproperty announces is used. 

In the case of Result form this subproperty summarises is used. """@en ;
  rdfs:isDefinedBy <http://data.europa.eu/a4g/ontology> ;
  rdfs:label "Relates to"@en ;
  skos:definition """Associated to. 

Additional information: 

In the case of a Planning form this subproperty notifies is used. 

In the case of Competition form this subproperty announces is used. 

In the case of Result form this subproperty summarises is used. """@en ;
  skos:prefLabel "Relates to"@en ;
.
epo:requires
  rdf:type owl:ObjectProperty ;
  rdfs:isDefinedBy <http://data.europa.eu/a4g/ontology> ;
  rdfs:label "Requires"@en ;
  skos:prefLabel "Requires"@en ;
.
epo:restrictedCommunicationJustification
  rdf:type owl:ObjectProperty ;
  rdfs:isDefinedBy <http://data.europa.eu/a4g/ontology> ;
  rdfs:label "Restricted communication justification"@en ;
  skos:prefLabel "Restricted communication justification"@en ;
.
epo:rewardedWith
  rdf:type owl:ObjectProperty ;
  rdfs:isDefinedBy <http://data.europa.eu/a4g/ontology> ;
  rdfs:label "Rewarded with"@en ;
  skos:prefLabel "Rewarded with"@en ;
.
epo:setsRulesOf
  rdf:type owl:ObjectProperty ;
  rdfs:isDefinedBy <http://data.europa.eu/a4g/ontology> ;
  rdfs:label "Sets rules of"@en ;
  skos:prefLabel "Sets rules of"@en ;
.
epo:specifies
  rdf:type owl:ObjectProperty ;
  rdfs:isDefinedBy <http://data.europa.eu/a4g/ontology> ;
  rdfs:label "Specifies"@en ;
  skos:prefLabel "Specifies"@en ;
.
epo:specifiesSubcontractors
  rdf:type owl:ObjectProperty ;
  rdfs:isDefinedBy <http://data.europa.eu/a4g/ontology> ;
  rdfs:label "Specifies subcontractors"@en ;
  skos:prefLabel "Specifies subcontractors"@en ;
.
epo:submits
  rdf:type owl:ObjectProperty ;
  rdfs:isDefinedBy <http://data.europa.eu/a4g/ontology> ;
  rdfs:label "Submits"@en ;
  skos:prefLabel "Submits"@en ;
.
epo:submitsDocument
  rdf:type owl:ObjectProperty ;
  rdfs:comment """The transmitter of documents. 

Additional Information

An example of transmitters are TeD eSenders, which are usually either the Buyer or a Service Provider acting on behalf of the Buyer, qualified by the Publication Office of the European Union.

"""@en ;
  rdfs:isDefinedBy <http://data.europa.eu/a4g/ontology> ;
  rdfs:label "Submits document"@en ;
  skos:definition """The transmitter of documents. 

Additional Information

An example of transmitters are TeD eSenders, which are usually either the Buyer or a Service Provider acting on behalf of the Buyer, qualified by the Publication Office of the European Union.

"""@en ;
  skos:prefLabel "Submits document"@en ;
.
epo:substantiates
  rdf:type owl:ObjectProperty ;
  rdfs:isDefinedBy <http://data.europa.eu/a4g/ontology> ;
  rdfs:label "Substantiates"@en ;
  skos:prefLabel "Substantiates"@en ;
.
epo:toBeEvaluatedBy
  rdf:type owl:ObjectProperty ;
  rdfs:isDefinedBy <http://data.europa.eu/a4g/ontology> ;
  rdfs:label "To be evaluated by"@en ;
  skos:prefLabel "To be evaluated by"@en ;
.
epo:unknown
  rdf:type skos:Concept ;
  rdfs:isDefinedBy <http://data.europa.eu/a4g/ontology> ;
  rdfs:label "Unknown"@en ;
  skos:inScheme <http://publications.europa.eu/resource/authority/Cpv> ;
  skos:prefLabel "Unknown"@en ;
.
epo:usedForReductionOfCandidates
  rdf:type owl:ObjectProperty ;
  rdfs:isDefinedBy <http://data.europa.eu/a4g/ontology> ;
  rdfs:label "Used for reduction of candidates"@en ;
  skos:prefLabel "Used for reduction of candidates"@en ;
.
epo:uses
  rdf:type owl:ObjectProperty ;
  rdfs:comment """

Additional Information
This property allows to obtain the estimated value of both a group of lots used in a Framework Agreement and the estimated value of each individual lot; which helps to compare the difference between the estimated value of the group against the addition of each lot estimated value.

"""@en ;
  rdfs:isDefinedBy <http://data.europa.eu/a4g/ontology> ;
  rdfs:label "Uses"@en ;
  skos:definition """

Additional Information
This property allows to obtain the estimated value of both a group of lots used in a Framework Agreement and the estimated value of each individual lot; which helps to compare the difference between the estimated value of the group against the addition of each lot estimated value.

"""@en ;
  skos:prefLabel "Uses"@en ;
.
epo:usesAdhoc
  rdf:type owl:ObjectProperty ;
  rdfs:isDefinedBy <http://data.europa.eu/a4g/ontology> ;
  rdfs:label "Uses adhoc"@en ;
  skos:prefLabel "Uses adhoc"@en ;
.
epo:withdraws
  rdf:type owl:ObjectProperty ;
  rdfs:isDefinedBy <http://data.europa.eu/a4g/ontology> ;
  rdfs:label "Withdraws"@en ;
  skos:prefLabel "Withdraws"@en ;
.
<http://data.europa.eu/m8g/Criterion>
  rdf:type owl:Class ;
  rdfs:comment """A condition that needs to be answered for evaluation purposes.

Additional Information: this can be used for transparency and evaluation of  PRICE CRITERIA
(list of criteria related to price) Selection and Award Criterion that are weighted.

(WG approval 22/06/2018)"""@en ;
  rdfs:isDefinedBy <http://data.europa.eu/a4g/ontology> ;
  rdfs:label "Criterion"@en ;
  skos:definition """A condition that needs to be answered for evaluation purposes.

Additional Information: this can be used for transparency and evaluation of  PRICE CRITERIA
(list of criteria related to price) Selection and Award Criterion that are weighted.

(WG approval 22/06/2018)"""@en ;
  skos:prefLabel "Criterion"@en ;
.
<http://data.europa.eu/m8g/Criterion-group-property-type>
  rdf:type skos:ConceptScheme ;
  rdfs:comment "A code categorising the data structure category, how to use or process it, etc."@en ;
  rdfs:isDefinedBy <http://data.europa.eu/a4g/ontology> ;
  rdfs:label "Criterion-group-property-type"@en ;
  skos:definition "A code categorising the data structure category, how to use or process it, etc."@en ;
  skos:prefLabel "Criterion-group-property-type" ;
.
<http://data.europa.eu/m8g/CriterionPropertyGroup>
  rdf:type owl:Class ;
  rdfs:comment """An organised structure of related criterion properties.

(WG approval 22/06/2018)"""@en ;
  rdfs:isDefinedBy <http://data.europa.eu/a4g/ontology> ;
  rdfs:label "Criterion property group"@en ;
  skos:definition """An organised structure of related criterion properties.

(WG approval 22/06/2018)"""@en ;
  skos:prefLabel "Criterion property group"@en ;
.
<http://data.europa.eu/m8g/DatumValue>
  rdf:type owl:Class ;
  rdfs:comment """The value  provided for a criterion property.

(WG approval 22/06/2018)
"""@en ;
  rdfs:isDefinedBy <http://data.europa.eu/a4g/ontology> ;
  rdfs:label "Datum value"@en ;
  skos:definition """The value  provided for a criterion property.

(WG approval 22/06/2018)
"""@en ;
  skos:prefLabel "Datum value"@en ;
.
<http://data.europa.eu/m8g/Evidence>
  rdf:type owl:Class ;
  rdfs:comment """Something which proves that something else exists or is true, in particular an evidence is used to prove that a specific criterion is met by someone of by something.

To be checked"""@en ;
  rdfs:isDefinedBy <http://data.europa.eu/a4g/ontology> ;
  rdfs:label "Evidence"@en ;
  skos:definition """Something which proves that something else exists or is true, in particular an evidence is used to prove that a specific criterion is met by someone of by something.

To be checked"""@en ;
  skos:prefLabel "Evidence"@en ;
.
<http://data.europa.eu/m8g/Property>
  rdf:type owl:Class ;
  rdfs:comment """Specific information needed to measure a criterion.

(WG approval 22/06/2018)"""@en ;
  rdfs:isDefinedBy <http://data.europa.eu/a4g/ontology> ;
  rdfs:label "Property"@en ;
  skos:definition """Specific information needed to measure a criterion.

(WG approval 22/06/2018)"""@en ;
  skos:prefLabel "Property"@en ;
.
<http://data.europa.eu/m8g/asksForData>
  rdf:type owl:ObjectProperty ;
  rdfs:isDefinedBy <http://data.europa.eu/a4g/ontology> ;
  rdfs:label "Asks for data"@en ;
  skos:prefLabel "Asks for data"@en ;
.
<http://data.europa.eu/m8g/basesOnEvidence>
  rdf:type owl:ObjectProperty ;
  rdfs:isDefinedBy <http://data.europa.eu/a4g/ontology> ;
  rdfs:label "Bases on evidence"@en ;
  skos:prefLabel "Bases on evidence"@en ;
.
<http://data.europa.eu/m8g/delegatesAncillaryActivitiesOn>
  rdf:type owl:ObjectProperty ;
  rdfs:isDefinedBy <http://data.europa.eu/a4g/ontology> ;
  rdfs:label "Delegates ancillary activities on"@en ;
  skos:prefLabel "Delegates ancillary activities on"@en ;
.
<http://data.europa.eu/m8g/expressesRequirement>
  rdf:type owl:ObjectProperty ;
  rdfs:isDefinedBy <http://data.europa.eu/a4g/ontology> ;
  rdfs:label "Expresses requirement"@en ;
  skos:prefLabel "Expresses requirement"@en ;
.
<http://data.europa.eu/m8g/has>
  rdf:type owl:ObjectProperty ;
  rdfs:isDefinedBy <http://data.europa.eu/a4g/ontology> ;
  rdfs:label "Has"@en ;
  skos:prefLabel "Has"@en ;
.
<http://data.europa.eu/m8g/hasAmount>
  rdf:type owl:ObjectProperty ;
  rdfs:isDefinedBy <http://data.europa.eu/a4g/ontology> ;
  rdfs:label "Amount"@en ;
  skos:prefLabel "Amount"@en ;
.
<http://data.europa.eu/m8g/hasCode>
  rdf:type owl:ObjectProperty ;
  rdfs:isDefinedBy <http://data.europa.eu/a4g/ontology> ;
  rdfs:label "Code"@en ;
  skos:prefLabel "Code"@en ;
.
<http://data.europa.eu/m8g/hasConfidentialityLevelType>
  rdf:type owl:ObjectProperty ;
  rdfs:isDefinedBy <http://data.europa.eu/a4g/ontology> ;
  rdfs:label "Confidentiality level type"@en ;
  rdfs:label "Has confidentiality level type"@en ;
  skos:prefLabel "Confidentiality level type"@en ;
  skos:prefLabel "Has confidentiality level type"@en ;
.
<http://data.europa.eu/m8g/hasConstraint>
  rdf:type owl:ObjectProperty ;
  rdfs:isDefinedBy <http://data.europa.eu/a4g/ontology> ;
  rdfs:label "Has constraint"@en ;
  skos:prefLabel "Has constraint"@en ;
.
<http://data.europa.eu/m8g/hasCriterionGroupPropertyType>
  rdf:type owl:ObjectProperty ;
  rdfs:isDefinedBy <http://data.europa.eu/a4g/ontology> ;
  rdfs:label "Criterion group property type"@en ;
  rdfs:label "Has criterion group property type"@en ;
  skos:prefLabel "Criterion group property type"@en ;
  skos:prefLabel "Has criterion group property type"@en ;
.
<http://data.europa.eu/m8g/hasCriterionProperty>
  rdf:type owl:ObjectProperty ;
  rdfs:isDefinedBy <http://data.europa.eu/a4g/ontology> ;
  rdfs:label "Has criterion property"@en ;
  skos:prefLabel "Has criterion property"@en ;
.
<http://data.europa.eu/m8g/hasDate>
  rdf:type owl:DatatypeProperty ;
  rdfs:isDefinedBy <http://data.europa.eu/a4g/ontology> ;
  rdfs:label "Date"@en ;
  skos:prefLabel "Date"@en ;
.
<http://data.europa.eu/m8g/hasDescription>
  rdf:type owl:DatatypeProperty ;
  rdfs:comment "A narrative description describing the content of the group of properties inside a criterion."@en ;
  rdfs:comment """Self-explanatory text about a concept.
"""@en ;
  rdfs:isDefinedBy <http://data.europa.eu/a4g/ontology> ;
  rdfs:label "Description"@en ;
  skos:definition "A narrative description describing the content of the group of properties inside a criterion."@en ;
  skos:definition """Self-explanatory text about a concept.
"""@en ;
  skos:prefLabel "Description"@en ;
.
<http://data.europa.eu/m8g/hasID>
  rdf:type owl:ObjectProperty ;
  rdfs:isDefinedBy <http://data.europa.eu/a4g/ontology> ;
  rdfs:label "I d"@en ;
  skos:prefLabel "I d"@en ;
.
<http://data.europa.eu/m8g/hasIdentifier>
  rdf:type owl:ObjectProperty ;
  rdfs:comment "Identifies unambiguously and uniquely a particular structure of data inside the group and across all procurement procedures."@en ;
  rdfs:comment "Identifies unambiguously and uniquely a particular structure of data inside the group."@en ;
  rdfs:isDefinedBy <http://data.europa.eu/a4g/ontology> ;
  rdfs:label "Identifier"@en ;
  skos:definition "Identifies unambiguously and uniquely a particular structure of data inside the group and across all procurement procedures."@en ;
  skos:definition "Identifies unambiguously and uniquely a particular structure of data inside the group."@en ;
  skos:prefLabel "Identifier"@en ;
.
<http://data.europa.eu/m8g/hasIndicator>
  rdf:type rdf:Property ;
  rdfs:isDefinedBy <http://data.europa.eu/a4g/ontology> ;
  rdfs:label "Indicator"@en ;
  skos:prefLabel "Indicator"@en ;
.
<http://data.europa.eu/m8g/hasInformationRequirement>
  rdf:type owl:ObjectProperty ;
  rdfs:isDefinedBy <http://data.europa.eu/a4g/ontology> ;
  rdfs:label "Has information requirement"@en ;
  skos:prefLabel "Has information requirement"@en ;
.
<http://data.europa.eu/m8g/hasName>
  rdf:type owl:DatatypeProperty ;
  rdfs:comment "A short text representing the group of properties inside a criterion."@en ;
  rdfs:isDefinedBy <http://data.europa.eu/a4g/ontology> ;
  rdfs:label "Name"@en ;
  skos:definition "A short text representing the group of properties inside a criterion."@en ;
  skos:prefLabel "Name"@en ;
.
<http://data.europa.eu/m8g/hasPropertySubgroup>
  rdf:type owl:ObjectProperty ;
  rdfs:isDefinedBy <http://data.europa.eu/a4g/ontology> ;
  rdfs:label "Has property subgroup"@en ;
  skos:prefLabel "Has property subgroup"@en ;
.
<http://data.europa.eu/m8g/hasQuantity>
  rdf:type owl:ObjectProperty ;
  rdfs:isDefinedBy <http://data.europa.eu/a4g/ontology> ;
  rdfs:label "Quantity"@en ;
  skos:prefLabel "Quantity"@en ;
.
<http://data.europa.eu/m8g/hasSub>
  rdf:type owl:ObjectProperty ;
  rdfs:isDefinedBy <http://data.europa.eu/a4g/ontology> ;
  rdfs:label "Has sub"@en ;
  skos:prefLabel "Has sub"@en ;
.
<http://data.europa.eu/m8g/hasText>
  rdf:type owl:DatatypeProperty ;
  rdfs:isDefinedBy <http://data.europa.eu/a4g/ontology> ;
  rdfs:label "Text"@en ;
  skos:prefLabel "Text"@en ;
.
<http://data.europa.eu/m8g/hasTime>
  rdf:type rdf:Property ;
  rdfs:isDefinedBy <http://data.europa.eu/a4g/ontology> ;
  rdfs:label "Time"@en ;
  skos:prefLabel "Time"@en ;
.
<http://data.europa.eu/m8g/hasURI>
  rdf:type rdf:Property ;
  rdfs:isDefinedBy <http://data.europa.eu/a4g/ontology> ;
  rdfs:label "U r i"@en ;
  skos:prefLabel "U r i"@en ;
.
<http://data.europa.eu/m8g/isPeriod>
  rdf:type owl:ObjectProperty ;
  rdfs:isDefinedBy <http://data.europa.eu/a4g/ontology> ;
  rdfs:label "Is period"@en ;
  skos:prefLabel "Is period"@en ;
.
<http://data.europa.eu/m8g/proofs>
  rdf:type owl:ObjectProperty ;
  rdfs:isDefinedBy <http://data.europa.eu/a4g/ontology> ;
  rdfs:label "Proofs"@en ;
  skos:prefLabel "Proofs"@en ;
.
<http://data.europa.eu/m8g/providesEvidence>
  rdf:type owl:ObjectProperty ;
  rdfs:isDefinedBy <http://data.europa.eu/a4g/ontology> ;
  rdfs:label "Provides evidence"@en ;
  skos:prefLabel "Provides evidence"@en ;
.
<http://data.europa.eu/m8g/refinesRequirement>
  rdf:type owl:ObjectProperty ;
  rdfs:isDefinedBy <http://data.europa.eu/a4g/ontology> ;
  rdfs:label "Refines requirement"@en ;
  skos:prefLabel "Refines requirement"@en ;
.
<http://data.europa.eu/m8g/respondsQuestion>
  rdf:type owl:ObjectProperty ;
  rdfs:isDefinedBy <http://data.europa.eu/a4g/ontology> ;
  rdfs:label "Responds question"@en ;
  skos:prefLabel "Responds question"@en ;
.
<http://publications.europa.eu/resource/authority/Accessibility>
  rdf:type skos:ConceptScheme ;
  rdfs:comment """Source: EU Vocabularies authority table \"<xref scope=\"external\" href=\"https://op.europa.eu/web/eu-vocabularies/at-dataset/-/resource/dataset/accessibility\"><foreign otherprops=\"#0000ff\"><u>Accessibility</u></foreign></xref>\" (https://op.europa.eu/web/eu-vocabularies/at-dataset/-/resource/dataset/accessibility).
"""@en ;
  rdfs:isDefinedBy <http://data.europa.eu/a4g/ontology> ;
  rdfs:label "Accessibility"@en ;
  skos:definition """Source: EU Vocabularies authority table \"<xref scope=\"external\" href=\"https://op.europa.eu/web/eu-vocabularies/at-dataset/-/resource/dataset/accessibility\"><foreign otherprops=\"#0000ff\"><u>Accessibility</u></foreign></xref>\" (https://op.europa.eu/web/eu-vocabularies/at-dataset/-/resource/dataset/accessibility).
"""@en ;
  skos:prefLabel "Accessibility" ;
.
<http://publications.europa.eu/resource/authority/Applicability>
  rdf:type skos:ConceptScheme ;
  rdfs:comment """Source: EU Vocabularies authority table \"<xref scope=\"external\" href=\"https://op.europa.eu/web/eu-vocabularies/at-dataset/-/resource/dataset/applicability\"><foreign otherprops=\"#0000ff\"><u>Applicability</u></foreign></xref>\" (https://op.europa.eu/web/eu-vocabularies/at-dataset/-/resource/dataset/applicability).

"""@en ;
  rdfs:isDefinedBy <http://data.europa.eu/a4g/ontology> ;
  rdfs:label "Applicability"@en ;
  skos:definition """Source: EU Vocabularies authority table \"<xref scope=\"external\" href=\"https://op.europa.eu/web/eu-vocabularies/at-dataset/-/resource/dataset/applicability\"><foreign otherprops=\"#0000ff\"><u>Applicability</u></foreign></xref>\" (https://op.europa.eu/web/eu-vocabularies/at-dataset/-/resource/dataset/applicability).

"""@en ;
  skos:prefLabel "Applicability" ;
.
<http://publications.europa.eu/resource/authority/Award-criterion-type>
  rdf:type skos:ConceptScheme ;
  rdfs:comment """Source: EU Vocabularies authority table \"<xref scope=\"external\" href=\"https://op.europa.eu/web/eu-vocabularies/at-dataset/-/resource/dataset/award-criterion-type\"><foreign otherprops=\"#0000ff\"><u>Award criterion type</u></foreign></xref>\" (https://op.europa.eu/web/eu-vocabularies/at-dataset/-/resource/dataset/award-criterion-type).
"""@en ;
  rdfs:isDefinedBy <http://data.europa.eu/a4g/ontology> ;
  rdfs:label "Award-criterion-type"@en ;
  skos:definition """Source: EU Vocabularies authority table \"<xref scope=\"external\" href=\"https://op.europa.eu/web/eu-vocabularies/at-dataset/-/resource/dataset/award-criterion-type\"><foreign otherprops=\"#0000ff\"><u>Award criterion type</u></foreign></xref>\" (https://op.europa.eu/web/eu-vocabularies/at-dataset/-/resource/dataset/award-criterion-type).
"""@en ;
  skos:prefLabel "Award-criterion-type" ;
.
<http://publications.europa.eu/resource/authority/Buyer-legal-type>
  rdf:type skos:ConceptScheme ;
  rdfs:comment """Source: EU Vocabularies authority table \"<xref scope=\"external\" href=\"https://op.europa.eu/web/eu-vocabularies/at-dataset/-/resource/dataset/buyer-legal-type\"><foreign otherprops=\"#0000ff\"><u>Buyer legal type</u></foreign></xref>\" (https://op.europa.eu/web/eu-vocabularies/at-dataset/-/resource/dataset/buyer-legal-type).
"""@en ;
  rdfs:isDefinedBy <http://data.europa.eu/a4g/ontology> ;
  rdfs:label "Buyer-legal-type"@en ;
  skos:definition """Source: EU Vocabularies authority table \"<xref scope=\"external\" href=\"https://op.europa.eu/web/eu-vocabularies/at-dataset/-/resource/dataset/buyer-legal-type\"><foreign otherprops=\"#0000ff\"><u>Buyer legal type</u></foreign></xref>\" (https://op.europa.eu/web/eu-vocabularies/at-dataset/-/resource/dataset/buyer-legal-type).
"""@en ;
  skos:prefLabel "Buyer-legal-type" ;
.
<http://publications.europa.eu/resource/authority/Communication-justification>
  rdf:type skos:ConceptScheme ;
  rdfs:comment """Source: EU Vocabularies authority table \"<xref scope=\"external\" href=\"https://op.europa.eu/web/eu-vocabularies/at-dataset/-/resource/dataset/communication-justification\"><foreign otherprops=\"#0000ff\"><u>Communication justification</u></foreign></xref>\" (https://op.europa.eu/web/eu-vocabularies/at-dataset/-/resource/dataset/communication-justification).
"""@en ;
  rdfs:isDefinedBy <http://data.europa.eu/a4g/ontology> ;
  rdfs:label "Communication-justification"@en ;
  skos:definition """Source: EU Vocabularies authority table \"<xref scope=\"external\" href=\"https://op.europa.eu/web/eu-vocabularies/at-dataset/-/resource/dataset/communication-justification\"><foreign otherprops=\"#0000ff\"><u>Communication justification</u></foreign></xref>\" (https://op.europa.eu/web/eu-vocabularies/at-dataset/-/resource/dataset/communication-justification).
"""@en ;
  skos:prefLabel "Communication-justification" ;
.
<http://publications.europa.eu/resource/authority/Contract-nature>
  rdf:type skos:ConceptScheme ;
  rdfs:comment "Source: EU Vocabularies authority table \"<xref scope=\"external\" href=\"https://op.europa.eu/web/eu-vocabularies/at-dataset/-/resource/dataset/contract-nature\"><foreign otherprops=\"#0000ff\"><u>Contract nature</u></foreign></xref>\" (https://op.europa.eu/web/eu-vocabularies/at-dataset/-/resource/dataset/contract-nature)."@en ;
  rdfs:isDefinedBy <http://data.europa.eu/a4g/ontology> ;
  rdfs:label "Contract-nature"@en ;
  skos:definition "Source: EU Vocabularies authority table \"<xref scope=\"external\" href=\"https://op.europa.eu/web/eu-vocabularies/at-dataset/-/resource/dataset/contract-nature\"><foreign otherprops=\"#0000ff\"><u>Contract nature</u></foreign></xref>\" (https://op.europa.eu/web/eu-vocabularies/at-dataset/-/resource/dataset/contract-nature)."@en ;
  skos:prefLabel "Contract-nature" ;
.
<http://publications.europa.eu/resource/authority/Country>
  rdf:type skos:ConceptScheme ;
  rdfs:comment """A country is one of the political units which the world is divided into, covering a particular area of land.

Compulsory use of the code list from the ISO 3166-1 alpha-3.

Source: EU Vocabularies authority table \"<xref scope=\"external\" href=\"https://op.europa.eu/web/eu-vocabularies/at-dataset/-/resource/dataset/country\"><foreign otherprops=\"#0000ff\"><u>Country</u></foreign></xref>\" (https://op.europa.eu/web/eu-vocabularies/at-dataset/-/resource/dataset/country)."""@en ;
  rdfs:isDefinedBy <http://data.europa.eu/a4g/ontology> ;
  rdfs:label "Country"@en ;
  skos:definition """A country is one of the political units which the world is divided into, covering a particular area of land.

Compulsory use of the code list from the ISO 3166-1 alpha-3.

Source: EU Vocabularies authority table \"<xref scope=\"external\" href=\"https://op.europa.eu/web/eu-vocabularies/at-dataset/-/resource/dataset/country\"><foreign otherprops=\"#0000ff\"><u>Country</u></foreign></xref>\" (https://op.europa.eu/web/eu-vocabularies/at-dataset/-/resource/dataset/country)."""@en ;
  skos:prefLabel "Country" ;
.
<http://publications.europa.eu/resource/authority/Cpv>
  rdf:type skos:ConceptScheme ;
  rdfs:comment """The CPV establishes a single classification system for public procurement aimed at standardising the references used by procuring entities to describe the purpose of procurement contracts and procurement projects.

Compulsory use of Common Procurement Vocabulary (CPV) codes (Regulation (EC) No 213/2008)

Source: <xref scope=\"external\" href=\"https://eur-lex.europa.eu/legal-content/EN/TXT/?uri=CELEX:32008R0213\"><foreign otherprops=\"#0000ff\"><u>Commision Regulation (EC) No 213/2008</u></foreign></xref> (https://eur-lex.europa.eu/legal-content/EN/TXT/?uri=CELEX:32008R0213) """@en ;
  rdfs:isDefinedBy <http://data.europa.eu/a4g/ontology> ;
  rdfs:label "Cpv"@en ;
  skos:definition """The CPV establishes a single classification system for public procurement aimed at standardising the references used by procuring entities to describe the purpose of procurement contracts and procurement projects.

Compulsory use of Common Procurement Vocabulary (CPV) codes (Regulation (EC) No 213/2008)

Source: <xref scope=\"external\" href=\"https://eur-lex.europa.eu/legal-content/EN/TXT/?uri=CELEX:32008R0213\"><foreign otherprops=\"#0000ff\"><u>Commision Regulation (EC) No 213/2008</u></foreign></xref> (https://eur-lex.europa.eu/legal-content/EN/TXT/?uri=CELEX:32008R0213) """@en ;
  skos:prefLabel "Cpv" ;
.
<http://publications.europa.eu/resource/authority/Currency>
  rdf:type skos:ConceptScheme ;
  rdfs:comment """The Currencies Named Authority List (NAL) or Common Authority Table (CAT) is a controlled vocabulary listing currencies with their authority code and labels in the 24 official languages of the EU (when available). The list is based on the ISO standard ISO 4217. This NAL is maintained by the Publications Office of the EU in its Metadata Registry (MDR).

Source: EU Vocabularies authority table \"<xref scope=\"external\" href=\"https://op.europa.eu/web/eu-vocabularies/at-dataset/-/resource/dataset/currency\"><foreign otherprops=\"#0000ff\"><u>Currency</u></foreign></xref>\" (https://op.europa.eu/web/eu-vocabularies/at-dataset/-/resource/dataset/currency).
"""@en ;
  rdfs:isDefinedBy <http://data.europa.eu/a4g/ontology> ;
  rdfs:label "Currency"@en ;
  skos:definition """The Currencies Named Authority List (NAL) or Common Authority Table (CAT) is a controlled vocabulary listing currencies with their authority code and labels in the 24 official languages of the EU (when available). The list is based on the ISO standard ISO 4217. This NAL is maintained by the Publications Office of the EU in its Metadata Registry (MDR).

Source: EU Vocabularies authority table \"<xref scope=\"external\" href=\"https://op.europa.eu/web/eu-vocabularies/at-dataset/-/resource/dataset/currency\"><foreign otherprops=\"#0000ff\"><u>Currency</u></foreign></xref>\" (https://op.europa.eu/web/eu-vocabularies/at-dataset/-/resource/dataset/currency).
"""@en ;
  skos:prefLabel "Currency" ;
.
<http://publications.europa.eu/resource/authority/Direct-award-justification>
  rdf:type skos:ConceptScheme ;
  rdfs:comment """Justifications for the choice of the negotiated procedure without prior publication of a call for competition or concession.

Source: EU Vocabularies authority table \"<xref scope=\"external\" href=\"https://op.europa.eu/web/eu-vocabularies/at-dataset/-/resource/dataset/direct-award-justification\"><foreign otherprops=\"#0000ff\"><u>Direct Award Justification</u></foreign></xref>\" (https://op.europa.eu/web/eu-vocabularies/at-dataset/-/resource/dataset/direct-award-justification).
"""@en ;
  rdfs:isDefinedBy <http://data.europa.eu/a4g/ontology> ;
  rdfs:label "Direct-award-justification"@en ;
  skos:definition """Justifications for the choice of the negotiated procedure without prior publication of a call for competition or concession.

Source: EU Vocabularies authority table \"<xref scope=\"external\" href=\"https://op.europa.eu/web/eu-vocabularies/at-dataset/-/resource/dataset/direct-award-justification\"><foreign otherprops=\"#0000ff\"><u>Direct Award Justification</u></foreign></xref>\" (https://op.europa.eu/web/eu-vocabularies/at-dataset/-/resource/dataset/direct-award-justification).
"""@en ;
  skos:prefLabel "Direct-award-justification" ;
.
<http://publications.europa.eu/resource/authority/Dps-usage>
  rdf:type skos:ConceptScheme ;
  rdfs:comment """Source: EU Vocabularies authority table \"<xref scope=\"external\" href=\"https://op.europa.eu/en/web/eu-vocabularies/at-dataset/-/resource/dataset/dps-usage\"><foreign otherprops=\"#0000ff\"><u>DPS Usage</u></foreign></xref>\" (https://op.europa.eu/en/web/eu-vocabularies/at-dataset/-/resource/dataset/dps-usage).
"""@en ;
  rdfs:isDefinedBy <http://data.europa.eu/a4g/ontology> ;
  rdfs:label "Dps-usage"@en ;
  skos:definition """Source: EU Vocabularies authority table \"<xref scope=\"external\" href=\"https://op.europa.eu/en/web/eu-vocabularies/at-dataset/-/resource/dataset/dps-usage\"><foreign otherprops=\"#0000ff\"><u>DPS Usage</u></foreign></xref>\" (https://op.europa.eu/en/web/eu-vocabularies/at-dataset/-/resource/dataset/dps-usage).
"""@en ;
  skos:prefLabel "Dps-usage" ;
.
<http://publications.europa.eu/resource/authority/Economic-operator-size>
  rdf:type skos:ConceptScheme ;
  rdfs:comment """Source: EU Vocabularies authority table \"<xref scope=\"external\" href=\"https://op.europa.eu/en/web/eu-vocabularies/at-dataset/-/resource/dataset/economic-operator-size\"><foreign otherprops=\"#0000ff\"><u>Economic Operator Size</u></foreign></xref>\" (https://op.europa.eu/en/web/eu-vocabularies/at-dataset/-/resource/dataset/economic-operator-size).

"""@en ;
  rdfs:isDefinedBy <http://data.europa.eu/a4g/ontology> ;
  rdfs:label "Economic-operator-size"@en ;
  skos:definition """Source: EU Vocabularies authority table \"<xref scope=\"external\" href=\"https://op.europa.eu/en/web/eu-vocabularies/at-dataset/-/resource/dataset/economic-operator-size\"><foreign otherprops=\"#0000ff\"><u>Economic Operator Size</u></foreign></xref>\" (https://op.europa.eu/en/web/eu-vocabularies/at-dataset/-/resource/dataset/economic-operator-size).

"""@en ;
  skos:prefLabel "Economic-operator-size" ;
.
<http://publications.europa.eu/resource/authority/Environmental-impact>
  rdf:type skos:ConceptScheme ;
  rdfs:comment """Requesting compliance with an ISO 14024 Type I environmental label 

Requesting compliance with the eco-management and audit scheme (EMAS), established by Regulation (EC) No 1221/2009 

Requesting compliance with an ISO 14001 environmental management system, other than the eco-management and audit scheme (EMAS) established by Regulation (EC) No 1221/2009 

Requesting compliance with the highest energy efficiency class (as defined by various legislation such as, for example, Regulation (EU) 626/2011 on air conditioners)

Requesting, for the majority of the relevant purchase, the compliance with Regulation (EC) 834/2007 on organic production and labelling of organic products 

Other

Source: EU Vocabularies authority table \"<xref scope=\"external\" href=\"https://op.europa.eu/en/web/eu-vocabularies/at-dataset/-/resource/dataset/environmental-impact\"><foreign otherprops=\"#0000ff\"><u>Environmental Impact</u></foreign></xref>\" (https://op.europa.eu/en/web/eu-vocabularies/at-dataset/-/resource/dataset/environmental-impact)."""@en ;
  rdfs:isDefinedBy <http://data.europa.eu/a4g/ontology> ;
  rdfs:label "Environmental-impact"@en ;
  skos:definition """Requesting compliance with an ISO 14024 Type I environmental label 

Requesting compliance with the eco-management and audit scheme (EMAS), established by Regulation (EC) No 1221/2009 

Requesting compliance with an ISO 14001 environmental management system, other than the eco-management and audit scheme (EMAS) established by Regulation (EC) No 1221/2009 

Requesting compliance with the highest energy efficiency class (as defined by various legislation such as, for example, Regulation (EU) 626/2011 on air conditioners)

Requesting, for the majority of the relevant purchase, the compliance with Regulation (EC) 834/2007 on organic production and labelling of organic products 

Other

Source: EU Vocabularies authority table \"<xref scope=\"external\" href=\"https://op.europa.eu/en/web/eu-vocabularies/at-dataset/-/resource/dataset/environmental-impact\"><foreign otherprops=\"#0000ff\"><u>Environmental Impact</u></foreign></xref>\" (https://op.europa.eu/en/web/eu-vocabularies/at-dataset/-/resource/dataset/environmental-impact)."""@en ;
  skos:prefLabel "Environmental-impact" ;
.
<http://publications.europa.eu/resource/authority/Innovative-acquisition>
  rdf:type skos:ConceptScheme ;
  rdfs:isDefinedBy <http://data.europa.eu/a4g/ontology> ;
  rdfs:label "Innovative-acquisition"@en ;
  skos:prefLabel "Innovative-acquisition" ;
.
<http://publications.europa.eu/resource/authority/Language>
  rdf:type skos:ConceptScheme ;
  rdfs:comment """Source: EU Vocabularies authority table \"<xref scope=\"external\" href=\"https://op.europa.eu/en/web/eu-vocabularies/at-dataset/-/resource/dataset/language\"><foreign otherprops=\"#0000ff\"><u>Language</u></foreign></xref>\" (https://op.europa.eu/en/web/eu-vocabularies/at-dataset/-/resource/dataset/language).
"""@en ;
  rdfs:isDefinedBy <http://data.europa.eu/a4g/ontology> ;
  rdfs:label "Language"@en ;
  skos:definition """Source: EU Vocabularies authority table \"<xref scope=\"external\" href=\"https://op.europa.eu/en/web/eu-vocabularies/at-dataset/-/resource/dataset/language\"><foreign otherprops=\"#0000ff\"><u>Language</u></foreign></xref>\" (https://op.europa.eu/en/web/eu-vocabularies/at-dataset/-/resource/dataset/language).
"""@en ;
  skos:prefLabel "Language" ;
.
<http://publications.europa.eu/resource/authority/Legal-basis>
  rdf:type skos:ConceptScheme ;
  rdfs:comment """Based on Legal Basis list defined by MDR.

Source: EU Vocabularies authority table \"<xref scope=\"external\" href=\"https://op.europa.eu/en/web/eu-vocabularies/at-dataset/-/resource/dataset/legal-basis\"><foreign otherprops=\"#0000ff\"><u>Legal Basis</u></foreign></xref>\" (https://op.europa.eu/en/web/eu-vocabularies/at-dataset/-/resource/dataset/legal-basis).
"""@en ;
  rdfs:isDefinedBy <http://data.europa.eu/a4g/ontology> ;
  rdfs:label "Legal-basis"@en ;
  skos:definition """Based on Legal Basis list defined by MDR.

Source: EU Vocabularies authority table \"<xref scope=\"external\" href=\"https://op.europa.eu/en/web/eu-vocabularies/at-dataset/-/resource/dataset/legal-basis\"><foreign otherprops=\"#0000ff\"><u>Legal Basis</u></foreign></xref>\" (https://op.europa.eu/en/web/eu-vocabularies/at-dataset/-/resource/dataset/legal-basis).
"""@en ;
  skos:prefLabel "Legal-basis" ;
.
<http://publications.europa.eu/resource/authority/Main-activity>
  rdf:type skos:ConceptScheme ;
  rdfs:comment """Source: EU Vocabularies authority table \"<xref scope=\"external\" href=\"https://op.europa.eu/en/web/eu-vocabularies/at-dataset/-/resource/dataset/main-activity\"><foreign otherprops=\"#0000ff\"><u>Main Activity</u></foreign></xref>\" (https://op.europa.eu/en/web/eu-vocabularies/at-dataset/-/resource/dataset/main-activity).
"""@en ;
  rdfs:isDefinedBy <http://data.europa.eu/a4g/ontology> ;
  rdfs:label "Main-activity"@en ;
  skos:definition """Source: EU Vocabularies authority table \"<xref scope=\"external\" href=\"https://op.europa.eu/en/web/eu-vocabularies/at-dataset/-/resource/dataset/main-activity\"><foreign otherprops=\"#0000ff\"><u>Main Activity</u></foreign></xref>\" (https://op.europa.eu/en/web/eu-vocabularies/at-dataset/-/resource/dataset/main-activity).
"""@en ;
  skos:prefLabel "Main-activity" ;
.
<http://publications.europa.eu/resource/authority/Measurement-unit>
  rdf:type skos:ConceptScheme ;
  rdfs:comment """Source: EU Vocabularies authority table \"<xref scope=\"external\" href=\"https://op.europa.eu/en/web/eu-vocabularies/at-dataset/-/resource/dataset/measurement-unit\"><foreign otherprops=\"#0000ff\"><u>Measurement Unit</u></foreign></xref>\" (https://op.europa.eu/en/web/eu-vocabularies/at-dataset/-/resource/dataset/measurement-unit).

"""@en ;
  rdfs:isDefinedBy <http://data.europa.eu/a4g/ontology> ;
  rdfs:label "Measurement-unit"@en ;
  skos:definition """Source: EU Vocabularies authority table \"<xref scope=\"external\" href=\"https://op.europa.eu/en/web/eu-vocabularies/at-dataset/-/resource/dataset/measurement-unit\"><foreign otherprops=\"#0000ff\"><u>Measurement Unit</u></foreign></xref>\" (https://op.europa.eu/en/web/eu-vocabularies/at-dataset/-/resource/dataset/measurement-unit).

"""@en ;
  skos:prefLabel "Measurement-unit" ;
.
<http://publications.europa.eu/resource/authority/Missing-info-submission>
  rdf:type skos:ConceptScheme ;
  rdfs:comment """Source: EU Vocabularies authority table \"<xref scope=\"external\" href=\"https://op.europa.eu/en/web/eu-vocabularies/at-dataset/-/resource/dataset/missing-info-submission\"><foreign otherprops=\"#0000ff\"><u>Missing Information Submission</u></foreign></xref>\" (https://op.europa.eu/en/web/eu-vocabularies/at-dataset/-/resource/dataset/missing-info-submission).
"""@en ;
  rdfs:isDefinedBy <http://data.europa.eu/a4g/ontology> ;
  rdfs:label "Missing-info-submission"@en ;
  skos:definition """Source: EU Vocabularies authority table \"<xref scope=\"external\" href=\"https://op.europa.eu/en/web/eu-vocabularies/at-dataset/-/resource/dataset/missing-info-submission\"><foreign otherprops=\"#0000ff\"><u>Missing Information Submission</u></foreign></xref>\" (https://op.europa.eu/en/web/eu-vocabularies/at-dataset/-/resource/dataset/missing-info-submission).
"""@en ;
  skos:prefLabel "Missing-info-submission" ;
.
<http://publications.europa.eu/resource/authority/Modification-justification>
  rdf:type skos:ConceptScheme ;
  rdfs:comment "Source: EU Vocabularies authority table \"<xref scope=\"external\" href=\"https://op.europa.eu/en/web/eu-vocabularies/at-dataset/-/resource/dataset/modification-justification\"><foreign otherprops=\"#0000ff\"><u>Modification Justification</u></foreign></xref>\" (https://op.europa.eu/en/web/eu-vocabularies/at-dataset/-/resource/dataset/modification-justification)"@en ;
  rdfs:isDefinedBy <http://data.europa.eu/a4g/ontology> ;
  rdfs:label "Modification-justification"@en ;
  skos:definition "Source: EU Vocabularies authority table \"<xref scope=\"external\" href=\"https://op.europa.eu/en/web/eu-vocabularies/at-dataset/-/resource/dataset/modification-justification\"><foreign otherprops=\"#0000ff\"><u>Modification Justification</u></foreign></xref>\" (https://op.europa.eu/en/web/eu-vocabularies/at-dataset/-/resource/dataset/modification-justification)"@en ;
  skos:prefLabel "Modification-justification" ;
.
<http://publications.europa.eu/resource/authority/Non-award-justification>
  rdf:type skos:ConceptScheme ;
  rdfs:comment """Source: EU Vocabularies authority table \"<xref scope=\"external\" href=\"https://op.europa.eu/en/web/eu-vocabularies/at-dataset/-/resource/dataset/non-award-justification\"><foreign otherprops=\"#0000ff\"><u>Non Award Justification</u></foreign></xref>\" (https://op.europa.eu/en/web/eu-vocabularies/at-dataset/-/resource/dataset/non-award-justification)
"""@en ;
  rdfs:isDefinedBy <http://data.europa.eu/a4g/ontology> ;
  rdfs:label "Non-award-justification"@en ;
  skos:definition """Source: EU Vocabularies authority table \"<xref scope=\"external\" href=\"https://op.europa.eu/en/web/eu-vocabularies/at-dataset/-/resource/dataset/non-award-justification\"><foreign otherprops=\"#0000ff\"><u>Non Award Justification</u></foreign></xref>\" (https://op.europa.eu/en/web/eu-vocabularies/at-dataset/-/resource/dataset/non-award-justification)
"""@en ;
  skos:prefLabel "Non-award-justification" ;
.
<http://publications.europa.eu/resource/authority/Non-publication-justification>
  rdf:type skos:ConceptScheme ;
  rdfs:comment "Source: EU Vocabularies authority table \"<xref scope=\"external\" href=\"https://op.europa.eu/en/web/eu-vocabularies/at-dataset/-/resource/dataset/non-publication-justification\"><foreign otherprops=\"#0000ff\"><u>Non Publication Justification</u></foreign></xref>\" (https://op.europa.eu/en/web/eu-vocabularies/at-dataset/-/resource/dataset/non-publication-justification)"@en ;
  rdfs:isDefinedBy <http://data.europa.eu/a4g/ontology> ;
  rdfs:label "Non-publication-justification"@en ;
  skos:definition "Source: EU Vocabularies authority table \"<xref scope=\"external\" href=\"https://op.europa.eu/en/web/eu-vocabularies/at-dataset/-/resource/dataset/non-publication-justification\"><foreign otherprops=\"#0000ff\"><u>Non Publication Justification</u></foreign></xref>\" (https://op.europa.eu/en/web/eu-vocabularies/at-dataset/-/resource/dataset/non-publication-justification)"@en ;
  skos:prefLabel "Non-publication-justification" ;
.
<http://publications.europa.eu/resource/authority/Number-fixed>
  rdf:type skos:ConceptScheme ;
  rdfs:comment """Source: EU Vocabularies authority table \"<xref scope=\"external\" href=\"https://op.europa.eu/en/web/eu-vocabularies/at-dataset/-/resource/dataset/number-fixed\"><foreign otherprops=\"#0000ff\"><u>Number fixed</u></foreign></xref>\" (https://op.europa.eu/en/web/eu-vocabularies/at-dataset/-/resource/dataset/number-fixed)
"""@en ;
  rdfs:isDefinedBy <http://data.europa.eu/a4g/ontology> ;
  rdfs:label "Number-fixed"@en ;
  skos:definition """Source: EU Vocabularies authority table \"<xref scope=\"external\" href=\"https://op.europa.eu/en/web/eu-vocabularies/at-dataset/-/resource/dataset/number-fixed\"><foreign otherprops=\"#0000ff\"><u>Number fixed</u></foreign></xref>\" (https://op.europa.eu/en/web/eu-vocabularies/at-dataset/-/resource/dataset/number-fixed)
"""@en ;
  skos:prefLabel "Number-fixed" ;
.
<http://publications.europa.eu/resource/authority/Number-threshold>
  rdf:type skos:ConceptScheme ;
  rdfs:comment """Source: EU Vocabularies authority table \"<xref scope=\"external\" href=\"https://op.europa.eu/en/web/eu-vocabularies/at-dataset/-/resource/dataset/number-threshold\"><foreign otherprops=\"#0000ff\"><u>Number threshold</u></foreign></xref>\" (https://op.europa.eu/en/web/eu-vocabularies/at-dataset/-/resource/dataset/number-threshold)
"""@en ;
  rdfs:isDefinedBy <http://data.europa.eu/a4g/ontology> ;
  rdfs:label "Number-threshold"@en ;
  skos:definition """Source: EU Vocabularies authority table \"<xref scope=\"external\" href=\"https://op.europa.eu/en/web/eu-vocabularies/at-dataset/-/resource/dataset/number-threshold\"><foreign otherprops=\"#0000ff\"><u>Number threshold</u></foreign></xref>\" (https://op.europa.eu/en/web/eu-vocabularies/at-dataset/-/resource/dataset/number-threshold)
"""@en ;
  skos:prefLabel "Number-threshold" ;
.
<http://publications.europa.eu/resource/authority/Number-weight>
  rdf:type skos:ConceptScheme ;
  rdfs:comment """Source: EU Vocabularies authority table \"<xref scope=\"external\" href=\"https://op.europa.eu/en/web/eu-vocabularies/at-dataset/-/resource/dataset/number-weight\"><foreign otherprops=\"#0000ff\"><u>Number weight</u></foreign></xref>\" (https://op.europa.eu/en/web/eu-vocabularies/at-dataset/-/resource/dataset/number-weight)
"""@en ;
  rdfs:isDefinedBy <http://data.europa.eu/a4g/ontology> ;
  rdfs:label "Number-weight"@en ;
  skos:definition """Source: EU Vocabularies authority table \"<xref scope=\"external\" href=\"https://op.europa.eu/en/web/eu-vocabularies/at-dataset/-/resource/dataset/number-weight\"><foreign otherprops=\"#0000ff\"><u>Number weight</u></foreign></xref>\" (https://op.europa.eu/en/web/eu-vocabularies/at-dataset/-/resource/dataset/number-weight)
"""@en ;
  skos:prefLabel "Number-weight" ;
.
<http://publications.europa.eu/resource/authority/Other-place-service>
  rdf:type skos:ConceptScheme ;
  rdfs:comment """Source: EU Vocabularies authority table \"<xref scope=\"external\" href=\"https://op.europa.eu/en/web/eu-vocabularies/at-dataset/-/resource/dataset/other-place-service\"><foreign otherprops=\"#0000ff\"><u>Other Place Service</u></foreign></xref>\" (https://op.europa.eu/en/web/eu-vocabularies/at-dataset/-/resource/dataset/other-place-service)
"""@en ;
  rdfs:isDefinedBy <http://data.europa.eu/a4g/ontology> ;
  rdfs:label "Other-place-service"@en ;
  skos:definition """Source: EU Vocabularies authority table \"<xref scope=\"external\" href=\"https://op.europa.eu/en/web/eu-vocabularies/at-dataset/-/resource/dataset/other-place-service\"><foreign otherprops=\"#0000ff\"><u>Other Place Service</u></foreign></xref>\" (https://op.europa.eu/en/web/eu-vocabularies/at-dataset/-/resource/dataset/other-place-service)
"""@en ;
  skos:prefLabel "Other-place-service" ;
.
<http://publications.europa.eu/resource/authority/Permission>
  rdf:type skos:ConceptScheme ;
  rdfs:comment """
Statement by the Procuring Entity about whether it may apply modifications to the procurement procedure that would alter the overall nature of the contract or the framework agreement.

(Pending to review by the WG)

Source: EU Vocabularies authority table \"<xref scope=\"external\" href=\"https://op.europa.eu/en/web/eu-vocabularies/at-dataset/-/resource/dataset/permission\"><foreign otherprops=\"#0000ff\"><u>Permission</u></foreign></xref>\" (https://op.europa.eu/en/web/eu-vocabularies/at-dataset/-/resource/dataset/permission)
"""@en ;
  rdfs:isDefinedBy <http://data.europa.eu/a4g/ontology> ;
  rdfs:label "Permission"@en ;
  skos:definition """
Statement by the Procuring Entity about whether it may apply modifications to the procurement procedure that would alter the overall nature of the contract or the framework agreement.

(Pending to review by the WG)

Source: EU Vocabularies authority table \"<xref scope=\"external\" href=\"https://op.europa.eu/en/web/eu-vocabularies/at-dataset/-/resource/dataset/permission\"><foreign otherprops=\"#0000ff\"><u>Permission</u></foreign></xref>\" (https://op.europa.eu/en/web/eu-vocabularies/at-dataset/-/resource/dataset/permission)
"""@en ;
  skos:prefLabel "Permission" ;
.
<http://publications.europa.eu/resource/authority/Procurement-procedure-type>
  rdf:type skos:ConceptScheme ;
  rdfs:comment """It specifies the sort of procurement procedure, which will regulate the conditions and deadlines that apply to the process.

Source: EU Vocabularies authority table \"<xref scope=\"external\" href=\"https://op.europa.eu/en/web/eu-vocabularies/at-dataset/-/resource/dataset/procurement-procedure-type\"><foreign otherprops=\"#0000ff\"><u>Procurement Procedure Type</u></foreign></xref>\" (https://op.europa.eu/en/web/eu-vocabularies/at-dataset/-/resource/dataset/procurement-procedure-type)
"""@en ;
  rdfs:isDefinedBy <http://data.europa.eu/a4g/ontology> ;
  rdfs:label "Procurement-procedure-type"@en ;
  skos:definition """It specifies the sort of procurement procedure, which will regulate the conditions and deadlines that apply to the process.

Source: EU Vocabularies authority table \"<xref scope=\"external\" href=\"https://op.europa.eu/en/web/eu-vocabularies/at-dataset/-/resource/dataset/procurement-procedure-type\"><foreign otherprops=\"#0000ff\"><u>Procurement Procedure Type</u></foreign></xref>\" (https://op.europa.eu/en/web/eu-vocabularies/at-dataset/-/resource/dataset/procurement-procedure-type)
"""@en ;
  skos:prefLabel "Procurement-procedure-type" ;
.
<http://publications.europa.eu/resource/authority/Requirement-stage>
  rdf:type skos:ConceptScheme ;
  rdfs:isDefinedBy <http://data.europa.eu/a4g/ontology> ;
  rdfs:label "Requirement-stage"@en ;
  skos:prefLabel "Requirement-stage" ;
.
<http://publications.europa.eu/resource/authority/Reserved-procurement>
  rdf:type skos:ConceptScheme ;
  rdfs:comment """Source: EU Vocabularies authority table \"<xref scope=\"external\" href=\"https://op.europa.eu/en/web/eu-vocabularies/at-dataset/-/resource/dataset/reserved-procurement\"><foreign otherprops=\"#0000ff\"><u>Reserved Procurement</u></foreign></xref>\" (https://op.europa.eu/en/web/eu-vocabularies/at-dataset/-/resource/dataset/reserved-procurement)
"""@en ;
  rdfs:isDefinedBy <http://data.europa.eu/a4g/ontology> ;
  rdfs:label "Reserved-procurement"@en ;
  skos:definition """Source: EU Vocabularies authority table \"<xref scope=\"external\" href=\"https://op.europa.eu/en/web/eu-vocabularies/at-dataset/-/resource/dataset/reserved-procurement\"><foreign otherprops=\"#0000ff\"><u>Reserved Procurement</u></foreign></xref>\" (https://op.europa.eu/en/web/eu-vocabularies/at-dataset/-/resource/dataset/reserved-procurement)
"""@en ;
  skos:prefLabel "Reserved-procurement" ;
.
<http://publications.europa.eu/resource/authority/Selection-criterion>
  rdf:type skos:ConceptScheme ;
  rdfs:comment """Source: EU Vocabularies authority table \"<xref scope=\"external\" href=\"https://op.europa.eu/en/web/eu-vocabularies/at-dataset/-/resource/dataset/selection-criterion\"><foreign otherprops=\"#0000ff\"><u>Selection Criterion</u></foreign></xref>\" (https://op.europa.eu/en/web/eu-vocabularies/at-dataset/-/resource/dataset/selection-criterion)
"""@en ;
  rdfs:isDefinedBy <http://data.europa.eu/a4g/ontology> ;
  rdfs:label "Selection-criterion"@en ;
  skos:definition """Source: EU Vocabularies authority table \"<xref scope=\"external\" href=\"https://op.europa.eu/en/web/eu-vocabularies/at-dataset/-/resource/dataset/selection-criterion\"><foreign otherprops=\"#0000ff\"><u>Selection Criterion</u></foreign></xref>\" (https://op.europa.eu/en/web/eu-vocabularies/at-dataset/-/resource/dataset/selection-criterion)
"""@en ;
  skos:prefLabel "Selection-criterion" ;
.
<http://publications.europa.eu/resource/authority/Social-objective>
  rdf:type skos:ConceptScheme ;
  rdfs:comment """Source: EU Vocabularies authority table \"<xref scope=\"external\" href=\"https://op.europa.eu/en/web/eu-vocabularies/at-dataset/-/resource/dataset/social-objective\"><foreign otherprops=\"#0000ff\"><u>Social Objective</u></foreign></xref>\" (https://op.europa.eu/en/web/eu-vocabularies/at-dataset/-/resource/dataset/social-objective)
"""@en ;
  rdfs:isDefinedBy <http://data.europa.eu/a4g/ontology> ;
  rdfs:label "Social-objective"@en ;
  skos:definition """Source: EU Vocabularies authority table \"<xref scope=\"external\" href=\"https://op.europa.eu/en/web/eu-vocabularies/at-dataset/-/resource/dataset/social-objective\"><foreign otherprops=\"#0000ff\"><u>Social Objective</u></foreign></xref>\" (https://op.europa.eu/en/web/eu-vocabularies/at-dataset/-/resource/dataset/social-objective)
"""@en ;
  skos:prefLabel "Social-objective" ;
.
<http://publications.europa.eu/resource/authority/Strategic-procurement>
  rdf:type skos:ConceptScheme ;
  rdfs:comment "Source: EU Vocabularies authority table \"<xref scope=\"external\" href=\"https://op.europa.eu/en/web/eu-vocabularies/at-dataset/-/resource/dataset/strategic-procurement\"><foreign otherprops=\"#0000ff\"><u>Strategic Procurement</u></foreign></xref>\" (https://op.europa.eu/en/web/eu-vocabularies/at-dataset/-/resource/dataset/strategic-procurement)"@en ;
  rdfs:isDefinedBy <http://data.europa.eu/a4g/ontology> ;
  rdfs:label "Strategic-procurement"@en ;
  skos:definition "Source: EU Vocabularies authority table \"<xref scope=\"external\" href=\"https://op.europa.eu/en/web/eu-vocabularies/at-dataset/-/resource/dataset/strategic-procurement\"><foreign otherprops=\"#0000ff\"><u>Strategic Procurement</u></foreign></xref>\" (https://op.europa.eu/en/web/eu-vocabularies/at-dataset/-/resource/dataset/strategic-procurement)"@en ;
  skos:prefLabel "Strategic-procurement" ;
.
<http://publications.europa.eu/resource/authority/Subcontracting-indication>
  rdf:type skos:ConceptScheme ;
  rdfs:comment """Source: EU Vocabularies authority table \"<xref scope=\"external\" href=\"https://op.europa.eu/en/web/eu-vocabularies/at-dataset/-/resource/dataset/subcontracting-indication\"><foreign otherprops=\"#0000ff\"><u>Subcontracting indication</u></foreign></xref>\" (https://op.europa.eu/en/web/eu-vocabularies/at-dataset/-/resource/dataset/subcontracting-indication)
"""@en ;
  rdfs:isDefinedBy <http://data.europa.eu/a4g/ontology> ;
  rdfs:label "Subcontracting-indication"@en ;
  skos:definition """Source: EU Vocabularies authority table \"<xref scope=\"external\" href=\"https://op.europa.eu/en/web/eu-vocabularies/at-dataset/-/resource/dataset/subcontracting-indication\"><foreign otherprops=\"#0000ff\"><u>Subcontracting indication</u></foreign></xref>\" (https://op.europa.eu/en/web/eu-vocabularies/at-dataset/-/resource/dataset/subcontracting-indication)
"""@en ;
  skos:prefLabel "Subcontracting-indication" ;
.
<http://publications.europa.eu/resource/authority/Subcontracting-obligation>
  rdf:type skos:ConceptScheme ;
  rdfs:comment """Codes and values used to show the obligation of the economic operator to subcontract parts of the original contract to third parties. 

WG Approval 17/09/2019 

Source: EU Vocabularies authority table \"<xref scope=\"external\" href=\"https://op.europa.eu/en/web/eu-vocabularies/at-dataset/-/resource/dataset/subcontracting-obligation\"><foreign otherprops=\"#0000ff\"><u>Subcontracting obligation</u></foreign></xref>\" (https://op.europa.eu/en/web/eu-vocabularies/at-dataset/-/resource/dataset/subcontracting-obligation)
"""@en ;
  rdfs:isDefinedBy <http://data.europa.eu/a4g/ontology> ;
  rdfs:label "Subcontracting-obligation"@en ;
  skos:definition """Codes and values used to show the obligation of the economic operator to subcontract parts of the original contract to third parties. 

WG Approval 17/09/2019 

Source: EU Vocabularies authority table \"<xref scope=\"external\" href=\"https://op.europa.eu/en/web/eu-vocabularies/at-dataset/-/resource/dataset/subcontracting-obligation\"><foreign otherprops=\"#0000ff\"><u>Subcontracting obligation</u></foreign></xref>\" (https://op.europa.eu/en/web/eu-vocabularies/at-dataset/-/resource/dataset/subcontracting-obligation)
"""@en ;
  skos:prefLabel "Subcontracting-obligation" ;
.
<http://publications.europa.eu/resource/authority/Timeperiods>
  rdf:type skos:ConceptScheme ;
  rdfs:comment """This code list is used by the Duration Measure attribute 'unitCode'.

Source: EU Vocabularies authority table \"<xref scope=\"external\" href=\"https://op.europa.eu/en/web/eu-vocabularies/at-dataset/-/resource/dataset/timeperiods\"><foreign otherprops=\"#0000ff\"><u>Timeperiods</u></foreign></xref>\" (https://op.europa.eu/en/web/eu-vocabularies/at-dataset/-/resource/dataset/timeperiods)
"""@en ;
  rdfs:isDefinedBy <http://data.europa.eu/a4g/ontology> ;
  rdfs:label "Timeperiods"@en ;
  skos:definition """This code list is used by the Duration Measure attribute 'unitCode'.

Source: EU Vocabularies authority table \"<xref scope=\"external\" href=\"https://op.europa.eu/en/web/eu-vocabularies/at-dataset/-/resource/dataset/timeperiods\"><foreign otherprops=\"#0000ff\"><u>Timeperiods</u></foreign></xref>\" (https://op.europa.eu/en/web/eu-vocabularies/at-dataset/-/resource/dataset/timeperiods)
"""@en ;
  skos:prefLabel "Timeperiods" ;
.
<http://publications.europa.eu/resource/authority/Usage>
  rdf:type skos:ConceptScheme ;
  rdfs:comment "Source: EU Vocabularies authority table \"<xref scope=\"external\" href=\"https://op.europa.eu/en/web/eu-vocabularies/at-dataset/-/resource/dataset/usage\"><foreign otherprops=\"#0000ff\"><u>Usage</u></foreign></xref>\" (https://op.europa.eu/en/web/eu-vocabularies/at-dataset/-/resource/dataset/usage)"@en ;
  rdfs:isDefinedBy <http://data.europa.eu/a4g/ontology> ;
  rdfs:label "Usage"@en ;
  skos:definition "Source: EU Vocabularies authority table \"<xref scope=\"external\" href=\"https://op.europa.eu/en/web/eu-vocabularies/at-dataset/-/resource/dataset/usage\"><foreign otherprops=\"#0000ff\"><u>Usage</u></foreign></xref>\" (https://op.europa.eu/en/web/eu-vocabularies/at-dataset/-/resource/dataset/usage)"@en ;
  skos:prefLabel "Usage" ;
.
<http://publications.europa.eu/resource/authority/Winner-selection-status>
  rdf:type skos:ConceptScheme ;
  rdfs:comment "Source: EU Vocabularies authority table \"<xref scope=\"external\" href=\"https://op.europa.eu/en/web/eu-vocabularies/at-dataset/-/resource/dataset/winner-selection-status\"><foreign otherprops=\"#0000ff\"><u>Winner Selection Status</u></foreign></xref>\" (https://op.europa.eu/en/web/eu-vocabularies/at-dataset/-/resource/dataset/winner-selection-status)"@en ;
  rdfs:isDefinedBy <http://data.europa.eu/a4g/ontology> ;
  rdfs:label "Winner-selection-status"@en ;
  skos:definition "Source: EU Vocabularies authority table \"<xref scope=\"external\" href=\"https://op.europa.eu/en/web/eu-vocabularies/at-dataset/-/resource/dataset/winner-selection-status\"><foreign otherprops=\"#0000ff\"><u>Winner Selection Status</u></foreign></xref>\" (https://op.europa.eu/en/web/eu-vocabularies/at-dataset/-/resource/dataset/winner-selection-status)"@en ;
  skos:prefLabel "Winner-selection-status" ;
.
dct:Agent
  rdf:type owl:Class ;
  rdfs:isDefinedBy <http://data.europa.eu/a4g/ontology> ;
  rdfs:label "Agent"@en ;
  rdfs:subClassOf foaf:Agent ;
  owl:disjointWith org:Organization ;
  owl:disjointWith foaf:Group ;
  owl:disjointWith foaf:Organization ;
  owl:disjointWith foaf:Person ;
  skos:prefLabel "Agent"@en ;
.
<http://www.unece.org/cefact#Amount>
  rdf:type owl:Class ;
  rdfs:isDefinedBy <http://data.europa.eu/a4g/ontology> ;
  rdfs:label "Amount"@en ;
  skos:prefLabel "Amount"@en ;
.
<http://www.unece.org/cefact#Code>
  rdf:type owl:Class ;
  rdfs:isDefinedBy <http://data.europa.eu/a4g/ontology> ;
  rdfs:label "Code"@en ;
  skos:prefLabel "Code"@en ;
.
<http://www.unece.org/cefact#Identifier>
  rdf:type owl:Class ;
  rdfs:isDefinedBy <http://data.europa.eu/a4g/ontology> ;
  rdfs:label "Identifier"@en ;
  skos:prefLabel "Identifier"@en ;
.
<http://www.unece.org/cefact#Indicator>
  rdf:type rdfs:Datatype ;
  rdfs:isDefinedBy <http://data.europa.eu/a4g/ontology> ;
  rdfs:label "Indicator"@en ;
  skos:prefLabel "Indicator"@en ;
.
<http://www.unece.org/cefact#Measure>
  rdf:type owl:Class ;
  rdfs:isDefinedBy <http://data.europa.eu/a4g/ontology> ;
  rdfs:label "Measure"@en ;
  skos:prefLabel "Measure"@en ;
.
<http://www.unece.org/cefact#Numeric>
  rdf:type rdfs:Datatype ;
  rdfs:isDefinedBy <http://data.europa.eu/a4g/ontology> ;
  rdfs:label "Numeric"@en ;
  skos:prefLabel "Numeric"@en ;
.
<http://www.unece.org/cefact#Quantity>
  rdf:type owl:Class ;
  rdfs:isDefinedBy <http://data.europa.eu/a4g/ontology> ;
  rdfs:label "Quantity"@en ;
  skos:prefLabel "Quantity"@en ;
.
<http://www.unece.org/cefact#Text>
  rdf:type owl:Class ;
  rdfs:isDefinedBy <http://data.europa.eu/a4g/ontology> ;
  rdfs:label "Text"@en ;
  skos:prefLabel "Text"@en ;
.
xsd:Date
  rdf:type rdfs:Datatype ;
  rdfs:isDefinedBy <http://data.europa.eu/a4g/ontology> ;
  rdfs:label "Date"@en ;
  skos:prefLabel "Date"@en ;
.
xsd:DateTime
  rdf:type rdfs:Datatype ;
  rdfs:isDefinedBy <http://data.europa.eu/a4g/ontology> ;
  rdfs:label "Date time"@en ;
  skos:prefLabel "Date time"@en ;
.
xsd:Decimal
  rdf:type rdfs:Datatype ;
  rdfs:isDefinedBy <http://data.europa.eu/a4g/ontology> ;
  rdfs:label "Decimal"@en ;
  skos:prefLabel "Decimal"@en ;
.
xsd:Text
  rdf:type rdfs:Datatype ;
  rdfs:isDefinedBy <http://data.europa.eu/a4g/ontology> ;
  rdfs:label "Text"@en ;
  skos:prefLabel "Text"@en ;
.
xsd:Time
  rdf:type rdfs:Datatype ;
  rdfs:isDefinedBy <http://data.europa.eu/a4g/ontology> ;
  rdfs:label "Time"@en ;
  skos:prefLabel "Time"@en ;
.
org:FormalOrganization
  rdf:type owl:Class ;
  rdfs:isDefinedBy <http://data.europa.eu/a4g/ontology> ;
  rdfs:label "Formal organization"@en ;
  rdfs:subClassOf org:Organization ;
  owl:disjointWith epo:Organisation ;
  owl:disjointWith org:OrganizationalCollaboration ;
  owl:disjointWith org:OrganizationalUnit ;
  skos:prefLabel "Formal organization"@en ;
.
org:Organization
  rdf:type owl:Class ;
  rdfs:isDefinedBy <http://data.europa.eu/a4g/ontology> ;
  rdfs:label "Organization"@en ;
  rdfs:subClassOf foaf:Agent ;
  rdfs:subClassOf foaf:Organization ;
  owl:disjointWith dct:Agent ;
  owl:disjointWith foaf:Group ;
  owl:disjointWith foaf:Organization ;
  owl:disjointWith foaf:Person ;
  skos:prefLabel "Organization"@en ;
.
org:OrganizationalCollaboration
  rdf:type owl:Class ;
  rdfs:isDefinedBy <http://data.europa.eu/a4g/ontology> ;
  rdfs:label "Organizational collaboration"@en ;
  rdfs:subClassOf org:Organization ;
  owl:disjointWith epo:Organisation ;
  owl:disjointWith org:FormalOrganization ;
  owl:disjointWith org:OrganizationalUnit ;
  skos:prefLabel "Organizational collaboration"@en ;
.
org:OrganizationalUnit
  rdf:type owl:Class ;
  rdfs:isDefinedBy <http://data.europa.eu/a4g/ontology> ;
  rdfs:label "Organizational unit"@en ;
  rdfs:subClassOf org:Organization ;
  owl:disjointWith epo:Organisation ;
  owl:disjointWith org:FormalOrganization ;
  owl:disjointWith org:OrganizationalCollaboration ;
  skos:prefLabel "Organizational unit"@en ;
.
org:Site
  rdf:type owl:Class ;
  rdfs:isDefinedBy <http://data.europa.eu/a4g/ontology> ;
  rdfs:label "Site"@en ;
  skos:prefLabel "Site"@en ;
.
org:hasName
  rdf:type owl:ObjectProperty ;
  rdfs:isDefinedBy <http://data.europa.eu/a4g/ontology> ;
  rdfs:label "Has name"@en ;
  skos:prefLabel "Has name"@en ;
.
org:hasUnit
  rdf:type owl:ObjectProperty ;
  rdfs:isDefinedBy <http://data.europa.eu/a4g/ontology> ;
  rdfs:label "Has unit"@en ;
  skos:prefLabel "Has unit"@en ;
.
org:unitOf
  rdf:type owl:ObjectProperty ;
  rdfs:isDefinedBy <http://data.europa.eu/a4g/ontology> ;
  rdfs:label "Unit of"@en ;
  skos:prefLabel "Unit of"@en ;
.
<http://www.w3.org/ns/regorg#hasRegisteredOrganization>
  rdf:type owl:ObjectProperty ;
  rdfs:isDefinedBy <http://data.europa.eu/a4g/ontology> ;
  rdfs:label "Has registered organization"@en ;
  skos:prefLabel "Has registered organization"@en ;
.
foaf:Agent
  rdf:type owl:Class ;
  rdfs:isDefinedBy <http://data.europa.eu/a4g/ontology> ;
  rdfs:label "Agent"@en ;
  skos:prefLabel "Agent"@en ;
.
foaf:Document
  rdf:type owl:Class ;
  rdfs:isDefinedBy <http://data.europa.eu/a4g/ontology> ;
  rdfs:label "Document"@en ;
  skos:prefLabel "Document"@en ;
.
foaf:Group
  rdf:type owl:Class ;
  rdfs:isDefinedBy <http://data.europa.eu/a4g/ontology> ;
  rdfs:label "Group"@en ;
  rdfs:subClassOf foaf:Agent ;
  owl:disjointWith dct:Agent ;
  owl:disjointWith org:Organization ;
  owl:disjointWith foaf:Organization ;
  owl:disjointWith foaf:Person ;
  skos:prefLabel "Group"@en ;
.
foaf:Organization
  rdf:type owl:Class ;
  rdfs:isDefinedBy <http://data.europa.eu/a4g/ontology> ;
  rdfs:label "Organization"@en ;
  rdfs:subClassOf foaf:Agent ;
  owl:disjointWith dct:Agent ;
  owl:disjointWith org:Organization ;
  owl:disjointWith foaf:Group ;
  owl:disjointWith foaf:Person ;
  skos:prefLabel "Organization"@en ;
.
foaf:Person
  rdf:type owl:Class ;
  rdfs:isDefinedBy <http://data.europa.eu/a4g/ontology> ;
  rdfs:label "Person"@en ;
  rdfs:subClassOf foaf:Agent ;
  owl:disjointWith dct:Agent ;
  owl:disjointWith org:Organization ;
  owl:disjointWith foaf:Group ;
  owl:disjointWith foaf:Organization ;
  skos:prefLabel "Person"@en ;
.
foaf:Project
  rdf:type owl:Class ;
  rdfs:isDefinedBy <http://data.europa.eu/a4g/ontology> ;
  rdfs:label "Project"@en ;
  skos:prefLabel "Project"@en ;
.
foaf:member
  rdf:type owl:ObjectProperty ;
  rdfs:isDefinedBy <http://data.europa.eu/a4g/ontology> ;
  rdfs:label "Member"@en ;
  skos:prefLabel "Member"@en ;
.
<https://github.com/ESPD/ESPD-EDM/Confidentiality-level>
  rdf:type skos:ConceptScheme ;
  rdfs:isDefinedBy <http://data.europa.eu/a4g/ontology> ;
  rdfs:label "Confidentiality-level"@en ;
  skos:prefLabel "Confidentiality-level" ;
.
